<?xml version="1.0"?>
<rdf:RDF xmlns="http://www.semanticweb.org/sc3/ontologies/2022/0/Planning-Ontology#"
     xml:base="http://www.semanticweb.org/sc3/ontologies/2022/0/Planning-Ontology"
     xmlns:owl="http://www.w3.org/2002/07/owl#"
     xmlns:rdf="http://www.w3.org/1999/02/22-rdf-syntax-ns#"
     xmlns:sc3="http://www.semanticweb.org/sc3/ontologies/2022/0/Planning-Ontology#sc3:"
     xmlns:xml="http://www.w3.org/XML/1998/namespace"
     xmlns:xsd="http://www.w3.org/2001/XMLSchema#"
     xmlns:rdfs="http://www.w3.org/2000/01/rdf-schema#"
     xmlns:skos="http://www.w3.org/2004/02/skos/core#"
     xmlns:time="http://www.w3.org/2006/time#"
     xmlns:terms="http://purl.org/dc/terms/"
     xmlns:Planning-Ontology="http://www.semanticweb.org/sc3/ontologies/2022/0/Planning-Ontology#">
    <owl:Ontology rdf:about="http://www.semanticweb.org/sc3/ontologies/2022/0/Planning-Ontology">
        <owl:imports rdf:resource="http://www.semanticweb.org/sc3/ontologies/2022/0/ozone-ontology"/>
        <owl:imports rdf:resource="http://www.w3.org/2006/time#2016"/>
    </owl:Ontology>
    


    <!-- 
    ///////////////////////////////////////////////////////////////////////////////////////
    //
    // Annotation properties
    //
    ///////////////////////////////////////////////////////////////////////////////////////
     -->


    


    <!-- http://www.semanticweb.org/sc3/ontologies/2022/0/Planning-Ontology#sc3:formula -->


    <owl:AnnotationProperty rdf:about="http://www.semanticweb.org/sc3/ontologies/2022/0/Planning-Ontology#sc3:formula"/>
    


    <!-- 
    ///////////////////////////////////////////////////////////////////////////////////////
    //
    // Datatypes
    //
    ///////////////////////////////////////////////////////////////////////////////////////
     -->


    


    <!-- http://www.w3.org/2001/XMLSchema#dateTimeStamp -->


    <rdf:Description rdf:about="http://www.w3.org/2001/XMLSchema#dateTimeStamp">
        <rdfs:label xml:lang="es">sello de tiempo</rdfs:label>
    </rdf:Description>
    


    <!-- http://www.w3.org/2001/XMLSchema#duration -->


    <rdfs:Datatype rdf:about="http://www.w3.org/2001/XMLSchema#duration"/>
    


    <!-- http://www.w3.org/2006/time#generalDay -->


    <rdfs:Datatype rdf:about="http://www.w3.org/2006/time#generalDay">
        <rdfs:comment xml:lang="en">Day of month - formulated as a text string with a pattern constraint to reproduce the same lexical form as gDay, except that values up to 99 are permitted, in order to support calendars with more than 31 days in a month. 
Note that the value-space is not defined, so a generic OWL2 processor cannot compute ordering relationships of values of this type.</rdfs:comment>
        <rdfs:comment xml:lang="es">Día del mes - formulado como una cadena de texto con una restricción patrón para reproducir la misma forma léxica que gDay, excepto que se permiten valores hasta el 99, con el propósito de proporcionar soporte a calendarios con meses con más de 31 días.
            Nótese que el espacio de valores no está definido, por tanto, un procesador genérico de OWL2 no puede computar relaciones de orden de valores de este tipo.</rdfs:comment>
        <rdfs:label xml:lang="es">Día generalizado</rdfs:label>
        <rdfs:label xml:lang="en">Generalized day</rdfs:label>
        <skos:definition xml:lang="en">Day of month - formulated as a text string with a pattern constraint to reproduce the same lexical form as gDay, except that values up to 99 are permitted, in order to support calendars with more than 31 days in a month. 
Note that the value-space is not defined, so a generic OWL2 processor cannot compute ordering relationships of values of this type.</skos:definition>
        <skos:definition xml:lang="es">Día del mes - formulado como una cadena de texto con una restricción patrón para reproducir la misma forma léxica que gDay, excepto que se permiten valores hasta el 99, con el propósito de proporcionar soporte a calendarios con meses con más de 31 días.
            Nótese que el espacio de valores no está definido, por tanto, un procesador genérico de OWL2 no puede computar relaciones de orden de valores de este tipo.</skos:definition>
    </rdfs:Datatype>
    


    <!-- http://www.w3.org/2006/time#generalMonth -->


    <rdfs:Datatype rdf:about="http://www.w3.org/2006/time#generalMonth">
        <rdfs:comment xml:lang="es">Mes del año - formulado como una cadena de texto con una restricción patrón para reproducir la misma forma léxica que gMonth, excepto que se permiten valores hasta el 20, con el propósito de proporcionar soporte a calendarios con años con más de 12 meses.
            Nótese que el espacio de valores no está definido, por tanto, un procesador genérico de OWL2 no puede computar relaciones de orden de valores de este tipo.</rdfs:comment>
        <rdfs:comment xml:lang="en">Month of year - formulated as a text string with a pattern constraint to reproduce the same lexical form as gMonth, except that values up to 20 are permitted, in order to support calendars with more than 12 months in the year. 
Note that the value-space is not defined, so a generic OWL2 processor cannot compute ordering relationships of values of this type.</rdfs:comment>
        <rdfs:label xml:lang="en">Generalized month</rdfs:label>
        <rdfs:label xml:lang="es">Mes generalizado</rdfs:label>
        <skos:definition xml:lang="es">Mes del año - formulado como una cadena de texto con una restricción patrón para reproducir la misma forma léxica que gMonth, excepto que se permiten valores hasta el 20, con el propósito de proporcionar soporte a calendarios con años con más de 12 meses.
            Nótese que el espacio de valores no está definido, por tanto, un procesador genérico de OWL2 no puede computar relaciones de orden de valores de este tipo.</skos:definition>
        <skos:definition xml:lang="en">Month of year - formulated as a text string with a pattern constraint to reproduce the same lexical form as gMonth, except that values up to 20 are permitted, in order to support calendars with more than 12 months in the year. 
Note that the value-space is not defined, so a generic OWL2 processor cannot compute ordering relationships of values of this type.</skos:definition>
    </rdfs:Datatype>
    


    <!-- http://www.w3.org/2006/time#generalYear -->


    <rdfs:Datatype rdf:about="http://www.w3.org/2006/time#generalYear">
        <rdfs:comment xml:lang="es">Número de año - formulado como una cadena de texto con una restricción patrón para reproducir la misma forma léxica que gYear, aunque no está restringido a valores del calendario gregoriano.
            Nótese que el espacio de valores no está definido, por tanto, un procesador genérico de OWL2 no puede computar relaciones de orden de valores de este tipo.</rdfs:comment>
        <rdfs:comment xml:lang="en">Year number - formulated as a text string with a pattern constraint to reproduce the same lexical form as gYear, but not restricted to values from the Gregorian calendar. 
Note that the value-space is not defined, so a generic OWL2 processor cannot compute ordering relationships of values of this type.</rdfs:comment>
        <rdfs:label xml:lang="es">Año generalizado</rdfs:label>
        <rdfs:label xml:lang="en">Generalized year</rdfs:label>
        <skos:definition xml:lang="es">Número de año - formulado como una cadena de texto con una restricción patrón para reproducir la misma forma léxica que gYear, aunque no está restringido a valores del calendario gregoriano.
            Nótese que el espacio de valores no está definido, por tanto, un procesador genérico de OWL2 no puede computar relaciones de orden de valores de este tipo.</skos:definition>
        <skos:definition xml:lang="en">Year number - formulated as a text string with a pattern constraint to reproduce the same lexical form as gYear, but not restricted to values from the Gregorian calendar. 
Note that the value-space is not defined, so a generic OWL2 processor cannot compute ordering relationships of values of this type.</skos:definition>
    </rdfs:Datatype>
    


    <!-- 
    ///////////////////////////////////////////////////////////////////////////////////////
    //
    // Object Properties
    //
    ///////////////////////////////////////////////////////////////////////////////////////
     -->


    


    <!-- http://www.semanticweb.org/sc3/ontologies/2022/0/Planning-Ontology#hasActivities -->


    <owl:ObjectProperty rdf:about="http://www.semanticweb.org/sc3/ontologies/2022/0/Planning-Ontology#hasActivities">
        <rdfs:subPropertyOf rdf:resource="http://www.w3.org/2002/07/owl#topObjectProperty"/>
        <rdfs:domain rdf:resource="http://www.semanticweb.org/sc3/ontologies/2022/0/Planning-Ontology#PlanningObject"/>
        <rdfs:domain rdf:resource="http://www.semanticweb.org/sc3/ontologies/2022/0/Planning-Ontology#RequiredCapacity"/>
        <rdfs:domain rdf:resource="http://www.semanticweb.org/sc3/ontologies/2022/0/ozone-ontology#Product"/>
        <rdfs:range rdf:resource="http://www.semanticweb.org/sc3/ontologies/2022/0/Planning-Ontology#Activity"/>
        <rdfs:comment>This property describes the set of activities that must be carried out to produce the goods that are associated with the PLANNING OBJECT.

Moreover, there are additional parameters for most types of PLANNING OBJECTS.</rdfs:comment>
    </owl:ObjectProperty>
    


    <!-- http://www.semanticweb.org/sc3/ontologies/2022/0/Planning-Ontology#hasBillOfMaterial -->


    <owl:ObjectProperty rdf:about="http://www.semanticweb.org/sc3/ontologies/2022/0/Planning-Ontology#hasBillOfMaterial">
        <rdfs:domain rdf:resource="http://www.semanticweb.org/sc3/ontologies/2022/0/Planning-Ontology#Part"/>
        <rdfs:domain rdf:resource="http://www.semanticweb.org/sc3/ontologies/2022/0/ozone-ontology#Product"/>
        <rdfs:range rdf:resource="http://www.semanticweb.org/sc3/ontologies/2022/0/Planning-Ontology#BillOfMaterial"/>
        <rdfs:comment>A set of potentially alternative BOMs can be used to meet the demand of a certain product</rdfs:comment>
    </owl:ObjectProperty>
    


    <!-- http://www.semanticweb.org/sc3/ontologies/2022/0/Planning-Ontology#hasBin -->


    <owl:ObjectProperty rdf:about="http://www.semanticweb.org/sc3/ontologies/2022/0/Planning-Ontology#hasBin">
        <rdfs:domain rdf:resource="http://www.semanticweb.org/sc3/ontologies/2022/0/Planning-Ontology#Binning"/>
        <rdfs:range rdf:resource="http://www.semanticweb.org/sc3/ontologies/2022/0/Planning-Ontology#Bin"/>
    </owl:ObjectProperty>
    


    <!-- http://www.semanticweb.org/sc3/ontologies/2022/0/Planning-Ontology#hasCapacity -->


    <owl:ObjectProperty rdf:about="http://www.semanticweb.org/sc3/ontologies/2022/0/Planning-Ontology#hasCapacity">
        <rdfs:domain rdf:resource="http://www.semanticweb.org/sc3/ontologies/2022/0/Planning-Ontology#Process"/>
        <rdfs:domain rdf:resource="http://www.semanticweb.org/sc3/ontologies/2022/0/ozone-ontology#Resource"/>
        <rdfs:range rdf:resource="http://www.semanticweb.org/sc3/ontologies/2022/0/Planning-Ontology#AvailableCapacity"/>
    </owl:ObjectProperty>
    


    <!-- http://www.semanticweb.org/sc3/ontologies/2022/0/Planning-Ontology#hasChildProductAggregate -->


    <owl:ObjectProperty rdf:about="http://www.semanticweb.org/sc3/ontologies/2022/0/Planning-Ontology#hasChildProductAggregate">
        <rdfs:domain rdf:resource="http://www.semanticweb.org/sc3/ontologies/2022/0/Planning-Ontology#ProductHierarchy"/>
        <rdfs:range rdf:resource="http://www.semanticweb.org/sc3/ontologies/2022/0/Planning-Ontology#ProductHierarchy"/>
    </owl:ObjectProperty>
    


    <!-- http://www.semanticweb.org/sc3/ontologies/2022/0/Planning-Ontology#hasComponentLocation -->


    <owl:ObjectProperty rdf:about="http://www.semanticweb.org/sc3/ontologies/2022/0/Planning-Ontology#hasComponentLocation">
        <rdfs:domain rdf:resource="http://www.semanticweb.org/sc3/ontologies/2022/0/Planning-Ontology#BillOfMaterial"/>
        <rdfs:range rdf:resource="http://www.semanticweb.org/sc3/ontologies/2022/0/Planning-Ontology#Location"/>
    </owl:ObjectProperty>
    


    <!-- http://www.semanticweb.org/sc3/ontologies/2022/0/Planning-Ontology#hasComponentPart -->


    <owl:ObjectProperty rdf:about="http://www.semanticweb.org/sc3/ontologies/2022/0/Planning-Ontology#hasComponentPart">
        <rdfs:subPropertyOf rdf:resource="http://www.w3.org/2002/07/owl#topObjectProperty"/>
        <rdfs:domain rdf:resource="http://www.semanticweb.org/sc3/ontologies/2022/0/Planning-Ontology#BillOfMaterial"/>
        <rdfs:domain rdf:resource="http://www.semanticweb.org/sc3/ontologies/2022/0/Planning-Ontology#Process"/>
        <rdfs:range rdf:resource="http://www.semanticweb.org/sc3/ontologies/2022/0/Planning-Ontology#ComponentPart"/>
    </owl:ObjectProperty>
    


    <!-- http://www.semanticweb.org/sc3/ontologies/2022/0/Planning-Ontology#hasComponentProcess -->


    <owl:ObjectProperty rdf:about="http://www.semanticweb.org/sc3/ontologies/2022/0/Planning-Ontology#hasComponentProcess">
        <rdfs:domain rdf:resource="http://www.semanticweb.org/sc3/ontologies/2022/0/Planning-Ontology#BillOfMaterial"/>
        <rdfs:range rdf:resource="http://www.semanticweb.org/sc3/ontologies/2022/0/Planning-Ontology#Process"/>
    </owl:ObjectProperty>
    


    <!-- http://www.semanticweb.org/sc3/ontologies/2022/0/Planning-Ontology#hasConnection -->


    <owl:ObjectProperty rdf:about="http://www.semanticweb.org/sc3/ontologies/2022/0/Planning-Ontology#hasConnection">
        <rdfs:subPropertyOf rdf:resource="http://www.w3.org/2002/07/owl#topObjectProperty"/>
        <rdfs:domain rdf:resource="http://www.semanticweb.org/sc3/ontologies/2022/0/Planning-Ontology#DecisionMakingUnit"/>
        <rdfs:domain rdf:resource="http://www.semanticweb.org/sc3/ontologies/2022/0/Planning-Ontology#PlanningProcess"/>
        <rdfs:range rdf:resource="http://www.semanticweb.org/sc3/ontologies/2022/0/Planning-Ontology#Edge"/>
        <rdfs:comment>If a vertex provides instruction or a reaction to another vertex than the two vertices are connected by a directed edge.</rdfs:comment>
    </owl:ObjectProperty>
    


    <!-- http://www.semanticweb.org/sc3/ontologies/2022/0/Planning-Ontology#hasConstraint -->


    <owl:ObjectProperty rdf:about="http://www.semanticweb.org/sc3/ontologies/2022/0/Planning-Ontology#hasConstraint"/>
    


    <!-- http://www.semanticweb.org/sc3/ontologies/2022/0/Planning-Ontology#hasCriterias -->


    <owl:ObjectProperty rdf:about="http://www.semanticweb.org/sc3/ontologies/2022/0/Planning-Ontology#hasCriterias">
        <rdfs:domain rdf:resource="http://www.semanticweb.org/sc3/ontologies/2022/0/Planning-Ontology#PlaningPurpose"/>
        <rdfs:range rdf:resource="http://www.semanticweb.org/sc3/ontologies/2022/0/Planning-Ontology#Criteria"/>
        <rdfs:comment>A criterion is assigned to each performance measure that belongs to a PLANNING PURPOSE. Typical criteria are maximization, minimization, i.e. if an optimization problem is considered, or larger or smaller than a prescribed value of the certain performance measure, a so-called target, i.e. if a satisfaction problem is solved. In a multi-criteria setting, the dominance concept for plans is of interest.</rdfs:comment>
    </owl:ObjectProperty>
    


    <!-- http://www.semanticweb.org/sc3/ontologies/2022/0/Planning-Ontology#hasDMUa -->


    <owl:ObjectProperty rdf:about="http://www.semanticweb.org/sc3/ontologies/2022/0/Planning-Ontology#hasDMUa">
        <rdfs:subPropertyOf rdf:resource="http://www.w3.org/2002/07/owl#topObjectProperty"/>
        <rdfs:domain rdf:resource="http://www.semanticweb.org/sc3/ontologies/2022/0/Planning-Ontology#Vertex"/>
        <rdfs:range rdf:resource="http://www.semanticweb.org/sc3/ontologies/2022/0/Planning-Ontology#DecisionMakingUnit"/>
        <rdfs:comment>First DMU of the Vertex</rdfs:comment>
    </owl:ObjectProperty>
    


    <!-- http://www.semanticweb.org/sc3/ontologies/2022/0/Planning-Ontology#hasDMUb -->


    <owl:ObjectProperty rdf:about="http://www.semanticweb.org/sc3/ontologies/2022/0/Planning-Ontology#hasDMUb">
        <rdfs:subPropertyOf rdf:resource="http://www.w3.org/2002/07/owl#topObjectProperty"/>
        <rdfs:domain rdf:resource="http://www.semanticweb.org/sc3/ontologies/2022/0/Planning-Ontology#Edge"/>
        <rdfs:range rdf:resource="http://www.semanticweb.org/sc3/ontologies/2022/0/Planning-Ontology#DecisionMakingUnit"/>
        <rdfs:comment>Second DMU of the Vertex</rdfs:comment>
    </owl:ObjectProperty>
    


    <!-- http://www.semanticweb.org/sc3/ontologies/2022/0/Planning-Ontology#hasDecisionMakerType -->


    <owl:ObjectProperty rdf:about="http://www.semanticweb.org/sc3/ontologies/2022/0/Planning-Ontology#hasDecisionMakerType">
        <rdfs:subPropertyOf rdf:resource="http://www.w3.org/2002/07/owl#topObjectProperty"/>
        <rdfs:domain rdf:resource="http://www.semanticweb.org/sc3/ontologies/2022/0/Planning-Ontology#DecisionMakingUnit"/>
        <rdfs:range rdf:resource="http://www.semanticweb.org/sc3/ontologies/2022/0/Planning-Ontology#DecisionMakerType"/>
        <rdfs:comment>Specifies the concrete type of a DMU</rdfs:comment>
    </owl:ObjectProperty>
    


    <!-- http://www.semanticweb.org/sc3/ontologies/2022/0/Planning-Ontology#hasDecisionMakingInitiative -->


    <owl:ObjectProperty rdf:about="http://www.semanticweb.org/sc3/ontologies/2022/0/Planning-Ontology#hasDecisionMakingInitiative">
        <rdfs:subPropertyOf rdf:resource="http://www.w3.org/2002/07/owl#topObjectProperty"/>
        <rdfs:domain rdf:resource="http://www.semanticweb.org/sc3/ontologies/2022/0/Planning-Ontology#DecisionMakingUnit"/>
        <rdfs:range rdf:resource="http://www.semanticweb.org/sc3/ontologies/2022/0/Planning-Ontology#DecisionMakingInitiative"/>
        <rdfs:comment>We distinguish fully autonomous DECISION-MAKING UNITS from DECISION-MAKING UNITS where the decision-making activities are triggered by other DECISION-MAKING UNITS. Note that the decision-making initiative can change over time in a situation-dependent manner.</rdfs:comment>
    </owl:ObjectProperty>
    


    <!-- http://www.semanticweb.org/sc3/ontologies/2022/0/Planning-Ontology#hasDecisionMakingUnit -->


    <owl:ObjectProperty rdf:about="http://www.semanticweb.org/sc3/ontologies/2022/0/Planning-Ontology#hasDecisionMakingUnit">
        <rdfs:subPropertyOf rdf:resource="http://www.w3.org/2002/07/owl#topObjectProperty"/>
        <rdfs:domain rdf:resource="http://www.semanticweb.org/sc3/ontologies/2022/0/Planning-Ontology#PlanningSituation"/>
        <rdfs:domain rdf:resource="http://www.semanticweb.org/sc3/ontologies/2022/0/Planning-Ontology#Vertex"/>
        <rdfs:range rdf:resource="http://www.semanticweb.org/sc3/ontologies/2022/0/Planning-Ontology#DecisionMakingUnit"/>
        <rdfs:comment>This property describes the set of DECISION-MAKING UNITS that constitutes the planning situation. We refer to the elements of the set as vertices.</rdfs:comment>
    </owl:ObjectProperty>
    


    <!-- http://www.semanticweb.org/sc3/ontologies/2022/0/Planning-Ontology#hasDecisionMakingUnitCharcters -->


    <owl:ObjectProperty rdf:about="http://www.semanticweb.org/sc3/ontologies/2022/0/Planning-Ontology#hasDecisionMakingUnitCharcters">
        <rdfs:subPropertyOf rdf:resource="http://www.w3.org/2002/07/owl#topObjectProperty"/>
        <rdfs:domain rdf:resource="http://www.semanticweb.org/sc3/ontologies/2022/0/Planning-Ontology#PlanningSituation"/>
        <rdfs:range rdf:resource="http://www.semanticweb.org/sc3/ontologies/2022/0/Planning-Ontology#DecisonMakingUnitCharacter"/>
    </owl:ObjectProperty>
    


    <!-- http://www.semanticweb.org/sc3/ontologies/2022/0/Planning-Ontology#hasDefined -->


    <owl:ObjectProperty rdf:about="http://www.semanticweb.org/sc3/ontologies/2022/0/Planning-Ontology#hasDefined">
        <rdfs:subPropertyOf rdf:resource="http://www.w3.org/2002/07/owl#topObjectProperty"/>
        <rdfs:domain rdf:resource="http://www.semanticweb.org/sc3/ontologies/2022/0/Planning-Ontology#PlanExecutuon"/>
        <rdfs:range rdf:resource="http://www.semanticweb.org/sc3/ontologies/2022/0/Planning-Ontology#PerformanceMeasure"/>
        <rdfs:comment>Values for certain PERFORMANCE MEASURES can be computed after a plan is executed. This always requires that the consequences of a PLAN are assessed in the base system.</rdfs:comment>
    </owl:ObjectProperty>
    


    <!-- http://www.semanticweb.org/sc3/ontologies/2022/0/Planning-Ontology#hasEarliestReleaseDate -->


    <owl:ObjectProperty rdf:about="http://www.semanticweb.org/sc3/ontologies/2022/0/Planning-Ontology#hasEarliestReleaseDate">
        <rdfs:subPropertyOf rdf:resource="http://www.w3.org/2002/07/owl#topObjectProperty"/>
        <rdfs:domain rdf:resource="http://www.semanticweb.org/sc3/ontologies/2022/0/Planning-Ontology#PlanningObject"/>
        <rdfs:range rdf:resource="http://www.w3.org/2006/time#TemporalDuration"/>
    </owl:ObjectProperty>
    


    <!-- http://www.semanticweb.org/sc3/ontologies/2022/0/Planning-Ontology#hasEventTrigger -->


    <owl:ObjectProperty rdf:about="http://www.semanticweb.org/sc3/ontologies/2022/0/Planning-Ontology#hasEventTrigger">
        <rdfs:subPropertyOf rdf:resource="http://www.w3.org/2002/07/owl#topObjectProperty"/>
        <rdfs:domain rdf:resource="http://www.semanticweb.org/sc3/ontologies/2022/0/Planning-Ontology#PlanningProcess"/>
        <rdfs:range rdf:resource="http://www.semanticweb.org/sc3/ontologies/2022/0/Planning-Ontology#Trigger"/>
        <rdfs:comment>This property determines which events result in replanning (Vieria et al. 2003). For instance, replanning can be the result of the breakdown of a bottleneck resource.</rdfs:comment>
    </owl:ObjectProperty>
    


    <!-- http://www.semanticweb.org/sc3/ontologies/2022/0/Planning-Ontology#hasFrozenFence -->


    <owl:ObjectProperty rdf:about="http://www.semanticweb.org/sc3/ontologies/2022/0/Planning-Ontology#hasFrozenFence">
        <rdfs:subPropertyOf rdf:resource="http://www.w3.org/2002/07/owl#topObjectProperty"/>
        <rdfs:domain rdf:resource="http://www.semanticweb.org/sc3/ontologies/2022/0/Planning-Ontology#PlanningProcess"/>
        <rdfs:range rdf:resource="http://www.semanticweb.org/sc3/ontologies/2022/0/Planning-Ontology#PlanningDecision"/>
        <rdfs:comment>This property specifies which planning decisions are remain unchanged in the case of replanning activities.</rdfs:comment>
    </owl:ObjectProperty>
    


    <!-- http://www.semanticweb.org/sc3/ontologies/2022/0/Planning-Ontology#hasHierarchicalSituation -->


    <owl:ObjectProperty rdf:about="http://www.semanticweb.org/sc3/ontologies/2022/0/Planning-Ontology#hasHierarchicalSituation">
        <rdfs:subPropertyOf rdf:resource="http://www.w3.org/2002/07/owl#topObjectProperty"/>
        <rdfs:domain rdf:resource="http://www.semanticweb.org/sc3/ontologies/2022/0/Planning-Ontology#PlanningSituation"/>
        <rdfs:range rdf:resource="http://www.semanticweb.org/sc3/ontologies/2022/0/Planning-Ontology#HierarchicalSituation"/>
    </owl:ObjectProperty>
    


    <!-- http://www.semanticweb.org/sc3/ontologies/2022/0/Planning-Ontology#hasInvolvedPlanningObjects -->


    <owl:ObjectProperty rdf:about="http://www.semanticweb.org/sc3/ontologies/2022/0/Planning-Ontology#hasInvolvedPlanningObjects">
        <rdfs:subPropertyOf rdf:resource="http://www.w3.org/2002/07/owl#topObjectProperty"/>
        <rdfs:domain rdf:resource="http://www.semanticweb.org/sc3/ontologies/2022/0/Planning-Ontology#PlanningInstance"/>
        <rdfs:range rdf:resource="http://www.semanticweb.org/sc3/ontologies/2022/0/Planning-Ontology#PlanningObject"/>
        <rdfs:comment>This property specifies the involved PLANNING OBJECTS.</rdfs:comment>
    </owl:ObjectProperty>
    


    <!-- http://www.semanticweb.org/sc3/ontologies/2022/0/Planning-Ontology#hasLocation -->


    <owl:ObjectProperty rdf:about="http://www.semanticweb.org/sc3/ontologies/2022/0/Planning-Ontology#hasLocation">
        <rdfs:subPropertyOf rdf:resource="http://www.w3.org/2002/07/owl#topObjectProperty"/>
        <rdfs:domain rdf:resource="http://www.semanticweb.org/sc3/ontologies/2022/0/Planning-Ontology#BillOfMaterial"/>
        <rdfs:domain rdf:resource="http://www.semanticweb.org/sc3/ontologies/2022/0/Planning-Ontology#Binning"/>
        <rdfs:domain rdf:resource="http://www.semanticweb.org/sc3/ontologies/2022/0/Planning-Ontology#Capacity"/>
        <rdfs:domain rdf:resource="http://www.semanticweb.org/sc3/ontologies/2022/0/Planning-Ontology#FrozenFence"/>
        <rdfs:domain rdf:resource="http://www.semanticweb.org/sc3/ontologies/2022/0/Planning-Ontology#Inventory"/>
        <rdfs:domain rdf:resource="http://www.semanticweb.org/sc3/ontologies/2022/0/Planning-Ontology#InventoryPolicy"/>
        <rdfs:domain rdf:resource="http://www.semanticweb.org/sc3/ontologies/2022/0/Planning-Ontology#LotSizingRule"/>
        <rdfs:domain rdf:resource="http://www.semanticweb.org/sc3/ontologies/2022/0/Planning-Ontology#PlanningObject"/>
        <rdfs:domain rdf:resource="http://www.semanticweb.org/sc3/ontologies/2022/0/Planning-Ontology#Process"/>
        <rdfs:domain rdf:resource="http://www.semanticweb.org/sc3/ontologies/2022/0/Planning-Ontology#ProjectedWip"/>
        <rdfs:domain rdf:resource="http://www.semanticweb.org/sc3/ontologies/2022/0/Planning-Ontology#Substitution"/>
        <rdfs:domain rdf:resource="http://www.semanticweb.org/sc3/ontologies/2022/0/Planning-Ontology#SupplyInformation"/>
        <rdfs:domain rdf:resource="http://www.semanticweb.org/sc3/ontologies/2022/0/Planning-Ontology#Yield"/>
        <rdfs:domain rdf:resource="http://www.semanticweb.org/sc3/ontologies/2022/0/ozone-ontology#Product"/>
        <rdfs:range rdf:resource="http://www.semanticweb.org/sc3/ontologies/2022/0/Planning-Ontology#Location"/>
        <rdfs:comment>This property describes the place or places, for instance nodes of the semiconductor supply chain or specific machines of a work center where the ACTIVITIES associated with the PLANNING OBJECT have to be executed.</rdfs:comment>
    </owl:ObjectProperty>
    


    <!-- http://www.semanticweb.org/sc3/ontologies/2022/0/Planning-Ontology#hasObjectives -->


    <owl:ObjectProperty rdf:about="http://www.semanticweb.org/sc3/ontologies/2022/0/Planning-Ontology#hasObjectives">
        <rdfs:domain rdf:resource="http://www.semanticweb.org/sc3/ontologies/2022/0/Planning-Ontology#PlanningProcess"/>
        <rdfs:range rdf:resource="http://www.semanticweb.org/sc3/ontologies/2022/0/Planning-Ontology#PlaningPurpose"/>
        <rdfs:comment>: The property specifies the objectives of a certain planning activity.
Moreover, there are additional parameters for most types of PLANNING PROCESS.</rdfs:comment>
    </owl:ObjectProperty>
    


    <!-- http://www.semanticweb.org/sc3/ontologies/2022/0/Planning-Ontology#hasOperations -->


    <owl:ObjectProperty rdf:about="http://www.semanticweb.org/sc3/ontologies/2022/0/Planning-Ontology#hasOperations">
        <rdfs:domain rdf:resource="http://www.semanticweb.org/sc3/ontologies/2022/0/Planning-Ontology#Route"/>
        <rdfs:range rdf:resource="http://www.semanticweb.org/sc3/ontologies/2022/0/Planning-Ontology#MacroOperation"/>
    </owl:ObjectProperty>
    


    <!-- http://www.semanticweb.org/sc3/ontologies/2022/0/Planning-Ontology#hasOrder -->


    <owl:ObjectProperty rdf:about="http://www.semanticweb.org/sc3/ontologies/2022/0/Planning-Ontology#hasOrder">
        <rdfs:domain rdf:resource="http://www.semanticweb.org/sc3/ontologies/2022/0/Planning-Ontology#In-TransitInventory"/>
        <rdfs:range rdf:resource="http://www.semanticweb.org/sc3/ontologies/2022/0/Planning-Ontology#Order"/>
    </owl:ObjectProperty>
    


    <!-- http://www.semanticweb.org/sc3/ontologies/2022/0/Planning-Ontology#hasOwner -->


    <owl:ObjectProperty rdf:about="http://www.semanticweb.org/sc3/ontologies/2022/0/Planning-Ontology#hasOwner">
        <rdfs:subPropertyOf rdf:resource="http://www.w3.org/2002/07/owl#topObjectProperty"/>
        <rdfs:domain rdf:resource="http://www.semanticweb.org/sc3/ontologies/2022/0/Planning-Ontology#PlanningObject"/>
        <rdfs:range rdf:resource="http://www.semanticweb.org/sc3/ontologies/2022/0/Planning-Ontology#Owner"/>
        <rdfs:comment>A PLANNING OBJECT is rarely considered in isolation. Usually it belongs to a set of PLANNING OBJECTS, for example, a planning instance.</rdfs:comment>
    </owl:ObjectProperty>
    


    <!-- http://www.semanticweb.org/sc3/ontologies/2022/0/Planning-Ontology#hasParentProductAggregate -->


    <owl:ObjectProperty rdf:about="http://www.semanticweb.org/sc3/ontologies/2022/0/Planning-Ontology#hasParentProductAggregate">
        <rdfs:domain rdf:resource="http://www.semanticweb.org/sc3/ontologies/2022/0/Planning-Ontology#ProductHierarchy"/>
        <rdfs:range rdf:resource="http://www.semanticweb.org/sc3/ontologies/2022/0/Planning-Ontology#ProductHierarchy"/>
    </owl:ObjectProperty>
    


    <!-- http://www.semanticweb.org/sc3/ontologies/2022/0/Planning-Ontology#hasPart -->


    <owl:ObjectProperty rdf:about="http://www.semanticweb.org/sc3/ontologies/2022/0/Planning-Ontology#hasPart">
        <rdfs:domain rdf:resource="http://www.semanticweb.org/sc3/ontologies/2022/0/Planning-Ontology#Bin"/>
        <rdfs:domain rdf:resource="http://www.semanticweb.org/sc3/ontologies/2022/0/Planning-Ontology#Binning"/>
        <rdfs:domain rdf:resource="http://www.semanticweb.org/sc3/ontologies/2022/0/Planning-Ontology#ProjectedWip"/>
        <rdfs:domain rdf:resource="http://www.semanticweb.org/sc3/ontologies/2022/0/Planning-Ontology#Yield"/>
        <rdfs:range rdf:resource="http://www.semanticweb.org/sc3/ontologies/2022/0/Planning-Ontology#Part"/>
    </owl:ObjectProperty>
    


    <!-- http://www.semanticweb.org/sc3/ontologies/2022/0/Planning-Ontology#hasPerformanceMeasures -->


    <owl:ObjectProperty rdf:about="http://www.semanticweb.org/sc3/ontologies/2022/0/Planning-Ontology#hasPerformanceMeasures">
        <rdfs:subPropertyOf rdf:resource="http://www.w3.org/2002/07/owl#topObjectProperty"/>
        <rdfs:domain rdf:resource="http://www.semanticweb.org/sc3/ontologies/2022/0/Planning-Ontology#PlaningPurpose"/>
        <rdfs:range rdf:resource="http://www.semanticweb.org/sc3/ontologies/2022/0/Planning-Ontology#PerformanceMeasure"/>
        <rdfs:comment>Each PLANNING PURPOSE is determined by a set of performance measures. Each measure is defined by a calculation procedure. Performance measures can be blended using weights to express the importance of the different measures.</rdfs:comment>
    </owl:ObjectProperty>
    


    <!-- http://www.semanticweb.org/sc3/ontologies/2022/0/Planning-Ontology#hasPeriodicTrigger -->


    <owl:ObjectProperty rdf:about="http://www.semanticweb.org/sc3/ontologies/2022/0/Planning-Ontology#hasPeriodicTrigger">
        <rdfs:subPropertyOf rdf:resource="http://www.w3.org/2002/07/owl#topObjectProperty"/>
        <rdfs:domain rdf:resource="http://www.semanticweb.org/sc3/ontologies/2022/0/Planning-Ontology#PlanningProcess"/>
        <rdfs:range rdf:resource="http://www.semanticweb.org/sc3/ontologies/2022/0/Planning-Ontology#Trigger"/>
        <rdfs:comment>This property defines after which amount of time a replanning activity is initiated in a periodic manner (Vieria et al. 2003). Rolling horizon approaches are triggered by such a periodic approach.</rdfs:comment>
    </owl:ObjectProperty>
    


    <!-- http://www.semanticweb.org/sc3/ontologies/2022/0/Planning-Ontology#hasPlan -->


    <owl:ObjectProperty rdf:about="http://www.semanticweb.org/sc3/ontologies/2022/0/Planning-Ontology#hasPlan">
        <rdfs:subPropertyOf rdf:resource="http://www.w3.org/2002/07/owl#topObjectProperty"/>
        <rdfs:domain rdf:resource="http://www.semanticweb.org/sc3/ontologies/2022/0/Planning-Ontology#PlanningProcess"/>
        <rdfs:range rdf:resource="http://www.semanticweb.org/sc3/ontologies/2022/0/Planning-Ontology#Plan"/>
        <rdfs:comment>Activities associated with a PLANNING PROCESS require an instance of the concept PLAN.</rdfs:comment>
    </owl:ObjectProperty>
    


    <!-- http://www.semanticweb.org/sc3/ontologies/2022/0/Planning-Ontology#hasPlanningConstraints -->


    <owl:ObjectProperty rdf:about="http://www.semanticweb.org/sc3/ontologies/2022/0/Planning-Ontology#hasPlanningConstraints">
        <rdfs:subPropertyOf rdf:resource="http://www.w3.org/2002/07/owl#topObjectProperty"/>
        <rdfs:domain rdf:resource="http://www.semanticweb.org/sc3/ontologies/2022/0/Planning-Ontology#PlanningInstance"/>
        <rdfs:range rdf:resource="http://www.semanticweb.org/sc3/ontologies/2022/0/Planning-Ontology#PlanningConstraint"/>
        <rdfs:comment>This property specifies which constraints must be ensured.</rdfs:comment>
    </owl:ObjectProperty>
    


    <!-- http://www.semanticweb.org/sc3/ontologies/2022/0/Planning-Ontology#hasPlanningInstance -->


    <owl:ObjectProperty rdf:about="http://www.semanticweb.org/sc3/ontologies/2022/0/Planning-Ontology#hasPlanningInstance">
        <rdfs:subPropertyOf rdf:resource="http://www.w3.org/2002/07/owl#topObjectProperty"/>
        <rdfs:domain rdf:resource="http://www.semanticweb.org/sc3/ontologies/2022/0/Planning-Ontology#PlanningProcess"/>
        <rdfs:range rdf:resource="http://www.semanticweb.org/sc3/ontologies/2022/0/Planning-Ontology#PlanningInstance"/>
        <rdfs:comment>Activities associated with PLANNING PROCESS require an instance of the concept PLANNING INSTANCE.</rdfs:comment>
    </owl:ObjectProperty>
    


    <!-- http://www.semanticweb.org/sc3/ontologies/2022/0/Planning-Ontology#hasPlanningObject -->


    <owl:ObjectProperty rdf:about="http://www.semanticweb.org/sc3/ontologies/2022/0/Planning-Ontology#hasPlanningObject">
        <rdfs:domain rdf:resource="http://www.semanticweb.org/sc3/ontologies/2022/0/Planning-Ontology#FrozenFence"/>
        <rdfs:range rdf:resource="http://www.semanticweb.org/sc3/ontologies/2022/0/Planning-Ontology#PlanningObject"/>
    </owl:ObjectProperty>
    


    <!-- http://www.semanticweb.org/sc3/ontologies/2022/0/Planning-Ontology#hasPlanningObjects -->


    <owl:ObjectProperty rdf:about="http://www.semanticweb.org/sc3/ontologies/2022/0/Planning-Ontology#hasPlanningObjects">
        <rdfs:subPropertyOf rdf:resource="http://www.w3.org/2002/07/owl#topObjectProperty"/>
        <rdfs:domain rdf:resource="http://www.semanticweb.org/sc3/ontologies/2022/0/Planning-Ontology#Part"/>
        <rdfs:domain rdf:resource="http://www.semanticweb.org/sc3/ontologies/2022/0/Planning-Ontology#PlaningPurpose"/>
        <rdfs:range rdf:resource="http://www.semanticweb.org/sc3/ontologies/2022/0/Planning-Ontology#PlanningObject"/>
        <rdfs:comment>A set of planning objects is required to determine the performance measure values belonging to the PLANNING PURPOSE. The set of planning objects is often determined by the planning window.</rdfs:comment>
    </owl:ObjectProperty>
    


    <!-- http://www.semanticweb.org/sc3/ontologies/2022/0/Planning-Ontology#hasPlanningProcess -->


    <owl:ObjectProperty rdf:about="http://www.semanticweb.org/sc3/ontologies/2022/0/Planning-Ontology#hasPlanningProcess">
        <rdfs:subPropertyOf rdf:resource="http://www.w3.org/2002/07/owl#topObjectProperty"/>
        <rdfs:domain rdf:resource="http://www.semanticweb.org/sc3/ontologies/2022/0/Planning-Ontology#DecisionMakingUnit"/>
        <rdfs:range rdf:resource="http://www.semanticweb.org/sc3/ontologies/2022/0/Planning-Ontology#PlanningProcess"/>
        <rdfs:comment>This property specifies under which circumstances which (re)planning activities are performed by a DECISION-MAKING UNIT.</rdfs:comment>
    </owl:ObjectProperty>
    


    <!-- http://www.semanticweb.org/sc3/ontologies/2022/0/Planning-Ontology#hasPlanningPurpose -->


    <owl:ObjectProperty rdf:about="http://www.semanticweb.org/sc3/ontologies/2022/0/Planning-Ontology#hasPlanningPurpose">
        <rdfs:domain rdf:resource="http://www.semanticweb.org/sc3/ontologies/2022/0/Planning-Ontology#PlanningProcess"/>
        <rdfs:range rdf:resource="http://www.semanticweb.org/sc3/ontologies/2022/0/Planning-Ontology#PlaningPurpose"/>
    </owl:ObjectProperty>
    


    <!-- http://www.semanticweb.org/sc3/ontologies/2022/0/Planning-Ontology#hasPredecessor -->


    <owl:ObjectProperty rdf:about="http://www.semanticweb.org/sc3/ontologies/2022/0/Planning-Ontology#hasPredecessor">
        <rdfs:domain rdf:resource="http://www.semanticweb.org/sc3/ontologies/2022/0/Planning-Ontology#Location"/>
        <rdfs:range rdf:resource="http://www.semanticweb.org/sc3/ontologies/2022/0/Planning-Ontology#Location"/>
    </owl:ObjectProperty>
    


    <!-- http://www.semanticweb.org/sc3/ontologies/2022/0/Planning-Ontology#hasProcess -->


    <owl:ObjectProperty rdf:about="http://www.semanticweb.org/sc3/ontologies/2022/0/Planning-Ontology#hasProcess">
        <rdfs:domain rdf:resource="http://www.semanticweb.org/sc3/ontologies/2022/0/Planning-Ontology#BillOfMaterial"/>
        <rdfs:domain rdf:resource="http://www.semanticweb.org/sc3/ontologies/2022/0/Planning-Ontology#Binning"/>
        <rdfs:domain rdf:resource="http://www.semanticweb.org/sc3/ontologies/2022/0/Planning-Ontology#RequiredCapacity"/>
        <rdfs:domain rdf:resource="http://www.semanticweb.org/sc3/ontologies/2022/0/Planning-Ontology#Yield"/>
        <rdfs:range rdf:resource="http://www.semanticweb.org/sc3/ontologies/2022/0/Planning-Ontology#Process"/>
    </owl:ObjectProperty>
    


    <!-- http://www.semanticweb.org/sc3/ontologies/2022/0/Planning-Ontology#hasProduct -->


    <owl:ObjectProperty rdf:about="http://www.semanticweb.org/sc3/ontologies/2022/0/Planning-Ontology#hasProduct">
        <rdfs:domain rdf:resource="http://www.semanticweb.org/sc3/ontologies/2022/0/Planning-Ontology#BillOfMaterial"/>
        <rdfs:domain rdf:resource="http://www.semanticweb.org/sc3/ontologies/2022/0/Planning-Ontology#Binning"/>
        <rdfs:domain rdf:resource="http://www.semanticweb.org/sc3/ontologies/2022/0/Planning-Ontology#Capacity"/>
        <rdfs:domain rdf:resource="http://www.semanticweb.org/sc3/ontologies/2022/0/Planning-Ontology#In-TransitInventory"/>
        <rdfs:domain rdf:resource="http://www.semanticweb.org/sc3/ontologies/2022/0/Planning-Ontology#Inventory"/>
        <rdfs:domain rdf:resource="http://www.semanticweb.org/sc3/ontologies/2022/0/Planning-Ontology#InventoryPolicy"/>
        <rdfs:domain rdf:resource="http://www.semanticweb.org/sc3/ontologies/2022/0/Planning-Ontology#LotSizingRule"/>
        <rdfs:domain rdf:resource="http://www.semanticweb.org/sc3/ontologies/2022/0/Planning-Ontology#Part"/>
        <rdfs:domain rdf:resource="http://www.semanticweb.org/sc3/ontologies/2022/0/Planning-Ontology#PlanningObject"/>
        <rdfs:domain rdf:resource="http://www.semanticweb.org/sc3/ontologies/2022/0/Planning-Ontology#Process"/>
        <rdfs:domain rdf:resource="http://www.semanticweb.org/sc3/ontologies/2022/0/Planning-Ontology#ProductAggregate"/>
        <rdfs:domain rdf:resource="http://www.semanticweb.org/sc3/ontologies/2022/0/Planning-Ontology#ProjectedWip"/>
        <rdfs:domain rdf:resource="http://www.semanticweb.org/sc3/ontologies/2022/0/Planning-Ontology#Substitution"/>
        <rdfs:domain rdf:resource="http://www.semanticweb.org/sc3/ontologies/2022/0/Planning-Ontology#SupplyInformation"/>
        <rdfs:domain rdf:resource="http://www.semanticweb.org/sc3/ontologies/2022/0/ozone-ontology#Demand"/>
        <rdfs:range rdf:resource="http://www.semanticweb.org/sc3/ontologies/2022/0/ozone-ontology#Product"/>
    </owl:ObjectProperty>
    


    <!-- http://www.semanticweb.org/sc3/ontologies/2022/0/Planning-Ontology#hasReceivingLocation -->


    <owl:ObjectProperty rdf:about="http://www.semanticweb.org/sc3/ontologies/2022/0/Planning-Ontology#hasReceivingLocation">
        <rdfs:domain rdf:resource="http://www.semanticweb.org/sc3/ontologies/2022/0/Planning-Ontology#In-TransitInventory"/>
        <rdfs:range rdf:resource="http://www.semanticweb.org/sc3/ontologies/2022/0/Planning-Ontology#Location"/>
    </owl:ObjectProperty>
    


    <!-- http://www.semanticweb.org/sc3/ontologies/2022/0/Planning-Ontology#hasReplanningDegree -->


    <owl:ObjectProperty rdf:about="http://www.semanticweb.org/sc3/ontologies/2022/0/Planning-Ontology#hasReplanningDegree">
        <rdfs:subPropertyOf rdf:resource="http://www.w3.org/2002/07/owl#topObjectProperty"/>
        <rdfs:domain rdf:resource="http://www.semanticweb.org/sc3/ontologies/2022/0/Planning-Ontology#PlanningProcess"/>
        <rdfs:range rdf:resource="http://www.semanticweb.org/sc3/ontologies/2022/0/Planning-Ontology#ReplanningDegree"/>
        <rdfs:comment>he degree distinguishes replanning from scratch and repair of existing plans (Vieria et al. 2003).</rdfs:comment>
    </owl:ObjectProperty>
    


    <!-- http://www.semanticweb.org/sc3/ontologies/2022/0/Planning-Ontology#hasResources -->


    <owl:ObjectProperty rdf:about="http://www.semanticweb.org/sc3/ontologies/2022/0/Planning-Ontology#hasResources">
        <rdfs:subPropertyOf rdf:resource="http://www.w3.org/2002/07/owl#topObjectProperty"/>
        <rdfs:domain rdf:resource="http://www.semanticweb.org/sc3/ontologies/2022/0/Planning-Ontology#Capacity"/>
        <rdfs:domain rdf:resource="http://www.semanticweb.org/sc3/ontologies/2022/0/ozone-ontology#Product"/>
        <rdfs:range rdf:resource="http://www.semanticweb.org/sc3/ontologies/2022/0/ozone-ontology#Resource"/>
        <rdfs:comment>the  set  of  resources  that  can be  utilized  to  execute  various  ACTIVITIES  of  the PRODUCT  plan.</rdfs:comment>
    </owl:ObjectProperty>
    


    <!-- http://www.semanticweb.org/sc3/ontologies/2022/0/Planning-Ontology#hasScope -->


    <owl:ObjectProperty rdf:about="http://www.semanticweb.org/sc3/ontologies/2022/0/Planning-Ontology#hasScope">
        <rdfs:subPropertyOf rdf:resource="http://www.w3.org/2002/07/owl#topObjectProperty"/>
        <rdfs:domain rdf:resource="http://www.semanticweb.org/sc3/ontologies/2022/0/Planning-Ontology#DecisionMakingUnit"/>
        <rdfs:range rdf:resource="http://www.semanticweb.org/sc3/ontologies/2022/0/Planning-Ontology#PlanningFunction"/>
        <rdfs:comment>This property defines which planning function is addressed by the DECISION-MAKING UNIT (planning scope). It also described to which part of the base system the DECISION-MAKING UNIT belongs (physical scope).</rdfs:comment>
    </owl:ObjectProperty>
    


    <!-- http://www.semanticweb.org/sc3/ontologies/2022/0/Planning-Ontology#hasSetOfPlanningObjects -->


    <owl:ObjectProperty rdf:about="http://www.semanticweb.org/sc3/ontologies/2022/0/Planning-Ontology#hasSetOfPlanningObjects">
        <rdfs:subPropertyOf rdf:resource="http://www.w3.org/2002/07/owl#topObjectProperty"/>
        <rdfs:domain rdf:resource="http://www.semanticweb.org/sc3/ontologies/2022/0/Planning-Ontology#Plan"/>
        <rdfs:range rdf:resource="http://www.semanticweb.org/sc3/ontologies/2022/0/Planning-Ontology#PlanningObject"/>
        <rdfs:comment>This property specifies a set of planning objects from a given planning instance where all attributes are supplied with values that are determined as the result of a planning decisions.</rdfs:comment>
    </owl:ObjectProperty>
    


    <!-- http://www.semanticweb.org/sc3/ontologies/2022/0/Planning-Ontology#hasSubProcesses -->


    <owl:ObjectProperty rdf:about="http://www.semanticweb.org/sc3/ontologies/2022/0/Planning-Ontology#hasSubProcesses">
        <rdfs:domain rdf:resource="http://www.semanticweb.org/sc3/ontologies/2022/0/Planning-Ontology#Process"/>
        <rdfs:range rdf:resource="http://www.semanticweb.org/sc3/ontologies/2022/0/Planning-Ontology#Process"/>
    </owl:ObjectProperty>
    


    <!-- http://www.semanticweb.org/sc3/ontologies/2022/0/Planning-Ontology#hasSubstitutes -->


    <owl:ObjectProperty rdf:about="http://www.semanticweb.org/sc3/ontologies/2022/0/Planning-Ontology#hasSubstitutes">
        <rdfs:domain rdf:resource="http://www.semanticweb.org/sc3/ontologies/2022/0/Planning-Ontology#Substitution"/>
        <rdfs:range rdf:resource="http://www.semanticweb.org/sc3/ontologies/2022/0/ozone-ontology#Product"/>
    </owl:ObjectProperty>
    


    <!-- http://www.semanticweb.org/sc3/ontologies/2022/0/Planning-Ontology#hasSuccessor -->


    <owl:ObjectProperty rdf:about="http://www.semanticweb.org/sc3/ontologies/2022/0/Planning-Ontology#hasSuccessor">
        <rdfs:domain rdf:resource="http://www.semanticweb.org/sc3/ontologies/2022/0/Planning-Ontology#Location"/>
        <rdfs:range rdf:resource="http://www.semanticweb.org/sc3/ontologies/2022/0/Planning-Ontology#Location"/>
    </owl:ObjectProperty>
    


    <!-- http://www.semanticweb.org/sc3/ontologies/2022/0/Planning-Ontology#hasSupplyingLocation -->


    <owl:ObjectProperty rdf:about="http://www.semanticweb.org/sc3/ontologies/2022/0/Planning-Ontology#hasSupplyingLocation">
        <rdfs:domain rdf:resource="http://www.semanticweb.org/sc3/ontologies/2022/0/Planning-Ontology#In-TransitInventory"/>
        <rdfs:range rdf:resource="http://www.semanticweb.org/sc3/ontologies/2022/0/Planning-Ontology#Location"/>
    </owl:ObjectProperty>
    


    <!-- http://www.semanticweb.org/sc3/ontologies/2022/0/Planning-Ontology#hasTargets -->


    <owl:ObjectProperty rdf:about="http://www.semanticweb.org/sc3/ontologies/2022/0/Planning-Ontology#hasTargets">
        <rdfs:subPropertyOf rdf:resource="http://www.w3.org/2002/07/owl#topObjectProperty"/>
        <rdfs:domain rdf:resource="http://www.semanticweb.org/sc3/ontologies/2022/0/Planning-Ontology#PlaningPurpose"/>
        <rdfs:range rdf:resource="http://www.semanticweb.org/sc3/ontologies/2022/0/Planning-Ontology#Target"/>
    </owl:ObjectProperty>
    


    <!-- http://www.semanticweb.org/sc3/ontologies/2022/0/Planning-Ontology#hasTrigger -->


    <owl:ObjectProperty rdf:about="http://www.semanticweb.org/sc3/ontologies/2022/0/Planning-Ontology#hasTrigger">
        <rdfs:domain rdf:resource="http://www.semanticweb.org/sc3/ontologies/2022/0/Planning-Ontology#PlanningProcess"/>
        <rdfs:range rdf:resource="http://www.semanticweb.org/sc3/ontologies/2022/0/Planning-Ontology#Trigger"/>
    </owl:ObjectProperty>
    


    <!-- http://www.semanticweb.org/sc3/ontologies/2022/0/Planning-Ontology#hasVertex -->


    <owl:ObjectProperty rdf:about="http://www.semanticweb.org/sc3/ontologies/2022/0/Planning-Ontology#hasVertex">
        <rdfs:domain rdf:resource="http://www.semanticweb.org/sc3/ontologies/2022/0/Planning-Ontology#PlanningSituation"/>
        <rdfs:range rdf:resource="http://www.semanticweb.org/sc3/ontologies/2022/0/Planning-Ontology#Vertex"/>
    </owl:ObjectProperty>
    


    <!-- http://www.semanticweb.org/sc3/ontologies/2022/0/Planning-Ontology#hasYield -->


    <owl:ObjectProperty rdf:about="http://www.semanticweb.org/sc3/ontologies/2022/0/Planning-Ontology#hasYield">
        <rdfs:domain rdf:resource="http://www.semanticweb.org/sc3/ontologies/2022/0/Planning-Ontology#Process"/>
        <rdfs:range rdf:resource="http://www.semanticweb.org/sc3/ontologies/2022/0/Planning-Ontology#Yield"/>
    </owl:ObjectProperty>
    


    <!-- http://www.semanticweb.org/sc3/ontologies/2022/0/Planning-Ontology#usesPlanningApproach -->


    <owl:ObjectProperty rdf:about="http://www.semanticweb.org/sc3/ontologies/2022/0/Planning-Ontology#usesPlanningApproach">
        <rdfs:subPropertyOf rdf:resource="http://www.w3.org/2002/07/owl#topObjectProperty"/>
        <rdfs:domain rdf:resource="http://www.semanticweb.org/sc3/ontologies/2022/0/Planning-Ontology#PlanningProcess"/>
        <rdfs:range rdf:resource="http://www.semanticweb.org/sc3/ontologies/2022/0/Planning-Ontology#PlanningApproach"/>
        <rdfs:comment>This property defines which algorithm is used to make the required decisions.</rdfs:comment>
    </owl:ObjectProperty>
    


    <!-- http://www.w3.org/2002/07/owl#topObjectProperty -->


    <rdf:Description rdf:about="http://www.w3.org/2002/07/owl#topObjectProperty">
        <rdfs:range rdf:resource="http://www.w3.org/2006/time#TemporalEntity"/>
    </rdf:Description>
    


    <!-- http://www.w3.org/2006/time#after -->


    <owl:ObjectProperty rdf:about="http://www.w3.org/2006/time#after">
        <rdfs:domain rdf:resource="http://www.w3.org/2006/time#TemporalEntity"/>
        <rdfs:range rdf:resource="http://www.w3.org/2006/time#TemporalEntity"/>
        <rdfs:comment xml:lang="es">Asume una dirección en el tiempo. Si una entidad temporal T1 está después de otra entidad temporal T2, entonces el principio de T1 está después del final de T2.</rdfs:comment>
        <rdfs:comment xml:lang="en">Gives directionality to time. If a temporal entity T1 is after another temporal entity T2, then the beginning of T1 is after the end of T2.</rdfs:comment>
        <rdfs:label xml:lang="en">after</rdfs:label>
        <rdfs:label xml:lang="es">después</rdfs:label>
        <skos:definition xml:lang="es">Asume una dirección en el tiempo. Si una entidad temporal T1 está después de otra entidad temporal T2, entonces el principio de T1 está después del final de T2.</skos:definition>
        <skos:definition xml:lang="en">Gives directionality to time. If a temporal entity T1 is after another temporal entity T2, then the beginning of T1 is after the end of T2.</skos:definition>
    </owl:ObjectProperty>
    


    <!-- http://www.w3.org/2006/time#before -->


    <owl:ObjectProperty rdf:about="http://www.w3.org/2006/time#before">
        <owl:inverseOf rdf:resource="http://www.w3.org/2006/time#after"/>
        <rdf:type rdf:resource="http://www.w3.org/2002/07/owl#TransitiveProperty"/>
        <rdfs:domain rdf:resource="http://www.w3.org/2006/time#TemporalEntity"/>
        <rdfs:range rdf:resource="http://www.w3.org/2006/time#TemporalEntity"/>
        <rdfs:comment xml:lang="es">Asume una dirección en el tiempo. Si una entidad temporal T1 está antes que otra entidad temporal T2, entonces el final de T1 está antes que el principio de T2. Así, &quot;antes&quot; se puede considerar básica para instantes y derivada para intervalos.</rdfs:comment>
        <rdfs:comment xml:lang="en">Gives directionality to time. If a temporal entity T1 is before another temporal entity T2, then the end of T1 is before the beginning of T2. Thus, &quot;before&quot; can be considered to be basic to instants and derived for intervals.</rdfs:comment>
        <rdfs:label xml:lang="es">antes</rdfs:label>
        <rdfs:label xml:lang="en">before</rdfs:label>
        <skos:definition xml:lang="es">Asume una dirección en el tiempo. Si una entidad temporal T1 está antes que otra entidad temporal T2, entonces el final de T1 está antes que el principio de T2. Así, &quot;antes&quot; se puede considerar básica para instantes y derivada para intervalos.</skos:definition>
        <skos:definition xml:lang="en">Gives directionality to time. If a temporal entity T1 is before another temporal entity T2, then the end of T1 is before the beginning of T2. Thus, &quot;before&quot; can be considered to be basic to instants and derived for intervals.</skos:definition>
    </owl:ObjectProperty>
    


    <!-- http://www.w3.org/2006/time#dayOfWeek -->


    <owl:ObjectProperty rdf:about="http://www.w3.org/2006/time#dayOfWeek">
        <rdfs:domain rdf:resource="http://www.w3.org/2006/time#GeneralDateTimeDescription"/>
        <rdfs:range rdf:resource="http://www.w3.org/2006/time#DayOfWeek"/>
        <rdfs:comment xml:lang="en">The day of week, whose value is a member of the class time:DayOfWeek</rdfs:comment>
        <rdfs:comment>El día de la semana, cuyo valor es un miembro de la clase &apos;día de la semana&apos;.</rdfs:comment>
        <rdfs:label xml:lang="en">day of week</rdfs:label>
        <rdfs:label xml:lang="es">día de la semana</rdfs:label>
        <skos:definition xml:lang="es">El día de la semana, cuyo valor es un miembro de la clase &apos;día de la semana&apos;.</skos:definition>
        <skos:definition xml:lang="en">The day of week, whose value is a member of the class time:DayOfWeek</skos:definition>
    </owl:ObjectProperty>
    


    <!-- http://www.w3.org/2006/time#hasBeginning -->


    <owl:ObjectProperty rdf:about="http://www.w3.org/2006/time#hasBeginning">
        <rdfs:subPropertyOf rdf:resource="http://www.w3.org/2006/time#hasTime"/>
        <rdfs:domain rdf:resource="http://www.w3.org/2006/time#TemporalEntity"/>
        <rdfs:range rdf:resource="http://www.w3.org/2006/time#Instant"/>
        <rdfs:comment xml:lang="en">Beginning of a temporal entity</rdfs:comment>
        <rdfs:comment xml:lang="es">Comienzo de una entidad temporal.</rdfs:comment>
        <rdfs:label xml:lang="en">has beginning</rdfs:label>
        <rdfs:label xml:lang="es">tiene principio</rdfs:label>
        <skos:definition xml:lang="en">Beginning of a temporal entity.</skos:definition>
        <skos:definition xml:lang="es">Comienzo de una entidad temporal.</skos:definition>
    </owl:ObjectProperty>
    


    <!-- http://www.w3.org/2006/time#hasDateTimeDescription -->


    <owl:ObjectProperty rdf:about="http://www.w3.org/2006/time#hasDateTimeDescription">
        <rdfs:domain rdf:resource="http://www.w3.org/2006/time#DateTimeInterval"/>
        <rdfs:range rdf:resource="http://www.w3.org/2006/time#GeneralDateTimeDescription"/>
        <rdfs:comment xml:lang="es">Valor de intervalo de fecha-hora expresado como un valor estructurado. El principio y el final del intervalo coincide con los límites del elemento más corto en la descripción.</rdfs:comment>
        <rdfs:comment xml:lang="en">Value of DateTimeInterval expressed as a structured value. The beginning and end of the interval coincide with the limits of the shortest element in the description.</rdfs:comment>
        <rdfs:label xml:lang="en">has Date-Time description</rdfs:label>
        <rdfs:label xml:lang="es">tiene descripción fecha-hora</rdfs:label>
        <skos:definition xml:lang="es">Valor de intervalo de fecha-hora expresado como un valor estructurado. El principio y el final del intervalo coincide con los límites del elemento más corto en la descripción.</skos:definition>
        <skos:definition xml:lang="en">Value of DateTimeInterval expressed as a structured value. The beginning and end of the interval coincide with the limits of the shortest element in the description.</skos:definition>
    </owl:ObjectProperty>
    


    <!-- http://www.w3.org/2006/time#hasDuration -->


    <owl:ObjectProperty rdf:about="http://www.w3.org/2006/time#hasDuration">
        <rdfs:subPropertyOf rdf:resource="http://www.w3.org/2006/time#hasTemporalDuration"/>
        <rdfs:range rdf:resource="http://www.w3.org/2006/time#Duration"/>
        <rdfs:comment xml:lang="es">Duración de una entidad temporal, expresada como un valor escalado o un valor nominal.</rdfs:comment>
        <rdfs:comment xml:lang="en">Duration of a temporal entity, expressed as a scaled value or nominal value</rdfs:comment>
        <rdfs:label xml:lang="en">has duration</rdfs:label>
        <rdfs:label xml:lang="es">tiene duración</rdfs:label>
        <skos:definition xml:lang="es">Duración de una entidad temporal, evento o actividad, o cosa, expresada como un valor escalado.</skos:definition>
        <skos:definition xml:lang="en">Duration of a temporal entity, event or activity, or thing, expressed as a scaled value</skos:definition>
    </owl:ObjectProperty>
    


    <!-- http://www.w3.org/2006/time#hasDurationDescription -->


    <owl:ObjectProperty rdf:about="http://www.w3.org/2006/time#hasDurationDescription">
        <rdfs:subPropertyOf rdf:resource="http://www.w3.org/2006/time#hasTemporalDuration"/>
        <rdfs:range rdf:resource="http://www.w3.org/2006/time#GeneralDurationDescription"/>
        <rdfs:comment xml:lang="es">Duración de una entidad temporal, expresada utilizando una descripción estructurada.</rdfs:comment>
        <rdfs:comment xml:lang="en">Duration of a temporal entity, expressed using a structured description</rdfs:comment>
        <rdfs:label xml:lang="en">has duration description</rdfs:label>
        <rdfs:label xml:lang="es">tiene descripción de duración</rdfs:label>
        <skos:definition xml:lang="es">Duración de una entidad temporal, expresada utilizando una descripción estructurada.</skos:definition>
        <skos:definition xml:lang="en">Duration of a temporal entity, expressed using a structured description</skos:definition>
    </owl:ObjectProperty>
    


    <!-- http://www.w3.org/2006/time#hasEnd -->


    <owl:ObjectProperty rdf:about="http://www.w3.org/2006/time#hasEnd">
        <rdfs:subPropertyOf rdf:resource="http://www.w3.org/2006/time#hasTime"/>
        <rdfs:domain rdf:resource="http://www.w3.org/2006/time#TemporalEntity"/>
        <rdfs:range rdf:resource="http://www.w3.org/2006/time#Instant"/>
        <rdfs:comment xml:lang="en">End of a temporal entity.</rdfs:comment>
        <rdfs:comment xml:lang="es">Final de una entidad temporal.</rdfs:comment>
        <rdfs:label xml:lang="en">has end</rdfs:label>
        <rdfs:label xml:lang="es">tiene fin</rdfs:label>
        <skos:definition xml:lang="en">End of a temporal entity.</skos:definition>
        <skos:definition xml:lang="es">Final de una entidad temporal.</skos:definition>
    </owl:ObjectProperty>
    


    <!-- http://www.w3.org/2006/time#hasTRS -->


    <owl:ObjectProperty rdf:about="http://www.w3.org/2006/time#hasTRS">
        <rdf:type rdf:resource="http://www.w3.org/2002/07/owl#FunctionalProperty"/>
        <rdfs:domain>
            <owl:Class>
                <owl:unionOf rdf:parseType="Collection">
                    <rdf:Description rdf:about="http://www.w3.org/2006/time#GeneralDurationDescription"/>
                    <rdf:Description rdf:about="http://www.w3.org/2006/time#TemporalPosition"/>
                </owl:unionOf>
            </owl:Class>
        </rdfs:domain>
        <rdfs:range rdf:resource="http://www.w3.org/2006/time#TRS"/>
        <rdfs:comment xml:lang="es">El sistema de referencia temporal utilizado por una posición temporal o descripción de extensión.</rdfs:comment>
        <rdfs:comment xml:lang="en">The temporal reference system used by a temporal position or extent description. </rdfs:comment>
        <rdfs:label xml:lang="en">Temporal reference system used</rdfs:label>
        <rdfs:label xml:lang="es">sistema de referencia temporal utilizado</rdfs:label>
        <skos:definition xml:lang="es">El sistema de referencia temporal utilizado por una posición temporal o descripción de extensión.</skos:definition>
        <skos:definition xml:lang="en">The temporal reference system used by a temporal position or extent description. </skos:definition>
    </owl:ObjectProperty>
    


    <!-- http://www.w3.org/2006/time#hasTemporalDuration -->


    <owl:ObjectProperty rdf:about="http://www.w3.org/2006/time#hasTemporalDuration">
        <rdfs:domain rdf:resource="http://www.w3.org/2006/time#TemporalEntity"/>
        <rdfs:range rdf:resource="http://www.w3.org/2006/time#TemporalDuration"/>
        <rdfs:comment xml:lang="es">Duración de una entidad temporal.</rdfs:comment>
        <rdfs:comment xml:lang="en">Duration of a temporal entity.</rdfs:comment>
        <rdfs:label xml:lang="en">has temporal duration</rdfs:label>
        <rdfs:label xml:lang="es">tiene duración temporal</rdfs:label>
        <skos:definition xml:lang="es">Duración de una entidad temporal.</skos:definition>
        <skos:definition xml:lang="en">Duration of a temporal entity.</skos:definition>
    </owl:ObjectProperty>
    


    <!-- http://www.w3.org/2006/time#hasTime -->


    <owl:ObjectProperty rdf:about="http://www.w3.org/2006/time#hasTime">
        <rdfs:range rdf:resource="http://www.w3.org/2006/time#TemporalEntity"/>
        <rdfs:comment xml:lang="es">Proporciona soporte a la asociación de una entidad temporal (instante o intervalo) a cualquier cosa.</rdfs:comment>
        <rdfs:comment xml:lang="en">Supports the association of a temporal entity (instant or interval) to any thing</rdfs:comment>
        <rdfs:label xml:lang="en">has time</rdfs:label>
        <rdfs:label xml:lang="es">tiene tiempo</rdfs:label>
        <skos:definition xml:lang="es">Proporciona soporte a la asociación de una entidad temporal (instante o intervalo) a cualquier cosa.</skos:definition>
        <skos:definition xml:lang="en">Supports the association of a temporal entity (instant or interval) to any thing</skos:definition>
        <skos:editorialNote xml:lang="es">Característica arriesgada -añadida en la revisión del 2017 que no ha sido todavía utilizada de forma amplia.</skos:editorialNote>
        <skos:editorialNote xml:lang="en">Feature at risk - added in 2017 revision, and not yet widely used. </skos:editorialNote>
    </owl:ObjectProperty>
    


    <!-- http://www.w3.org/2006/time#inDateTime -->


    <owl:ObjectProperty rdf:about="http://www.w3.org/2006/time#inDateTime">
        <rdfs:subPropertyOf rdf:resource="http://www.w3.org/2006/time#inTemporalPosition"/>
        <rdfs:domain rdf:resource="http://www.w3.org/2006/time#Instant"/>
        <rdfs:range rdf:resource="http://www.w3.org/2006/time#GeneralDateTimeDescription"/>
        <rdfs:comment xml:lang="es">Posición de un instante, expresada utilizando una descripción estructurada.</rdfs:comment>
        <rdfs:comment xml:lang="en">Position of an instant, expressed using a structured description</rdfs:comment>
        <rdfs:label xml:lang="es">en descripción de fecha-hora</rdfs:label>
        <rdfs:label xml:lang="en">in date-time description</rdfs:label>
        <skos:definition xml:lang="es">Posición de un instante, expresada utilizando una descripción estructurada.</skos:definition>
        <skos:definition xml:lang="en">Position of an instant, expressed using a structured description</skos:definition>
    </owl:ObjectProperty>
    


    <!-- http://www.w3.org/2006/time#inTemporalPosition -->


    <owl:ObjectProperty rdf:about="http://www.w3.org/2006/time#inTemporalPosition">
        <rdfs:domain rdf:resource="http://www.w3.org/2006/time#Instant"/>
        <rdfs:range rdf:resource="http://www.w3.org/2006/time#TemporalPosition"/>
        <rdfs:comment xml:lang="es">Posición de un instante de tiempo.</rdfs:comment>
        <rdfs:comment xml:lang="en">Position of a time instant</rdfs:comment>
        <rdfs:label xml:lang="en">Temporal position</rdfs:label>
        <rdfs:label xml:lang="es">posición temporal</rdfs:label>
        <skos:definition xml:lang="es">Posición de un instante de tiempo.</skos:definition>
        <skos:definition xml:lang="en">Position of a time instant</skos:definition>
    </owl:ObjectProperty>
    


    <!-- http://www.w3.org/2006/time#inTimePosition -->


    <owl:ObjectProperty rdf:about="http://www.w3.org/2006/time#inTimePosition">
        <rdfs:subPropertyOf rdf:resource="http://www.w3.org/2006/time#inTemporalPosition"/>
        <rdfs:domain rdf:resource="http://www.w3.org/2006/time#Instant"/>
        <rdfs:range rdf:resource="http://www.w3.org/2006/time#TimePosition"/>
        <rdfs:comment xml:lang="es">Posición de un instante, expresada como una coordenada temporal o un valor nominal.</rdfs:comment>
        <rdfs:comment xml:lang="en">Position of an instant, expressed as a temporal coordinate or nominal value</rdfs:comment>
        <rdfs:label xml:lang="en">Time position</rdfs:label>
        <rdfs:label xml:lang="es">posición de tiempo</rdfs:label>
        <skos:definition xml:lang="es">Posición de un instante, expresada como una coordenada temporal o un valor nominal.</skos:definition>
        <skos:definition xml:lang="en">Position of a time instant expressed as a TimePosition</skos:definition>
    </owl:ObjectProperty>
    


    <!-- http://www.w3.org/2006/time#inside -->


    <owl:ObjectProperty rdf:about="http://www.w3.org/2006/time#inside">
        <rdfs:domain rdf:resource="http://www.w3.org/2006/time#Interval"/>
        <rdfs:range rdf:resource="http://www.w3.org/2006/time#Instant"/>
        <rdfs:comment xml:lang="en">An instant that falls inside the interval. It is not intended to include beginnings and ends of intervals.</rdfs:comment>
        <rdfs:comment xml:lang="es">Un instante que cae dentro del intervalo. Se asume que no es ni el principio ni el final de ningún intervalo.</rdfs:comment>
        <rdfs:label xml:lang="en">has time instant inside</rdfs:label>
        <rdfs:label xml:lang="es">tiene instante de tiempo dentro</rdfs:label>
        <skos:definition xml:lang="en">An instant that falls inside the interval. It is not intended to include beginnings and ends of intervals.</skos:definition>
        <skos:definition xml:lang="es">Un instante que cae dentro del intervalo. Se asume que no es ni el principio ni el final de ningún intervalo.</skos:definition>
    </owl:ObjectProperty>
    


    <!-- http://www.w3.org/2006/time#intervalAfter -->


    <owl:ObjectProperty rdf:about="http://www.w3.org/2006/time#intervalAfter">
        <rdfs:subPropertyOf rdf:resource="http://www.w3.org/2006/time#after"/>
        <rdfs:subPropertyOf rdf:resource="http://www.w3.org/2006/time#intervalDisjoint"/>
        <owl:inverseOf rdf:resource="http://www.w3.org/2006/time#intervalBefore"/>
        <rdfs:domain rdf:resource="http://www.w3.org/2006/time#ProperInterval"/>
        <rdfs:range rdf:resource="http://www.w3.org/2006/time#ProperInterval"/>
        <rdfs:comment xml:lang="en">If a proper interval T1 is intervalAfter another proper interval T2, then the beginning of T1 is after the end of T2.</rdfs:comment>
        <rdfs:comment>Si un intervalo propio T1 es posterior a otro intervalo propio T2, entonces el principio de T1 está después que el final de T2.</rdfs:comment>
        <rdfs:label xml:lang="en">interval after</rdfs:label>
        <rdfs:label xml:lang="es">intervalo posterior</rdfs:label>
        <skos:definition xml:lang="en">If a proper interval T1 is intervalAfter another proper interval T2, then the beginning of T1 is after the end of T2.</skos:definition>
        <skos:definition xml:lang="es">Si un intervalo propio T1 es posterior a otro intervalo propio T2, entonces el principio de T1 está después que el final de T2.</skos:definition>
    </owl:ObjectProperty>
    


    <!-- http://www.w3.org/2006/time#intervalBefore -->


    <owl:ObjectProperty rdf:about="http://www.w3.org/2006/time#intervalBefore">
        <rdfs:subPropertyOf rdf:resource="http://www.w3.org/2006/time#before"/>
        <rdfs:subPropertyOf rdf:resource="http://www.w3.org/2006/time#intervalDisjoint"/>
        <rdfs:domain rdf:resource="http://www.w3.org/2006/time#ProperInterval"/>
        <rdfs:range rdf:resource="http://www.w3.org/2006/time#ProperInterval"/>
        <rdfs:comment xml:lang="en">If a proper interval T1 is intervalBefore another proper interval T2, then the end of T1 is before the beginning of T2.</rdfs:comment>
        <rdfs:comment xml:lang="es">Si un intervalo propio T1 está antes que otro intervalo propio T2, entonces el final de T1 está antes que el principio de T2.</rdfs:comment>
        <rdfs:label xml:lang="en">interval before</rdfs:label>
        <rdfs:label xml:lang="es">intervalo anterior</rdfs:label>
        <skos:definition xml:lang="en">If a proper interval T1 is intervalBefore another proper interval T2, then the end of T1 is before the beginning of T2.</skos:definition>
        <skos:definition xml:lang="es">Si un intervalo propio T1 está antes que otro intervalo propio T2, entonces el final de T1 está antes que el principio de T2.</skos:definition>
    </owl:ObjectProperty>
    


    <!-- http://www.w3.org/2006/time#intervalContains -->


    <owl:ObjectProperty rdf:about="http://www.w3.org/2006/time#intervalContains">
        <rdfs:domain rdf:resource="http://www.w3.org/2006/time#ProperInterval"/>
        <rdfs:range rdf:resource="http://www.w3.org/2006/time#ProperInterval"/>
        <rdfs:comment xml:lang="en">If a proper interval T1 is intervalContains another proper interval T2, then the beginning of T1 is before the beginning of T2, and the end of T1 is after the end of T2.</rdfs:comment>
        <rdfs:comment xml:lang="es">Si un intervalo propio T1 contiene otro intervalo propio T2, entonces el principio de T1 está antes que el principio de T2, y el final de T1 está después del final de T2.</rdfs:comment>
        <rdfs:label xml:lang="en">interval contains</rdfs:label>
        <rdfs:label xml:lang="es">intervalo contiene</rdfs:label>
        <skos:definition xml:lang="en">If a proper interval T1 is intervalContains another proper interval T2, then the beginning of T1 is before the beginning of T2, and the end of T1 is after the end of T2.</skos:definition>
        <skos:definition xml:lang="es">Si un intervalo propio T1 contiene otro intervalo propio T2, entonces el principio de T1 está antes que el principio de T2, y el final de T1 está después del final de T2.</skos:definition>
    </owl:ObjectProperty>
    


    <!-- http://www.w3.org/2006/time#intervalDisjoint -->


    <owl:ObjectProperty rdf:about="http://www.w3.org/2006/time#intervalDisjoint">
        <rdfs:domain rdf:resource="http://www.w3.org/2006/time#ProperInterval"/>
        <rdfs:range rdf:resource="http://www.w3.org/2006/time#ProperInterval"/>
        <rdfs:comment xml:lang="en">If a proper interval T1 is intervalDisjoint another proper interval T2, then the beginning of T1 is after the end of T2, or the end of T1 is before the beginning of T2, i.e. the intervals do not overlap in any way, but their ordering relationship is not known.</rdfs:comment>
        <rdfs:comment xml:lang="es">Si un intervalo propio T1 es disjunto con otro intervalo propio T2, entonces el principio de T1 está después del final de T2, o el final de T1 está antes que el principio de T2, es decir, los intervalos no se solapan de ninguna forma, aunque su relación de orden no se conozca.</rdfs:comment>
        <rdfs:label xml:lang="en">interval disjoint</rdfs:label>
        <rdfs:label xml:lang="es">intervalo disjunto</rdfs:label>
        <skos:definition xml:lang="en">If a proper interval T1 is intervalDisjoint another proper interval T2, then the beginning of T1 is after the end of T2, or the end of T1 is before the beginning of T2, i.e. the intervals do not overlap in any way, but their ordering relationship is not known.</skos:definition>
        <skos:definition xml:lang="es">Si un intervalo propio T1 es disjunto con otro intervalo propio T2, entonces el principio de T1 está después del final de T2, o el final de T1 está antes que el principio de T2, es decir, los intervalos no se solapan de ninguna forma, aunque su relación de orden no se conozca.</skos:definition>
        <skos:note xml:lang="es">Esta relación entre intervalos no estaba incluida en las 13 relaciones básicas definidas por Allen (1984), pero está definida en T.3 como la unión de &apos;intervalo anterior&apos; con &apos;intervalo posterior&apos;. Sin embargo, esto está fuera de la expresividad de OWL2, por tanto, está implementado como una propiedad explícita, con &apos;intervalo anterior&apos; e &apos;intervalo posterior&apos; como sub-propiedades.</skos:note>
        <skos:note xml:lang="en">This interval relation is not included in the 13 basic relationships defined in Allen (1984), but is defined in (T.3) as the union of :intervalBefore v :intervalAfter . However, that is outside OWL2 expressivity, so is implemented as an explicit property, with :intervalBefore , :intervalAfter as sub-properties</skos:note>
    </owl:ObjectProperty>
    


    <!-- http://www.w3.org/2006/time#intervalDuring -->


    <owl:ObjectProperty rdf:about="http://www.w3.org/2006/time#intervalDuring">
        <rdfs:subPropertyOf rdf:resource="http://www.w3.org/2006/time#intervalIn"/>
        <owl:inverseOf rdf:resource="http://www.w3.org/2006/time#intervalContains"/>
        <rdfs:domain rdf:resource="http://www.w3.org/2006/time#ProperInterval"/>
        <rdfs:range rdf:resource="http://www.w3.org/2006/time#ProperInterval"/>
        <rdfs:comment xml:lang="en">If a proper interval T1 is intervalDuring another proper interval T2, then the beginning of T1 is after the beginning of T2, and the end of T1 is before the end of T2.</rdfs:comment>
        <rdfs:comment xml:lang="es">Si un intervalo propio T1 está durante otro intervalo propio T2, entonces del principio de T1 está después del principio de T2, y el final de T1 está antes que el final de T2.</rdfs:comment>
        <rdfs:label xml:lang="en">interval during</rdfs:label>
        <rdfs:label xml:lang="es">intervalo durante</rdfs:label>
        <skos:definition xml:lang="en">If a proper interval T1 is intervalDuring another proper interval T2, then the beginning of T1 is after the beginning of T2, and the end of T1 is before the end of T2.</skos:definition>
        <skos:definition xml:lang="es">Si un intervalo propio T1 está durante otro intervalo propio T2, entonces del principio de T1 está después del principio de T2, y el final de T1 está antes que el final de T2.</skos:definition>
    </owl:ObjectProperty>
    


    <!-- http://www.w3.org/2006/time#intervalEquals -->


    <owl:ObjectProperty rdf:about="http://www.w3.org/2006/time#intervalEquals">
        <rdfs:domain rdf:resource="http://www.w3.org/2006/time#ProperInterval"/>
        <rdfs:range rdf:resource="http://www.w3.org/2006/time#ProperInterval"/>
        <owl:propertyDisjointWith rdf:resource="http://www.w3.org/2006/time#intervalIn"/>
        <rdfs:comment xml:lang="en">If a proper interval T1 is intervalEquals another proper interval T2, then the beginning of T1 is coincident with the beginning of T2, and the end of T1 is coincident with the end of T2.</rdfs:comment>
        <rdfs:comment xml:lang="es">Si un intervalo propio T1 es igual a otro intervalo propio T2, entonces el principio de T1 coincide con el principio de T2, y el final de T1 coincide con el final de T2.</rdfs:comment>
        <rdfs:label xml:lang="en">interval equals</rdfs:label>
        <rdfs:label xml:lang="es">intervalo igual</rdfs:label>
        <skos:definition xml:lang="en">If a proper interval T1 is intervalEquals another proper interval T2, then the beginning of T1 is coincident with the beginning of T2, and the end of T1 is coincident with the end of T2.</skos:definition>
        <skos:definition xml:lang="es">Si un intervalo propio T1 es igual a otro intervalo propio T2, entonces el principio de T1 coincide con el principio de T2, y el final de T1 coincide con el final de T2.</skos:definition>
    </owl:ObjectProperty>
    


    <!-- http://www.w3.org/2006/time#intervalFinishedBy -->


    <owl:ObjectProperty rdf:about="http://www.w3.org/2006/time#intervalFinishedBy">
        <owl:inverseOf rdf:resource="http://www.w3.org/2006/time#intervalFinishes"/>
        <rdfs:domain rdf:resource="http://www.w3.org/2006/time#ProperInterval"/>
        <rdfs:range rdf:resource="http://www.w3.org/2006/time#ProperInterval"/>
        <rdfs:comment xml:lang="en">If a proper interval T1 is intervalFinishedBy another proper interval T2, then the beginning of T1 is before the beginning of T2, and the end of T1 is coincident with the end of T2.</rdfs:comment>
        <rdfs:comment xml:lang="es">Si un intervalo propio T1 está terminado por otro intervalo propio T2, entonces el principio de T1 está antes que el principio de T2, y el final de T1 coincide con el final de T2.</rdfs:comment>
        <rdfs:label xml:lang="en">interval finished by</rdfs:label>
        <rdfs:label xml:lang="es">intervalo terminado por</rdfs:label>
        <skos:definition xml:lang="en">If a proper interval T1 is intervalFinishedBy another proper interval T2, then the beginning of T1 is before the beginning of T2, and the end of T1 is coincident with the end of T2.</skos:definition>
        <skos:definition xml:lang="es">Si un intervalo propio T1 está terminado por otro intervalo propio T2, entonces el principio de T1 está antes que el principio de T2, y el final de T1 coincide con el final de T2.</skos:definition>
    </owl:ObjectProperty>
    


    <!-- http://www.w3.org/2006/time#intervalFinishes -->


    <owl:ObjectProperty rdf:about="http://www.w3.org/2006/time#intervalFinishes">
        <rdfs:subPropertyOf rdf:resource="http://www.w3.org/2006/time#intervalIn"/>
        <rdfs:domain rdf:resource="http://www.w3.org/2006/time#ProperInterval"/>
        <rdfs:range rdf:resource="http://www.w3.org/2006/time#ProperInterval"/>
        <rdfs:comment xml:lang="en">If a proper interval T1 is intervalFinishes another proper interval T2, then the beginning of T1 is after the beginning of T2, and the end of T1 is coincident with the end of T2.</rdfs:comment>
        <rdfs:comment xml:lang="es">Si un intervalo propio T1 termina otro intervalo propio T2, entonces del principio de T1 está después del principio de T2, y el final de T1 coincide con el final de T2.</rdfs:comment>
        <rdfs:label xml:lang="en">interval finishes</rdfs:label>
        <rdfs:label xml:lang="es">intervalo termina</rdfs:label>
        <skos:definition xml:lang="en">If a proper interval T1 is intervalFinishes another proper interval T2, then the beginning of T1 is after the beginning of T2, and the end of T1 is coincident with the end of T2.</skos:definition>
        <skos:definition xml:lang="es">Si un intervalo propio T1 termina otro intervalo propio T2, entonces del principio de T1 está después del principio de T2, y el final de T1 coincide con el final de T2.</skos:definition>
    </owl:ObjectProperty>
    


    <!-- http://www.w3.org/2006/time#intervalIn -->


    <owl:ObjectProperty rdf:about="http://www.w3.org/2006/time#intervalIn">
        <rdfs:domain rdf:resource="http://www.w3.org/2006/time#ProperInterval"/>
        <rdfs:range rdf:resource="http://www.w3.org/2006/time#ProperInterval"/>
        <rdfs:comment xml:lang="en">If a proper interval T1 is intervalIn another proper interval T2, then the beginning of T1 is after the beginning of T2 or is coincident with the beginning of T2, and the end of T1 is before the end of T2, or is coincident with the end of T2, except that end of T1 may not be coincident with the end of T2 if the beginning of T1 is coincident with the beginning of T2.</rdfs:comment>
        <rdfs:comment xml:lang="es">Si un intervalo propio T1 es un intervalo interior a otro intervalo propio T2, entonces el principio de T1 está después del principio de T2 o coincide con el principio de T2, y el final de T1 está antes que el final de T2, o coincide con el final de T2, excepto que el final de T1 puede no coincidir con el final de T2 si el principio de T1 coincide con el principio de T2.</rdfs:comment>
        <rdfs:label xml:lang="en">interval in</rdfs:label>
        <rdfs:label xml:lang="es">intervalo interior</rdfs:label>
        <skos:definition xml:lang="en">If a proper interval T1 is intervalIn another proper interval T2, then the beginning of T1 is after the beginning of T2 or is coincident with the beginning of T2, and the end of T1 is before the end of T2, or is coincident with the end of T2, except that end of T1 may not be coincident with the end of T2 if the beginning of T1 is coincident with the beginning of T2.</skos:definition>
        <skos:definition xml:lang="es">Si un intervalo propio T1 es un intervalo interior a otro intervalo propio T2, entonces el principio de T1 está después del principio de T2 o coincide con el principio de T2, y el final de T1 está antes que el final de T2, o coincide con el final de T2, excepto que el final de T1 puede no coincidir con el final de T2 si el principio de T1 coincide con el principio de T2.</skos:definition>
        <skos:note xml:lang="es">Esta relación entre intervalos no estaba incluida en las 13 relaciones básicas definidas por Allen (1984), pero se hace referencia a ella como &quot;una relación importante&quot; en Allen y Ferguson (1997). Es la unión disjunta de &apos;intervalo empieza&apos;, &apos;intervalo durante&apos; y con &apos;intervalo termina&apos;. Sin embargo, esto está fuera de la expresividad de OWL2, por tanto, se implementa como una propiedad explícita, con &apos;intervalo empieza&apos;, &apos;intervalo durante&apos; e &apos;intervalo termina&apos; como sub-propiedades.</skos:note>
        <skos:note xml:lang="en">This interval relation is not included in the 13 basic relationships defined in Allen (1984), but is referred to as &apos;an important relationship&apos; in Allen and Ferguson (1997). It is the disjoint union of :intervalStarts v :intervalDuring v :intervalFinishes . However, that is outside OWL2 expressivity, so is implemented as an explicit property, with :intervalStarts , :intervalDuring , :intervalFinishes as sub-properties</skos:note>
    </owl:ObjectProperty>
    


    <!-- http://www.w3.org/2006/time#intervalMeets -->


    <owl:ObjectProperty rdf:about="http://www.w3.org/2006/time#intervalMeets">
        <rdfs:domain rdf:resource="http://www.w3.org/2006/time#ProperInterval"/>
        <rdfs:range rdf:resource="http://www.w3.org/2006/time#ProperInterval"/>
        <rdfs:comment xml:lang="en">If a proper interval T1 is intervalMeets another proper interval T2, then the end of T1 is coincident with the beginning of T2.</rdfs:comment>
        <rdfs:comment xml:lang="es">Si un intervalo propio T1 se encuentra con otro intervalo propio T2, entonces el final de T1 coincide con el principio de T2.</rdfs:comment>
        <rdfs:label xml:lang="en">interval meets</rdfs:label>
        <rdfs:label xml:lang="es">intervalo se encuentra</rdfs:label>
        <skos:definition xml:lang="en">If a proper interval T1 is intervalMeets another proper interval T2, then the end of T1 is coincident with the beginning of T2.</skos:definition>
        <skos:definition xml:lang="es">Si un intervalo propio T1 se encuentra con otro intervalo propio T2, entonces el final de T1 coincide con el principio de T2.</skos:definition>
    </owl:ObjectProperty>
    


    <!-- http://www.w3.org/2006/time#intervalMetBy -->


    <owl:ObjectProperty rdf:about="http://www.w3.org/2006/time#intervalMetBy">
        <owl:inverseOf rdf:resource="http://www.w3.org/2006/time#intervalMeets"/>
        <rdfs:domain rdf:resource="http://www.w3.org/2006/time#ProperInterval"/>
        <rdfs:range rdf:resource="http://www.w3.org/2006/time#ProperInterval"/>
        <rdfs:comment xml:lang="en">If a proper interval T1 is intervalMetBy another proper interval T2, then the beginning of T1 is coincident with the end of T2.</rdfs:comment>
        <rdfs:comment xml:lang="es">Si un intervalo propio T1 es &apos;intervalo encontrado por&apos; otro intervalo propio T2, entonces el principio de T1 coincide con el final de T2.</rdfs:comment>
        <rdfs:label xml:lang="en">interval met by</rdfs:label>
        <rdfs:label xml:lang="es">intervalo encontrado por</rdfs:label>
        <skos:definition xml:lang="en">If a proper interval T1 is intervalMetBy another proper interval T2, then the beginning of T1 is coincident with the end of T2.</skos:definition>
        <skos:definition xml:lang="es">Si un intervalo propio T1 es &apos;intervalo encontrado por&apos; otro intervalo propio T2, entonces el principio de T1 coincide con el final de T2.</skos:definition>
    </owl:ObjectProperty>
    


    <!-- http://www.w3.org/2006/time#intervalOverlappedBy -->


    <owl:ObjectProperty rdf:about="http://www.w3.org/2006/time#intervalOverlappedBy">
        <rdfs:domain rdf:resource="http://www.w3.org/2006/time#ProperInterval"/>
        <rdfs:range rdf:resource="http://www.w3.org/2006/time#ProperInterval"/>
        <rdfs:comment xml:lang="en">If a proper interval T1 is intervalOverlappedBy another proper interval T2, then the beginning of T1 is after the beginning of T2, the beginning of T1 is before the end of T2, and the end of T1 is after the end of T2.</rdfs:comment>
        <rdfs:comment xml:lang="es">Si un intervalo propio T1 es &apos;intervalo solapado por&apos; otro intervalo propio T2, entonces el principio de T1 es posterior al principio de T2, y el principio de T1 es anterior al final de T2, y el final de T1 es posterior al final de T2.</rdfs:comment>
        <rdfs:label xml:lang="en">interval overlapped by</rdfs:label>
        <rdfs:label xml:lang="es">intervalo solapado por</rdfs:label>
        <skos:definition xml:lang="en">If a proper interval T1 is intervalOverlappedBy another proper interval T2, then the beginning of T1 is after the beginning of T2, the beginning of T1 is before the end of T2, and the end of T1 is after the end of T2.</skos:definition>
        <skos:definition xml:lang="es">Si un intervalo propio T1 es &apos;intervalo solapado por&apos; otro intervalo propio T2, entonces el principio de T1 es posterior al principio de T2, y el principio de T1 es anterior al final de T2, y el final de T1 es posterior al final de T2.</skos:definition>
    </owl:ObjectProperty>
    


    <!-- http://www.w3.org/2006/time#intervalOverlaps -->


    <owl:ObjectProperty rdf:about="http://www.w3.org/2006/time#intervalOverlaps">
        <owl:inverseOf rdf:resource="http://www.w3.org/2006/time#intervalOverlappedBy"/>
        <rdfs:domain rdf:resource="http://www.w3.org/2006/time#ProperInterval"/>
        <rdfs:range rdf:resource="http://www.w3.org/2006/time#ProperInterval"/>
        <rdfs:comment xml:lang="es">Asume una dirección en el tiempo. Si una entidad temporal T1 está después de otra entidad temporal T2, entonces el principio de T1 está después del final de T2.</rdfs:comment>
        <rdfs:comment xml:lang="en">If a proper interval T1 is intervalOverlaps another proper interval T2, then the beginning of T1 is before the beginning of T2, the end of T1 is after the beginning of T2, and the end of T1 is before the end of T2.</rdfs:comment>
        <rdfs:comment xml:lang="es">Si un intervalo propio T1 se solapa con otro intervalo propio T2, entonces el principio de T1 es anterior al principio de T2, el final de T1 es posterior al principio de T2, y el final de T1 es anterior al final de T2.</rdfs:comment>
        <rdfs:label xml:lang="en">interval overlaps</rdfs:label>
        <rdfs:label xml:lang="es">intervalo se solapa</rdfs:label>
        <skos:definition xml:lang="en">If a proper interval T1 is intervalOverlaps another proper interval T2, then the beginning of T1 is before the beginning of T2, the end of T1 is after the beginning of T2, and the end of T1 is before the end of T2.</skos:definition>
        <skos:definition xml:lang="es">Si un intervalo propio T1 se solapa con otro intervalo propio T2, entonces el principio de T1 es anterior al principio de T2, el final de T1 es posterior al principio de T2, y el final de T1 es anterior al final de T2.</skos:definition>
    </owl:ObjectProperty>
    


    <!-- http://www.w3.org/2006/time#intervalStartedBy -->


    <owl:ObjectProperty rdf:about="http://www.w3.org/2006/time#intervalStartedBy">
        <rdfs:domain rdf:resource="http://www.w3.org/2006/time#ProperInterval"/>
        <rdfs:range rdf:resource="http://www.w3.org/2006/time#ProperInterval"/>
        <rdfs:comment xml:lang="en">If a proper interval T1 is intervalStarted another proper interval T2, then the beginning of T1 is coincident with the beginning of T2, and the end of T1 is after the end of T2.</rdfs:comment>
        <rdfs:comment xml:lang="es">Si un intervalo propio T1 es empezado por otro intervalo propio T2, entonces el principio de T1 coincide con el principio de T2, y el final de T1 es posterior al final de T2.</rdfs:comment>
        <rdfs:label xml:lang="en">interval started by</rdfs:label>
        <skos:definition xml:lang="en">If a proper interval T1 is intervalStarted another proper interval T2, then the beginning of T1 is coincident with the beginning of T2, and the end of T1 is after the end of T2.</skos:definition>
        <skos:definition xml:lang="es">Si un intervalo propio T1 es empezado por otro intervalo propio T2, entonces el principio de T1 coincide con el principio de T2, y el final de T1 es posterior al final de T2.</skos:definition>
    </owl:ObjectProperty>
    


    <!-- http://www.w3.org/2006/time#intervalStarts -->


    <owl:ObjectProperty rdf:about="http://www.w3.org/2006/time#intervalStarts">
        <rdfs:subPropertyOf rdf:resource="http://www.w3.org/2006/time#intervalIn"/>
        <owl:inverseOf rdf:resource="http://www.w3.org/2006/time#intervalStartedBy"/>
        <rdfs:domain rdf:resource="http://www.w3.org/2006/time#ProperInterval"/>
        <rdfs:range rdf:resource="http://www.w3.org/2006/time#ProperInterval"/>
        <rdfs:comment xml:lang="en">If a proper interval T1 is intervalStarts another proper interval T2, then the beginning of T1 is coincident with the beginning of T2, and the end of T1 is before the end of T2.</rdfs:comment>
        <rdfs:comment xml:lang="es">Si un intervalo propio T1 empieza otro intervalo propio T2, entonces del principio de T1 con el principio de T2, y el final de T1 es anterior al final de T2.</rdfs:comment>
        <rdfs:label xml:lang="en">interval starts</rdfs:label>
        <rdfs:label xml:lang="es">intervalo empieza</rdfs:label>
        <skos:definition xml:lang="en">If a proper interval T1 is intervalStarts another proper interval T2, then the beginning of T1 is coincident with the beginning of T2, and the end of T1 is before the end of T2.</skos:definition>
        <skos:definition xml:lang="es">Si un intervalo propio T1 empieza otro intervalo propio T2, entonces del principio de T1 con el final de T2, y el final de T1 es anterior al final de T2.</skos:definition>
    </owl:ObjectProperty>
    


    <!-- http://www.w3.org/2006/time#monthOfYear -->


    <owl:ObjectProperty rdf:about="http://www.w3.org/2006/time#monthOfYear">
        <rdfs:domain rdf:resource="http://www.w3.org/2006/time#GeneralDateTimeDescription"/>
        <rdfs:range rdf:resource="http://www.w3.org/2006/time#MonthOfYear"/>
        <rdfs:comment xml:lang="es">El mes del año, cuyo valor es un miembro de la clase &apos;mes del año&apos;.</rdfs:comment>
        <rdfs:comment xml:lang="en">The month of the year, whose value is a member of the class time:MonthOfYear</rdfs:comment>
        <rdfs:label xml:lang="es">mes del año</rdfs:label>
        <rdfs:label xml:lang="en">month of year</rdfs:label>
        <skos:definition xml:lang="es">El mes del año, cuyo valor es un miembro de la clase &apos;mes del año&apos;.</skos:definition>
        <skos:definition xml:lang="en">The month of the year, whose value is a member of the class time:MonthOfYear</skos:definition>
        <skos:editorialNote xml:lang="es">Característica arriesgada - añadida en la revisión de 2017, y todavía no ampliamente utilizada.</skos:editorialNote>
        <skos:editorialNote xml:lang="en">Feature at risk - added in 2017 revision, and not yet widely used. </skos:editorialNote>
    </owl:ObjectProperty>
    


    <!-- http://www.w3.org/2006/time#timeZone -->


    <owl:ObjectProperty rdf:about="http://www.w3.org/2006/time#timeZone">
        <rdfs:domain rdf:resource="http://www.w3.org/2006/time#GeneralDateTimeDescription"/>
        <rdfs:range rdf:resource="http://www.w3.org/2006/time#TimeZone"/>
        <rdfs:comment xml:lang="en">The time zone for clock elements in the temporal position</rdfs:comment>
        <rdfs:label xml:lang="es">en huso horario</rdfs:label>
        <rdfs:label xml:lang="en">in time zone</rdfs:label>
        <skos:historyNote xml:lang="es">En la versión original de OWL-Time de 2006, el rango de &apos;en huso horario&apos; se definió en un espacio de nombres diferente &quot;http://www.w3.org/2006/timezone#&quot;.
            Un axioma de alineación permite que los datos codificados de acuerdo con la versión anterior sean consistentes con la ontología actualizada.</skos:historyNote>
        <skos:historyNote>In the original 2006 version of OWL-Time, the range of time:timeZone was a TimeZone class in a separate namespace &quot;http://www.w3.org/2006/timezone#&quot;. 
An alignment axiom 
	tzont:TimeZone rdfs:subClassOf time:TimeZone . 
allows data encoded according to the previous version to be consistent with the updated ontology. </skos:historyNote>
        <skos:note xml:lang="es">IANA mantiene una base de datos de husos horarios. Éstas están bien mantenidas y generalmente se consideran autorizadas, pero los ítems individuales no están disponibles en URIs individuales, por tanto, no se pueden utilizar directamente en datos expresados utilizando OWL-Time.
            La BDPedia proporciona un conjunto de recursos correspondientes a los husos horarios de IANA, con una URI para cada uno (por ejemplo, http://dbpedia.org/resource/Australia/Eucla). El Servicio de Reloj Mundial también proporciona una lista de husos horarios con la descripción de cada uno de los disponibles como una página Web individual con una URI adecuada individual (por ejemplo, https://www.timeanddate.com/time/zones/acwst). Éstos, y otros recursos similares, se puden usar como un valor de la propiedad &apos;huso horario&apos;.</skos:note>
        <skos:note>IANA maintains a database of timezones. These are well maintained and generally considered authoritative, but individual items are not available at individual URIs, so cannot be used directly in data expressed using OWL-Time.

DBPedia provides a set of resources corresponding to the IANA timezones, with a URI for each (e.g. http://dbpedia.org/resource/Australia/Eucla). The World Clock service also provides a list of time zones with the description of each available as an individual webpage with a convenient individual URI (e.g. https://www.timeanddate.com/time/zones/acwst). These or other, similar, resources might be used as a value of the time:timeZone property.</skos:note>
    </owl:ObjectProperty>
    


    <!-- http://www.w3.org/2006/time#unitType -->


    <owl:ObjectProperty rdf:about="http://www.w3.org/2006/time#unitType">
        <rdfs:domain>
            <owl:Class>
                <owl:unionOf rdf:parseType="Collection">
                    <rdf:Description rdf:about="http://www.w3.org/2006/time#Duration"/>
                    <rdf:Description rdf:about="http://www.w3.org/2006/time#GeneralDateTimeDescription"/>
                </owl:unionOf>
            </owl:Class>
        </rdfs:domain>
        <rdfs:range rdf:resource="http://www.w3.org/2006/time#TemporalUnit"/>
        <rdfs:comment xml:lang="es">La unidad de tiempo que proporciona la precisión de un valor fecha-hora o la escala de una extensión temporal.</rdfs:comment>
        <rdfs:comment xml:lang="en">The temporal unit which provides the precision of a date-time value or scale of a temporal extent</rdfs:comment>
        <rdfs:label xml:lang="en">temporal unit type</rdfs:label>
        <rdfs:label xml:lang="es">tipo de unidad temporal</rdfs:label>
    </owl:ObjectProperty>
    


    <!-- 
    ///////////////////////////////////////////////////////////////////////////////////////
    //
    // Data properties
    //
    ///////////////////////////////////////////////////////////////////////////////////////
     -->


    


    <!-- http://www.semanticweb.org/sc3/ontologies/2022/0/Planning-Ontology#hasAnticipationCapabilities -->


    <owl:DatatypeProperty rdf:about="http://www.semanticweb.org/sc3/ontologies/2022/0/Planning-Ontology#hasAnticipationCapabilities">
        <rdfs:subPropertyOf rdf:resource="http://www.w3.org/2002/07/owl#topDataProperty"/>
        <rdfs:domain rdf:resource="http://www.semanticweb.org/sc3/ontologies/2022/0/Planning-Ontology#DecisionMakingUnit"/>
        <rdfs:range rdf:resource="http://www.w3.org/2001/XMLSchema#string"/>
        <rdfs:comment>Anticipatory activities are used by a DECISION-MAKING UNIT to take into account the characteristics and the situation of other DECISION-MAKING UNITs in course of its own decision making (Schneeweiss 2003).</rdfs:comment>
    </owl:DatatypeProperty>
    


    <!-- http://www.semanticweb.org/sc3/ontologies/2022/0/Planning-Ontology#hasAvailabilityDate -->


    <owl:DatatypeProperty rdf:about="http://www.semanticweb.org/sc3/ontologies/2022/0/Planning-Ontology#hasAvailabilityDate">
        <rdfs:domain rdf:resource="http://www.semanticweb.org/sc3/ontologies/2022/0/Planning-Ontology#SupplyInformation"/>
        <rdfs:range rdf:resource="http://www.w3.org/2001/XMLSchema#string"/>
    </owl:DatatypeProperty>
    


    <!-- http://www.semanticweb.org/sc3/ontologies/2022/0/Planning-Ontology#hasBinningPercentage -->


    <owl:DatatypeProperty rdf:about="http://www.semanticweb.org/sc3/ontologies/2022/0/Planning-Ontology#hasBinningPercentage">
        <rdfs:domain rdf:resource="http://www.semanticweb.org/sc3/ontologies/2022/0/Planning-Ontology#Process"/>
        <rdfs:range rdf:resource="http://www.w3.org/2001/XMLSchema#int"/>
    </owl:DatatypeProperty>
    


    <!-- http://www.semanticweb.org/sc3/ontologies/2022/0/Planning-Ontology#hasCapacityUnit -->


    <owl:DatatypeProperty rdf:about="http://www.semanticweb.org/sc3/ontologies/2022/0/Planning-Ontology#hasCapacityUnit">
        <rdfs:domain rdf:resource="http://www.semanticweb.org/sc3/ontologies/2022/0/Planning-Ontology#Capacity"/>
        <rdfs:range rdf:resource="http://www.w3.org/2001/XMLSchema#string"/>
    </owl:DatatypeProperty>
    


    <!-- http://www.semanticweb.org/sc3/ontologies/2022/0/Planning-Ontology#hasCommitDate -->


    <owl:DatatypeProperty rdf:about="http://www.semanticweb.org/sc3/ontologies/2022/0/Planning-Ontology#hasCommitDate">
        <rdfs:domain rdf:resource="http://www.semanticweb.org/sc3/ontologies/2022/0/ozone-ontology#Demand"/>
        <rdfs:range rdf:resource="http://www.w3.org/2001/XMLSchema#string"/>
    </owl:DatatypeProperty>
    


    <!-- http://www.semanticweb.org/sc3/ontologies/2022/0/Planning-Ontology#hasConsumedQuantity -->


    <owl:DatatypeProperty rdf:about="http://www.semanticweb.org/sc3/ontologies/2022/0/Planning-Ontology#hasConsumedQuantity">
        <rdfs:domain rdf:resource="http://www.semanticweb.org/sc3/ontologies/2022/0/Planning-Ontology#RequiredCapacity"/>
        <rdfs:range rdf:resource="http://www.w3.org/2001/XMLSchema#int"/>
    </owl:DatatypeProperty>
    


    <!-- http://www.semanticweb.org/sc3/ontologies/2022/0/Planning-Ontology#hasCosts -->


    <owl:DatatypeProperty rdf:about="http://www.semanticweb.org/sc3/ontologies/2022/0/Planning-Ontology#hasCosts">
        <rdfs:subPropertyOf rdf:resource="http://www.w3.org/2002/07/owl#topDataProperty"/>
        <rdfs:domain rdf:resource="http://www.semanticweb.org/sc3/ontologies/2022/0/Planning-Ontology#PlaningPurpose"/>
        <rdfs:domain rdf:resource="http://www.semanticweb.org/sc3/ontologies/2022/0/Planning-Ontology#Substitution"/>
        <rdfs:range rdf:resource="http://www.w3.org/2001/XMLSchema#string"/>
        <rdfs:comment>Cost refers to the amount of money that is needed to do a certain action for a unit of a certain good, for instance, store or produce a unit of a product.</rdfs:comment>
    </owl:DatatypeProperty>
    


    <!-- http://www.semanticweb.org/sc3/ontologies/2022/0/Planning-Ontology#hasCurrentStockLevel -->


    <owl:DatatypeProperty rdf:about="http://www.semanticweb.org/sc3/ontologies/2022/0/Planning-Ontology#hasCurrentStockLevel">
        <rdfs:domain rdf:resource="http://www.semanticweb.org/sc3/ontologies/2022/0/Planning-Ontology#Inventory"/>
        <rdfs:range rdf:resource="http://www.w3.org/2001/XMLSchema#int"/>
    </owl:DatatypeProperty>
    


    <!-- http://www.semanticweb.org/sc3/ontologies/2022/0/Planning-Ontology#hasDecision-Rights -->


    <owl:DatatypeProperty rdf:about="http://www.semanticweb.org/sc3/ontologies/2022/0/Planning-Ontology#hasDecision-Rights">
        <rdfs:subPropertyOf rdf:resource="http://www.w3.org/2002/07/owl#topDataProperty"/>
        <rdfs:domain rdf:resource="http://www.semanticweb.org/sc3/ontologies/2022/0/Planning-Ontology#DecisionMakingUnit"/>
        <rdfs:range rdf:resource="http://www.w3.org/2001/XMLSchema#string"/>
        <rdfs:comment>This property will allow a DECISION-MAKING UNIT to negotiate the instruction provided by other DECISION-MAKING UNIT. In a conventional or strict hierarchical setting, negotiations of instruction provided by superior DECISION-MAKING UNITs are impossible. In a distributed hierarchical setting in the sense of Schneeweiss (2003) reactions of the DECISION-MAKING UNIT which can lead to negotiations are possible (Schneeweiss 2003).</rdfs:comment>
    </owl:DatatypeProperty>
    


    <!-- http://www.semanticweb.org/sc3/ontologies/2022/0/Planning-Ontology#hasDecisionTime -->


    <owl:DatatypeProperty rdf:about="http://www.semanticweb.org/sc3/ontologies/2022/0/Planning-Ontology#hasDecisionTime">
        <rdfs:subPropertyOf rdf:resource="http://www.w3.org/2002/07/owl#topDataProperty"/>
        <rdfs:domain rdf:resource="http://www.semanticweb.org/sc3/ontologies/2022/0/Planning-Ontology#DecisionMakingUnit"/>
        <rdfs:range rdf:resource="http://www.w3.org/2001/XMLSchema#string"/>
        <rdfs:comment>This property describes the point of time when a decision is made by the DECISION-MAKING UNIT.</rdfs:comment>
    </owl:DatatypeProperty>
    


    <!-- http://www.semanticweb.org/sc3/ontologies/2022/0/Planning-Ontology#hasDemandClass -->


    <owl:DatatypeProperty rdf:about="http://www.semanticweb.org/sc3/ontologies/2022/0/Planning-Ontology#hasDemandClass">
        <rdfs:domain rdf:resource="http://www.semanticweb.org/sc3/ontologies/2022/0/ozone-ontology#Demand"/>
        <rdfs:range rdf:resource="http://www.w3.org/2001/XMLSchema#string"/>
    </owl:DatatypeProperty>
    


    <!-- http://www.semanticweb.org/sc3/ontologies/2022/0/Planning-Ontology#hasDistribution -->


    <owl:DatatypeProperty rdf:about="http://www.semanticweb.org/sc3/ontologies/2022/0/Planning-Ontology#hasDistribution">
        <rdfs:domain rdf:resource="http://www.semanticweb.org/sc3/ontologies/2022/0/Planning-Ontology#Binning"/>
        <rdfs:range rdf:resource="http://www.w3.org/2001/XMLSchema#int"/>
    </owl:DatatypeProperty>
    


    <!-- http://www.semanticweb.org/sc3/ontologies/2022/0/Planning-Ontology#hasDueDate -->


    <owl:DatatypeProperty rdf:about="http://www.semanticweb.org/sc3/ontologies/2022/0/Planning-Ontology#hasDueDate">
        <rdfs:subPropertyOf rdf:resource="http://www.w3.org/2002/07/owl#topDataProperty"/>
        <rdfs:domain rdf:resource="http://www.semanticweb.org/sc3/ontologies/2022/0/Planning-Ontology#Activity"/>
        <rdfs:domain rdf:resource="http://www.semanticweb.org/sc3/ontologies/2022/0/Planning-Ontology#Part"/>
        <rdfs:domain rdf:resource="http://www.semanticweb.org/sc3/ontologies/2022/0/Planning-Ontology#PlanningObject"/>
        <rdfs:domain rdf:resource="http://www.semanticweb.org/sc3/ontologies/2022/0/Planning-Ontology#SupplyInformation"/>
        <rdfs:range rdf:resource="http://www.w3.org/2001/XMLSchema#dateTime"/>
        <rdfs:comment>This is the latest time where the activities associated with a PLANNING OBJECT have to be finished. Note that the parameter DUE DATE is exogenous, i.e. given, in contrast to the property TIME.</rdfs:comment>
    </owl:DatatypeProperty>
    


    <!-- http://www.semanticweb.org/sc3/ontologies/2022/0/Planning-Ontology#hasEarliestReleaseDate -->


    <owl:DatatypeProperty rdf:about="http://www.semanticweb.org/sc3/ontologies/2022/0/Planning-Ontology#hasEarliestReleaseDate">
        <rdfs:domain rdf:resource="http://www.semanticweb.org/sc3/ontologies/2022/0/Planning-Ontology#Part"/>
        <rdfs:range rdf:resource="http://www.w3.org/2001/XMLSchema#string"/>
    </owl:DatatypeProperty>
    


    <!-- http://www.semanticweb.org/sc3/ontologies/2022/0/Planning-Ontology#hasEffectiveDate -->


    <owl:DatatypeProperty rdf:about="http://www.semanticweb.org/sc3/ontologies/2022/0/Planning-Ontology#hasEffectiveDate">
        <rdfs:domain rdf:resource="http://www.semanticweb.org/sc3/ontologies/2022/0/Planning-Ontology#Yield"/>
        <rdfs:range rdf:resource="http://www.w3.org/2001/XMLSchema#string"/>
    </owl:DatatypeProperty>
    


    <!-- http://www.semanticweb.org/sc3/ontologies/2022/0/Planning-Ontology#hasEffectiveStartDate -->


    <owl:DatatypeProperty rdf:about="http://www.semanticweb.org/sc3/ontologies/2022/0/Planning-Ontology#hasEffectiveStartDate">
        <rdfs:domain rdf:resource="http://www.semanticweb.org/sc3/ontologies/2022/0/Planning-Ontology#Capacity"/>
        <rdfs:range rdf:resource="http://www.w3.org/2001/XMLSchema#string"/>
    </owl:DatatypeProperty>
    


    <!-- http://www.semanticweb.org/sc3/ontologies/2022/0/Planning-Ontology#hasEndDate -->


    <owl:DatatypeProperty rdf:about="http://www.semanticweb.org/sc3/ontologies/2022/0/Planning-Ontology#hasEndDate">
        <rdfs:domain rdf:resource="http://www.semanticweb.org/sc3/ontologies/2022/0/Planning-Ontology#Binning"/>
        <rdfs:domain rdf:resource="http://www.semanticweb.org/sc3/ontologies/2022/0/Planning-Ontology#FrozenFence"/>
        <rdfs:domain rdf:resource="http://www.semanticweb.org/sc3/ontologies/2022/0/Planning-Ontology#InventoryPolicy"/>
        <rdfs:domain rdf:resource="http://www.semanticweb.org/sc3/ontologies/2022/0/Planning-Ontology#LotSizingRule"/>
        <rdfs:domain rdf:resource="http://www.semanticweb.org/sc3/ontologies/2022/0/Planning-Ontology#Substitution"/>
        <rdfs:range rdf:resource="http://www.w3.org/2001/XMLSchema#string"/>
    </owl:DatatypeProperty>
    


    <!-- http://www.semanticweb.org/sc3/ontologies/2022/0/Planning-Ontology#hasEndTime -->


    <owl:DatatypeProperty rdf:about="http://www.semanticweb.org/sc3/ontologies/2022/0/Planning-Ontology#hasEndTime">
        <rdfs:subPropertyOf rdf:resource="http://www.w3.org/2002/07/owl#topDataProperty"/>
        <rdfs:domain rdf:resource="http://www.semanticweb.org/sc3/ontologies/2022/0/Planning-Ontology#PlanningConstraint"/>
        <rdfs:range rdf:resource="http://www.w3.org/2001/XMLSchema#string"/>
        <rdfs:comment>This is the latest point in time when the PLANNING CONSTRAINT is active.</rdfs:comment>
    </owl:DatatypeProperty>
    


    <!-- http://www.semanticweb.org/sc3/ontologies/2022/0/Planning-Ontology#hasFeasibilityStatus -->


    <owl:DatatypeProperty rdf:about="http://www.semanticweb.org/sc3/ontologies/2022/0/Planning-Ontology#hasFeasibilityStatus">
        <rdfs:subPropertyOf rdf:resource="http://www.w3.org/2002/07/owl#topDataProperty"/>
        <rdfs:domain rdf:resource="http://www.semanticweb.org/sc3/ontologies/2022/0/Planning-Ontology#Plan"/>
        <rdfs:range rdf:resource="http://www.w3.org/2001/XMLSchema#string"/>
        <rdfs:comment>A PLAN is feasible if all PLANNING CONSTAINTS of the PLANNING INSTANCE on which the plan is based are fulfilled, otherwise, the plan is infeasible.</rdfs:comment>
    </owl:DatatypeProperty>
    


    <!-- http://www.semanticweb.org/sc3/ontologies/2022/0/Planning-Ontology#hasHardConstraints -->


    <owl:DatatypeProperty rdf:about="http://www.semanticweb.org/sc3/ontologies/2022/0/Planning-Ontology#hasHardConstraints">
        <rdfs:subPropertyOf rdf:resource="http://www.w3.org/2002/07/owl#topDataProperty"/>
        <rdfs:domain rdf:resource="http://www.semanticweb.org/sc3/ontologies/2022/0/Planning-Ontology#PlanningConstraint"/>
        <rdfs:range rdf:resource="http://www.w3.org/2001/XMLSchema#string"/>
        <rdfs:comment>PLANNING CONSTRAINTS with this property cannot be violated.</rdfs:comment>
    </owl:DatatypeProperty>
    


    <!-- http://www.semanticweb.org/sc3/ontologies/2022/0/Planning-Ontology#hasIdentifier -->


    <owl:DatatypeProperty rdf:about="http://www.semanticweb.org/sc3/ontologies/2022/0/Planning-Ontology#hasIdentifier">
        <rdfs:subPropertyOf rdf:resource="http://www.w3.org/2002/07/owl#topDataProperty"/>
        <rdfs:domain rdf:resource="http://www.semanticweb.org/sc3/ontologies/2022/0/Planning-Ontology#PlanningObject"/>
        <rdfs:range rdf:resource="http://www.w3.org/2001/XMLSchema#string"/>
        <rdfs:comment>Each PLANNING OBJECT has a unique identifier, abbreviated by ID.</rdfs:comment>
    </owl:DatatypeProperty>
    


    <!-- http://www.semanticweb.org/sc3/ontologies/2022/0/Planning-Ontology#hasInformationStatus -->


    <owl:DatatypeProperty rdf:about="http://www.semanticweb.org/sc3/ontologies/2022/0/Planning-Ontology#hasInformationStatus">
        <rdfs:subPropertyOf rdf:resource="http://www.w3.org/2002/07/owl#topDataProperty"/>
        <rdfs:domain rdf:resource="http://www.semanticweb.org/sc3/ontologies/2022/0/Planning-Ontology#DecisionMakingUnit"/>
        <rdfs:range rdf:resource="http://www.w3.org/2001/XMLSchema#string"/>
        <rdfs:comment>This property describes the own internal, but also the external situation of the DECISION-MAKING UNIT. At the same time, it describes information about the internal and external situation of other DECISION-MAKING UNITs and their information status (Schneeweiss 2003).</rdfs:comment>
    </owl:DatatypeProperty>
    


    <!-- http://www.semanticweb.org/sc3/ontologies/2022/0/Planning-Ontology#hasLeadTime -->


    <owl:DatatypeProperty rdf:about="http://www.semanticweb.org/sc3/ontologies/2022/0/Planning-Ontology#hasLeadTime">
        <rdfs:domain rdf:resource="http://www.semanticweb.org/sc3/ontologies/2022/0/Planning-Ontology#Process"/>
        <rdfs:range rdf:resource="http://www.w3.org/2001/XMLSchema#int"/>
    </owl:DatatypeProperty>
    


    <!-- http://www.semanticweb.org/sc3/ontologies/2022/0/Planning-Ontology#hasLevel -->


    <owl:DatatypeProperty rdf:about="http://www.semanticweb.org/sc3/ontologies/2022/0/Planning-Ontology#hasLevel">
        <rdfs:subPropertyOf rdf:resource="http://www.w3.org/2002/07/owl#topDataProperty"/>
        <rdfs:domain rdf:resource="http://www.semanticweb.org/sc3/ontologies/2022/0/Planning-Ontology#Edge"/>
        <rdfs:domain rdf:resource="http://www.semanticweb.org/sc3/ontologies/2022/0/Planning-Ontology#PlanningSituation"/>
        <rdfs:range rdf:resource="http://www.w3.org/2001/XMLSchema#string"/>
        <rdfs:comment>Each vertex has a level. The highest level is assigned to vertices that do not receive instructions from other vertices. The vertices belonging to the second highest level receive instructions only from vertices of the highest level. This definition can be repeated in a recursive manner. Reactions are only possible from vertices of level k-1 to vertices of level k or level k-1.</rdfs:comment>
    </owl:DatatypeProperty>
    


    <!-- http://www.semanticweb.org/sc3/ontologies/2022/0/Planning-Ontology#hasMaximumCapacity -->


    <owl:DatatypeProperty rdf:about="http://www.semanticweb.org/sc3/ontologies/2022/0/Planning-Ontology#hasMaximumCapacity">
        <rdfs:domain rdf:resource="http://www.semanticweb.org/sc3/ontologies/2022/0/Planning-Ontology#AvailableCapacity"/>
        <rdfs:range rdf:resource="http://www.w3.org/2001/XMLSchema#int"/>
    </owl:DatatypeProperty>
    


    <!-- http://www.semanticweb.org/sc3/ontologies/2022/0/Planning-Ontology#hasMaximumComputingTime -->


    <owl:DatatypeProperty rdf:about="http://www.semanticweb.org/sc3/ontologies/2022/0/Planning-Ontology#hasMaximumComputingTime">
        <rdfs:subPropertyOf rdf:resource="http://www.w3.org/2002/07/owl#topDataProperty"/>
        <rdfs:domain rdf:resource="http://www.semanticweb.org/sc3/ontologies/2022/0/Planning-Ontology#PlanningProcess"/>
        <rdfs:range rdf:resource="http://www.w3.org/2001/XMLSchema#string"/>
        <rdfs:comment>This property specifies which maximum time is allowed to perform a certain planning activity.</rdfs:comment>
    </owl:DatatypeProperty>
    


    <!-- http://www.semanticweb.org/sc3/ontologies/2022/0/Planning-Ontology#hasMaximumLotSize -->


    <owl:DatatypeProperty rdf:about="http://www.semanticweb.org/sc3/ontologies/2022/0/Planning-Ontology#hasMaximumLotSize">
        <rdfs:domain rdf:resource="http://www.semanticweb.org/sc3/ontologies/2022/0/Planning-Ontology#LotSizingRule"/>
        <rdfs:range rdf:resource="http://www.w3.org/2001/XMLSchema#int"/>
    </owl:DatatypeProperty>
    


    <!-- http://www.semanticweb.org/sc3/ontologies/2022/0/Planning-Ontology#hasMaximumSupply -->


    <owl:DatatypeProperty rdf:about="http://www.semanticweb.org/sc3/ontologies/2022/0/Planning-Ontology#hasMaximumSupply">
        <rdfs:domain rdf:resource="http://www.semanticweb.org/sc3/ontologies/2022/0/Planning-Ontology#SupplyInformation"/>
        <rdfs:range rdf:resource="http://www.w3.org/2001/XMLSchema#string"/>
    </owl:DatatypeProperty>
    


    <!-- http://www.semanticweb.org/sc3/ontologies/2022/0/Planning-Ontology#hasMinimumCapacity -->


    <owl:DatatypeProperty rdf:about="http://www.semanticweb.org/sc3/ontologies/2022/0/Planning-Ontology#hasMinimumCapacity">
        <rdfs:domain rdf:resource="http://www.semanticweb.org/sc3/ontologies/2022/0/Planning-Ontology#AvailableCapacity"/>
        <rdfs:range rdf:resource="http://www.w3.org/2001/XMLSchema#int"/>
    </owl:DatatypeProperty>
    


    <!-- http://www.semanticweb.org/sc3/ontologies/2022/0/Planning-Ontology#hasMinimumLotSize -->


    <owl:DatatypeProperty rdf:about="http://www.semanticweb.org/sc3/ontologies/2022/0/Planning-Ontology#hasMinimumLotSize">
        <rdfs:domain rdf:resource="http://www.semanticweb.org/sc3/ontologies/2022/0/Planning-Ontology#LotSizingRule"/>
        <rdfs:range rdf:resource="http://www.w3.org/2001/XMLSchema#int"/>
    </owl:DatatypeProperty>
    


    <!-- http://www.semanticweb.org/sc3/ontologies/2022/0/Planning-Ontology#hasMinimumSupply -->


    <owl:DatatypeProperty rdf:about="http://www.semanticweb.org/sc3/ontologies/2022/0/Planning-Ontology#hasMinimumSupply">
        <rdfs:domain rdf:resource="http://www.semanticweb.org/sc3/ontologies/2022/0/Planning-Ontology#SupplyInformation"/>
        <rdfs:range rdf:resource="http://www.w3.org/2001/XMLSchema#string"/>
    </owl:DatatypeProperty>
    


    <!-- http://www.semanticweb.org/sc3/ontologies/2022/0/Planning-Ontology#hasOffsetPeriods -->


    <owl:DatatypeProperty rdf:about="http://www.semanticweb.org/sc3/ontologies/2022/0/Planning-Ontology#hasOffsetPeriods">
        <rdfs:domain rdf:resource="http://www.semanticweb.org/sc3/ontologies/2022/0/Planning-Ontology#RequiredCapacity"/>
        <rdfs:range rdf:resource="http://www.w3.org/2001/XMLSchema#int"/>
    </owl:DatatypeProperty>
    


    <!-- http://www.semanticweb.org/sc3/ontologies/2022/0/Planning-Ontology#hasOrigin -->


    <owl:DatatypeProperty rdf:about="http://www.semanticweb.org/sc3/ontologies/2022/0/Planning-Ontology#hasOrigin">
        <rdfs:domain rdf:resource="http://www.semanticweb.org/sc3/ontologies/2022/0/ozone-ontology#Demand"/>
        <rdfs:range rdf:resource="http://www.w3.org/2001/XMLSchema#string"/>
    </owl:DatatypeProperty>
    


    <!-- http://www.semanticweb.org/sc3/ontologies/2022/0/Planning-Ontology#hasPartType -->


    <owl:DatatypeProperty rdf:about="http://www.semanticweb.org/sc3/ontologies/2022/0/Planning-Ontology#hasPartType">
        <rdfs:domain rdf:resource="http://www.semanticweb.org/sc3/ontologies/2022/0/Planning-Ontology#ProjectedWip"/>
        <rdfs:range rdf:resource="http://www.w3.org/2001/XMLSchema#string"/>
    </owl:DatatypeProperty>
    


    <!-- http://www.semanticweb.org/sc3/ontologies/2022/0/Planning-Ontology#hasPenalityCosts -->


    <owl:DatatypeProperty rdf:about="http://www.semanticweb.org/sc3/ontologies/2022/0/Planning-Ontology#hasPenalityCosts">
        <rdfs:subPropertyOf rdf:resource="http://www.w3.org/2002/07/owl#topDataProperty"/>
        <rdfs:domain rdf:resource="http://www.semanticweb.org/sc3/ontologies/2022/0/Planning-Ontology#PlaningPurpose"/>
        <rdfs:range rdf:resource="http://www.w3.org/2001/XMLSchema#string"/>
        <rdfs:comment>If CONSTRAINTS are violated by a plan penalties might be used to change the performance measure values to express that the violations are undesired.</rdfs:comment>
    </owl:DatatypeProperty>
    


    <!-- http://www.semanticweb.org/sc3/ontologies/2022/0/Planning-Ontology#hasPerformanceCriteria -->


    <owl:DatatypeProperty rdf:about="http://www.semanticweb.org/sc3/ontologies/2022/0/Planning-Ontology#hasPerformanceCriteria">
        <rdfs:domain rdf:resource="http://www.semanticweb.org/sc3/ontologies/2022/0/Planning-Ontology#PlaningPurpose"/>
        <rdfs:range rdf:resource="http://www.w3.org/2001/XMLSchema#string"/>
    </owl:DatatypeProperty>
    


    <!-- http://www.semanticweb.org/sc3/ontologies/2022/0/Planning-Ontology#hasPerformanceMeasure -->


    <owl:DatatypeProperty rdf:about="http://www.semanticweb.org/sc3/ontologies/2022/0/Planning-Ontology#hasPerformanceMeasure">
        <rdfs:domain rdf:resource="http://www.semanticweb.org/sc3/ontologies/2022/0/Planning-Ontology#PlaningPurpose"/>
        <rdfs:range rdf:resource="http://www.w3.org/2001/XMLSchema#string"/>
    </owl:DatatypeProperty>
    


    <!-- http://www.semanticweb.org/sc3/ontologies/2022/0/Planning-Ontology#hasPeriod -->


    <owl:DatatypeProperty rdf:about="http://www.semanticweb.org/sc3/ontologies/2022/0/Planning-Ontology#hasPeriod">
        <rdfs:range rdf:resource="http://www.w3.org/2001/XMLSchema#int"/>
    </owl:DatatypeProperty>
    


    <!-- http://www.semanticweb.org/sc3/ontologies/2022/0/Planning-Ontology#hasPlanningPeriod -->


    <owl:DatatypeProperty rdf:about="http://www.semanticweb.org/sc3/ontologies/2022/0/Planning-Ontology#hasPlanningPeriod">
        <rdfs:subPropertyOf rdf:resource="http://www.w3.org/2002/07/owl#topDataProperty"/>
        <rdfs:domain rdf:resource="http://www.semanticweb.org/sc3/ontologies/2022/0/Planning-Ontology#PlanningInstance"/>
        <rdfs:range rdf:resource="http://www.w3.org/2001/XMLSchema#int"/>
        <rdfs:comment>This property defines a certain fraction of a planning window. Equidistant periods are common for many supply chain planning problems.</rdfs:comment>
    </owl:DatatypeProperty>
    


    <!-- http://www.semanticweb.org/sc3/ontologies/2022/0/Planning-Ontology#hasPlanningWindow -->


    <owl:DatatypeProperty rdf:about="http://www.semanticweb.org/sc3/ontologies/2022/0/Planning-Ontology#hasPlanningWindow">
        <rdfs:subPropertyOf rdf:resource="http://www.w3.org/2002/07/owl#topDataProperty"/>
        <rdfs:domain rdf:resource="http://www.semanticweb.org/sc3/ontologies/2022/0/Planning-Ontology#PlaningPurpose"/>
        <rdfs:domain rdf:resource="http://www.semanticweb.org/sc3/ontologies/2022/0/Planning-Ontology#PlanningInstance"/>
        <rdfs:range rdf:resource="http://www.w3.org/2001/XMLSchema#int"/>
        <rdfs:comment>A planning window described for which amount of periods or which time span the performance measure values have to be calculated. In some situations, the planning window will determine the set of planning objects, for instance, lots completed within the planning window.</rdfs:comment>
    </owl:DatatypeProperty>
    


    <!-- http://www.semanticweb.org/sc3/ontologies/2022/0/Planning-Ontology#hasPriority -->


    <owl:DatatypeProperty rdf:about="http://www.semanticweb.org/sc3/ontologies/2022/0/Planning-Ontology#hasPriority">
        <rdfs:subPropertyOf rdf:resource="http://www.w3.org/2002/07/owl#topDataProperty"/>
        <rdfs:domain rdf:resource="http://www.semanticweb.org/sc3/ontologies/2022/0/Planning-Ontology#PlanningObject"/>
        <rdfs:range rdf:resource="http://www.w3.org/2001/XMLSchema#int"/>
        <rdfs:comment>This property describes the relative importance of the PLANNING OBJECT. It provided the base for establishing a partial ordering of the importance of the set of planning objects.</rdfs:comment>
    </owl:DatatypeProperty>
    


    <!-- http://www.semanticweb.org/sc3/ontologies/2022/0/Planning-Ontology#hasProjectedDate -->


    <owl:DatatypeProperty rdf:about="http://www.semanticweb.org/sc3/ontologies/2022/0/Planning-Ontology#hasProjectedDate">
        <rdfs:domain rdf:resource="http://www.semanticweb.org/sc3/ontologies/2022/0/Planning-Ontology#In-TransitInventory"/>
        <rdfs:domain rdf:resource="http://www.semanticweb.org/sc3/ontologies/2022/0/Planning-Ontology#ProjectedWip"/>
        <rdfs:range rdf:resource="http://www.w3.org/2001/XMLSchema#string"/>
    </owl:DatatypeProperty>
    


    <!-- http://www.semanticweb.org/sc3/ontologies/2022/0/Planning-Ontology#hasProjectedQuantity -->


    <owl:DatatypeProperty rdf:about="http://www.semanticweb.org/sc3/ontologies/2022/0/Planning-Ontology#hasProjectedQuantity">
        <rdfs:domain rdf:resource="http://www.semanticweb.org/sc3/ontologies/2022/0/Planning-Ontology#In-TransitInventory"/>
        <rdfs:domain rdf:resource="http://www.semanticweb.org/sc3/ontologies/2022/0/Planning-Ontology#ProjectedWip"/>
        <rdfs:range rdf:resource="http://www.w3.org/2001/XMLSchema#int"/>
    </owl:DatatypeProperty>
    


    <!-- http://www.semanticweb.org/sc3/ontologies/2022/0/Planning-Ontology#hasQuantity -->


    <owl:DatatypeProperty rdf:about="http://www.semanticweb.org/sc3/ontologies/2022/0/Planning-Ontology#hasQuantity">
        <rdfs:subPropertyOf rdf:resource="http://www.w3.org/2002/07/owl#topDataProperty"/>
        <rdfs:domain rdf:resource="http://www.semanticweb.org/sc3/ontologies/2022/0/Planning-Ontology#PlanningObject"/>
        <rdfs:domain rdf:resource="http://www.semanticweb.org/sc3/ontologies/2022/0/ozone-ontology#Demand"/>
        <rdfs:range rdf:resource="http://www.w3.org/2001/XMLSchema#int"/>
        <rdfs:comment>This property describes given, i.e. fixed, size of a PLANNING OBJECT, for instance, the number of wafers that belong to a lot. Note that the parameter QUANTITY is exogenous, i.e. given, in contrast to the property QUANTITY where the amount of the quantity has to be decided.</rdfs:comment>
    </owl:DatatypeProperty>
    


    <!-- http://www.semanticweb.org/sc3/ontologies/2022/0/Planning-Ontology#hasReleaseDate -->


    <owl:DatatypeProperty rdf:about="http://www.semanticweb.org/sc3/ontologies/2022/0/Planning-Ontology#hasReleaseDate">
        <rdfs:subPropertyOf rdf:resource="http://www.w3.org/2002/07/owl#topDataProperty"/>
        <rdfs:domain rdf:resource="http://www.semanticweb.org/sc3/ontologies/2022/0/Planning-Ontology#Activity"/>
        <rdfs:domain rdf:resource="http://www.semanticweb.org/sc3/ontologies/2022/0/Planning-Ontology#PlanningObject"/>
        <rdfs:range rdf:resource="http://www.w3.org/2001/XMLSchema#dateTime"/>
    </owl:DatatypeProperty>
    


    <!-- http://www.semanticweb.org/sc3/ontologies/2022/0/Planning-Ontology#hasRequestedDate -->


    <owl:DatatypeProperty rdf:about="http://www.semanticweb.org/sc3/ontologies/2022/0/Planning-Ontology#hasRequestedDate">
        <rdfs:domain rdf:resource="http://www.semanticweb.org/sc3/ontologies/2022/0/ozone-ontology#Demand"/>
        <rdfs:range rdf:resource="http://www.w3.org/2001/XMLSchema#string"/>
    </owl:DatatypeProperty>
    


    <!-- http://www.semanticweb.org/sc3/ontologies/2022/0/Planning-Ontology#hasRevenue -->


    <owl:DatatypeProperty rdf:about="http://www.semanticweb.org/sc3/ontologies/2022/0/Planning-Ontology#hasRevenue">
        <rdfs:subPropertyOf rdf:resource="http://www.w3.org/2002/07/owl#topDataProperty"/>
        <rdfs:domain rdf:resource="http://www.semanticweb.org/sc3/ontologies/2022/0/Planning-Ontology#PlaningPurpose"/>
        <rdfs:range rdf:resource="http://www.w3.org/2001/XMLSchema#string"/>
        <rdfs:comment>Revenue refers to the amount of income, earning generated by the sale of one unit of a certain good.</rdfs:comment>
    </owl:DatatypeProperty>
    


    <!-- http://www.semanticweb.org/sc3/ontologies/2022/0/Planning-Ontology#hasSafetyStockLevel -->


    <owl:DatatypeProperty rdf:about="http://www.semanticweb.org/sc3/ontologies/2022/0/Planning-Ontology#hasSafetyStockLevel">
        <rdfs:domain rdf:resource="http://www.semanticweb.org/sc3/ontologies/2022/0/Planning-Ontology#InventoryPolicy"/>
        <rdfs:range rdf:resource="http://www.w3.org/2001/XMLSchema#int"/>
    </owl:DatatypeProperty>
    


    <!-- http://www.semanticweb.org/sc3/ontologies/2022/0/Planning-Ontology#hasSafetyStockTime -->


    <owl:DatatypeProperty rdf:about="http://www.semanticweb.org/sc3/ontologies/2022/0/Planning-Ontology#hasSafetyStockTime">
        <rdfs:domain rdf:resource="http://www.semanticweb.org/sc3/ontologies/2022/0/Planning-Ontology#InventoryPolicy"/>
        <rdfs:range rdf:resource="http://www.w3.org/2001/XMLSchema#string"/>
    </owl:DatatypeProperty>
    


    <!-- http://www.semanticweb.org/sc3/ontologies/2022/0/Planning-Ontology#hasSetOfConnections -->


    <owl:DatatypeProperty rdf:about="http://www.semanticweb.org/sc3/ontologies/2022/0/Planning-Ontology#hasSetOfConnections">
        <rdfs:subPropertyOf rdf:resource="http://www.w3.org/2002/07/owl#topDataProperty"/>
        <rdfs:domain rdf:resource="http://www.semanticweb.org/sc3/ontologies/2022/0/Planning-Ontology#PlanningSituation"/>
        <rdfs:range rdf:resource="http://www.w3.org/2001/XMLSchema#string"/>
    </owl:DatatypeProperty>
    


    <!-- http://www.semanticweb.org/sc3/ontologies/2022/0/Planning-Ontology#hasSoftConstraints -->


    <owl:DatatypeProperty rdf:about="http://www.semanticweb.org/sc3/ontologies/2022/0/Planning-Ontology#hasSoftConstraints">
        <rdfs:subPropertyOf rdf:resource="http://www.w3.org/2002/07/owl#topDataProperty"/>
        <rdfs:domain rdf:resource="http://www.semanticweb.org/sc3/ontologies/2022/0/Planning-Ontology#PlanningConstraint"/>
        <rdfs:range rdf:resource="http://www.w3.org/2001/XMLSchema#string"/>
        <rdfs:comment>PLANNING CONSTRAINTS with this property can be violated. This means that the degree of violation is typically penalized in a related criterion or performance measure.</rdfs:comment>
    </owl:DatatypeProperty>
    


    <!-- http://www.semanticweb.org/sc3/ontologies/2022/0/Planning-Ontology#hasStartDate -->


    <owl:DatatypeProperty rdf:about="http://www.semanticweb.org/sc3/ontologies/2022/0/Planning-Ontology#hasStartDate">
        <rdfs:domain rdf:resource="http://www.semanticweb.org/sc3/ontologies/2022/0/Planning-Ontology#Binning"/>
        <rdfs:domain rdf:resource="http://www.semanticweb.org/sc3/ontologies/2022/0/Planning-Ontology#InventoryPolicy"/>
        <rdfs:domain rdf:resource="http://www.semanticweb.org/sc3/ontologies/2022/0/Planning-Ontology#LotSizingRule"/>
        <rdfs:domain rdf:resource="http://www.semanticweb.org/sc3/ontologies/2022/0/Planning-Ontology#Substitution"/>
        <rdfs:range rdf:resource="http://www.w3.org/2001/XMLSchema#string"/>
    </owl:DatatypeProperty>
    


    <!-- http://www.semanticweb.org/sc3/ontologies/2022/0/Planning-Ontology#hasStartTime -->


    <owl:DatatypeProperty rdf:about="http://www.semanticweb.org/sc3/ontologies/2022/0/Planning-Ontology#hasStartTime">
        <rdfs:subPropertyOf rdf:resource="http://www.w3.org/2002/07/owl#topDataProperty"/>
        <rdfs:domain rdf:resource="http://www.semanticweb.org/sc3/ontologies/2022/0/Planning-Ontology#PlanningConstraint"/>
        <rdfs:range rdf:resource="http://www.w3.org/2001/XMLSchema#string"/>
        <rdfs:comment>This is the earliest point in time when the PLANNING CONSTRAINT is active.</rdfs:comment>
    </owl:DatatypeProperty>
    


    <!-- http://www.semanticweb.org/sc3/ontologies/2022/0/Planning-Ontology#hasSubstitutionQuantity -->


    <owl:DatatypeProperty rdf:about="http://www.semanticweb.org/sc3/ontologies/2022/0/Planning-Ontology#hasSubstitutionQuantity">
        <rdfs:domain rdf:resource="http://www.semanticweb.org/sc3/ontologies/2022/0/Planning-Ontology#Substitution"/>
        <rdfs:range rdf:resource="http://www.w3.org/2001/XMLSchema#int"/>
    </owl:DatatypeProperty>
    


    <!-- http://www.semanticweb.org/sc3/ontologies/2022/0/Planning-Ontology#hasTime -->


    <owl:DatatypeProperty rdf:about="http://www.semanticweb.org/sc3/ontologies/2022/0/Planning-Ontology#hasTime">
        <rdfs:subPropertyOf rdf:resource="http://www.w3.org/2002/07/owl#topDataProperty"/>
        <rdfs:domain rdf:resource="http://www.semanticweb.org/sc3/ontologies/2022/0/Planning-Ontology#PlanningObject"/>
        <rdfs:range rdf:resource="http://www.w3.org/2001/XMLSchema#string"/>
        <rdfs:comment>This property is required to manage timing aspects of a PLANNING OBJECT. It can be a release time, a finishing time, a single start time, or a set of start time for certain ACTIVITIES to be fulfilled.</rdfs:comment>
    </owl:DatatypeProperty>
    


    <!-- http://www.semanticweb.org/sc3/ontologies/2022/0/Planning-Ontology#hasType -->


    <owl:DatatypeProperty rdf:about="http://www.semanticweb.org/sc3/ontologies/2022/0/Planning-Ontology#hasType">
        <rdfs:domain rdf:resource="http://www.semanticweb.org/sc3/ontologies/2022/0/Planning-Ontology#InventoryPolicy"/>
        <rdfs:domain rdf:resource="http://www.semanticweb.org/sc3/ontologies/2022/0/Planning-Ontology#Order"/>
        <rdfs:domain rdf:resource="http://www.semanticweb.org/sc3/ontologies/2022/0/Planning-Ontology#SupplyInformation"/>
        <rdfs:range rdf:resource="http://www.w3.org/2001/XMLSchema#string"/>
    </owl:DatatypeProperty>
    


    <!-- http://www.semanticweb.org/sc3/ontologies/2022/0/Planning-Ontology#hasWeights -->


    <owl:DatatypeProperty rdf:about="http://www.semanticweb.org/sc3/ontologies/2022/0/Planning-Ontology#hasWeights">
        <rdfs:subPropertyOf rdf:resource="http://www.w3.org/2002/07/owl#topDataProperty"/>
        <rdfs:domain rdf:resource="http://www.semanticweb.org/sc3/ontologies/2022/0/Planning-Ontology#PlaningPurpose"/>
        <rdfs:range rdf:resource="http://www.w3.org/2001/XMLSchema#int"/>
        <rdfs:comment>Weights can be used to express preferences of the decision makers among the different performance measures and related criteria. This is, for instance, useful if a lexicographic approach is used.</rdfs:comment>
    </owl:DatatypeProperty>
    


    <!-- http://www.semanticweb.org/sc3/ontologies/2022/0/Planning-Ontology#numberOfOperationsOnSameResource -->


    <owl:DatatypeProperty rdf:about="http://www.semanticweb.org/sc3/ontologies/2022/0/Planning-Ontology#numberOfOperationsOnSameResource">
        <rdfs:domain rdf:resource="http://www.semanticweb.org/sc3/ontologies/2022/0/ozone-ontology#Product"/>
        <rdfs:range rdf:resource="http://www.w3.org/2001/XMLSchema#int"/>
    </owl:DatatypeProperty>
    


    <!-- http://www.w3.org/2002/07/owl#topDataProperty -->


    <rdf:Description rdf:about="http://www.w3.org/2002/07/owl#topDataProperty">
        <rdfs:comment>This is the earliest time where the activities associated with a PLANNING OBJECT can start. Note that the parameter RELEASE DATE is exogenous, i.e. given, in contrast to the property TIME.</rdfs:comment>
    </rdf:Description>
    


    <!-- http://www.w3.org/2006/time#day -->


    <owl:DatatypeProperty rdf:about="http://www.w3.org/2006/time#day">
        <rdfs:domain rdf:resource="http://www.w3.org/2006/time#GeneralDateTimeDescription"/>
        <rdfs:comment xml:lang="en">Day position in a calendar-clock system.

The range of this property is not specified, so can be replaced by any specific representation of a calendar day from any calendar. </rdfs:comment>
        <rdfs:comment xml:lang="es">Posición de día en un sistema calendario-reloj.</rdfs:comment>
        <rdfs:label xml:lang="en">day</rdfs:label>
        <rdfs:label xml:lang="es">día</rdfs:label>
        <skos:definition xml:lang="en">Day position in a calendar-clock system.

The range of this property is not specified, so can be replaced by any specific representation of a calendar day from any calendar. </skos:definition>
        <skos:definition xml:lang="es">Posición de día en un sistema calendario-reloj.

El rango de esta propiedad no está especificado, por tanto, se puede reemplazar por una representación específica de un día de calendario de cualquier calendario.</skos:definition>
    </owl:DatatypeProperty>
    


    <!-- http://www.w3.org/2006/time#dayOfYear -->


    <owl:DatatypeProperty rdf:about="http://www.w3.org/2006/time#dayOfYear">
        <rdfs:domain rdf:resource="http://www.w3.org/2006/time#GeneralDateTimeDescription"/>
        <rdfs:range rdf:resource="http://www.w3.org/2001/XMLSchema#nonNegativeInteger"/>
        <rdfs:comment xml:lang="es">El número de día en el año.</rdfs:comment>
        <rdfs:comment xml:lang="en">The number of the day within the year</rdfs:comment>
        <rdfs:label xml:lang="en">day of year</rdfs:label>
        <rdfs:label xml:lang="es">día del año</rdfs:label>
        <skos:definition xml:lang="es">El número de día en el año.</skos:definition>
        <skos:definition xml:lang="en">The number of the day within the year</skos:definition>
    </owl:DatatypeProperty>
    


    <!-- http://www.w3.org/2006/time#days -->


    <owl:DatatypeProperty rdf:about="http://www.w3.org/2006/time#days">
        <rdfs:domain rdf:resource="http://www.w3.org/2006/time#GeneralDurationDescription"/>
        <rdfs:range rdf:resource="http://www.w3.org/2001/XMLSchema#decimal"/>
        <rdfs:comment xml:lang="es">Longitud de, o elemento de la longitud de, una extensión temporal expresada en días.</rdfs:comment>
        <rdfs:comment xml:lang="en">length of, or element of the length of, a temporal extent expressed in days</rdfs:comment>
        <rdfs:label xml:lang="en">days duration</rdfs:label>
        <rdfs:label xml:lang="es">duración en días</rdfs:label>
        <skos:definition xml:lang="es">Longitud de, o elemento de la longitud de, una extensión temporal expresada en días.</skos:definition>
        <skos:definition xml:lang="en">length of, or element of the length of, a temporal extent expressed in days</skos:definition>
    </owl:DatatypeProperty>
    


    <!-- http://www.w3.org/2006/time#hasXSDDuration -->


    <owl:DatatypeProperty rdf:about="http://www.w3.org/2006/time#hasXSDDuration">
        <rdfs:domain rdf:resource="http://www.w3.org/2006/time#TemporalEntity"/>
        <rdfs:range rdf:resource="http://www.w3.org/2001/XMLSchema#duration"/>
        <rdfs:comment xml:lang="es">Extensión de una entidad temporal, expresada utilizando xsd:duration.</rdfs:comment>
        <rdfs:comment xml:lang="en">Extent of a temporal entity, expressed using xsd:duration</rdfs:comment>
        <rdfs:label xml:lang="en">has XSD duration</rdfs:label>
        <rdfs:label xml:lang="es">tiene duración XSD</rdfs:label>
        <skos:definition xml:lang="es">Extensión de una entidad temporal, expresada utilizando xsd:duration.</skos:definition>
        <skos:definition xml:lang="en">Extent of a temporal entity, expressed using xsd:duration</skos:definition>
        <skos:editorialNote xml:lang="es">Característica arriesgada - añadida en la revisión de 2017, y todavía no ampliamente utilizada.</skos:editorialNote>
        <skos:editorialNote xml:lang="en">Feature at risk - added in 2017 revision, and not yet widely used. </skos:editorialNote>
    </owl:DatatypeProperty>
    


    <!-- http://www.w3.org/2006/time#hour -->


    <owl:DatatypeProperty rdf:about="http://www.w3.org/2006/time#hour">
        <rdfs:domain rdf:resource="http://www.w3.org/2006/time#GeneralDateTimeDescription"/>
        <rdfs:range rdf:resource="http://www.w3.org/2001/XMLSchema#nonNegativeInteger"/>
        <rdfs:comment xml:lang="en">Hour position in a calendar-clock system.</rdfs:comment>
        <rdfs:comment xml:lang="es">Posición de hora en un sistema calendario-reloj.</rdfs:comment>
        <rdfs:label xml:lang="es">hora</rdfs:label>
        <rdfs:label xml:lang="en">hour</rdfs:label>
        <skos:definition xml:lang="en">Hour position in a calendar-clock system.</skos:definition>
        <skos:definition xml:lang="es">Posición de hora en un sistema calendario-reloj.</skos:definition>
    </owl:DatatypeProperty>
    


    <!-- http://www.w3.org/2006/time#hours -->


    <owl:DatatypeProperty rdf:about="http://www.w3.org/2006/time#hours">
        <rdfs:domain rdf:resource="http://www.w3.org/2006/time#GeneralDurationDescription"/>
        <rdfs:range rdf:resource="http://www.w3.org/2001/XMLSchema#decimal"/>
        <rdfs:comment xml:lang="es">Longitud de, o elemento de la longitud de, una extensión temporal expresada en horas.</rdfs:comment>
        <rdfs:comment xml:lang="en">length of, or element of the length of, a temporal extent expressed in hours</rdfs:comment>
        <rdfs:label xml:lang="es">duración en horas</rdfs:label>
        <rdfs:label xml:lang="en">hours duration</rdfs:label>
        <skos:definition xml:lang="es">Longitud de, o elemento de la longitud de, una extensión temporal expresada en horas.</skos:definition>
        <skos:definition xml:lang="en">length of, or element of the length of, a temporal extent expressed in hours</skos:definition>
    </owl:DatatypeProperty>
    


    <!-- http://www.w3.org/2006/time#inXSDDate -->


    <owl:DatatypeProperty rdf:about="http://www.w3.org/2006/time#inXSDDate">
        <rdfs:domain rdf:resource="http://www.w3.org/2006/time#Instant"/>
        <rdfs:range rdf:resource="http://www.w3.org/2001/XMLSchema#date"/>
        <rdfs:comment xml:lang="es">Posición de un instante, expresado utilizando xsd:date.</rdfs:comment>
        <rdfs:comment xml:lang="en">Position of an instant, expressed using xsd:date</rdfs:comment>
        <rdfs:label xml:lang="es">en fecha XSD</rdfs:label>
        <rdfs:label xml:lang="en">in XSD date</rdfs:label>
        <skos:definition xml:lang="es">Posición de un instante, expresado utilizando xsd:date.</skos:definition>
        <skos:definition xml:lang="en">Position of an instant, expressed using xsd:date</skos:definition>
    </owl:DatatypeProperty>
    


    <!-- http://www.w3.org/2006/time#inXSDDateTime -->


    <owl:DatatypeProperty rdf:about="http://www.w3.org/2006/time#inXSDDateTime">
        <rdfs:domain rdf:resource="http://www.w3.org/2006/time#Instant"/>
        <rdfs:range rdf:resource="http://www.w3.org/2001/XMLSchema#dateTime"/>
        <rdfs:comment xml:lang="es">Posición de un instante, expresado utilizando xsd:dateTime.</rdfs:comment>
        <rdfs:comment xml:lang="en">Position of an instant, expressed using xsd:dateTime</rdfs:comment>
        <rdfs:label xml:lang="es">en fecha-tiempo XSD</rdfs:label>
        <rdfs:label xml:lang="en">in XSD Date-Time</rdfs:label>
        <owl:deprecated rdf:datatype="http://www.w3.org/2001/XMLSchema#boolean">true</owl:deprecated>
        <skos:definition xml:lang="es">Posición de un instante, expresado utilizando xsd:dateTime.</skos:definition>
        <skos:definition xml:lang="en">Position of an instant, expressed using xsd:dateTime</skos:definition>
        <skos:note xml:lang="es">La propiedad &apos;en fecha-hora XSD&apos; ha sido reemplazada por &apos;en fecha-sello de tiempo XSD&apos; que hace obligatorio el campo &apos;huso horario&apos;.</skos:note>
        <skos:note xml:lang="en">The property :inXSDDateTime is replaced by :inXSDDateTimeStamp which makes the time-zone field mandatory.</skos:note>
    </owl:DatatypeProperty>
    


    <!-- http://www.w3.org/2006/time#inXSDDateTimeStamp -->


    <owl:DatatypeProperty rdf:about="http://www.w3.org/2006/time#inXSDDateTimeStamp">
        <rdfs:domain rdf:resource="http://www.w3.org/2006/time#Instant"/>
        <rdfs:range rdf:resource="http://www.w3.org/2001/XMLSchema#dateTimeStamp"/>
        <rdfs:comment xml:lang="es">Posición de un instante, expresado utilizando xsd:dateTimeStamp.</rdfs:comment>
        <rdfs:comment xml:lang="en">Position of an instant, expressed using xsd:dateTimeStamp</rdfs:comment>
        <rdfs:label xml:lang="es">en fecha-sello de tiempo XSD</rdfs:label>
        <rdfs:label xml:lang="en">in XSD Date-Time-Stamp</rdfs:label>
        <skos:definition xml:lang="es">Posición de un instante, expresado utilizando xsd:dateTimeStamp.</skos:definition>
        <skos:definition xml:lang="en">Position of an instant, expressed using xsd:dateTimeStamp</skos:definition>
    </owl:DatatypeProperty>
    


    <!-- http://www.w3.org/2006/time#inXSDgYear -->


    <owl:DatatypeProperty rdf:about="http://www.w3.org/2006/time#inXSDgYear">
        <rdfs:domain rdf:resource="http://www.w3.org/2006/time#Instant"/>
        <rdfs:range rdf:resource="http://www.w3.org/2001/XMLSchema#gYear"/>
        <rdfs:comment xml:lang="es">Posición de un instante, expresado utilizando xsd:gYear.</rdfs:comment>
        <rdfs:comment xml:lang="en">Position of an instant, expressed using xsd:gYear</rdfs:comment>
        <rdfs:label xml:lang="es">en año gregoriano XSD</rdfs:label>
        <rdfs:label xml:lang="en">in XSD g-Year</rdfs:label>
        <skos:definition xml:lang="es">Posición de un instante, expresado utilizando xsd:gYear.</skos:definition>
        <skos:definition xml:lang="en">Position of an instant, expressed using xsd:gYear</skos:definition>
    </owl:DatatypeProperty>
    


    <!-- http://www.w3.org/2006/time#inXSDgYearMonth -->


    <owl:DatatypeProperty rdf:about="http://www.w3.org/2006/time#inXSDgYearMonth">
        <rdfs:domain rdf:resource="http://www.w3.org/2006/time#Instant"/>
        <rdfs:range rdf:resource="http://www.w3.org/2001/XMLSchema#gYearMonth"/>
        <rdfs:comment xml:lang="es">Posición de un instante, expresado utilizando xsd:gYearMonth.</rdfs:comment>
        <rdfs:comment xml:lang="en">Position of an instant, expressed using xsd:gYearMonth</rdfs:comment>
        <rdfs:label xml:lang="es">en año-mes gregoriano XSD</rdfs:label>
        <rdfs:label xml:lang="en">in XSD g-YearMonth</rdfs:label>
        <skos:definition xml:lang="es">Posición de un instante, expresado utilizando xsd:gYearMonth.</skos:definition>
        <skos:definition xml:lang="en">Position of an instant, expressed using xsd:gYearMonth</skos:definition>
    </owl:DatatypeProperty>
    


    <!-- http://www.w3.org/2006/time#minute -->


    <owl:DatatypeProperty rdf:about="http://www.w3.org/2006/time#minute">
        <rdfs:domain rdf:resource="http://www.w3.org/2006/time#GeneralDateTimeDescription"/>
        <rdfs:range rdf:resource="http://www.w3.org/2001/XMLSchema#nonNegativeInteger"/>
        <rdfs:comment xml:lang="en">Minute position in a calendar-clock system.</rdfs:comment>
        <rdfs:comment xml:lang="es">Posición de minuto en un sistema calendario-reloj.</rdfs:comment>
        <rdfs:label xml:lang="en">minute</rdfs:label>
        <rdfs:label xml:lang="es">minuto</rdfs:label>
        <skos:definition xml:lang="en">Minute position in a calendar-clock system.</skos:definition>
        <skos:definition xml:lang="es">Posición de minuto en un sistema calendario-reloj.</skos:definition>
    </owl:DatatypeProperty>
    


    <!-- http://www.w3.org/2006/time#minutes -->


    <owl:DatatypeProperty rdf:about="http://www.w3.org/2006/time#minutes">
        <rdfs:domain rdf:resource="http://www.w3.org/2006/time#GeneralDurationDescription"/>
        <rdfs:range rdf:resource="http://www.w3.org/2001/XMLSchema#decimal"/>
        <rdfs:comment xml:lang="es">Longitud de, o elemento de la longitud de, una extensión temporal expresada en minutos.</rdfs:comment>
        <rdfs:comment xml:lang="en">length, or element of, a temporal extent expressed in minutes</rdfs:comment>
        <rdfs:label xml:lang="en">minutes</rdfs:label>
        <rdfs:label xml:lang="es">minutos</rdfs:label>
        <skos:definition xml:lang="es">Longitud de, o elemento de la longitud de, una extensión temporal expresada en minutos.</skos:definition>
        <skos:definition xml:lang="en">length, or element of, a temporal extent expressed in minutes</skos:definition>
    </owl:DatatypeProperty>
    


    <!-- http://www.w3.org/2006/time#month -->


    <owl:DatatypeProperty rdf:about="http://www.w3.org/2006/time#month">
        <rdfs:domain rdf:resource="http://www.w3.org/2006/time#GeneralDateTimeDescription"/>
        <rdfs:comment xml:lang="en">Month position in a calendar-clock system.

The range of this property is not specified, so can be replaced by any specific representation of a calendar month from any calendar. </rdfs:comment>
        <rdfs:comment xml:lang="es">Posición de mes en un sistema calendario-reloj.
    El rango de esta propiedad no está especificado, por tanto, se puede reemplazar por cualquier representación específica de un mes de calendario de un calendario cualquiera.</rdfs:comment>
        <rdfs:label xml:lang="es">mes</rdfs:label>
        <rdfs:label xml:lang="en">month</rdfs:label>
        <skos:definition xml:lang="en">Month position in a calendar-clock system.

The range of this property is not specified, so can be replaced by any specific representation of a calendar month from any calendar. </skos:definition>
        <skos:definition xml:lang="es">Posición de mes en un sistema calendario-reloj.
            El rango de esta propiedad no está especificado, por tanto, se puede reemplazar por cualquier representación específica de un mes de calendario de un calendario cualquiera.</skos:definition>
    </owl:DatatypeProperty>
    


    <!-- http://www.w3.org/2006/time#months -->


    <owl:DatatypeProperty rdf:about="http://www.w3.org/2006/time#months">
        <rdfs:domain rdf:resource="http://www.w3.org/2006/time#GeneralDurationDescription"/>
        <rdfs:range rdf:resource="http://www.w3.org/2001/XMLSchema#decimal"/>
        <rdfs:comment xml:lang="es">Longitud de, o elemento de la longitud de, una extensión temporal expresada en meses.</rdfs:comment>
        <rdfs:comment xml:lang="en">length of, or element of the length of, a temporal extent expressed in months</rdfs:comment>
        <rdfs:label xml:lang="es">duración en meses</rdfs:label>
        <rdfs:label xml:lang="en">months duration</rdfs:label>
        <skos:definition xml:lang="es">Longitud de, o elemento de la longitud de, una extensión temporal expresada en meses.</skos:definition>
        <skos:definition xml:lang="en">length of, or element of the length of, a temporal extent expressed in months</skos:definition>
    </owl:DatatypeProperty>
    


    <!-- http://www.w3.org/2006/time#nominalPosition -->


    <owl:DatatypeProperty rdf:about="http://www.w3.org/2006/time#nominalPosition">
        <rdfs:domain rdf:resource="http://www.w3.org/2006/time#TimePosition"/>
        <rdfs:range rdf:resource="http://www.w3.org/2001/XMLSchema#string"/>
        <rdfs:comment xml:lang="es">El valor (nominal) que indica posición temporal en un sistema de referencia ordinal.</rdfs:comment>
        <rdfs:comment xml:lang="en">The (nominal) value indicating temporal position in an ordinal reference system </rdfs:comment>
        <rdfs:label xml:lang="en">Name of temporal position</rdfs:label>
        <rdfs:label xml:lang="es">nombre de posición temporal</rdfs:label>
        <skos:definition xml:lang="es">El valor (nominal) que indica posición temporal en un sistema de referencia ordinal.</skos:definition>
        <skos:definition xml:lang="en">The (nominal) value indicating temporal position in an ordinal reference system </skos:definition>
    </owl:DatatypeProperty>
    


    <!-- http://www.w3.org/2006/time#numericDuration -->


    <owl:DatatypeProperty rdf:about="http://www.w3.org/2006/time#numericDuration">
        <rdfs:domain rdf:resource="http://www.w3.org/2006/time#Duration"/>
        <rdfs:range rdf:resource="http://www.w3.org/2001/XMLSchema#decimal"/>
        <rdfs:comment xml:lang="es">Valor de una extensión temporal expresada como un número decimal escalado por una unidad de tiempo.</rdfs:comment>
        <rdfs:comment xml:lang="en">Value of a temporal extent expressed as a decimal number scaled by a temporal unit</rdfs:comment>
        <rdfs:label xml:lang="en">Numeric value of temporal duration</rdfs:label>
        <rdfs:label xml:lang="es">valor numérico de duración temporal</rdfs:label>
        <skos:definition xml:lang="es">Valor de una extensión temporal expresada como un número decimal escalado por una unidad de tiempo.</skos:definition>
        <skos:definition xml:lang="en">Value of a temporal extent expressed as a decimal number scaled by a temporal unit</skos:definition>
    </owl:DatatypeProperty>
    


    <!-- http://www.w3.org/2006/time#numericPosition -->


    <owl:DatatypeProperty rdf:about="http://www.w3.org/2006/time#numericPosition">
        <rdfs:domain rdf:resource="http://www.w3.org/2006/time#TimePosition"/>
        <rdfs:range rdf:resource="http://www.w3.org/2001/XMLSchema#decimal"/>
        <rdfs:comment xml:lang="es">El valor (numérico) que indica posición temporal en un sistema de referencia ordinal.</rdfs:comment>
        <rdfs:comment xml:lang="en">The (numeric) value indicating position within a temporal coordinate system </rdfs:comment>
        <rdfs:label xml:lang="en">Numeric value of temporal position</rdfs:label>
        <rdfs:label xml:lang="es">valor numérico de posición temporal</rdfs:label>
        <skos:definition xml:lang="es">El valor (numérico) que indica posición temporal en un sistema de referencia ordinal.</skos:definition>
        <skos:definition xml:lang="en">The (numeric) value indicating position within a temporal coordinate system </skos:definition>
    </owl:DatatypeProperty>
    


    <!-- http://www.w3.org/2006/time#second -->


    <owl:DatatypeProperty rdf:about="http://www.w3.org/2006/time#second">
        <rdfs:domain rdf:resource="http://www.w3.org/2006/time#GeneralDateTimeDescription"/>
        <rdfs:range rdf:resource="http://www.w3.org/2001/XMLSchema#decimal"/>
        <rdfs:comment xml:lang="es">Posición de segundo en un sistema calendario-reloj.</rdfs:comment>
        <rdfs:comment xml:lang="en">Second position in a calendar-clock system.</rdfs:comment>
        <rdfs:label xml:lang="en">second</rdfs:label>
        <rdfs:label xml:lang="es">segundo</rdfs:label>
    </owl:DatatypeProperty>
    


    <!-- http://www.w3.org/2006/time#seconds -->


    <owl:DatatypeProperty rdf:about="http://www.w3.org/2006/time#seconds">
        <rdfs:domain rdf:resource="http://www.w3.org/2006/time#GeneralDurationDescription"/>
        <rdfs:range rdf:resource="http://www.w3.org/2001/XMLSchema#decimal"/>
        <rdfs:comment xml:lang="es">Longitud de, o elemento de la longitud de, una extensión temporal expresada en segundos.</rdfs:comment>
        <rdfs:comment xml:lang="en">length of, or element of the length of, a temporal extent expressed in seconds</rdfs:comment>
        <rdfs:label xml:lang="es">duración en segundos</rdfs:label>
        <rdfs:label xml:lang="en">seconds duration</rdfs:label>
        <rdfs:seeAlso rdf:resource="http://www.bipm.org/en/publications/si-brochure/second.html"/>
    </owl:DatatypeProperty>
    


    <!-- http://www.w3.org/2006/time#week -->


    <owl:DatatypeProperty rdf:about="http://www.w3.org/2006/time#week">
        <rdfs:domain rdf:resource="http://www.w3.org/2006/time#GeneralDateTimeDescription"/>
        <rdfs:range rdf:resource="http://www.w3.org/2001/XMLSchema#nonNegativeInteger"/>
        <rdfs:comment xml:lang="es">Número de semana en el año.</rdfs:comment>
        <rdfs:comment xml:lang="en">Week number within the year.</rdfs:comment>
        <rdfs:label xml:lang="es">semana</rdfs:label>
        <rdfs:label xml:lang="en">week</rdfs:label>
        <skos:note xml:lang="en">Weeks are numbered differently depending on the calendar in use and the local language or cultural conventions (locale). ISO-8601 specifies that the first week of the year includes at least four days, and that Monday is the first day of the week. In that system, week 1 is the week that contains the first Thursday in the year.</skos:note>
        <skos:scopeNote xml:lang="es">Las semanas están numeradas de forma diferente dependiendo del calendario en uso y de las convenciones lingüísticas y culturales locales (locale en inglés). El ISO-8601 especifica que la primera semana del año incluye al menos cuatro días, y que el lunes es el primer día de la semana. En ese sistema, la semana 1 es la semana que contiene el primer jueves del año.</skos:scopeNote>
    </owl:DatatypeProperty>
    


    <!-- http://www.w3.org/2006/time#weeks -->


    <owl:DatatypeProperty rdf:about="http://www.w3.org/2006/time#weeks">
        <rdfs:domain rdf:resource="http://www.w3.org/2006/time#GeneralDurationDescription"/>
        <rdfs:range rdf:resource="http://www.w3.org/2001/XMLSchema#decimal"/>
        <rdfs:comment xml:lang="es">Longitud de, o elemento de la longitud de, una extensión temporal expresada en semanas.</rdfs:comment>
        <rdfs:comment xml:lang="en">length of, or element of the length of, a temporal extent expressed in weeks</rdfs:comment>
        <rdfs:label xml:lang="es">duración en semanas</rdfs:label>
        <rdfs:label xml:lang="en">weeks duration</rdfs:label>
    </owl:DatatypeProperty>
    


    <!-- http://www.w3.org/2006/time#xsdDateTime -->


    <owl:DatatypeProperty rdf:about="http://www.w3.org/2006/time#xsdDateTime">
        <rdfs:domain rdf:resource="http://www.w3.org/2006/time#DateTimeInterval"/>
        <rdfs:range rdf:resource="http://www.w3.org/2001/XMLSchema#dateTime"/>
        <rdfs:comment xml:lang="es">Valor de &apos;intervalo de fecha-hora&apos; expresado como un valor compacto.</rdfs:comment>
        <rdfs:comment xml:lang="en">Value of DateTimeInterval expressed as a compact value.</rdfs:comment>
        <rdfs:label xml:lang="en">has XSD date-time</rdfs:label>
        <rdfs:label xml:lang="es">tiene fecha-hora XSD</rdfs:label>
        <owl:deprecated rdf:datatype="http://www.w3.org/2001/XMLSchema#boolean">true</owl:deprecated>
        <skos:note xml:lang="en">Using xsd:dateTime in this place means that the duration of the interval is implicit: it corresponds to the length of the smallest non-zero element of the date-time literal. However, this rule cannot be used for intervals whose duration is more than one rank smaller than the starting time - e.g. the first minute or second of a day, the first hour of a month, or the first day of a year. In these cases the desired interval cannot be distinguished from the interval corresponding to the next rank up. Because of this essential ambiguity, use of this property is not recommended and it is deprecated.</skos:note>
        <skos:note>Utilizando xsd:dateTime en este lugar significa que la duración del intervalo está implícita: se corresponde con la longitud del elemento más pequeño distinto de cero del literal fecha-hora. Sin embargo, esta regla no se puede utilizar para intervalos cuya duración es mayor que un rango más pequeño que el tiempo de comienzo - p.ej. el primer minuto o segundo del día, la primera hora del mes, o el primer día del año. En estos casos el intervalo deseado no se puede distinguir del intervalo correspondiente al próximo rango más alto. Debido a esta ambigüedad esencial, no se recomienda el uso de esta propiedad y está desaprobada.</skos:note>
    </owl:DatatypeProperty>
    


    <!-- http://www.w3.org/2006/time#year -->


    <owl:DatatypeProperty rdf:about="http://www.w3.org/2006/time#year">
        <rdfs:domain rdf:resource="http://www.w3.org/2006/time#GeneralDateTimeDescription"/>
        <rdfs:comment xml:lang="es">Posición de año en un sistema calendario-reloj.

l rango de esta propiedad no está especificado, por tanto, se puede reemplazar por cualquier representación específica de un año de calendario de un calendario cualquiera.</rdfs:comment>
        <rdfs:comment xml:lang="en">Year position in a calendar-clock system.

The range of this property is not specified, so can be replaced by any specific representation of a calendar year from any calendar. </rdfs:comment>
        <rdfs:label xml:lang="en">year</rdfs:label>
    </owl:DatatypeProperty>
    


    <!-- http://www.w3.org/2006/time#years -->


    <owl:DatatypeProperty rdf:about="http://www.w3.org/2006/time#years">
        <rdfs:domain rdf:resource="http://www.w3.org/2006/time#GeneralDurationDescription"/>
        <rdfs:range rdf:resource="http://www.w3.org/2001/XMLSchema#decimal"/>
        <rdfs:comment xml:lang="es">Longitud de, o elemento de la longitud de, una extensión temporal expresada en años.</rdfs:comment>
        <rdfs:comment xml:lang="en">length of, or element of the length of, a temporal extent expressed in years</rdfs:comment>
        <rdfs:label xml:lang="es">duración en años</rdfs:label>
        <rdfs:label xml:lang="en">years duration</rdfs:label>
    </owl:DatatypeProperty>
    


    <!-- 
    ///////////////////////////////////////////////////////////////////////////////////////
    //
    // Classes
    //
    ///////////////////////////////////////////////////////////////////////////////////////
     -->


    


    <!-- http://www.semanticweb.org/sc3/ontologies/2022/0/Planning-Ontology#Activity -->


    <owl:Class rdf:about="http://www.semanticweb.org/sc3/ontologies/2022/0/Planning-Ontology#Activity"/>
    


    <!-- http://www.semanticweb.org/sc3/ontologies/2022/0/Planning-Ontology#Automated -->


    <owl:Class rdf:about="http://www.semanticweb.org/sc3/ontologies/2022/0/Planning-Ontology#Automated">
        <rdfs:subClassOf rdf:resource="http://www.semanticweb.org/sc3/ontologies/2022/0/Planning-Ontology#DecisionMakerType"/>
    </owl:Class>
    


    <!-- http://www.semanticweb.org/sc3/ontologies/2022/0/Planning-Ontology#Autonomous -->


    <owl:Class rdf:about="http://www.semanticweb.org/sc3/ontologies/2022/0/Planning-Ontology#Autonomous">
        <rdfs:subClassOf rdf:resource="http://www.semanticweb.org/sc3/ontologies/2022/0/Planning-Ontology#DecisionMakingInitiative"/>
    </owl:Class>
    


    <!-- http://www.semanticweb.org/sc3/ontologies/2022/0/Planning-Ontology#AvailableCapacity -->


    <owl:Class rdf:about="http://www.semanticweb.org/sc3/ontologies/2022/0/Planning-Ontology#AvailableCapacity">
        <rdfs:subClassOf rdf:resource="http://www.semanticweb.org/sc3/ontologies/2022/0/Planning-Ontology#Capacity"/>
        <rdfs:comment>: The AVAILABLE CAPACITY describes the ability of a resource within a period of time to perform activities or processes. Elmaghraby (2011) refers to this as operational capacity, i.e. the productive capacity that is obtained from the nominal capacity by subtracting the anticipated and unavoidable loss in productivity, for instance, due to machine breakdowns in a wafer fab.</rdfs:comment>
    </owl:Class>
    


    <!-- http://www.semanticweb.org/sc3/ontologies/2022/0/Planning-Ontology#BillOfMaterial -->


    <owl:Class rdf:about="http://www.semanticweb.org/sc3/ontologies/2022/0/Planning-Ontology#BillOfMaterial">
        <rdfs:comment>A BILL OF MATERIALS (BOM) describes the component products used to make another product. Substitution, often associated with binning, is based on the possibility that alternative items might be used to finish a process step.</rdfs:comment>
    </owl:Class>
    


    <!-- http://www.semanticweb.org/sc3/ontologies/2022/0/Planning-Ontology#Bin -->


    <owl:Class rdf:about="http://www.semanticweb.org/sc3/ontologies/2022/0/Planning-Ontology#Bin"/>
    


    <!-- http://www.semanticweb.org/sc3/ontologies/2022/0/Planning-Ontology#Binning -->


    <owl:Class rdf:about="http://www.semanticweb.org/sc3/ontologies/2022/0/Planning-Ontology#Binning">
        <rdfs:comment>BINNING refers to the process of testing and categorizing parts against defined measures and sort them into different bins (Degbotse 2013). Each bin belongs to certain levels of defined measures (e.g. chip speed, current, voltage, energy consumption). Binning is often combined with SUBSTITUTION.</rdfs:comment>
    </owl:Class>
    


    <!-- http://www.semanticweb.org/sc3/ontologies/2022/0/Planning-Ontology#Capacity -->


    <owl:Class rdf:about="http://www.semanticweb.org/sc3/ontologies/2022/0/Planning-Ontology#Capacity"/>
    


    <!-- http://www.semanticweb.org/sc3/ontologies/2022/0/Planning-Ontology#ComponentPart -->


    <owl:Class rdf:about="http://www.semanticweb.org/sc3/ontologies/2022/0/Planning-Ontology#ComponentPart">
        <rdfs:subClassOf rdf:resource="http://www.semanticweb.org/sc3/ontologies/2022/0/Planning-Ontology#Part"/>
    </owl:Class>
    


    <!-- http://www.semanticweb.org/sc3/ontologies/2022/0/Planning-Ontology#Criteria -->


    <owl:Class rdf:about="http://www.semanticweb.org/sc3/ontologies/2022/0/Planning-Ontology#Criteria">
        <rdfs:comment>Typical criteria are maximization, minimization, i.e. if an optimization problem is considered, or larger or smaller than a prescribed value of the certain performance measure, a so-called target, i.e. if a satisfaction problem is solved. In a multi-criteria setting, the dominance concept for plans is of interest.</rdfs:comment>
    </owl:Class>
    


    <!-- http://www.semanticweb.org/sc3/ontologies/2022/0/Planning-Ontology#DecisionMakerType -->


    <owl:Class rdf:about="http://www.semanticweb.org/sc3/ontologies/2022/0/Planning-Ontology#DecisionMakerType">
        <rdfs:comment>We distinguish human decision-makers (human DECISION-MAKING UNITS) from fully automated DECISION-MAKING UNITS where computers make fully automated decisions. Between these two extremes there are semi-automated decisions, where a computer provides several decision alternatives and a human decision-maker chooses among them. Note that the decision-maker type can change over time.</rdfs:comment>
    </owl:Class>
    


    <!-- http://www.semanticweb.org/sc3/ontologies/2022/0/Planning-Ontology#DecisionMakingInitiative -->


    <owl:Class rdf:about="http://www.semanticweb.org/sc3/ontologies/2022/0/Planning-Ontology#DecisionMakingInitiative">
        <rdfs:comment>We distinguish fully autonomous DECISION-MAKING UNITS from DECISION-MAKING UNITS where the decision-making activities are triggered by other DECISION-MAKING UNITS. Note that the decision-making initiative can change over time in a situation-dependent manner.</rdfs:comment>
    </owl:Class>
    


    <!-- http://www.semanticweb.org/sc3/ontologies/2022/0/Planning-Ontology#DecisionMakingUnit -->


    <owl:Class rdf:about="http://www.semanticweb.org/sc3/ontologies/2022/0/Planning-Ontology#DecisionMakingUnit">
        <rdfs:comment>The DECISION-MAKING UNIT specifies an instance that makes decisions.</rdfs:comment>
    </owl:Class>
    


    <!-- http://www.semanticweb.org/sc3/ontologies/2022/0/Planning-Ontology#DecisonMakingUnitCharacter -->


    <owl:Class rdf:about="http://www.semanticweb.org/sc3/ontologies/2022/0/Planning-Ontology#DecisonMakingUnitCharacter">
        <rdfs:comment>In an ANTAGO¬NISTIC SETTING, the different DECISION-MAKING UNITS try to meet their own objectives which are in conflict. In a non-antagonistic setting, the DECISION-MAKING UNITS do not exploit their private knowledge in an opportunistic way.</rdfs:comment>
    </owl:Class>
    


    <!-- http://www.semanticweb.org/sc3/ontologies/2022/0/Planning-Ontology#Dependent -->


    <owl:Class rdf:about="http://www.semanticweb.org/sc3/ontologies/2022/0/Planning-Ontology#Dependent">
        <rdfs:subClassOf rdf:resource="http://www.semanticweb.org/sc3/ontologies/2022/0/Planning-Ontology#DecisionMakingInitiative"/>
    </owl:Class>
    


    <!-- http://www.semanticweb.org/sc3/ontologies/2022/0/Planning-Ontology#DistributedHierarchicalSituation -->


    <owl:Class rdf:about="http://www.semanticweb.org/sc3/ontologies/2022/0/Planning-Ontology#DistributedHierarchicalSituation">
        <rdfs:subClassOf rdf:resource="http://www.semanticweb.org/sc3/ontologies/2022/0/Planning-Ontology#HierarchicalSituation"/>
        <rdfs:comment>In this situation, edges referring to instructions and reactions are possible.</rdfs:comment>
    </owl:Class>
    


    <!-- http://www.semanticweb.org/sc3/ontologies/2022/0/Planning-Ontology#Edge -->


    <owl:Class rdf:about="http://www.semanticweb.org/sc3/ontologies/2022/0/Planning-Ontology#Edge"/>
    


    <!-- http://www.semanticweb.org/sc3/ontologies/2022/0/Planning-Ontology#FrozenFence -->


    <owl:Class rdf:about="http://www.semanticweb.org/sc3/ontologies/2022/0/Planning-Ontology#FrozenFence">
        <rdfs:comment>FROZEN FENCE is used to set a frozen interval  in which decision making is not allowed to change the previously determined values.</rdfs:comment>
    </owl:Class>
    


    <!-- http://www.semanticweb.org/sc3/ontologies/2022/0/Planning-Ontology#HeterarchicalSituation -->


    <owl:Class rdf:about="http://www.semanticweb.org/sc3/ontologies/2022/0/Planning-Ontology#HeterarchicalSituation">
        <rdfs:subClassOf rdf:resource="http://www.semanticweb.org/sc3/ontologies/2022/0/Planning-Ontology#HierarchicalSituation"/>
        <rdfs:comment>All the vertices have level 1.</rdfs:comment>
    </owl:Class>
    


    <!-- http://www.semanticweb.org/sc3/ontologies/2022/0/Planning-Ontology#HierarchicalSituation -->


    <owl:Class rdf:about="http://www.semanticweb.org/sc3/ontologies/2022/0/Planning-Ontology#HierarchicalSituation"/>
    


    <!-- http://www.semanticweb.org/sc3/ontologies/2022/0/Planning-Ontology#Human -->


    <owl:Class rdf:about="http://www.semanticweb.org/sc3/ontologies/2022/0/Planning-Ontology#Human">
        <rdfs:subClassOf rdf:resource="http://www.semanticweb.org/sc3/ontologies/2022/0/Planning-Ontology#DecisionMakerType"/>
    </owl:Class>
    


    <!-- http://www.semanticweb.org/sc3/ontologies/2022/0/Planning-Ontology#In-TransitInventory -->


    <owl:Class rdf:about="http://www.semanticweb.org/sc3/ontologies/2022/0/Planning-Ontology#In-TransitInventory">
        <rdfs:comment>The IN-TRANSIT INVENTORY describes the quantity of a certain product that is shipped from one location to another. This quantity has left the inventory of one location, but has not yet been received into the inventory of the receiving location.</rdfs:comment>
    </owl:Class>
    


    <!-- http://www.semanticweb.org/sc3/ontologies/2022/0/Planning-Ontology#Inventory -->


    <owl:Class rdf:about="http://www.semanticweb.org/sc3/ontologies/2022/0/Planning-Ontology#Inventory">
        <rdfs:comment>The INVENTORY describes the quantity of a certain product that is available in stock to be used to meet demand.</rdfs:comment>
    </owl:Class>
    


    <!-- http://www.semanticweb.org/sc3/ontologies/2022/0/Planning-Ontology#InventoryPolicy -->


    <owl:Class rdf:about="http://www.semanticweb.org/sc3/ontologies/2022/0/Planning-Ontology#InventoryPolicy">
        <rdfs:comment>An INVENTORY POLICY indicates how much earlier or how much more (safety stock) needs to be built than that required to satisfy demand on time. Inventory Policies define the rules which have to be implemented at a specific inventory location such as safety stock or product mix for supporting the production process flow as well as fulfilling customer demand.</rdfs:comment>
    </owl:Class>
    


    <!-- http://www.semanticweb.org/sc3/ontologies/2022/0/Planning-Ontology#Location -->


    <owl:Class rdf:about="http://www.semanticweb.org/sc3/ontologies/2022/0/Planning-Ontology#Location">
        <rdfs:comment></rdfs:comment>
    </owl:Class>
    


    <!-- http://www.semanticweb.org/sc3/ontologies/2022/0/Planning-Ontology#LotSizingRule -->


    <owl:Class rdf:about="http://www.semanticweb.org/sc3/ontologies/2022/0/Planning-Ontology#LotSizingRule">
        <rdfs:comment>A LOT SIZING RULE defines a rule to specify the lot size for a specific part. The lot size on the other hand defines the number of pieces belonging to a part. The lot size is the result of applying lot sizing rules.</rdfs:comment>
    </owl:Class>
    


    <!-- http://www.semanticweb.org/sc3/ontologies/2022/0/Planning-Ontology#MacroOperation -->


    <owl:Class rdf:about="http://www.semanticweb.org/sc3/ontologies/2022/0/Planning-Ontology#MacroOperation"/>
    


    <!-- http://www.semanticweb.org/sc3/ontologies/2022/0/Planning-Ontology#Order -->


    <owl:Class rdf:about="http://www.semanticweb.org/sc3/ontologies/2022/0/Planning-Ontology#Order"/>
    


    <!-- http://www.semanticweb.org/sc3/ontologies/2022/0/Planning-Ontology#Owner -->


    <owl:Class rdf:about="http://www.semanticweb.org/sc3/ontologies/2022/0/Planning-Ontology#Owner"/>
    


    <!-- http://www.semanticweb.org/sc3/ontologies/2022/0/Planning-Ontology#Part -->


    <owl:Class rdf:about="http://www.semanticweb.org/sc3/ontologies/2022/0/Planning-Ontology#Part">
        <rdfs:comment>A PART represents a physical instance of a product in the manufacturing process. It therefore realizes a product. A part moves through the system and is manufactured according to its product specification. A part is associated to exactly one product. During the production process it is typically tested several times. The binning rules of the associated product specification can be applied to the respective part. A part can be substituted by another part according to the associated product specification</rdfs:comment>
    </owl:Class>
    


    <!-- http://www.semanticweb.org/sc3/ontologies/2022/0/Planning-Ontology#PerformanceMeasure -->


    <owl:Class rdf:about="http://www.semanticweb.org/sc3/ontologies/2022/0/Planning-Ontology#PerformanceMeasure">
        <rdfs:comment>Each measure is defined by a calculation procedure. Performance measures can be blended using weights to express the importance of the different measures.</rdfs:comment>
    </owl:Class>
    


    <!-- http://www.semanticweb.org/sc3/ontologies/2022/0/Planning-Ontology#Plan -->


    <owl:Class rdf:about="http://www.semanticweb.org/sc3/ontologies/2022/0/Planning-Ontology#Plan">
        <rdfs:comment>A PLAN is an activity specification with an intended purpose.</rdfs:comment>
    </owl:Class>
    


    <!-- http://www.semanticweb.org/sc3/ontologies/2022/0/Planning-Ontology#PlanExecutuon -->


    <owl:Class rdf:about="http://www.semanticweb.org/sc3/ontologies/2022/0/Planning-Ontology#PlanExecutuon">
        <rdfs:comment>A PLAN EXECUTION is related to performing the activities according to a PLAN either directly in the base system, for instance, releasing lots into a wafer fab, or as instructions for another DECISION-MAKING UNIT.</rdfs:comment>
    </owl:Class>
    


    <!-- http://www.semanticweb.org/sc3/ontologies/2022/0/Planning-Ontology#PlaningPurpose -->


    <owl:Class rdf:about="http://www.semanticweb.org/sc3/ontologies/2022/0/Planning-Ontology#PlaningPurpose">
        <rdfs:comment></rdfs:comment>
        <rdfs:comment>The PLANNING PURPOSE specifies the objectives of a certain planning activity. It is given by a set of performance measures that are related to a set of PLANNING OBJECTS.</rdfs:comment>
    </owl:Class>
    


    <!-- http://www.semanticweb.org/sc3/ontologies/2022/0/Planning-Ontology#PlanningApproach -->


    <owl:Class rdf:about="http://www.semanticweb.org/sc3/ontologies/2022/0/Planning-Ontology#PlanningApproach">
        <rdfs:comment>Specific planning algorithm which is used in a deticated planning process</rdfs:comment>
    </owl:Class>
    


    <!-- http://www.semanticweb.org/sc3/ontologies/2022/0/Planning-Ontology#PlanningConstraint -->


    <owl:Class rdf:about="http://www.semanticweb.org/sc3/ontologies/2022/0/Planning-Ontology#PlanningConstraint">
        <rdfs:comment>A PLANNING CONSTRAINT restricts the action space. This space is formed by alternative actions that are a result of the planning decisions (Schneeweis 2003). In the planning domain, PLANNING CONSTRAINTS, often the capacity offered by resources, limit the quantities that are assigned to the PLANNING OBJECTS or impact the temporal properties of PLANNING OBJECTS.</rdfs:comment>
    </owl:Class>
    


    <!-- http://www.semanticweb.org/sc3/ontologies/2022/0/Planning-Ontology#PlanningDecision -->


    <owl:Class rdf:about="http://www.semanticweb.org/sc3/ontologies/2022/0/Planning-Ontology#PlanningDecision">
        <rdfs:comment>Decisions determined by a Decision Making Unit</rdfs:comment>
    </owl:Class>
    


    <!-- http://www.semanticweb.org/sc3/ontologies/2022/0/Planning-Ontology#PlanningFunction -->


    <owl:Class rdf:about="http://www.semanticweb.org/sc3/ontologies/2022/0/Planning-Ontology#PlanningFunction">
        <rdfs:comment>Describes the different functions and its properies follwing the supply chain planning matrix.</rdfs:comment>
    </owl:Class>
    


    <!-- http://www.semanticweb.org/sc3/ontologies/2022/0/Planning-Ontology#PlanningInstance -->


    <owl:Class rdf:about="http://www.semanticweb.org/sc3/ontologies/2022/0/Planning-Ontology#PlanningInstance">
        <rdfs:comment>A PLANNING INSTANCE specifies the PLANNING OBJECTS and the values of related PLANNING CONSTRAINTS that form the basis for a planning decision.</rdfs:comment>
    </owl:Class>
    


    <!-- http://www.semanticweb.org/sc3/ontologies/2022/0/Planning-Ontology#PlanningObject -->


    <owl:Class rdf:about="http://www.semanticweb.org/sc3/ontologies/2022/0/Planning-Ontology#PlanningObject">
        <rdfs:comment>A PLANNING OBJECT specifies what has to be planned as an atomic unit. A single PLANNING OBJECT typically represents a quantity of a certain product or product aggregate to be released or completed within a certain period in a certain node of the semiconductor supply chain. Other PLANNING OBJECTS can be orders or lots. Values are assigned to the attributes of a PLANNING OBJECT as a result of a planning decision.</rdfs:comment>
    </owl:Class>
    


    <!-- http://www.semanticweb.org/sc3/ontologies/2022/0/Planning-Ontology#PlanningProcess -->


    <owl:Class rdf:about="http://www.semanticweb.org/sc3/ontologies/2022/0/Planning-Ontology#PlanningProcess">
        <rdfs:comment>The PLANNING PROCESS specifies under which circumstances which (re)planning activities are performed by a DECISION-MAKING UNIT.</rdfs:comment>
    </owl:Class>
    


    <!-- http://www.semanticweb.org/sc3/ontologies/2022/0/Planning-Ontology#PlanningSituation -->


    <owl:Class rdf:about="http://www.semanticweb.org/sc3/ontologies/2022/0/Planning-Ontology#PlanningSituation">
        <rdfs:comment>The PLANNING SITUATION describes the organization of several DECISION-MAKING UNITS and also its environment.</rdfs:comment>
    </owl:Class>
    


    <!-- http://www.semanticweb.org/sc3/ontologies/2022/0/Planning-Ontology#Process -->


    <owl:Class rdf:about="http://www.semanticweb.org/sc3/ontologies/2022/0/Planning-Ontology#Process">
        <rdfs:comment>A PROCESS specifies a method of making a product at a location. The process is expressed at a coarse level of granularity suitable for use in production planning.</rdfs:comment>
    </owl:Class>
    


    <!-- http://www.semanticweb.org/sc3/ontologies/2022/0/Planning-Ontology#ProductAggregate -->


    <owl:Class rdf:about="http://www.semanticweb.org/sc3/ontologies/2022/0/Planning-Ontology#ProductAggregate">
        <rdfs:comment>A PRODUCT AGGREGATE combines individual products into a few logical products groups. This results in a reduction of complexity, which enables a better overview.</rdfs:comment>
    </owl:Class>
    


    <!-- http://www.semanticweb.org/sc3/ontologies/2022/0/Planning-Ontology#ProductHierarchy -->


    <owl:Class rdf:about="http://www.semanticweb.org/sc3/ontologies/2022/0/Planning-Ontology#ProductHierarchy">
        <rdfs:comment>A PRODUCT HIERARCHY characterizes the top-down and bottom-up relationship between different product aggregates. It organizes the product aggregates according to defined criteria. A product aggregate is used to group different products based on certain criteria. The grouping criteria depend on the planning purpose (e.g. controlling, production). It is a certain view on a set of products.</rdfs:comment>
    </owl:Class>
    


    <!-- http://www.semanticweb.org/sc3/ontologies/2022/0/Planning-Ontology#ProjectedWip -->


    <owl:Class rdf:about="http://www.semanticweb.org/sc3/ontologies/2022/0/Planning-Ontology#ProjectedWip">
        <rdfs:comment>The PROJECTED WIP describes the quantity of a certain product that is anticipated to be received into inventory at a particular location at a particular time.</rdfs:comment>
    </owl:Class>
    


    <!-- http://www.semanticweb.org/sc3/ontologies/2022/0/Planning-Ontology#ReplanningDegree -->


    <owl:Class rdf:about="http://www.semanticweb.org/sc3/ontologies/2022/0/Planning-Ontology#ReplanningDegree">
        <rdfs:comment>The degree distinguishes replanning from scratch and repair of existing plans (Vieria et al. 2003).</rdfs:comment>
    </owl:Class>
    


    <!-- http://www.semanticweb.org/sc3/ontologies/2022/0/Planning-Ontology#RequiredCapacity -->


    <owl:Class rdf:about="http://www.semanticweb.org/sc3/ontologies/2022/0/Planning-Ontology#RequiredCapacity">
        <rdfs:subClassOf rdf:resource="http://www.semanticweb.org/sc3/ontologies/2022/0/Planning-Ontology#Capacity"/>
    </owl:Class>
    


    <!-- http://www.semanticweb.org/sc3/ontologies/2022/0/Planning-Ontology#Resource-Availability-Constraints -->


    <owl:Class rdf:about="http://www.semanticweb.org/sc3/ontologies/2022/0/Planning-Ontology#Resource-Availability-Constraints">
        <rdfs:subClassOf rdf:resource="http://www.semanticweb.org/sc3/ontologies/2022/0/Planning-Ontology#PlanningConstraint"/>
        <rdfs:comment>This type of constraints has an impact on the assignment of activities to RESOURCES and to START/END TIMES to ACTIVITIES.</rdfs:comment>
    </owl:Class>
    


    <!-- http://www.semanticweb.org/sc3/ontologies/2022/0/Planning-Ontology#Resource-Compatibility-Constraints -->


    <owl:Class rdf:about="http://www.semanticweb.org/sc3/ontologies/2022/0/Planning-Ontology#Resource-Compatibility-Constraints">
        <rdfs:subClassOf rdf:resource="http://www.semanticweb.org/sc3/ontologies/2022/0/Planning-Ontology#PlanningConstraint"/>
        <rdfs:comment>This type of constraints ensures that only allowed activities are performed using a given RESOURCE.</rdfs:comment>
    </owl:Class>
    


    <!-- http://www.semanticweb.org/sc3/ontologies/2022/0/Planning-Ontology#Route -->


    <owl:Class rdf:about="http://www.semanticweb.org/sc3/ontologies/2022/0/Planning-Ontology#Route"/>
    


    <!-- http://www.semanticweb.org/sc3/ontologies/2022/0/Planning-Ontology#SemiAutomated -->


    <owl:Class rdf:about="http://www.semanticweb.org/sc3/ontologies/2022/0/Planning-Ontology#SemiAutomated">
        <rdfs:subClassOf rdf:resource="http://www.semanticweb.org/sc3/ontologies/2022/0/Planning-Ontology#DecisionMakerType"/>
        <rdfs:comment>Between these two extremes there are semi-automated decisions, where a computer provides several decision alternatives and a human decision-maker chooses among them.</rdfs:comment>
    </owl:Class>
    


    <!-- http://www.semanticweb.org/sc3/ontologies/2022/0/Planning-Ontology#StrictHierarchicalSituation -->


    <owl:Class rdf:about="http://www.semanticweb.org/sc3/ontologies/2022/0/Planning-Ontology#StrictHierarchicalSituation">
        <rdfs:subClassOf rdf:resource="http://www.semanticweb.org/sc3/ontologies/2022/0/Planning-Ontology#HierarchicalSituation"/>
        <rdfs:comment>There are only edges between vertices of level k and vertices of level k-1, where k≥2.</rdfs:comment>
    </owl:Class>
    


    <!-- http://www.semanticweb.org/sc3/ontologies/2022/0/Planning-Ontology#Substitution -->


    <owl:Class rdf:about="http://www.semanticweb.org/sc3/ontologies/2022/0/Planning-Ontology#Substitution">
        <rdfs:comment>SUBSTITUTION refers to using alternative parts. Depending on the product, each one could be replaced by using specific alternatives at the same stage of production, e.g. final product, raw material, or semi-finished products (Degbotse 2013) in order to complete a manufacturing step or fulfill a customer order.</rdfs:comment>
    </owl:Class>
    


    <!-- http://www.semanticweb.org/sc3/ontologies/2022/0/Planning-Ontology#SupplyInformation -->


    <owl:Class rdf:about="http://www.semanticweb.org/sc3/ontologies/2022/0/Planning-Ontology#SupplyInformation">
        <rdfs:comment>SUPPLY INFORMATION provides information of the used and unused supply of a supply chain network.</rdfs:comment>
    </owl:Class>
    


    <!-- http://www.semanticweb.org/sc3/ontologies/2022/0/Planning-Ontology#Target -->


    <owl:Class rdf:about="http://www.semanticweb.org/sc3/ontologies/2022/0/Planning-Ontology#Target">
        <rdfs:comment>Targets are prescribed values for the different performance measures.</rdfs:comment>
    </owl:Class>
    


    <!-- http://www.semanticweb.org/sc3/ontologies/2022/0/Planning-Ontology#Temporal-Constraints -->


    <owl:Class rdf:about="http://www.semanticweb.org/sc3/ontologies/2022/0/Planning-Ontology#Temporal-Constraints">
        <rdfs:subClassOf rdf:resource="http://www.semanticweb.org/sc3/ontologies/2022/0/Planning-Ontology#PlanningConstraint"/>
        <rdfs:comment>This type of constraints restricts the values of temporal attributes, modeled by the property TIME, that belong to PLANNING OBJECTS. For instance, there might be a minimum amount of time between two consecutive operations of a certain product.</rdfs:comment>
    </owl:Class>
    


    <!-- http://www.semanticweb.org/sc3/ontologies/2022/0/Planning-Ontology#Trigger -->


    <owl:Class rdf:about="http://www.semanticweb.org/sc3/ontologies/2022/0/Planning-Ontology#Trigger">
        <rdfs:comment>A mechanism that initiates an action when an event occurs such as reaching a certain time or date or upon receiving some type of input. A trigger generally causes a program routine to be executed.</rdfs:comment>
    </owl:Class>
    


    <!-- http://www.semanticweb.org/sc3/ontologies/2022/0/Planning-Ontology#Vertex -->


    <owl:Class rdf:about="http://www.semanticweb.org/sc3/ontologies/2022/0/Planning-Ontology#Vertex"/>
    


    <!-- http://www.semanticweb.org/sc3/ontologies/2022/0/Planning-Ontology#Yield -->


    <owl:Class rdf:about="http://www.semanticweb.org/sc3/ontologies/2022/0/Planning-Ontology#Yield">
        <rdfs:comment>YIELD could be the fraction (percentage) of good dies resulting from total dies released.</rdfs:comment>
    </owl:Class>
    


    <!-- http://www.semanticweb.org/sc3/ontologies/2022/0/ozone-ontology#Demand -->


    <owl:Class rdf:about="http://www.semanticweb.org/sc3/ontologies/2022/0/ozone-ontology#Demand"/>
    


    <!-- http://www.semanticweb.org/sc3/ontologies/2022/0/ozone-ontology#Product -->


    <owl:Class rdf:about="http://www.semanticweb.org/sc3/ontologies/2022/0/ozone-ontology#Product"/>
    


    <!-- http://www.semanticweb.org/sc3/ontologies/2022/0/ozone-ontology#Resource -->


    <owl:Class rdf:about="http://www.semanticweb.org/sc3/ontologies/2022/0/ozone-ontology#Resource"/>
    


    <!-- http://www.w3.org/2006/time#DateTimeDescription -->


    <owl:Class rdf:about="http://www.w3.org/2006/time#DateTimeDescription">
        <rdfs:subClassOf rdf:resource="http://www.w3.org/2006/time#GeneralDateTimeDescription"/>
        <rdfs:subClassOf>
            <owl:Restriction>
                <owl:onProperty rdf:resource="http://www.w3.org/2006/time#hasTRS"/>
                <owl:hasValue rdf:resource="http://www.opengis.net/def/uom/ISO-8601/0/Gregorian"/>
            </owl:Restriction>
        </rdfs:subClassOf>
        <rdfs:subClassOf>
            <owl:Restriction>
                <owl:onProperty rdf:resource="http://www.w3.org/2006/time#day"/>
                <owl:allValuesFrom rdf:resource="http://www.w3.org/2001/XMLSchema#gDay"/>
            </owl:Restriction>
        </rdfs:subClassOf>
        <rdfs:subClassOf>
            <owl:Restriction>
                <owl:onProperty rdf:resource="http://www.w3.org/2006/time#month"/>
                <owl:allValuesFrom rdf:resource="http://www.w3.org/2001/XMLSchema#gMonth"/>
            </owl:Restriction>
        </rdfs:subClassOf>
        <rdfs:subClassOf>
            <owl:Restriction>
                <owl:onProperty rdf:resource="http://www.w3.org/2006/time#year"/>
                <owl:allValuesFrom rdf:resource="http://www.w3.org/2001/XMLSchema#gYear"/>
            </owl:Restriction>
        </rdfs:subClassOf>
        <rdfs:comment xml:lang="es">Descripción de fecha y tiempo estructurada con valores separados para los diferentes elementos de un sistema calendario-reloj. El sistema de referencia temporal está fijado al calendario gregoriano, y el rango de las propiedades año, mes, día restringidas a los correspondientes tipos del XML Schema xsd:gYear, xsd:gMonth y xsd:gDay respectivamente.</rdfs:comment>
        <rdfs:comment xml:lang="en">Description of date and time structured with separate values for the various elements of a calendar-clock system. The temporal reference system is fixed to Gregorian Calendar, and the range of year, month, day properties restricted to corresponding XML Schema types xsd:gYear, xsd:gMonth and xsd:gDay, respectively.</rdfs:comment>
        <rdfs:label xml:lang="en">Date-Time description</rdfs:label>
        <rdfs:label xml:lang="es">descripción de fecha-tiempo</rdfs:label>
        <skos:definition xml:lang="es">Descripción de fecha y tiempo estructurada con valores separados para los diferentes elementos de un sistema calendario-reloj. El sistema de referencia temporal está fijado al calendario gregoriano, y el rango de las propiedades año, mes, día restringidas a los correspondientes tipos del XML Schema xsd:gYear, xsd:gMonth y xsd:gDay respectivamente.</skos:definition>
        <skos:definition xml:lang="en">Description of date and time structured with separate values for the various elements of a calendar-clock system. The temporal reference system is fixed to Gregorian Calendar, and the range of year, month, day properties restricted to corresponding XML Schema types xsd:gYear, xsd:gMonth and xsd:gDay, respectively.</skos:definition>
    </owl:Class>
    


    <!-- http://www.w3.org/2006/time#DateTimeInterval -->


    <owl:Class rdf:about="http://www.w3.org/2006/time#DateTimeInterval">
        <rdfs:subClassOf rdf:resource="http://www.w3.org/2006/time#ProperInterval"/>
        <rdfs:comment xml:lang="es">&apos;intervalo de fecha-hora&apos; es una subclase de &apos;intervalo propio&apos;, definida utilizando el multi-elemento &apos;descripción de fecha-hora&apos;.</rdfs:comment>
        <rdfs:comment xml:lang="en">DateTimeInterval is a subclass of ProperInterval, defined using the multi-element DateTimeDescription.</rdfs:comment>
        <rdfs:label xml:lang="en">Date-time interval</rdfs:label>
        <rdfs:label xml:lang="es">intervalo de fecha-hora</rdfs:label>
        <skos:definition xml:lang="es">&apos;intervalo de fecha-hora&apos; es una subclase de &apos;intervalo propio&apos;, definida utilizando el multi-elemento &apos;descripción de fecha-hora&apos;.</skos:definition>
        <skos:definition xml:lang="en">DateTimeInterval is a subclass of ProperInterval, defined using the multi-element DateTimeDescription.</skos:definition>
        <skos:note xml:lang="es">&apos;intervalo de fecha-hora&apos; se puede utilizar sólo para un intervalo cuyos límites coinciden con un elemento de fecha-hora alineados con el calendario y la zona horaria indicados. Por ejemplo, aunque ambos tienen una duración de un día, el intervalo de 24 horas que empieza en la media noche del comienzo del 8 mayo en Europa Central se puede expresar como un &apos;intervalo de fecha-hora&apos;, el intervalo de 24 horas que empieza a las 1:30pm no.</skos:note>
        <skos:note xml:lang="en">:DateTimeInterval can only be used for an interval whose limits coincide with a date-time element aligned to the calendar and timezone indicated. For example, while both have a duration of one day, the 24-hour interval beginning at midnight at the beginning of 8 May in Central Europe can be expressed as a :DateTimeInterval, but the 24-hour interval starting at 1:30pm cannot.</skos:note>
    </owl:Class>
    


    <!-- http://www.w3.org/2006/time#DayOfWeek -->


    <owl:Class rdf:about="http://www.w3.org/2006/time#DayOfWeek">
        <rdfs:subClassOf rdf:resource="http://www.w3.org/2002/07/owl#Thing"/>
        <rdfs:comment xml:lang="es">El día de la semana</rdfs:comment>
        <rdfs:comment xml:lang="en">The day of week</rdfs:comment>
        <rdfs:label xml:lang="en">Day of week</rdfs:label>
        <rdfs:label xml:lang="es">día de la semana</rdfs:label>
        <skos:changeNote xml:lang="en">Remove enumeration from definition, in order to allow other days to be used when required in other calendars. 
NOTE: existing days are still present as members of the class, but the class membership is now open. 

In the original OWL-Time the following constraint appeared: 
  owl:oneOf (
      time:Monday
      time:Tuesday
      time:Wednesday
      time:Thursday
      time:Friday
      time:Saturday
      time:Sunday
    ) ;</skos:changeNote>
        <skos:definition xml:lang="es">El día de la semana</skos:definition>
        <skos:definition xml:lang="en">The day of week</skos:definition>
        <skos:note xml:lang="es">La pertenencia a la clase &apos;día de la semana&apos; está abierta, para permitir longitudes de semana alternativas y diferentes nombres de días.</skos:note>
        <skos:note xml:lang="en">Membership of the class :DayOfWeek is open, to allow for alternative week lengths and different day names.</skos:note>
    </owl:Class>
    


    <!-- http://www.w3.org/2006/time#Duration -->


    <owl:Class rdf:about="http://www.w3.org/2006/time#Duration">
        <rdfs:subClassOf rdf:resource="http://www.w3.org/2006/time#TemporalDuration"/>
        <rdfs:subClassOf>
            <owl:Restriction>
                <owl:onProperty rdf:resource="http://www.w3.org/2006/time#unitType"/>
                <owl:cardinality rdf:datatype="http://www.w3.org/2001/XMLSchema#nonNegativeInteger">1</owl:cardinality>
            </owl:Restriction>
        </rdfs:subClassOf>
        <rdfs:subClassOf>
            <owl:Restriction>
                <owl:onProperty rdf:resource="http://www.w3.org/2006/time#numericDuration"/>
                <owl:cardinality rdf:datatype="http://www.w3.org/2001/XMLSchema#nonNegativeInteger">1</owl:cardinality>
            </owl:Restriction>
        </rdfs:subClassOf>
        <rdfs:comment xml:lang="es">Duración de una extensión temporal expresada como un número escalado por una unidad temporal.</rdfs:comment>
        <rdfs:comment xml:lang="en">Duration of a temporal extent expressed as a number scaled by a temporal unit</rdfs:comment>
        <rdfs:label xml:lang="en">Time duration</rdfs:label>
        <rdfs:label>duración de tiempo</rdfs:label>
        <skos:definition xml:lang="es">Duración de una extensión temporal expresada como un número escalado por una unidad temporal.</skos:definition>
        <skos:definition xml:lang="en">Duration of a temporal extent expressed as a number scaled by a temporal unit</skos:definition>
        <skos:note xml:lang="es">Alternativa a &apos;descripción de tiempo&apos; para proporcionar descripción soporte a una duración temporal diferente a utilizar un sistema de calendario/reloj.</skos:note>
        <skos:note xml:lang="en">Alternative to time:DurationDescription to support description of a temporal duration other than using a calendar/clock system.</skos:note>
    </owl:Class>
    


    <!-- http://www.w3.org/2006/time#DurationDescription -->


    <owl:Class rdf:about="http://www.w3.org/2006/time#DurationDescription">
        <rdfs:subClassOf rdf:resource="http://www.w3.org/2006/time#GeneralDurationDescription"/>
        <rdfs:subClassOf>
            <owl:Restriction>
                <owl:onProperty rdf:resource="http://www.w3.org/2006/time#hasTRS"/>
                <owl:hasValue rdf:resource="http://www.opengis.net/def/uom/ISO-8601/0/Gregorian"/>
            </owl:Restriction>
        </rdfs:subClassOf>
        <rdfs:subClassOf>
            <owl:Restriction>
                <owl:onProperty rdf:resource="http://www.w3.org/2006/time#days"/>
                <owl:allValuesFrom rdf:resource="http://www.w3.org/2001/XMLSchema#decimal"/>
            </owl:Restriction>
        </rdfs:subClassOf>
        <rdfs:subClassOf>
            <owl:Restriction>
                <owl:onProperty rdf:resource="http://www.w3.org/2006/time#hours"/>
                <owl:allValuesFrom rdf:resource="http://www.w3.org/2001/XMLSchema#decimal"/>
            </owl:Restriction>
        </rdfs:subClassOf>
        <rdfs:subClassOf>
            <owl:Restriction>
                <owl:onProperty rdf:resource="http://www.w3.org/2006/time#minutes"/>
                <owl:allValuesFrom rdf:resource="http://www.w3.org/2001/XMLSchema#decimal"/>
            </owl:Restriction>
        </rdfs:subClassOf>
        <rdfs:subClassOf>
            <owl:Restriction>
                <owl:onProperty rdf:resource="http://www.w3.org/2006/time#months"/>
                <owl:allValuesFrom rdf:resource="http://www.w3.org/2001/XMLSchema#decimal"/>
            </owl:Restriction>
        </rdfs:subClassOf>
        <rdfs:subClassOf>
            <owl:Restriction>
                <owl:onProperty rdf:resource="http://www.w3.org/2006/time#seconds"/>
                <owl:allValuesFrom rdf:resource="http://www.w3.org/2001/XMLSchema#decimal"/>
            </owl:Restriction>
        </rdfs:subClassOf>
        <rdfs:subClassOf>
            <owl:Restriction>
                <owl:onProperty rdf:resource="http://www.w3.org/2006/time#weeks"/>
                <owl:allValuesFrom rdf:resource="http://www.w3.org/2001/XMLSchema#decimal"/>
            </owl:Restriction>
        </rdfs:subClassOf>
        <rdfs:subClassOf>
            <owl:Restriction>
                <owl:onProperty rdf:resource="http://www.w3.org/2006/time#years"/>
                <owl:allValuesFrom rdf:resource="http://www.w3.org/2001/XMLSchema#decimal"/>
            </owl:Restriction>
        </rdfs:subClassOf>
        <rdfs:comment xml:lang="es">Descripción de extensión temporal estructurada con valores separados para los distintos elementos de un sistema de horario-calendario. El sistema de referencia temporal se fija al calendario gregoriano, y el intervalo de cada una de las propiedades numéricas se restringe a xsd:decimal.</rdfs:comment>
        <rdfs:comment xml:lang="en">Description of temporal extent structured with separate values for the various elements of a calendar-clock system. The temporal reference system is fixed to Gregorian Calendar, and the range of each of the numeric properties is restricted to xsd:decimal</rdfs:comment>
        <rdfs:label xml:lang="en">Duration description</rdfs:label>
        <rdfs:label xml:lang="es">descripción de duración</rdfs:label>
        <skos:definition xml:lang="es">Descripción de extensión temporal estructurada con valores separados para los distintos elementos de un sistema de horario-calendario. El sistema de referencia temporal se fija al calendario gregoriano, y el intervalo de cada una de las propiedades numéricas se restringe a xsd:decimal.</skos:definition>
        <skos:definition xml:lang="en">Description of temporal extent structured with separate values for the various elements of a calendar-clock system. The temporal reference system is fixed to Gregorian Calendar, and the range of each of the numeric properties is restricted to xsd:decimal</skos:definition>
        <skos:note xml:lang="es">En el calendario gregoriano la longitud de los meses no es fija. Por lo tanto, un valor como &quot;2,5 meses&quot; no se puede comparar exactamente con una duración similar expresada en términos de semanas o días.</skos:note>
        <skos:note xml:lang="en">In the Gregorian calendar the length of the month is not fixed. Therefore, a value like &quot;2.5 months&quot; cannot be exactly compared with a similar duration expressed in terms of weeks or days.</skos:note>
    </owl:Class>
    


    <!-- http://www.w3.org/2006/time#GeneralDateTimeDescription -->


    <owl:Class rdf:about="http://www.w3.org/2006/time#GeneralDateTimeDescription">
        <rdfs:subClassOf rdf:resource="http://www.w3.org/2006/time#TemporalPosition"/>
        <rdfs:subClassOf>
            <owl:Restriction>
                <owl:onProperty rdf:resource="http://www.w3.org/2006/time#unitType"/>
                <owl:cardinality rdf:datatype="http://www.w3.org/2001/XMLSchema#nonNegativeInteger">1</owl:cardinality>
            </owl:Restriction>
        </rdfs:subClassOf>
        <rdfs:subClassOf>
            <owl:Restriction>
                <owl:onProperty rdf:resource="http://www.w3.org/2006/time#dayOfWeek"/>
                <owl:maxCardinality rdf:datatype="http://www.w3.org/2001/XMLSchema#nonNegativeInteger">1</owl:maxCardinality>
            </owl:Restriction>
        </rdfs:subClassOf>
        <rdfs:subClassOf>
            <owl:Restriction>
                <owl:onProperty rdf:resource="http://www.w3.org/2006/time#monthOfYear"/>
                <owl:maxCardinality rdf:datatype="http://www.w3.org/2001/XMLSchema#nonNegativeInteger">1</owl:maxCardinality>
            </owl:Restriction>
        </rdfs:subClassOf>
        <rdfs:subClassOf>
            <owl:Restriction>
                <owl:onProperty rdf:resource="http://www.w3.org/2006/time#timeZone"/>
                <owl:maxCardinality rdf:datatype="http://www.w3.org/2001/XMLSchema#nonNegativeInteger">1</owl:maxCardinality>
            </owl:Restriction>
        </rdfs:subClassOf>
        <rdfs:subClassOf>
            <owl:Restriction>
                <owl:onProperty rdf:resource="http://www.w3.org/2006/time#day"/>
                <owl:maxCardinality rdf:datatype="http://www.w3.org/2001/XMLSchema#nonNegativeInteger">1</owl:maxCardinality>
            </owl:Restriction>
        </rdfs:subClassOf>
        <rdfs:subClassOf>
            <owl:Restriction>
                <owl:onProperty rdf:resource="http://www.w3.org/2006/time#dayOfYear"/>
                <owl:maxCardinality rdf:datatype="http://www.w3.org/2001/XMLSchema#nonNegativeInteger">1</owl:maxCardinality>
            </owl:Restriction>
        </rdfs:subClassOf>
        <rdfs:subClassOf>
            <owl:Restriction>
                <owl:onProperty rdf:resource="http://www.w3.org/2006/time#hour"/>
                <owl:maxCardinality rdf:datatype="http://www.w3.org/2001/XMLSchema#nonNegativeInteger">1</owl:maxCardinality>
            </owl:Restriction>
        </rdfs:subClassOf>
        <rdfs:subClassOf>
            <owl:Restriction>
                <owl:onProperty rdf:resource="http://www.w3.org/2006/time#minute"/>
                <owl:maxCardinality rdf:datatype="http://www.w3.org/2001/XMLSchema#nonNegativeInteger">1</owl:maxCardinality>
            </owl:Restriction>
        </rdfs:subClassOf>
        <rdfs:subClassOf>
            <owl:Restriction>
                <owl:onProperty rdf:resource="http://www.w3.org/2006/time#month"/>
                <owl:maxCardinality rdf:datatype="http://www.w3.org/2001/XMLSchema#nonNegativeInteger">1</owl:maxCardinality>
            </owl:Restriction>
        </rdfs:subClassOf>
        <rdfs:subClassOf>
            <owl:Restriction>
                <owl:onProperty rdf:resource="http://www.w3.org/2006/time#second"/>
                <owl:maxCardinality rdf:datatype="http://www.w3.org/2001/XMLSchema#nonNegativeInteger">1</owl:maxCardinality>
            </owl:Restriction>
        </rdfs:subClassOf>
        <rdfs:subClassOf>
            <owl:Restriction>
                <owl:onProperty rdf:resource="http://www.w3.org/2006/time#week"/>
                <owl:maxCardinality rdf:datatype="http://www.w3.org/2001/XMLSchema#nonNegativeInteger">1</owl:maxCardinality>
            </owl:Restriction>
        </rdfs:subClassOf>
        <rdfs:subClassOf>
            <owl:Restriction>
                <owl:onProperty rdf:resource="http://www.w3.org/2006/time#year"/>
                <owl:maxCardinality rdf:datatype="http://www.w3.org/2001/XMLSchema#nonNegativeInteger">1</owl:maxCardinality>
            </owl:Restriction>
        </rdfs:subClassOf>
        <rdfs:comment xml:lang="es">Descripción de fecha y hora estructurada con valores separados para los distintos elementos de un sistema calendario-reloj.</rdfs:comment>
        <rdfs:comment xml:lang="en">Description of date and time structured with separate values for the various elements of a calendar-clock system</rdfs:comment>
        <rdfs:label xml:lang="en">Generalized date-time description</rdfs:label>
        <rdfs:label xml:lang="es">descripción de fecha-hora generalizada</rdfs:label>
        <skos:definition xml:lang="en">Description of date and time structured with separate values for the various elements of a calendar-clock system</skos:definition>
        <skos:definition>Descripción de fecha y hora estructurada con valores separados para los distintos elementos de un sistema calendario-reloj.</skos:definition>
        <skos:note xml:lang="es">Algunas combinaciones de propiedades son redundantes - por ejemplo, dentro de un &apos;año&apos; especificado si se proporciona &apos;día del año&apos; entonces &apos;día&apos; y &apos;mes&apos; se pueden computar, y viceversa. Los valores individuales deberían ser consistentes entre ellos y con el calendario, indicado a través del valor de la propiedad &apos;tiene TRS&apos;.</skos:note>
        <skos:note>Some combinations of properties are redundant - for example, within a specified :year if :dayOfYear is provided then :day and :month can be computed, and vice versa. Individual values should be consistent with each other and the calendar, indicated through the value of the :hasTRS property.</skos:note>
    </owl:Class>
    


    <!-- http://www.w3.org/2006/time#GeneralDurationDescription -->


    <owl:Class rdf:about="http://www.w3.org/2006/time#GeneralDurationDescription">
        <rdfs:subClassOf rdf:resource="http://www.w3.org/2006/time#TemporalDuration"/>
        <rdfs:subClassOf>
            <owl:Restriction>
                <owl:onProperty rdf:resource="http://www.w3.org/2006/time#hasTRS"/>
                <owl:cardinality rdf:datatype="http://www.w3.org/2001/XMLSchema#nonNegativeInteger">1</owl:cardinality>
            </owl:Restriction>
        </rdfs:subClassOf>
        <rdfs:subClassOf>
            <owl:Restriction>
                <owl:onProperty rdf:resource="http://www.w3.org/2006/time#days"/>
                <owl:maxCardinality rdf:datatype="http://www.w3.org/2001/XMLSchema#nonNegativeInteger">1</owl:maxCardinality>
            </owl:Restriction>
        </rdfs:subClassOf>
        <rdfs:subClassOf>
            <owl:Restriction>
                <owl:onProperty rdf:resource="http://www.w3.org/2006/time#hours"/>
                <owl:maxCardinality rdf:datatype="http://www.w3.org/2001/XMLSchema#nonNegativeInteger">1</owl:maxCardinality>
            </owl:Restriction>
        </rdfs:subClassOf>
        <rdfs:subClassOf>
            <owl:Restriction>
                <owl:onProperty rdf:resource="http://www.w3.org/2006/time#minutes"/>
                <owl:maxCardinality rdf:datatype="http://www.w3.org/2001/XMLSchema#nonNegativeInteger">1</owl:maxCardinality>
            </owl:Restriction>
        </rdfs:subClassOf>
        <rdfs:subClassOf>
            <owl:Restriction>
                <owl:onProperty rdf:resource="http://www.w3.org/2006/time#months"/>
                <owl:maxCardinality rdf:datatype="http://www.w3.org/2001/XMLSchema#nonNegativeInteger">1</owl:maxCardinality>
            </owl:Restriction>
        </rdfs:subClassOf>
        <rdfs:subClassOf>
            <owl:Restriction>
                <owl:onProperty rdf:resource="http://www.w3.org/2006/time#seconds"/>
                <owl:maxCardinality rdf:datatype="http://www.w3.org/2001/XMLSchema#nonNegativeInteger">1</owl:maxCardinality>
            </owl:Restriction>
        </rdfs:subClassOf>
        <rdfs:subClassOf>
            <owl:Restriction>
                <owl:onProperty rdf:resource="http://www.w3.org/2006/time#weeks"/>
                <owl:maxCardinality rdf:datatype="http://www.w3.org/2001/XMLSchema#nonNegativeInteger">1</owl:maxCardinality>
            </owl:Restriction>
        </rdfs:subClassOf>
        <rdfs:subClassOf>
            <owl:Restriction>
                <owl:onProperty rdf:resource="http://www.w3.org/2006/time#years"/>
                <owl:maxCardinality rdf:datatype="http://www.w3.org/2001/XMLSchema#nonNegativeInteger">1</owl:maxCardinality>
            </owl:Restriction>
        </rdfs:subClassOf>
        <rdfs:comment xml:lang="es">Descripción de extensión temporal estructurada con valores separados para los distintos elementos de un sistema de horario-calendario.</rdfs:comment>
        <rdfs:comment xml:lang="en">Description of temporal extent structured with separate values for the various elements of a calendar-clock system.</rdfs:comment>
        <rdfs:label xml:lang="en">Generalized duration description</rdfs:label>
        <rdfs:label xml:lang="es">descripción de duración generalizada</rdfs:label>
        <skos:definition xml:lang="es">Descripción de extensión temporal estructurada con valores separados para los distintos elementos de un sistema de horario-calendario.</skos:definition>
        <skos:definition xml:lang="en">Description of temporal extent structured with separate values for the various elements of a calendar-clock system.</skos:definition>
        <skos:note xml:lang="es">La extensión de una duración de tiempo expresada como una &apos;descripción de duración general&apos; depende del Sistema de Referencia Temporal. En algunos calendarios la longitud de la semana o del mes no es constante a lo largo del año. Por tanto, un valor como &quot;25 meses&quot; puede no ser necesariamente ser comparado con un duración similar expresada en términos de semanas o días. Cuando se consideran calendarios que no están basados en el movimiento de la Tierra, se deben tomar incluso más precauciones en la comparación de duraciones.</skos:note>
        <skos:note xml:lang="en">The extent of a time duration expressed as a GeneralDurationDescription depends on the Temporal Reference System. In some calendars the length of the week or month is not constant within the year. Therefore, a value like &quot;2.5 months&quot; may not necessarily be exactly compared with a similar duration expressed in terms of weeks or days. When non-earth-based calendars are considered even more care must be taken in comparing durations.</skos:note>
    </owl:Class>
    


    <!-- http://www.w3.org/2006/time#Instant -->


    <owl:Class rdf:about="http://www.w3.org/2006/time#Instant">
        <rdfs:subClassOf rdf:resource="http://www.w3.org/2006/time#TemporalEntity"/>
        <owl:disjointWith rdf:resource="http://www.w3.org/2006/time#ProperInterval"/>
        <rdfs:comment xml:lang="en">A temporal entity with zero extent or duration</rdfs:comment>
        <rdfs:comment xml:lang="es">Una entidad temporal con una extensión o duración cero.</rdfs:comment>
        <rdfs:label xml:lang="en">Time instant</rdfs:label>
        <rdfs:label xml:lang="es">instante de tiempo.</rdfs:label>
        <skos:definition xml:lang="en">A temporal entity with zero extent or duration</skos:definition>
        <skos:definition xml:lang="es">Una entidad temporal con una extensión o duración cero.</skos:definition>
    </owl:Class>
    


    <!-- http://www.w3.org/2006/time#Interval -->


    <owl:Class rdf:about="http://www.w3.org/2006/time#Interval">
        <rdfs:subClassOf rdf:resource="http://www.w3.org/2006/time#TemporalEntity"/>
        <rdfs:comment xml:lang="en">A temporal entity with an extent or duration</rdfs:comment>
        <rdfs:comment xml:lang="es">Una entidad temporal con una extensión o duración.</rdfs:comment>
        <rdfs:label xml:lang="en">Time interval</rdfs:label>
        <rdfs:label xml:lang="es">intervalo de tiempo</rdfs:label>
        <skos:definition xml:lang="en">A temporal entity with an extent or duration</skos:definition>
        <skos:definition xml:lang="es">Una entidad temporal con una extensión o duración.</skos:definition>
    </owl:Class>
    


    <!-- http://www.w3.org/2006/time#January -->


    <owl:Class rdf:about="http://www.w3.org/2006/time#January">
        <rdfs:subClassOf rdf:resource="http://www.w3.org/2006/time#DateTimeDescription"/>
        <rdfs:subClassOf>
            <owl:Restriction>
                <owl:onProperty rdf:resource="http://www.w3.org/2006/time#unitType"/>
                <owl:hasValue rdf:resource="http://www.w3.org/2006/time#unitMonth"/>
            </owl:Restriction>
        </rdfs:subClassOf>
        <rdfs:subClassOf>
            <owl:Restriction>
                <owl:onProperty rdf:resource="http://www.w3.org/2006/time#month"/>
                <owl:hasValue>--01</owl:hasValue>
            </owl:Restriction>
        </rdfs:subClassOf>
        <rdfs:label>January</rdfs:label>
        <owl:deprecated rdf:datatype="http://www.w3.org/2001/XMLSchema#boolean">true</owl:deprecated>
        <skos:historyNote>This class was present in the 2006 version of OWL-Time. It was presented as an example of how DateTimeDescription could be specialized, but does not belong in the revised ontology. </skos:historyNote>
    </owl:Class>
    


    <!-- http://www.w3.org/2006/time#MonthOfYear -->


    <owl:Class rdf:about="http://www.w3.org/2006/time#MonthOfYear">
        <rdfs:subClassOf rdf:resource="http://www.w3.org/2006/time#DateTimeDescription"/>
        <rdfs:subClassOf>
            <owl:Restriction>
                <owl:onProperty rdf:resource="http://www.w3.org/2006/time#unitType"/>
                <owl:hasValue rdf:resource="http://www.w3.org/2006/time#unitMonth"/>
            </owl:Restriction>
        </rdfs:subClassOf>
        <rdfs:subClassOf>
            <owl:Restriction>
                <owl:onProperty rdf:resource="http://www.w3.org/2006/time#day"/>
                <owl:cardinality rdf:datatype="http://www.w3.org/2001/XMLSchema#nonNegativeInteger">0</owl:cardinality>
            </owl:Restriction>
        </rdfs:subClassOf>
        <rdfs:subClassOf>
            <owl:Restriction>
                <owl:onProperty rdf:resource="http://www.w3.org/2006/time#hour"/>
                <owl:cardinality rdf:datatype="http://www.w3.org/2001/XMLSchema#nonNegativeInteger">0</owl:cardinality>
            </owl:Restriction>
        </rdfs:subClassOf>
        <rdfs:subClassOf>
            <owl:Restriction>
                <owl:onProperty rdf:resource="http://www.w3.org/2006/time#minute"/>
                <owl:cardinality rdf:datatype="http://www.w3.org/2001/XMLSchema#nonNegativeInteger">0</owl:cardinality>
            </owl:Restriction>
        </rdfs:subClassOf>
        <rdfs:subClassOf>
            <owl:Restriction>
                <owl:onProperty rdf:resource="http://www.w3.org/2006/time#month"/>
                <owl:cardinality rdf:datatype="http://www.w3.org/2001/XMLSchema#nonNegativeInteger">1</owl:cardinality>
            </owl:Restriction>
        </rdfs:subClassOf>
        <rdfs:subClassOf>
            <owl:Restriction>
                <owl:onProperty rdf:resource="http://www.w3.org/2006/time#second"/>
                <owl:cardinality rdf:datatype="http://www.w3.org/2001/XMLSchema#nonNegativeInteger">0</owl:cardinality>
            </owl:Restriction>
        </rdfs:subClassOf>
        <rdfs:subClassOf>
            <owl:Restriction>
                <owl:onProperty rdf:resource="http://www.w3.org/2006/time#week"/>
                <owl:cardinality rdf:datatype="http://www.w3.org/2001/XMLSchema#nonNegativeInteger">0</owl:cardinality>
            </owl:Restriction>
        </rdfs:subClassOf>
        <rdfs:subClassOf>
            <owl:Restriction>
                <owl:onProperty rdf:resource="http://www.w3.org/2006/time#year"/>
                <owl:cardinality rdf:datatype="http://www.w3.org/2001/XMLSchema#nonNegativeInteger">0</owl:cardinality>
            </owl:Restriction>
        </rdfs:subClassOf>
        <rdfs:comment xml:lang="es">El mes del año.</rdfs:comment>
        <rdfs:comment xml:lang="en">The month of the year</rdfs:comment>
        <rdfs:label xml:lang="en">Month of year</rdfs:label>
        <rdfs:label xml:lang="es">mes del año</rdfs:label>
        <skos:definition xml:lang="es">El mes del año.</skos:definition>
        <skos:definition xml:lang="en">The month of the year</skos:definition>
        <skos:editorialNote xml:lang="es">Característica en riesgo - añadida en la revisión de 2017, y no utilizada todavía de forma amplia.</skos:editorialNote>
        <skos:editorialNote xml:lang="en">Feature at risk - added in 2017 revision, and not yet widely used. </skos:editorialNote>
        <skos:note xml:lang="es">La pertenencia a la clase &apos;mes del año&apos; está abierta, a permitir calendarios anuales alternativos y diferentes nombres de meses.</skos:note>
        <skos:note xml:lang="en">Membership of the class :MonthOfYear is open, to allow for alternative annual calendars and different month names.</skos:note>
    </owl:Class>
    


    <!-- http://www.w3.org/2006/time#ProperInterval -->


    <owl:Class rdf:about="http://www.w3.org/2006/time#ProperInterval">
        <rdfs:subClassOf rdf:resource="http://www.w3.org/2006/time#Interval"/>
        <rdfs:comment xml:lang="en">A temporal entity with non-zero extent or duration, i.e. for which the value of the beginning and end are different</rdfs:comment>
        <rdfs:comment xml:lang="es">Una entidad temporal con extensión o duración distinta de cero, es decir, para la cual los valores de principio y fin del intervalo son diferentes.</rdfs:comment>
        <rdfs:label xml:lang="en">Proper interval</rdfs:label>
        <rdfs:label xml:lang="es">intervalo propio</rdfs:label>
        <skos:definition xml:lang="en">A temporal entity with non-zero extent or duration, i.e. for which the value of the beginning and end are different</skos:definition>
        <skos:definition xml:lang="es">Una entidad temporal con extensión o duración distinta de cero, es decir, para la cual los valores de principio y fin del intervalo son diferentes.</skos:definition>
    </owl:Class>
    


    <!-- http://www.w3.org/2006/time#TRS -->


    <owl:Class rdf:about="http://www.w3.org/2006/time#TRS">
        <rdfs:comment xml:lang="en">A temporal reference system, such as a temporal coordinate system (with an origin, direction, and scale), a calendar-clock combination, or a (possibly hierarchical) ordinal system. 

This is a stub class, representing the set of all temporal reference systems.</rdfs:comment>
        <rdfs:comment xml:lang="es">Un sistema de referencia temporal, tal como un sistema de coordenadas temporales (con un origen, una dirección y una escala), una combinación calendario-reloj, o un sistema ordinal (posiblemente jerárquico).
        Esta clase comodín representa el conjunto de todos los sistemas de referencia temporal.</rdfs:comment>
        <rdfs:label xml:lang="en">Temporal Reference System</rdfs:label>
        <rdfs:label xml:lang="es">sistema de referencia temporal</rdfs:label>
        <skos:definition xml:lang="en">A temporal reference system, such as a temporal coordinate system (with an origin, direction, and scale), a calendar-clock combination, or a (possibly hierarchical) ordinal system. 

This is a stub class, representing the set of all temporal reference systems.</skos:definition>
        <skos:definition xml:lang="es">Un sistema de referencia temporal, tal como un sistema de coordenadas temporales (con un origen, una dirección y una escala), una combinación calendario-reloj, o un sistema ordinal (posiblemente jerárquico).
    Esta clase comodín representa el conjunto de todos los sistemas de referencia temporal.</skos:definition>
        <skos:note xml:lang="en">A taxonomy of temporal reference systems is provided in ISO 19108:2002 [ISO19108], including (a) calendar + clock systems; (b) temporal coordinate systems (i.e. numeric offset from an epoch); (c) temporal ordinal reference systems (i.e. ordered sequence of named intervals, not necessarily of equal duration).</skos:note>
        <skos:note xml:lang="es">En el ISO 19108:2002 [ISO19108] se proporciona una taxonomía de sistemas de referencia temporal, incluyendo (a) sistemas de calendario + reloj; (b) sistemas de coordenadas temporales (es decir, desplazamiento numérico a partir de una época); (c) sistemas de referencia ordinales temporales (es decir, secuencia ordenada de intervalos nombrados, no necesariamente de igual duración).</skos:note>
    </owl:Class>
    


    <!-- http://www.w3.org/2006/time#TemporalDuration -->


    <owl:Class rdf:about="http://www.w3.org/2006/time#TemporalDuration">
        <rdfs:comment xml:lang="es">Extensión de tiempo; duración de un intervalo de tiempo independiente de su posición de inicio particular.</rdfs:comment>
        <rdfs:comment xml:lang="en">Time extent; duration of a time interval separate from its particular start position</rdfs:comment>
        <rdfs:label xml:lang="en">Temporal duration</rdfs:label>
        <rdfs:label xml:lang="es">duración temporal</rdfs:label>
        <skos:definition xml:lang="es">Extensión de tiempo; duración de un intervalo de tiempo independiente de su posición de inicio particular.</skos:definition>
        <skos:definition xml:lang="en">Time extent; duration of a time interval separate from its particular start position</skos:definition>
    </owl:Class>
    


    <!-- http://www.w3.org/2006/time#TemporalEntity -->


    <owl:Class rdf:about="http://www.w3.org/2006/time#TemporalEntity">
        <owl:equivalentClass>
            <owl:Class>
                <owl:unionOf rdf:parseType="Collection">
                    <rdf:Description rdf:about="http://www.w3.org/2006/time#Instant"/>
                    <rdf:Description rdf:about="http://www.w3.org/2006/time#Interval"/>
                </owl:unionOf>
            </owl:Class>
        </owl:equivalentClass>
        <rdfs:subClassOf rdf:resource="http://www.w3.org/2002/07/owl#Thing"/>
        <rdfs:comment xml:lang="en">A temporal interval or instant.</rdfs:comment>
        <rdfs:comment xml:lang="es">Un intervalo temporal o un instante.</rdfs:comment>
        <rdfs:label xml:lang="en">Temporal entity</rdfs:label>
        <rdfs:label xml:lang="es">entidad temporal</rdfs:label>
        <skos:definition xml:lang="en">A temporal interval or instant.</skos:definition>
        <skos:definition xml:lang="es">Un intervalo temporal o un instante.</skos:definition>
    </owl:Class>
    


    <!-- http://www.w3.org/2006/time#TemporalPosition -->


    <owl:Class rdf:about="http://www.w3.org/2006/time#TemporalPosition">
        <rdfs:subClassOf>
            <owl:Restriction>
                <owl:onProperty rdf:resource="http://www.w3.org/2006/time#hasTRS"/>
                <owl:cardinality rdf:datatype="http://www.w3.org/2001/XMLSchema#nonNegativeInteger">1</owl:cardinality>
            </owl:Restriction>
        </rdfs:subClassOf>
        <rdfs:comment xml:lang="en">A position on a time-line</rdfs:comment>
        <rdfs:comment xml:lang="es">Una posición sobre una línea de tiempo.</rdfs:comment>
        <rdfs:label xml:lang="en">Temporal position</rdfs:label>
        <rdfs:label xml:lang="es">posición temporal</rdfs:label>
        <skos:definition xml:lang="en">A position on a time-line</skos:definition>
        <skos:definition xml:lang="es">Una posición sobre una línea de tiempo.</skos:definition>
    </owl:Class>
    


    <!-- http://www.w3.org/2006/time#TemporalUnit -->


    <owl:Class rdf:about="http://www.w3.org/2006/time#TemporalUnit">
        <rdfs:subClassOf rdf:resource="http://www.w3.org/2006/time#TemporalDuration"/>
        <rdfs:comment xml:lang="en">A standard duration, which provides a scale factor for a time extent, or the granularity or precision for a time position.</rdfs:comment>
        <rdfs:comment xml:lang="es">Una duración estándar, que proporciona un factor de escala para una extensión de tiempo, o la granularidad o precisión para una posición de tiempo.</rdfs:comment>
        <rdfs:label xml:lang="en">Temporal unit</rdfs:label>
        <rdfs:label xml:lang="es">unidad de tiempo</rdfs:label>
        <skos:changeNote xml:lang="en">Remove enumeration from definition, in order to allow other units to be used when required in other coordinate systems. 
NOTE: existing units are still present as members of the class, but the class membership is now open. 

In the original OWL-Time the following constraint appeared: 
  owl:oneOf (
      time:unitSecond
      time:unitMinute
      time:unitHour
      time:unitDay
      time:unitWeek
      time:unitMonth
      time:unitYear
    ) ;</skos:changeNote>
        <skos:definition xml:lang="en">A standard duration, which provides a scale factor for a time extent, or the granularity or precision for a time position.</skos:definition>
        <skos:definition xml:lang="es">Una duración estándar, que proporciona un factor de escala para una extensión de tiempo, o la granularidad o precisión para una posición de tiempo.</skos:definition>
        <skos:note xml:lang="es">La pertenencia de la clase &apos;unidad de tiempo&apos; está abierta, para permitir otras unidades de tiempo utilizadas en algunas aplicaciones técnicas (por ejemplo, millones de años o el mes Baha&apos;i).</skos:note>
        <skos:note xml:lang="en">Membership of the class TemporalUnit is open, to allow for other temporal units used in some technical applications (e.g. millions of years, Baha&apos;i month).</skos:note>
    </owl:Class>
    


    <!-- http://www.w3.org/2006/time#TimePosition -->


    <owl:Class rdf:about="http://www.w3.org/2006/time#TimePosition">
        <rdfs:subClassOf rdf:resource="http://www.w3.org/2006/time#TemporalPosition"/>
        <rdfs:subClassOf>
            <owl:Class>
                <owl:unionOf rdf:parseType="Collection">
                    <owl:Restriction>
                        <owl:onProperty rdf:resource="http://www.w3.org/2006/time#nominalPosition"/>
                        <owl:cardinality rdf:datatype="http://www.w3.org/2001/XMLSchema#nonNegativeInteger">1</owl:cardinality>
                    </owl:Restriction>
                    <owl:Restriction>
                        <owl:onProperty rdf:resource="http://www.w3.org/2006/time#numericPosition"/>
                        <owl:cardinality rdf:datatype="http://www.w3.org/2001/XMLSchema#nonNegativeInteger">1</owl:cardinality>
                    </owl:Restriction>
                </owl:unionOf>
            </owl:Class>
        </rdfs:subClassOf>
        <rdfs:comment xml:lang="en">A temporal position described using either a (nominal) value from an ordinal reference system, or a (numeric) value in a temporal coordinate system. </rdfs:comment>
        <rdfs:comment xml:lang="es">Una posición temporal descrita utilizando bien un valor (nominal) de un sistema de referencia ordinal, o un valor (numérico) en un sistema de coordenadas temporales.</rdfs:comment>
        <rdfs:label xml:lang="en">Time position</rdfs:label>
        <rdfs:label xml:lang="es">posición de tiempo</rdfs:label>
        <skos:definition xml:lang="en">A temporal position described using either a (nominal) value from an ordinal reference system, or a (numeric) value in a temporal coordinate system. </skos:definition>
        <skos:definition xml:lang="es">Una posición temporal descrita utilizando bien un valor (nominal) de un sistema de referencia ordinal, o un valor (numérico) en un sistema de coordenadas temporales.</skos:definition>
    </owl:Class>
    


    <!-- http://www.w3.org/2006/time#TimeZone -->


    <owl:Class rdf:about="http://www.w3.org/2006/time#TimeZone">
        <rdfs:comment xml:lang="en">A Time Zone specifies the amount by which the local time is offset from UTC. 
	A time zone is usually denoted geographically (e.g. Australian Eastern Daylight Time), with a constant value in a given region. 
The region where it applies and the offset from UTC are specified by a locally recognised governing authority.</rdfs:comment>
        <rdfs:comment xml:lang="es">Un huso horario especifica la cantidad en que la hora local está desplazada con respecto a UTC.
        Un huso horario normalmente se denota geográficamente (p.ej. el horario de verano del este de Australia), con un valor constante en una región dada.
        La región donde aplica y el desplazamiento desde UTC las especifica una autoridad gubernamental localmente reconocida.</rdfs:comment>
        <rdfs:label xml:lang="en">Time Zone</rdfs:label>
        <rdfs:label xml:lang="es">huso horario</rdfs:label>
        <skos:definition xml:lang="en">A Time Zone specifies the amount by which the local time is offset from UTC. 
	A time zone is usually denoted geographically (e.g. Australian Eastern Daylight Time), with a constant value in a given region. 
The region where it applies and the offset from UTC are specified by a locally recognised governing authority.</skos:definition>
        <skos:definition xml:lang="es">Un huso horario especifica la cantidad en que la hora local está desplazada con respecto a UTC.
    Un huso horario normalmente se denota geográficamente (p.ej. el horario de verano del este de Australia), con un valor constante en una región dada.
    La región donde aplica y el desplazamiento desde UTC las especifica una autoridad gubernamental localmente reconocida.</skos:definition>
        <skos:historyNote xml:lang="es">En la versión original de OWL-Time de 2006, se definió, en un espacio de nombres diferente &quot;http://www.w3.org/2006/timezone#&quot;, la clase &apos;huso horario&apos;, con varias propiedades específicas correspondientes a un modelo específico de huso horario.
    En la versión actual hay una clase con el mismo nombre local en el espacio de nombres de OWL-Time, eliminando la dependencia del espacio de nombres externo.
    Un axioma de alineación permite que los datos codificados de acuerdo con la versión anterior sean consistentes con la ontología actualizada.</skos:historyNote>
        <skos:historyNote>In the original 2006 version of OWL-Time, the TimeZone class, with several properties corresponding to a specific model of time-zones, was defined in a separate namespace &quot;http://www.w3.org/2006/timezone#&quot;. 

In the current version a class with same local name is put into the main OWL-Time namespace, removing the dependency on the external namespace. 

An alignment axiom 
	tzont:TimeZone rdfs:subClassOf time:TimeZone . 
allows data encoded according to the previous version to be consistent with the updated ontology. </skos:historyNote>
        <skos:note xml:lang="en">A designated timezone is associated with a geographic region. However, for a particular region the offset from UTC often varies seasonally, and the dates of the changes may vary from year to year. The timezone designation usually changes for the different seasons (e.g. Australian Eastern Standard Time vs. Australian Eastern Daylight Time). Furthermore, the offset for a timezone may change over longer timescales, though its designation might not.  

Detailed guidance about working with time zones is given in http://www.w3.org/TR/timezone/ .</skos:note>
        <skos:note xml:lang="en">An ontology for time zone descriptions was described in [owl-time-20060927] and provided as RDF in a separate namespace tzont:. However, that ontology was incomplete in scope, and the example datasets were selective. Furthermore, since the use of a class from an external ontology as the range of an ObjectProperty in OWL-Time creates a dependency, reference to the time zone class has been replaced with the &apos;stub&apos; class in the normative part of this version of OWL-Time.</skos:note>
        <skos:note xml:lang="es">Un huso horario designado está asociado con una región geográfica. Sin embargo, para una región particular el desplazamiento desde UTC a menudo varía según las estaciones, y las fechas de los cambios pueden variar de un año a otro. La designación de huso horario  normalmente cambia de una estación a otra (por ejemplo, el horario estándar frente al horario de verano ambos del este de Australia). Además, del desplazamiento para un huso horario puede cambiar sobre escalas de tiempo mayores, aunque su designación no lo haga.
    Se puede encontrar una guía detallada sobre el funcionamiento de husos horarios en http://www.w3.org/TR/timezone/.&quot;@es , &quot;En [owl-time-20060927] se describió una ontología para descripciones de husos horarios, y se proporcionó en un espacio de nombres separado tzont:. Sin embargo, dicha ontología estaba incompleta en su alcance, y el ejemplo de conjuntos de datos (datasets) era selectivo. Además, puesto que el uso de una clase de una ontología externa como el rango de una propiedad de objeto en OWL-Time crea una dependencia, la referencia a la clase huso horario se ha reemplazado por una clase que viene a ser un &quot;cajón de sastre&quot; en la en la parte normativa de esta versión de OWL-Time.</skos:note>
        <skos:scopeNote xml:lang="es">En esta implementación &apos;huso horario&apos; no tiene definidas propiedades. Se debería pensar como una superclase &quot;abstracta&quot; de todas las implementaciones de huso horario específicas.</skos:scopeNote>
        <skos:scopeNote>In this implementation TimeZone has no properties defined. It should be thought of as an &apos;abstract&apos; superclass of all specific timezone implementations.</skos:scopeNote>
    </owl:Class>
    


    <!-- http://www.w3.org/2006/time#Year -->


    <owl:Class rdf:about="http://www.w3.org/2006/time#Year">
        <rdfs:subClassOf rdf:resource="http://www.w3.org/2006/time#DurationDescription"/>
        <rdfs:subClassOf>
            <owl:Restriction>
                <owl:onProperty rdf:resource="http://www.w3.org/2006/time#days"/>
                <owl:cardinality rdf:datatype="http://www.w3.org/2001/XMLSchema#nonNegativeInteger">0</owl:cardinality>
            </owl:Restriction>
        </rdfs:subClassOf>
        <rdfs:subClassOf>
            <owl:Restriction>
                <owl:onProperty rdf:resource="http://www.w3.org/2006/time#hours"/>
                <owl:cardinality rdf:datatype="http://www.w3.org/2001/XMLSchema#nonNegativeInteger">0</owl:cardinality>
            </owl:Restriction>
        </rdfs:subClassOf>
        <rdfs:subClassOf>
            <owl:Restriction>
                <owl:onProperty rdf:resource="http://www.w3.org/2006/time#minutes"/>
                <owl:cardinality rdf:datatype="http://www.w3.org/2001/XMLSchema#nonNegativeInteger">0</owl:cardinality>
            </owl:Restriction>
        </rdfs:subClassOf>
        <rdfs:subClassOf>
            <owl:Restriction>
                <owl:onProperty rdf:resource="http://www.w3.org/2006/time#months"/>
                <owl:cardinality rdf:datatype="http://www.w3.org/2001/XMLSchema#nonNegativeInteger">0</owl:cardinality>
            </owl:Restriction>
        </rdfs:subClassOf>
        <rdfs:subClassOf>
            <owl:Restriction>
                <owl:onProperty rdf:resource="http://www.w3.org/2006/time#seconds"/>
                <owl:cardinality rdf:datatype="http://www.w3.org/2001/XMLSchema#nonNegativeInteger">0</owl:cardinality>
            </owl:Restriction>
        </rdfs:subClassOf>
        <rdfs:subClassOf>
            <owl:Restriction>
                <owl:onProperty rdf:resource="http://www.w3.org/2006/time#weeks"/>
                <owl:cardinality rdf:datatype="http://www.w3.org/2001/XMLSchema#nonNegativeInteger">0</owl:cardinality>
            </owl:Restriction>
        </rdfs:subClassOf>
        <rdfs:subClassOf>
            <owl:Restriction>
                <owl:onProperty rdf:resource="http://www.w3.org/2006/time#years"/>
                <owl:cardinality rdf:datatype="http://www.w3.org/2001/XMLSchema#nonNegativeInteger">1</owl:cardinality>
            </owl:Restriction>
        </rdfs:subClassOf>
        <rdfs:comment>Year duration</rdfs:comment>
        <rdfs:label xml:lang="en">Year</rdfs:label>
        <owl:deprecated rdf:datatype="http://www.w3.org/2001/XMLSchema#boolean">true</owl:deprecated>
        <skos:definition>Year duration</skos:definition>
        <skos:historyNote>Year was proposed in the 2006 version of OWL-Time as an example of how DurationDescription could be specialized to allow for a duration to be restricted to a number of years. 

It is deprecated in this edition of OWL-Time. </skos:historyNote>
        <skos:prefLabel xml:lang="it">Anno</skos:prefLabel>
        <skos:prefLabel xml:lang="fr">Année (calendrier)</skos:prefLabel>
        <skos:prefLabel xml:lang="pt">Ano</skos:prefLabel>
        <skos:prefLabel xml:lang="es">Año</skos:prefLabel>
        <skos:prefLabel xml:lang="nl">Jaar</skos:prefLabel>
        <skos:prefLabel xml:lang="de">Jahr</skos:prefLabel>
        <skos:prefLabel xml:lang="pl">Rok</skos:prefLabel>
        <skos:prefLabel xml:lang="en">Year</skos:prefLabel>
        <skos:prefLabel xml:lang="ru">Год</skos:prefLabel>
        <skos:prefLabel xml:lang="ar">سنة</skos:prefLabel>
        <skos:prefLabel xml:lang="ja">年</skos:prefLabel>
        <skos:prefLabel xml:lang="zh">年</skos:prefLabel>
    </owl:Class>
    


    <!-- 
    ///////////////////////////////////////////////////////////////////////////////////////
    //
    // Individuals
    //
    ///////////////////////////////////////////////////////////////////////////////////////
     -->


    


    <!-- http://www.semanticweb.org/sc3/ontologies/2022/0/Planning-Ontology#Activity_Etching -->


    <owl:NamedIndividual rdf:about="http://www.semanticweb.org/sc3/ontologies/2022/0/Planning-Ontology#Activity_Etching">
        <rdf:type rdf:resource="http://www.semanticweb.org/sc3/ontologies/2022/0/Planning-Ontology#Activity"/>
        <hasCapacity rdf:resource="http://www.semanticweb.org/sc3/ontologies/2022/0/Planning-Ontology#RequiredCap1"/>
        <hasResources rdf:resource="http://www.semanticweb.org/sc3/ontologies/2022/0/Planning-Ontology#FE_Aligner"/>
    </owl:NamedIndividual>
    


    <!-- http://www.semanticweb.org/sc3/ontologies/2022/0/Planning-Ontology#Activity_Oxide -->


    <owl:NamedIndividual rdf:about="http://www.semanticweb.org/sc3/ontologies/2022/0/Planning-Ontology#Activity_Oxide">
        <rdf:type rdf:resource="http://www.semanticweb.org/sc3/ontologies/2022/0/Planning-Ontology#Activity"/>
        <hasCapacity rdf:resource="http://www.semanticweb.org/sc3/ontologies/2022/0/Planning-Ontology#RequiredCap2"/>
        <hasResources rdf:resource="http://www.semanticweb.org/sc3/ontologies/2022/0/Planning-Ontology#FE_Implanter"/>
    </owl:NamedIndividual>
    


    <!-- http://www.semanticweb.org/sc3/ontologies/2022/0/Planning-Ontology#Activity_Photo -->


    <owl:NamedIndividual rdf:about="http://www.semanticweb.org/sc3/ontologies/2022/0/Planning-Ontology#Activity_Photo">
        <rdf:type rdf:resource="http://www.semanticweb.org/sc3/ontologies/2022/0/Planning-Ontology#Activity"/>
        <hasCapacity rdf:resource="http://www.semanticweb.org/sc3/ontologies/2022/0/Planning-Ontology#RequiredCap3"/>
        <hasResources rdf:resource="http://www.semanticweb.org/sc3/ontologies/2022/0/Planning-Ontology#FE_Stepper_1"/>
    </owl:NamedIndividual>
    


    <!-- http://www.semanticweb.org/sc3/ontologies/2022/0/Planning-Ontology#Activity_UV_Bake -->


    <owl:NamedIndividual rdf:about="http://www.semanticweb.org/sc3/ontologies/2022/0/Planning-Ontology#Activity_UV_Bake">
        <rdf:type rdf:resource="http://www.semanticweb.org/sc3/ontologies/2022/0/Planning-Ontology#Activity"/>
        <hasCapacity rdf:resource="http://www.semanticweb.org/sc3/ontologies/2022/0/Planning-Ontology#RequiredCap4"/>
        <hasResources rdf:resource="http://www.semanticweb.org/sc3/ontologies/2022/0/Planning-Ontology#FE_Stepper_2"/>
    </owl:NamedIndividual>
    


    <!-- http://www.semanticweb.org/sc3/ontologies/2022/0/Planning-Ontology#All_Planning_Objects_have_to_be_positive -->


    <owl:NamedIndividual rdf:about="http://www.semanticweb.org/sc3/ontologies/2022/0/Planning-Ontology#All_Planning_Objects_have_to_be_positive">
        <rdf:type rdf:resource="http://www.semanticweb.org/sc3/ontologies/2022/0/Planning-Ontology#PlanningConstraint"/>
        <sc3:formula>forall($g in Products, $t in PlanningHorizon, $j in Frontends) -&gt; FE_Y($j, $g, $t) &gt;= 0;
forall($g in Products, $t in PlanningHorizon, $j in Frontends) -&gt; FE_X($j, $g, $t) &gt;= 0;
forall($g in Products, $t in PlanningHorizon, $j in Frontends) -&gt; FE_Wip($j, $g, $t) &gt;= 0;
forall($g in Products, $t in PlanningHorizon) -&gt; FE_Inventory($g, $t) &gt;= 0;
forall($g in Products, $t in PlanningHorizon) -&gt; FE_Backlog($g, $t) &gt;= 0;</sc3:formula>
    </owl:NamedIndividual>
    


    <!-- http://www.semanticweb.org/sc3/ontologies/2022/0/Planning-Ontology#AvailableCap1 -->


    <owl:NamedIndividual rdf:about="http://www.semanticweb.org/sc3/ontologies/2022/0/Planning-Ontology#AvailableCap1">
        <rdf:type rdf:resource="http://www.semanticweb.org/sc3/ontologies/2022/0/Planning-Ontology#AvailableCapacity"/>
    </owl:NamedIndividual>
    


    <!-- http://www.semanticweb.org/sc3/ontologies/2022/0/Planning-Ontology#AvailableCap2 -->


    <owl:NamedIndividual rdf:about="http://www.semanticweb.org/sc3/ontologies/2022/0/Planning-Ontology#AvailableCap2">
        <rdf:type rdf:resource="http://www.semanticweb.org/sc3/ontologies/2022/0/Planning-Ontology#AvailableCapacity"/>
    </owl:NamedIndividual>
    


    <!-- http://www.semanticweb.org/sc3/ontologies/2022/0/Planning-Ontology#AvailableCap3 -->


    <owl:NamedIndividual rdf:about="http://www.semanticweb.org/sc3/ontologies/2022/0/Planning-Ontology#AvailableCap3">
        <rdf:type rdf:resource="http://www.semanticweb.org/sc3/ontologies/2022/0/Planning-Ontology#AvailableCapacity"/>
    </owl:NamedIndividual>
    


    <!-- http://www.semanticweb.org/sc3/ontologies/2022/0/Planning-Ontology#AvailableCap4 -->


    <owl:NamedIndividual rdf:about="http://www.semanticweb.org/sc3/ontologies/2022/0/Planning-Ontology#AvailableCap4">
        <rdf:type rdf:resource="http://www.semanticweb.org/sc3/ontologies/2022/0/Planning-Ontology#AvailableCapacity"/>
    </owl:NamedIndividual>
    


    <!-- http://www.semanticweb.org/sc3/ontologies/2022/0/Planning-Ontology#AvailableCap5 -->


    <owl:NamedIndividual rdf:about="http://www.semanticweb.org/sc3/ontologies/2022/0/Planning-Ontology#AvailableCap5">
        <rdf:type rdf:resource="http://www.semanticweb.org/sc3/ontologies/2022/0/Planning-Ontology#AvailableCapacity"/>
    </owl:NamedIndividual>
    


    <!-- http://www.semanticweb.org/sc3/ontologies/2022/0/Planning-Ontology#Bom_Product_1 -->


    <owl:NamedIndividual rdf:about="http://www.semanticweb.org/sc3/ontologies/2022/0/Planning-Ontology#Bom_Product_1">
        <rdf:type rdf:resource="http://www.semanticweb.org/sc3/ontologies/2022/0/Planning-Ontology#BillOfMaterial"/>
        <hasLocation rdf:resource="http://www.semanticweb.org/sc3/ontologies/2022/0/Planning-Ontology#Frontend_1"/>
        <hasProduct rdf:resource="http://www.semanticweb.org/sc3/ontologies/2022/0/Planning-Ontology#Product_1"/>
    </owl:NamedIndividual>
    


    <!-- http://www.semanticweb.org/sc3/ontologies/2022/0/Planning-Ontology#Borderless_FE1_zu_FE2 -->


    <owl:NamedIndividual rdf:about="http://www.semanticweb.org/sc3/ontologies/2022/0/Planning-Ontology#Borderless_FE1_zu_FE2">
        <rdf:type rdf:resource="http://www.semanticweb.org/sc3/ontologies/2022/0/Planning-Ontology#PlanningObject"/>
        <hasActivities rdf:resource="http://www.semanticweb.org/sc3/ontologies/2022/0/Planning-Ontology#Activity_Photo"/>
        <hasLocation rdf:resource="http://www.semanticweb.org/sc3/ontologies/2022/0/Planning-Ontology#Frontend_2"/>
        <hasOwner rdf:resource="http://www.semanticweb.org/sc3/ontologies/2022/0/Planning-Ontology#FE1"/>
        <hasProduct rdf:resource="http://www.semanticweb.org/sc3/ontologies/2022/0/Planning-Ontology#Product_1"/>
        <hasDueDate>1 week</hasDueDate>
        <hasQuantity rdf:datatype="http://www.w3.org/2001/XMLSchema#integer">10</hasQuantity>
    </owl:NamedIndividual>
    


    <!-- http://www.semanticweb.org/sc3/ontologies/2022/0/Planning-Ontology#Capacity_Restriction_Equation -->


    <owl:NamedIndividual rdf:about="http://www.semanticweb.org/sc3/ontologies/2022/0/Planning-Ontology#Capacity_Restriction_Equation">
        <rdf:type rdf:resource="http://www.semanticweb.org/sc3/ontologies/2022/0/Planning-Ontology#PlanningConstraint"/>
        <sc3:formula>forall($k in WorkCenters, $j in Frontends, t in PlanningHorizon) sum($g in Products, $l in OperationCountOnWorkCenter($j, $k, $g) -&gt;
		FE_Y($j, $g, $t, OperationsOnWorkCenter($j, $k, $g, $l)) * alpha($j, $g, OperationsOnWorkCenter($j, $k, $g, $l)) &lt;= WorkCenterCapacity($t, $j, $k);
	

WorkCenters (Resources)=FE_Aligner, FE_Stepper_2, FE_Stepper_1, FE_Implanter
Frontends= Frontend_1, Frontend_2;
Products= Product_1;
OperationCountOnWorkCenter=Product($numberOfOperationsOnSameResource);
alpha= Activity($hasRequiredCapacity(Product($hasActivities)));
WorkCenterCapacity= FE_Aligner($hasAvailableCapacity, $hasLocation), FE_Stepper_2($hasAvailableCapacity, $hasLocation), FE_Stepper_1($hasAvailableCapacity, $hasLocation), FE_Implanter($hasAvailableCapacity, $hasLocation);</sc3:formula>
    </owl:NamedIndividual>
    


    <!-- http://www.semanticweb.org/sc3/ontologies/2022/0/Planning-Ontology#FE1 -->


    <owl:NamedIndividual rdf:about="http://www.semanticweb.org/sc3/ontologies/2022/0/Planning-Ontology#FE1">
        <rdf:type rdf:resource="http://www.semanticweb.org/sc3/ontologies/2022/0/Planning-Ontology#Owner"/>
    </owl:NamedIndividual>
    


    <!-- http://www.semanticweb.org/sc3/ontologies/2022/0/Planning-Ontology#FE1_CostMinimization -->


    <owl:NamedIndividual rdf:about="http://www.semanticweb.org/sc3/ontologies/2022/0/Planning-Ontology#FE1_CostMinimization">
        <rdf:type rdf:resource="http://www.semanticweb.org/sc3/ontologies/2022/0/Planning-Ontology#PlaningPurpose"/>
        <hasCriterias rdf:resource="http://www.semanticweb.org/sc3/ontologies/2022/0/Planning-Ontology#Minimization"/>
        <hasPerformanceMeasures rdf:resource="http://www.semanticweb.org/sc3/ontologies/2022/0/Planning-Ontology#MinimizeBacklog"/>
        <hasPerformanceMeasures rdf:resource="http://www.semanticweb.org/sc3/ontologies/2022/0/Planning-Ontology#MinimizeInventoryLevel"/>
        <hasPerformanceMeasures rdf:resource="http://www.semanticweb.org/sc3/ontologies/2022/0/Planning-Ontology#MinimizeWipCosts"/>
        <hasPlanningObjects rdf:resource="http://www.semanticweb.org/sc3/ontologies/2022/0/Planning-Ontology#FE_Backlog"/>
        <hasPlanningObjects rdf:resource="http://www.semanticweb.org/sc3/ontologies/2022/0/Planning-Ontology#FE_Inventory"/>
        <hasPlanningObjects rdf:resource="http://www.semanticweb.org/sc3/ontologies/2022/0/Planning-Ontology#FE_Wip"/>
        <hasPlanningObjects rdf:resource="http://www.semanticweb.org/sc3/ontologies/2022/0/Planning-Ontology#FE_X"/>
        <hasPlanningObjects rdf:resource="http://www.semanticweb.org/sc3/ontologies/2022/0/Planning-Ontology#FE_Y"/>
        <hasCosts>backlog=150</hasCosts>
        <hasCosts>inventory=15</hasCosts>
        <hasCosts>wip=50</hasCosts>
        <hasPlanningWindow>12 weeks</hasPlanningWindow>
        <sc3:formula>sum($g in Products, $t in PlanningHorizon)--&gt; sum($j in Frontends) (WipCosts($g, $t) * FE_Wip($j, $g, $t)) + InventoryCosts($g, $t) * FE_Inventory($g, $t) + BacklogCosts($g, $t) * FE_Backlog($g, $t);

Frontends= Frontend_1, Frontend_2;
Products= Product_1;
InventoryCosts= $(hasCosts($inventory));
BacklogCosts= $(hasCosts($backlog));
WipCosts= $(hasCosts($wip));</sc3:formula>
    </owl:NamedIndividual>
    


    <!-- http://www.semanticweb.org/sc3/ontologies/2022/0/Planning-Ontology#FE2 -->


    <owl:NamedIndividual rdf:about="http://www.semanticweb.org/sc3/ontologies/2022/0/Planning-Ontology#FE2">
        <rdf:type rdf:resource="http://www.semanticweb.org/sc3/ontologies/2022/0/Planning-Ontology#Owner"/>
    </owl:NamedIndividual>
    


    <!-- http://www.semanticweb.org/sc3/ontologies/2022/0/Planning-Ontology#FE_Aligner -->


    <owl:NamedIndividual rdf:about="http://www.semanticweb.org/sc3/ontologies/2022/0/Planning-Ontology#FE_Aligner">
        <rdf:type rdf:resource="http://www.semanticweb.org/sc3/ontologies/2022/0/ozone-ontology#Resource"/>
        <hasCapacity rdf:resource="http://www.semanticweb.org/sc3/ontologies/2022/0/Planning-Ontology#AvailableCap1"/>
        <hasLocation rdf:resource="http://www.semanticweb.org/sc3/ontologies/2022/0/Planning-Ontology#Frontend_1"/>
    </owl:NamedIndividual>
    


    <!-- http://www.semanticweb.org/sc3/ontologies/2022/0/Planning-Ontology#FE_Backlog -->


    <owl:NamedIndividual rdf:about="http://www.semanticweb.org/sc3/ontologies/2022/0/Planning-Ontology#FE_Backlog">
        <rdf:type rdf:resource="http://www.semanticweb.org/sc3/ontologies/2022/0/Planning-Ontology#PlanningObject"/>
        <hasLocation rdf:resource="http://www.semanticweb.org/sc3/ontologies/2022/0/Planning-Ontology#Frontend_1"/>
        <hasLocation rdf:resource="http://www.semanticweb.org/sc3/ontologies/2022/0/Planning-Ontology#Frontend_2"/>
        <hasProduct rdf:resource="http://www.semanticweb.org/sc3/ontologies/2022/0/Planning-Ontology#Product_1"/>
        <hasPeriod></hasPeriod>
        <time:day></time:day>
    </owl:NamedIndividual>
    


    <!-- http://www.semanticweb.org/sc3/ontologies/2022/0/Planning-Ontology#FE_Implanter -->


    <owl:NamedIndividual rdf:about="http://www.semanticweb.org/sc3/ontologies/2022/0/Planning-Ontology#FE_Implanter">
        <rdf:type rdf:resource="http://www.semanticweb.org/sc3/ontologies/2022/0/ozone-ontology#Resource"/>
        <hasCapacity rdf:resource="http://www.semanticweb.org/sc3/ontologies/2022/0/Planning-Ontology#AvailableCap2"/>
        <hasLocation rdf:resource="http://www.semanticweb.org/sc3/ontologies/2022/0/Planning-Ontology#Frontend_1"/>
    </owl:NamedIndividual>
    


    <!-- http://www.semanticweb.org/sc3/ontologies/2022/0/Planning-Ontology#FE_Inventory -->


    <owl:NamedIndividual rdf:about="http://www.semanticweb.org/sc3/ontologies/2022/0/Planning-Ontology#FE_Inventory">
        <rdf:type rdf:resource="http://www.semanticweb.org/sc3/ontologies/2022/0/Planning-Ontology#PlanningObject"/>
        <hasLocation rdf:resource="http://www.semanticweb.org/sc3/ontologies/2022/0/Planning-Ontology#Frontend_1"/>
        <hasLocation rdf:resource="http://www.semanticweb.org/sc3/ontologies/2022/0/Planning-Ontology#Frontend_2"/>
        <hasProduct rdf:resource="http://www.semanticweb.org/sc3/ontologies/2022/0/Planning-Ontology#Product_1"/>
        <hasProduct rdf:resource="http://www.semanticweb.org/sc3/ontologies/2022/0/Planning-Ontology#Product_2"/>
        <hasPeriod></hasPeriod>
        <time:day></time:day>
    </owl:NamedIndividual>
    


    <!-- http://www.semanticweb.org/sc3/ontologies/2022/0/Planning-Ontology#FE_Stepper_1 -->


    <owl:NamedIndividual rdf:about="http://www.semanticweb.org/sc3/ontologies/2022/0/Planning-Ontology#FE_Stepper_1">
        <rdf:type rdf:resource="http://www.semanticweb.org/sc3/ontologies/2022/0/ozone-ontology#Resource"/>
        <hasCapacity rdf:resource="http://www.semanticweb.org/sc3/ontologies/2022/0/Planning-Ontology#AvailableCap3"/>
        <hasLocation rdf:resource="http://www.semanticweb.org/sc3/ontologies/2022/0/Planning-Ontology#Frontend_1"/>
    </owl:NamedIndividual>
    


    <!-- http://www.semanticweb.org/sc3/ontologies/2022/0/Planning-Ontology#FE_Stepper_2 -->


    <owl:NamedIndividual rdf:about="http://www.semanticweb.org/sc3/ontologies/2022/0/Planning-Ontology#FE_Stepper_2">
        <rdf:type rdf:resource="http://www.semanticweb.org/sc3/ontologies/2022/0/ozone-ontology#Resource"/>
        <hasCapacity rdf:resource="http://www.semanticweb.org/sc3/ontologies/2022/0/Planning-Ontology#AvailableCap4"/>
        <hasLocation rdf:resource="http://www.semanticweb.org/sc3/ontologies/2022/0/Planning-Ontology#Frontend_1"/>
    </owl:NamedIndividual>
    


    <!-- http://www.semanticweb.org/sc3/ontologies/2022/0/Planning-Ontology#FE_Wip -->


    <owl:NamedIndividual rdf:about="http://www.semanticweb.org/sc3/ontologies/2022/0/Planning-Ontology#FE_Wip">
        <rdf:type rdf:resource="http://www.semanticweb.org/sc3/ontologies/2022/0/Planning-Ontology#PlanningObject"/>
        <hasLocation rdf:resource="http://www.semanticweb.org/sc3/ontologies/2022/0/Planning-Ontology#Frontend_1"/>
        <hasLocation rdf:resource="http://www.semanticweb.org/sc3/ontologies/2022/0/Planning-Ontology#Frontend_2"/>
        <hasProduct rdf:resource="http://www.semanticweb.org/sc3/ontologies/2022/0/Planning-Ontology#Product_1"/>
        <hasProduct rdf:resource="http://www.semanticweb.org/sc3/ontologies/2022/0/Planning-Ontology#Product_2"/>
        <hasPeriod></hasPeriod>
        <time:day></time:day>
    </owl:NamedIndividual>
    


    <!-- http://www.semanticweb.org/sc3/ontologies/2022/0/Planning-Ontology#FE_X -->


    <owl:NamedIndividual rdf:about="http://www.semanticweb.org/sc3/ontologies/2022/0/Planning-Ontology#FE_X">
        <rdf:type rdf:resource="http://www.semanticweb.org/sc3/ontologies/2022/0/Planning-Ontology#PlanningObject"/>
        <hasLocation rdf:resource="http://www.semanticweb.org/sc3/ontologies/2022/0/Planning-Ontology#Frontend_1"/>
        <hasLocation rdf:resource="http://www.semanticweb.org/sc3/ontologies/2022/0/Planning-Ontology#Frontend_2"/>
        <hasProduct rdf:resource="http://www.semanticweb.org/sc3/ontologies/2022/0/Planning-Ontology#Product_1"/>
        <hasProduct rdf:resource="http://www.semanticweb.org/sc3/ontologies/2022/0/Planning-Ontology#Product_2"/>
        <hasPeriod></hasPeriod>
        <time:day></time:day>
    </owl:NamedIndividual>
    


    <!-- http://www.semanticweb.org/sc3/ontologies/2022/0/Planning-Ontology#FE_Y -->


    <owl:NamedIndividual rdf:about="http://www.semanticweb.org/sc3/ontologies/2022/0/Planning-Ontology#FE_Y">
        <rdf:type rdf:resource="http://www.semanticweb.org/sc3/ontologies/2022/0/Planning-Ontology#PlanningObject"/>
        <hasLocation rdf:resource="http://www.semanticweb.org/sc3/ontologies/2022/0/Planning-Ontology#Frontend_1"/>
        <hasLocation rdf:resource="http://www.semanticweb.org/sc3/ontologies/2022/0/Planning-Ontology#Frontend_2"/>
        <hasProduct rdf:resource="http://www.semanticweb.org/sc3/ontologies/2022/0/Planning-Ontology#Product_1"/>
        <hasProduct rdf:resource="http://www.semanticweb.org/sc3/ontologies/2022/0/Planning-Ontology#Product_2"/>
        <hasPeriod></hasPeriod>
        <time:day></time:day>
    </owl:NamedIndividual>
    


    <!-- http://www.semanticweb.org/sc3/ontologies/2022/0/Planning-Ontology#Frontend_1 -->


    <owl:NamedIndividual rdf:about="http://www.semanticweb.org/sc3/ontologies/2022/0/Planning-Ontology#Frontend_1">
        <rdf:type rdf:resource="http://www.semanticweb.org/sc3/ontologies/2022/0/Planning-Ontology#Location"/>
        <hasProduct rdf:resource="http://www.semanticweb.org/sc3/ontologies/2022/0/Planning-Ontology#Product_1"/>
    </owl:NamedIndividual>
    


    <!-- http://www.semanticweb.org/sc3/ontologies/2022/0/Planning-Ontology#Frontend_2 -->


    <owl:NamedIndividual rdf:about="http://www.semanticweb.org/sc3/ontologies/2022/0/Planning-Ontology#Frontend_2">
        <rdf:type rdf:resource="http://www.semanticweb.org/sc3/ontologies/2022/0/Planning-Ontology#Location"/>
        <hasLocation rdf:resource="http://www.semanticweb.org/sc3/ontologies/2022/0/Planning-Ontology#Frontend_1"/>
        <hasProduct rdf:resource="http://www.semanticweb.org/sc3/ontologies/2022/0/Planning-Ontology#Product_1"/>
    </owl:NamedIndividual>
    


    <!-- http://www.semanticweb.org/sc3/ontologies/2022/0/Planning-Ontology#Inventory_Balance_Equation -->


    <owl:NamedIndividual rdf:about="http://www.semanticweb.org/sc3/ontologies/2022/0/Planning-Ontology#Inventory_Balance_Equation">
        <rdf:type rdf:resource="http://www.semanticweb.org/sc3/ontologies/2022/0/Planning-Ontology#PlanningConstraint"/>
        <sc3:formula>forall($g in Products, $t in PlanningHorizon) -&gt; FE_Inventory($p, $t) = FE_Inventory($g, $t-1) + sum(j in Frontends)(FE_Y($j,$g,$t) - FE_Backlog($g, $t-1) + FE_Backlog($g, $t) + sum(j in Frontends)(Inventory_DB($j, $g, $t) - Demand($g, $t);

Frontends= Frontend_1, Frontend_2;
Products= Product_1;</sc3:formula>
    </owl:NamedIndividual>
    


    <!-- http://www.semanticweb.org/sc3/ontologies/2022/0/Planning-Ontology#Inventory_DB -->


    <owl:NamedIndividual rdf:about="http://www.semanticweb.org/sc3/ontologies/2022/0/Planning-Ontology#Inventory_DB">
        <rdf:type rdf:resource="http://www.semanticweb.org/sc3/ontologies/2022/0/Planning-Ontology#Inventory"/>
        <hasLocation rdf:resource="http://www.semanticweb.org/sc3/ontologies/2022/0/Planning-Ontology#Frontend_1"/>
        <hasLocation rdf:resource="http://www.semanticweb.org/sc3/ontologies/2022/0/Planning-Ontology#Frontend_2"/>
        <hasProduct rdf:resource="http://www.semanticweb.org/sc3/ontologies/2022/0/Planning-Ontology#Product_1"/>
        <hasProduct rdf:resource="http://www.semanticweb.org/sc3/ontologies/2022/0/Planning-Ontology#Product_2"/>
        <hasPeriod></hasPeriod>
        <time:day></time:day>
    </owl:NamedIndividual>
    


    <!-- http://www.semanticweb.org/sc3/ontologies/2022/0/Planning-Ontology#Material_Flow_Equation -->


    <owl:NamedIndividual rdf:about="http://www.semanticweb.org/sc3/ontologies/2022/0/Planning-Ontology#Material_Flow_Equation">
        <rdf:type rdf:resource="http://www.semanticweb.org/sc3/ontologies/2022/0/Planning-Ontology#PlanningConstraint"/>
        <sc3:formula>forall($g in Products, $j in Frontends, $t in PlanningHorizon, $l in Steps($j, $g) -&gt; FE_Y($j, $g, $t, $l) = FE_X($j, $g, $t - LeadTime($g, $l));
			

Frontends= Frontend_1, Frontend_2;
Products= Product_1;
Steps= Product($hasActivities);
LeadTime= Product($hasLeadTime);</sc3:formula>
    </owl:NamedIndividual>
    


    <!-- http://www.semanticweb.org/sc3/ontologies/2022/0/Planning-Ontology#Minimization -->


    <owl:NamedIndividual rdf:about="http://www.semanticweb.org/sc3/ontologies/2022/0/Planning-Ontology#Minimization">
        <rdf:type rdf:resource="http://www.semanticweb.org/sc3/ontologies/2022/0/Planning-Ontology#Criteria"/>
    </owl:NamedIndividual>
    


    <!-- http://www.semanticweb.org/sc3/ontologies/2022/0/Planning-Ontology#MinimizeBacklog -->


    <owl:NamedIndividual rdf:about="http://www.semanticweb.org/sc3/ontologies/2022/0/Planning-Ontology#MinimizeBacklog"/>
    


    <!-- http://www.semanticweb.org/sc3/ontologies/2022/0/Planning-Ontology#MinimizeInventoryLevel -->


    <owl:NamedIndividual rdf:about="http://www.semanticweb.org/sc3/ontologies/2022/0/Planning-Ontology#MinimizeInventoryLevel"/>
    


    <!-- http://www.semanticweb.org/sc3/ontologies/2022/0/Planning-Ontology#MinimizeWipCosts -->


    <owl:NamedIndividual rdf:about="http://www.semanticweb.org/sc3/ontologies/2022/0/Planning-Ontology#MinimizeWipCosts"/>
    


    <!-- http://www.semanticweb.org/sc3/ontologies/2022/0/Planning-Ontology#Part1_Product_1 -->


    <owl:NamedIndividual rdf:about="http://www.semanticweb.org/sc3/ontologies/2022/0/Planning-Ontology#Part1_Product_1">
        <rdf:type rdf:resource="http://www.semanticweb.org/sc3/ontologies/2022/0/Planning-Ontology#Part"/>
        <hasPlanningObject rdf:resource="http://www.semanticweb.org/sc3/ontologies/2022/0/Planning-Ontology#Borderless_FE1_zu_FE2"/>
        <hasProduct rdf:resource="http://www.semanticweb.org/sc3/ontologies/2022/0/Planning-Ontology#Product_1"/>
        <hasDueDate>1 week</hasDueDate>
    </owl:NamedIndividual>
    


    <!-- http://www.semanticweb.org/sc3/ontologies/2022/0/Planning-Ontology#Part2_Product_1 -->


    <owl:NamedIndividual rdf:about="http://www.semanticweb.org/sc3/ontologies/2022/0/Planning-Ontology#Part2_Product_1">
        <rdf:type rdf:resource="http://www.semanticweb.org/sc3/ontologies/2022/0/Planning-Ontology#Part"/>
        <hasPlanningObject rdf:resource="http://www.semanticweb.org/sc3/ontologies/2022/0/Planning-Ontology#Borderless_FE1_zu_FE2"/>
        <hasProduct rdf:resource="http://www.semanticweb.org/sc3/ontologies/2022/0/Planning-Ontology#Product_1"/>
        <hasDueDate>1 week</hasDueDate>
    </owl:NamedIndividual>
    


    <!-- http://www.semanticweb.org/sc3/ontologies/2022/0/Planning-Ontology#Part3_Product_1 -->


    <owl:NamedIndividual rdf:about="http://www.semanticweb.org/sc3/ontologies/2022/0/Planning-Ontology#Part3_Product_1">
        <rdf:type rdf:resource="http://www.semanticweb.org/sc3/ontologies/2022/0/Planning-Ontology#Part"/>
        <hasProduct rdf:resource="http://www.semanticweb.org/sc3/ontologies/2022/0/Planning-Ontology#Product_1"/>
        <hasDueDate>3 weeks</hasDueDate>
    </owl:NamedIndividual>
    


    <!-- http://www.semanticweb.org/sc3/ontologies/2022/0/Planning-Ontology#Part4_Product_1 -->


    <owl:NamedIndividual rdf:about="http://www.semanticweb.org/sc3/ontologies/2022/0/Planning-Ontology#Part4_Product_1">
        <rdf:type rdf:resource="http://www.semanticweb.org/sc3/ontologies/2022/0/Planning-Ontology#Part"/>
        <hasProduct rdf:resource="http://www.semanticweb.org/sc3/ontologies/2022/0/Planning-Ontology#Product_1"/>
        <hasDueDate>4 weeks</hasDueDate>
    </owl:NamedIndividual>
    


    <!-- http://www.semanticweb.org/sc3/ontologies/2022/0/Planning-Ontology#Part5_Product_1 -->


    <owl:NamedIndividual rdf:about="http://www.semanticweb.org/sc3/ontologies/2022/0/Planning-Ontology#Part5_Product_1">
        <rdf:type rdf:resource="http://www.semanticweb.org/sc3/ontologies/2022/0/Planning-Ontology#Part"/>
        <hasProduct rdf:resource="http://www.semanticweb.org/sc3/ontologies/2022/0/Planning-Ontology#Product_1"/>
        <hasDueDate>5 weeks</hasDueDate>
    </owl:NamedIndividual>
    


    <!-- http://www.semanticweb.org/sc3/ontologies/2022/0/Planning-Ontology#PeriodLength -->


    <owl:NamedIndividual rdf:about="http://www.semanticweb.org/sc3/ontologies/2022/0/Planning-Ontology#PeriodLength">
        <rdf:type rdf:resource="http://www.w3.org/2006/time#Interval"/>
        <time:days rdf:datatype="http://www.w3.org/2001/XMLSchema#integer">1</time:days>
    </owl:NamedIndividual>
    


    <!-- http://www.semanticweb.org/sc3/ontologies/2022/0/Planning-Ontology#PlanningInstance_Frontend_1 -->


    <owl:NamedIndividual rdf:about="http://www.semanticweb.org/sc3/ontologies/2022/0/Planning-Ontology#PlanningInstance_Frontend_1">
        <rdf:type rdf:resource="http://www.semanticweb.org/sc3/ontologies/2022/0/Planning-Ontology#PlanningInstance"/>
        <hasConstraint rdf:resource="http://www.semanticweb.org/sc3/ontologies/2022/0/Planning-Ontology#Capacity_Restriction_Equation"/>
        <hasConstraint rdf:resource="http://www.semanticweb.org/sc3/ontologies/2022/0/Planning-Ontology#Inventory_Balance_Equation"/>
        <hasConstraint rdf:resource="http://www.semanticweb.org/sc3/ontologies/2022/0/Planning-Ontology#Material_Flow_Equation"/>
        <hasConstraint rdf:resource="http://www.semanticweb.org/sc3/ontologies/2022/0/Planning-Ontology#Wip_Balance_Equation"/>
    </owl:NamedIndividual>
    


    <!-- http://www.semanticweb.org/sc3/ontologies/2022/0/Planning-Ontology#Process_Product_1 -->


    <owl:NamedIndividual rdf:about="http://www.semanticweb.org/sc3/ontologies/2022/0/Planning-Ontology#Process_Product_1"/>
    


    <!-- http://www.semanticweb.org/sc3/ontologies/2022/0/Planning-Ontology#Product_1 -->


    <owl:NamedIndividual rdf:about="http://www.semanticweb.org/sc3/ontologies/2022/0/Planning-Ontology#Product_1">
        <rdf:type rdf:resource="http://www.semanticweb.org/sc3/ontologies/2022/0/ozone-ontology#Product"/>
        <hasActivities rdf:resource="http://www.semanticweb.org/sc3/ontologies/2022/0/Planning-Ontology#Activity_Etching"/>
        <hasActivities rdf:resource="http://www.semanticweb.org/sc3/ontologies/2022/0/Planning-Ontology#Activity_Oxide"/>
        <hasActivities rdf:resource="http://www.semanticweb.org/sc3/ontologies/2022/0/Planning-Ontology#Activity_Photo"/>
        <hasActivities rdf:resource="http://www.semanticweb.org/sc3/ontologies/2022/0/Planning-Ontology#Activity_UV_Bake"/>
        <hasLocation rdf:resource="http://www.semanticweb.org/sc3/ontologies/2022/0/Planning-Ontology#Frontend_1"/>
        <hasProcess rdf:resource="http://www.semanticweb.org/sc3/ontologies/2022/0/Planning-Ontology#Process_Product_1"/>
        <hasProduct rdf:resource="http://www.semanticweb.org/sc3/ontologies/2022/0/Planning-Ontology#Product_1"/>
    </owl:NamedIndividual>
    


    <!-- http://www.semanticweb.org/sc3/ontologies/2022/0/Planning-Ontology#Product_2 -->


    <owl:NamedIndividual rdf:about="http://www.semanticweb.org/sc3/ontologies/2022/0/Planning-Ontology#Product_2">
        <rdf:type rdf:resource="http://www.semanticweb.org/sc3/ontologies/2022/0/ozone-ontology#Product"/>
    </owl:NamedIndividual>
    


    <!-- http://www.semanticweb.org/sc3/ontologies/2022/0/Planning-Ontology#RequiredCap1 -->


    <owl:NamedIndividual rdf:about="http://www.semanticweb.org/sc3/ontologies/2022/0/Planning-Ontology#RequiredCap1">
        <rdf:type rdf:resource="http://www.semanticweb.org/sc3/ontologies/2022/0/Planning-Ontology#RequiredCapacity"/>
    </owl:NamedIndividual>
    


    <!-- http://www.semanticweb.org/sc3/ontologies/2022/0/Planning-Ontology#RequiredCap2 -->


    <owl:NamedIndividual rdf:about="http://www.semanticweb.org/sc3/ontologies/2022/0/Planning-Ontology#RequiredCap2">
        <rdf:type rdf:resource="http://www.semanticweb.org/sc3/ontologies/2022/0/Planning-Ontology#RequiredCapacity"/>
    </owl:NamedIndividual>
    


    <!-- http://www.semanticweb.org/sc3/ontologies/2022/0/Planning-Ontology#RequiredCap3 -->


    <owl:NamedIndividual rdf:about="http://www.semanticweb.org/sc3/ontologies/2022/0/Planning-Ontology#RequiredCap3">
        <rdf:type rdf:resource="http://www.semanticweb.org/sc3/ontologies/2022/0/Planning-Ontology#RequiredCapacity"/>
    </owl:NamedIndividual>
    


    <!-- http://www.semanticweb.org/sc3/ontologies/2022/0/Planning-Ontology#RequiredCap4 -->


    <owl:NamedIndividual rdf:about="http://www.semanticweb.org/sc3/ontologies/2022/0/Planning-Ontology#RequiredCap4">
        <rdf:type rdf:resource="http://www.semanticweb.org/sc3/ontologies/2022/0/Planning-Ontology#RequiredCapacity"/>
    </owl:NamedIndividual>
    


    <!-- http://www.semanticweb.org/sc3/ontologies/2022/0/Planning-Ontology#SimulationHorizon -->


    <owl:NamedIndividual rdf:about="http://www.semanticweb.org/sc3/ontologies/2022/0/Planning-Ontology#SimulationHorizon">
        <rdf:type rdf:resource="http://www.w3.org/2006/time#Duration"/>
        <time:weeks rdf:datatype="http://www.w3.org/2001/XMLSchema#integer">26</time:weeks>
    </owl:NamedIndividual>
    


    <!-- http://www.semanticweb.org/sc3/ontologies/2022/0/Planning-Ontology#Wip_Balance_Equation -->


    <owl:NamedIndividual rdf:about="http://www.semanticweb.org/sc3/ontologies/2022/0/Planning-Ontology#Wip_Balance_Equation">
        <rdf:type rdf:resource="http://www.semanticweb.org/sc3/ontologies/2022/0/Planning-Ontology#PlanningConstraint"/>
        <sc3:formula>forall($g in Products, $t in PlanningHorizon, $j in Frontends) -&gt; FE_Wip($j, $g, $t) = FE_X($j, $g, $t) - FE_Y($j, $g, $t) + FE_Wip($j, $g, $t-1)

Frontends= Frontend_1, Frontend_2;
Products= Product_1;</sc3:formula>
    </owl:NamedIndividual>
    


    <!-- http://www.w3.org/2006/time#Friday -->


    <rdf:Description rdf:about="http://www.w3.org/2006/time#Friday">
        <rdf:type rdf:resource="http://www.w3.org/2006/time#DayOfWeek"/>
        <rdfs:label xml:lang="en">Friday</rdfs:label>
        <skos:prefLabel xml:lang="de">Freitag</skos:prefLabel>
        <skos:prefLabel xml:lang="en">Friday</skos:prefLabel>
        <skos:prefLabel xml:lang="pl">Piątek</skos:prefLabel>
        <skos:prefLabel xml:lang="pt">Sexta-feira</skos:prefLabel>
        <skos:prefLabel xml:lang="fr">Vendredi</skos:prefLabel>
        <skos:prefLabel xml:lang="it">Venerdì</skos:prefLabel>
        <skos:prefLabel xml:lang="es">Viernes</skos:prefLabel>
        <skos:prefLabel xml:lang="nl">Vrijdag</skos:prefLabel>
        <skos:prefLabel xml:lang="ru">Пятница</skos:prefLabel>
        <skos:prefLabel xml:lang="ar">الجمعة</skos:prefLabel>
        <skos:prefLabel xml:lang="zh">星期五</skos:prefLabel>
        <skos:prefLabel xml:lang="ja">金曜日</skos:prefLabel>
    </rdf:Description>
    


    <!-- http://www.w3.org/2006/time#Monday -->


    <rdf:Description rdf:about="http://www.w3.org/2006/time#Monday">
        <rdf:type rdf:resource="http://www.w3.org/2006/time#DayOfWeek"/>
        <rdfs:label xml:lang="en">Monday</rdfs:label>
        <skos:prefLabel xml:lang="fr">Lundi</skos:prefLabel>
        <skos:prefLabel xml:lang="it">Lunedì</skos:prefLabel>
        <skos:prefLabel xml:lang="es">Lunes</skos:prefLabel>
        <skos:prefLabel xml:lang="nl">Maandag</skos:prefLabel>
        <skos:prefLabel xml:lang="en">Monday</skos:prefLabel>
        <skos:prefLabel xml:lang="de">Montag</skos:prefLabel>
        <skos:prefLabel xml:lang="pl">Poniedziałek</skos:prefLabel>
        <skos:prefLabel xml:lang="pt">Segunda-feira</skos:prefLabel>
        <skos:prefLabel xml:lang="ru">Понедельник</skos:prefLabel>
        <skos:prefLabel xml:lang="ar">الاثنين</skos:prefLabel>
        <skos:prefLabel xml:lang="zh">星期一</skos:prefLabel>
        <skos:prefLabel xml:lang="ja">月曜日</skos:prefLabel>
    </rdf:Description>
    


    <!-- http://www.w3.org/2006/time#Saturday -->


    <rdf:Description rdf:about="http://www.w3.org/2006/time#Saturday">
        <rdf:type rdf:resource="http://www.w3.org/2006/time#DayOfWeek"/>
        <rdfs:label xml:lang="en">Saturday</rdfs:label>
        <skos:prefLabel xml:lang="it">Sabato</skos:prefLabel>
        <skos:prefLabel xml:lang="fr">Samedi</skos:prefLabel>
        <skos:prefLabel xml:lang="de">Samstag</skos:prefLabel>
        <skos:prefLabel xml:lang="en">Saturday</skos:prefLabel>
        <skos:prefLabel xml:lang="pl">Sobota</skos:prefLabel>
        <skos:prefLabel xml:lang="es">Sábado</skos:prefLabel>
        <skos:prefLabel xml:lang="pt">Sábado</skos:prefLabel>
        <skos:prefLabel xml:lang="nl">Zaterdag</skos:prefLabel>
        <skos:prefLabel xml:lang="ru">Суббота</skos:prefLabel>
        <skos:prefLabel xml:lang="ar">السبت</skos:prefLabel>
        <skos:prefLabel xml:lang="ja">土曜日</skos:prefLabel>
        <skos:prefLabel xml:lang="zh">星期六</skos:prefLabel>
    </rdf:Description>
    


    <!-- http://www.w3.org/2006/time#Sunday -->


    <rdf:Description rdf:about="http://www.w3.org/2006/time#Sunday">
        <rdf:type rdf:resource="http://www.w3.org/2006/time#DayOfWeek"/>
        <rdfs:label xml:lang="en">Sunday</rdfs:label>
        <skos:prefLabel xml:lang="fr">Dimanche</skos:prefLabel>
        <skos:prefLabel xml:lang="it">Domenica</skos:prefLabel>
        <skos:prefLabel xml:lang="es">Domingo</skos:prefLabel>
        <skos:prefLabel xml:lang="pt">Domingo</skos:prefLabel>
        <skos:prefLabel xml:lang="pl">Niedziela</skos:prefLabel>
        <skos:prefLabel xml:lang="de">Sonntag</skos:prefLabel>
        <skos:prefLabel xml:lang="en">Sunday</skos:prefLabel>
        <skos:prefLabel xml:lang="nl">Zondag</skos:prefLabel>
        <skos:prefLabel xml:lang="ru">Воскресенье</skos:prefLabel>
        <skos:prefLabel xml:lang="ar">الأحد (يوم)</skos:prefLabel>
        <skos:prefLabel xml:lang="ja">日曜日</skos:prefLabel>
        <skos:prefLabel xml:lang="zh">星期日</skos:prefLabel>
    </rdf:Description>
    


    <!-- http://www.w3.org/2006/time#Thursday -->


    <rdf:Description rdf:about="http://www.w3.org/2006/time#Thursday">
        <rdf:type rdf:resource="http://www.w3.org/2006/time#DayOfWeek"/>
        <rdfs:label xml:lang="en">Thursday</rdfs:label>
        <skos:prefLabel xml:lang="pl">Czwartek</skos:prefLabel>
        <skos:prefLabel xml:lang="nl">Donderdag</skos:prefLabel>
        <skos:prefLabel xml:lang="de">Donnerstag</skos:prefLabel>
        <skos:prefLabel xml:lang="it">Giovedì</skos:prefLabel>
        <skos:prefLabel xml:lang="fr">Jeudi</skos:prefLabel>
        <skos:prefLabel xml:lang="es">Jueves</skos:prefLabel>
        <skos:prefLabel xml:lang="pt">Quinta-feira</skos:prefLabel>
        <skos:prefLabel xml:lang="en">Thursday</skos:prefLabel>
        <skos:prefLabel xml:lang="ru">Четверг</skos:prefLabel>
        <skos:prefLabel xml:lang="ar">الخميس</skos:prefLabel>
        <skos:prefLabel xml:lang="zh">星期四</skos:prefLabel>
        <skos:prefLabel xml:lang="ja">木曜日</skos:prefLabel>
    </rdf:Description>
    


    <!-- http://www.w3.org/2006/time#Tuesday -->


    <rdf:Description rdf:about="http://www.w3.org/2006/time#Tuesday">
        <rdf:type rdf:resource="http://www.w3.org/2006/time#DayOfWeek"/>
        <rdfs:label xml:lang="en">Tuesday</rdfs:label>
        <skos:prefLabel xml:lang="de">Dienstag</skos:prefLabel>
        <skos:prefLabel xml:lang="nl">Dinsdag</skos:prefLabel>
        <skos:prefLabel xml:lang="fr">Mardi</skos:prefLabel>
        <skos:prefLabel xml:lang="it">Martedì</skos:prefLabel>
        <skos:prefLabel xml:lang="es">Martes</skos:prefLabel>
        <skos:prefLabel xml:lang="pt">Terça-feira</skos:prefLabel>
        <skos:prefLabel xml:lang="en">Tuesday</skos:prefLabel>
        <skos:prefLabel xml:lang="pl">Wtorek</skos:prefLabel>
        <skos:prefLabel xml:lang="ru">Вторник</skos:prefLabel>
        <skos:prefLabel xml:lang="ar">الثلاثاء</skos:prefLabel>
        <skos:prefLabel xml:lang="zh">星期二</skos:prefLabel>
        <skos:prefLabel xml:lang="ja">火曜日</skos:prefLabel>
    </rdf:Description>
    


    <!-- http://www.w3.org/2006/time#Wednesday -->


    <rdf:Description rdf:about="http://www.w3.org/2006/time#Wednesday">
        <rdf:type rdf:resource="http://www.w3.org/2006/time#DayOfWeek"/>
        <rdfs:label xml:lang="en">Wednesday</rdfs:label>
        <skos:prefLabel xml:lang="it">Mercoledì</skos:prefLabel>
        <skos:prefLabel xml:lang="fr">Mercredi</skos:prefLabel>
        <skos:prefLabel xml:lang="de">Mittwoch</skos:prefLabel>
        <skos:prefLabel xml:lang="es">Miércoles</skos:prefLabel>
        <skos:prefLabel xml:lang="pt">Quarta-feira</skos:prefLabel>
        <skos:prefLabel xml:lang="en">Wednesday</skos:prefLabel>
        <skos:prefLabel xml:lang="nl">Woensdag</skos:prefLabel>
        <skos:prefLabel xml:lang="pl">Środa</skos:prefLabel>
        <skos:prefLabel xml:lang="ru">Среда</skos:prefLabel>
        <skos:prefLabel xml:lang="ar">الأربعاء</skos:prefLabel>
        <skos:prefLabel xml:lang="zh">星期三</skos:prefLabel>
        <skos:prefLabel xml:lang="ja">水曜日</skos:prefLabel>
    </rdf:Description>
    


    <!-- http://www.w3.org/2006/time#unitDay -->


    <rdf:Description rdf:about="http://www.w3.org/2006/time#unitDay">
        <rdf:type rdf:resource="http://www.w3.org/2006/time#TemporalUnit"/>
        <time:days rdf:datatype="http://www.w3.org/2001/XMLSchema#decimal">1</time:days>
        <time:hours rdf:datatype="http://www.w3.org/2001/XMLSchema#decimal">0</time:hours>
        <time:minutes rdf:datatype="http://www.w3.org/2001/XMLSchema#decimal">0</time:minutes>
        <time:months rdf:datatype="http://www.w3.org/2001/XMLSchema#decimal">0</time:months>
        <time:seconds rdf:datatype="http://www.w3.org/2001/XMLSchema#decimal">0</time:seconds>
        <time:weeks rdf:datatype="http://www.w3.org/2001/XMLSchema#decimal">0</time:weeks>
        <time:years rdf:datatype="http://www.w3.org/2001/XMLSchema#decimal">0</time:years>
        <rdfs:label xml:lang="en">Day (unit of temporal duration)</rdfs:label>
        <skos:prefLabel xml:lang="de">Tag</skos:prefLabel>
        <skos:prefLabel xml:lang="nl">dag</skos:prefLabel>
        <skos:prefLabel xml:lang="en">day</skos:prefLabel>
        <skos:prefLabel xml:lang="pt">dia</skos:prefLabel>
        <skos:prefLabel xml:lang="pl">doba</skos:prefLabel>
        <skos:prefLabel xml:lang="es">día</skos:prefLabel>
        <skos:prefLabel xml:lang="it">giorno</skos:prefLabel>
        <skos:prefLabel xml:lang="fr">jour</skos:prefLabel>
        <skos:prefLabel xml:lang="ar">يوماً ما</skos:prefLabel>
        <skos:prefLabel xml:lang="jp">ある日</skos:prefLabel>
        <skos:prefLabel xml:lang="zh">一天</skos:prefLabel>
        <skos:prefLabel xml:lang="kr">언젠가</skos:prefLabel>
    </rdf:Description>
    


    <!-- http://www.w3.org/2006/time#unitHour -->


    <rdf:Description rdf:about="http://www.w3.org/2006/time#unitHour">
        <rdf:type rdf:resource="http://www.w3.org/2006/time#TemporalUnit"/>
        <time:days rdf:datatype="http://www.w3.org/2001/XMLSchema#decimal">0</time:days>
        <time:hours rdf:datatype="http://www.w3.org/2001/XMLSchema#decimal">1</time:hours>
        <time:minutes rdf:datatype="http://www.w3.org/2001/XMLSchema#decimal">0</time:minutes>
        <time:months rdf:datatype="http://www.w3.org/2001/XMLSchema#decimal">0</time:months>
        <time:seconds rdf:datatype="http://www.w3.org/2001/XMLSchema#decimal">0</time:seconds>
        <time:weeks rdf:datatype="http://www.w3.org/2001/XMLSchema#decimal">0</time:weeks>
        <time:years rdf:datatype="http://www.w3.org/2001/XMLSchema#decimal">0</time:years>
        <rdfs:label xml:lang="en">Hour (unit of temporal duration)</rdfs:label>
        <skos:prefLabel xml:lang="de">Stunde</skos:prefLabel>
        <skos:prefLabel xml:lang="pl">godzina</skos:prefLabel>
        <skos:prefLabel xml:lang="fr">heure</skos:prefLabel>
        <skos:prefLabel xml:lang="es">hora</skos:prefLabel>
        <skos:prefLabel xml:lang="pt">hora</skos:prefLabel>
        <skos:prefLabel xml:lang="en">hour</skos:prefLabel>
        <skos:prefLabel xml:lang="it">ora</skos:prefLabel>
        <skos:prefLabel xml:lang="nl">uur</skos:prefLabel>
        <skos:prefLabel xml:lang="ar">ساعة واحدة</skos:prefLabel>
        <skos:prefLabel xml:lang="zh">一小時</skos:prefLabel>
        <skos:prefLabel xml:lang="jp">一時間</skos:prefLabel>
        <skos:prefLabel xml:lang="kr">한 시간</skos:prefLabel>
        <skos:prefLabel>один час&quot;@ru</skos:prefLabel>
    </rdf:Description>
    


    <!-- http://www.w3.org/2006/time#unitMinute -->


    <rdf:Description rdf:about="http://www.w3.org/2006/time#unitMinute">
        <rdf:type rdf:resource="http://www.w3.org/2006/time#TemporalUnit"/>
        <time:days rdf:datatype="http://www.w3.org/2001/XMLSchema#decimal">0</time:days>
        <time:hours rdf:datatype="http://www.w3.org/2001/XMLSchema#decimal">0</time:hours>
        <time:minutes rdf:datatype="http://www.w3.org/2001/XMLSchema#decimal">1</time:minutes>
        <time:months rdf:datatype="http://www.w3.org/2001/XMLSchema#decimal">0</time:months>
        <time:seconds rdf:datatype="http://www.w3.org/2001/XMLSchema#decimal">0</time:seconds>
        <time:weeks rdf:datatype="http://www.w3.org/2001/XMLSchema#decimal">0</time:weeks>
        <time:years rdf:datatype="http://www.w3.org/2001/XMLSchema#decimal">0</time:years>
        <rdfs:label xml:lang="en">Minute (unit of temporal duration)</rdfs:label>
        <skos:prefLabel xml:lang="de">Minute</skos:prefLabel>
        <skos:prefLabel xml:lang="pl">minuta</skos:prefLabel>
        <skos:prefLabel xml:lang="en">minute</skos:prefLabel>
        <skos:prefLabel xml:lang="fr">minute</skos:prefLabel>
        <skos:prefLabel xml:lang="es">minuto</skos:prefLabel>
        <skos:prefLabel xml:lang="it">minuto</skos:prefLabel>
        <skos:prefLabel xml:lang="pt">minuto</skos:prefLabel>
        <skos:prefLabel xml:lang="nl">minuut</skos:prefLabel>
        <skos:prefLabel xml:lang="ru">одна минута</skos:prefLabel>
        <skos:prefLabel xml:lang="ar">دقيقة واحدة</skos:prefLabel>
        <skos:prefLabel xml:lang="jp">一分</skos:prefLabel>
        <skos:prefLabel xml:lang="zh">等一下</skos:prefLabel>
        <skos:prefLabel xml:lang="kr">분</skos:prefLabel>
    </rdf:Description>
    


    <!-- http://www.w3.org/2006/time#unitMonth -->


    <rdf:Description rdf:about="http://www.w3.org/2006/time#unitMonth">
        <rdf:type rdf:resource="http://www.w3.org/2006/time#TemporalUnit"/>
        <time:days rdf:datatype="http://www.w3.org/2001/XMLSchema#decimal">0</time:days>
        <time:hours rdf:datatype="http://www.w3.org/2001/XMLSchema#decimal">0</time:hours>
        <time:minutes rdf:datatype="http://www.w3.org/2001/XMLSchema#decimal">0</time:minutes>
        <time:months rdf:datatype="http://www.w3.org/2001/XMLSchema#decimal">1</time:months>
        <time:seconds rdf:datatype="http://www.w3.org/2001/XMLSchema#decimal">0</time:seconds>
        <time:weeks rdf:datatype="http://www.w3.org/2001/XMLSchema#decimal">0</time:weeks>
        <time:years rdf:datatype="http://www.w3.org/2001/XMLSchema#decimal">0</time:years>
        <rdfs:label xml:lang="en">Month (unit of temporal duration)</rdfs:label>
        <skos:prefLabel xml:lang="de">Monat</skos:prefLabel>
        <skos:prefLabel xml:lang="nl">maand</skos:prefLabel>
        <skos:prefLabel xml:lang="es">mes</skos:prefLabel>
        <skos:prefLabel xml:lang="it">mese</skos:prefLabel>
        <skos:prefLabel xml:lang="pl">miesiąc</skos:prefLabel>
        <skos:prefLabel xml:lang="fr">mois</skos:prefLabel>
        <skos:prefLabel xml:lang="en">month</skos:prefLabel>
        <skos:prefLabel xml:lang="ru">один месяц</skos:prefLabel>
        <skos:prefLabel xml:lang="ar">شهر واحد</skos:prefLabel>
        <skos:prefLabel xml:lang="jp">一か月</skos:prefLabel>
        <skos:prefLabel xml:lang="zh">一個月</skos:prefLabel>
        <skos:prefLabel xml:lang="kr">한달</skos:prefLabel>
    </rdf:Description>
    


    <!-- http://www.w3.org/2006/time#unitSecond -->


    <rdf:Description rdf:about="http://www.w3.org/2006/time#unitSecond">
        <rdf:type rdf:resource="http://www.w3.org/2006/time#TemporalUnit"/>
        <time:days rdf:datatype="http://www.w3.org/2001/XMLSchema#decimal">0</time:days>
        <time:hours rdf:datatype="http://www.w3.org/2001/XMLSchema#decimal">0</time:hours>
        <time:minutes rdf:datatype="http://www.w3.org/2001/XMLSchema#decimal">0</time:minutes>
        <time:months rdf:datatype="http://www.w3.org/2001/XMLSchema#decimal">0</time:months>
        <time:seconds rdf:datatype="http://www.w3.org/2001/XMLSchema#decimal">1</time:seconds>
        <time:weeks rdf:datatype="http://www.w3.org/2001/XMLSchema#decimal">0</time:weeks>
        <time:years rdf:datatype="http://www.w3.org/2001/XMLSchema#decimal">0</time:years>
        <rdfs:label xml:lang="en">Second (unit of temporal duration)</rdfs:label>
        <skos:prefLabel xml:lang="de">Sekunde</skos:prefLabel>
        <skos:prefLabel xml:lang="pl">Sekundę</skos:prefLabel>
        <skos:prefLabel xml:lang="en">second</skos:prefLabel>
        <skos:prefLabel xml:lang="fr">seconde</skos:prefLabel>
        <skos:prefLabel xml:lang="nl">seconde</skos:prefLabel>
        <skos:prefLabel xml:lang="it">secondo</skos:prefLabel>
        <skos:prefLabel xml:lang="es">segundo</skos:prefLabel>
        <skos:prefLabel xml:lang="pt">segundo</skos:prefLabel>
        <skos:prefLabel xml:lang="ar">ثانية واحدة</skos:prefLabel>
        <skos:prefLabel xml:lang="jp">一秒</skos:prefLabel>
        <skos:prefLabel xml:lang="zh">一秒</skos:prefLabel>
        <skos:prefLabel xml:lang="kr">일초</skos:prefLabel>
    </rdf:Description>
    


    <!-- http://www.w3.org/2006/time#unitWeek -->


    <rdf:Description rdf:about="http://www.w3.org/2006/time#unitWeek">
        <rdf:type rdf:resource="http://www.w3.org/2006/time#TemporalUnit"/>
        <time:days rdf:datatype="http://www.w3.org/2001/XMLSchema#decimal">0</time:days>
        <time:hours rdf:datatype="http://www.w3.org/2001/XMLSchema#decimal">0</time:hours>
        <time:minutes rdf:datatype="http://www.w3.org/2001/XMLSchema#decimal">0</time:minutes>
        <time:months rdf:datatype="http://www.w3.org/2001/XMLSchema#decimal">0</time:months>
        <time:seconds rdf:datatype="http://www.w3.org/2001/XMLSchema#decimal">0</time:seconds>
        <time:weeks rdf:datatype="http://www.w3.org/2001/XMLSchema#decimal">1</time:weeks>
        <time:years rdf:datatype="http://www.w3.org/2001/XMLSchema#decimal">0</time:years>
        <rdfs:label xml:lang="en">Week (unit of temporal duration)</rdfs:label>
        <skos:prefLabel xml:lang="de">Woche</skos:prefLabel>
        <skos:prefLabel xml:lang="fr">semaine</skos:prefLabel>
        <skos:prefLabel xml:lang="es">semana</skos:prefLabel>
        <skos:prefLabel xml:lang="pt">semana</skos:prefLabel>
        <skos:prefLabel xml:lang="it">settimana</skos:prefLabel>
        <skos:prefLabel xml:lang="pl">tydzień</skos:prefLabel>
        <skos:prefLabel xml:lang="en">week</skos:prefLabel>
        <skos:prefLabel xml:lang="nl">week</skos:prefLabel>
        <skos:prefLabel xml:lang="ru">одна неделя</skos:prefLabel>
        <skos:prefLabel xml:lang="ar">سبوع واحد</skos:prefLabel>
        <skos:prefLabel xml:lang="zh">一周</skos:prefLabel>
        <skos:prefLabel xml:lang="jp">一週間</skos:prefLabel>
        <skos:prefLabel xml:lang="kr">일주일</skos:prefLabel>
    </rdf:Description>
    


    <!-- http://www.w3.org/2006/time#unitYear -->


    <rdf:Description rdf:about="http://www.w3.org/2006/time#unitYear">
        <rdf:type rdf:resource="http://www.w3.org/2006/time#TemporalUnit"/>
        <time:days rdf:datatype="http://www.w3.org/2001/XMLSchema#decimal">0</time:days>
        <time:hours rdf:datatype="http://www.w3.org/2001/XMLSchema#decimal">0</time:hours>
        <time:minutes rdf:datatype="http://www.w3.org/2001/XMLSchema#decimal">0</time:minutes>
        <time:months rdf:datatype="http://www.w3.org/2001/XMLSchema#decimal">0</time:months>
        <time:seconds rdf:datatype="http://www.w3.org/2001/XMLSchema#decimal">0</time:seconds>
        <time:weeks rdf:datatype="http://www.w3.org/2001/XMLSchema#decimal">0</time:weeks>
        <time:years rdf:datatype="http://www.w3.org/2001/XMLSchema#decimal">1</time:years>
        <rdfs:label xml:lang="en">Year (unit of temporal duration)</rdfs:label>
        <skos:prefLabel xml:lang="kr">1 년</skos:prefLabel>
        <skos:prefLabel xml:lang="jp">1年</skos:prefLabel>
        <skos:prefLabel xml:lang="de">Jahr</skos:prefLabel>
        <skos:prefLabel xml:lang="fr">an</skos:prefLabel>
        <skos:prefLabel xml:lang="it">anno</skos:prefLabel>
        <skos:prefLabel xml:lang="pt">ano</skos:prefLabel>
        <skos:prefLabel xml:lang="nl">jaar</skos:prefLabel>
        <skos:prefLabel xml:lang="pl">rok</skos:prefLabel>
        <skos:prefLabel xml:lang="es">un año</skos:prefLabel>
        <skos:prefLabel xml:lang="en">year</skos:prefLabel>
        <skos:prefLabel xml:lang="ru">один год</skos:prefLabel>
        <skos:prefLabel xml:lang="ar">سنة واحدة</skos:prefLabel>
        <skos:prefLabel xml:lang="zh">一年</skos:prefLabel>
    </rdf:Description>
    <rdf:Description>
        <xsd:pattern>---(0[1-9]|[1-9][0-9])(Z|(\+|-)((0[0-9]|1[0-3]):[0-5][0-9]|14:00))?</xsd:pattern>
    </rdf:Description>
    <rdf:Description>
        <xsd:pattern>--(0[1-9]|1[0-9]|20)(Z|(\+|-)((0[0-9]|1[0-3]):[0-5][0-9]|14:00))?</xsd:pattern>
    </rdf:Description>
    <rdf:Description>
        <xsd:pattern>-?([1-9][0-9]{3,}|0[0-9]{3})(Z|(\+|-)((0[0-9]|1[0-3]):[0-5][0-9]|14:00))?</xsd:pattern>
    </rdf:Description>
    


    <!-- 
    ///////////////////////////////////////////////////////////////////////////////////////
    //
    // Annotations
    //
    ///////////////////////////////////////////////////////////////////////////////////////
     -->


    <rdf:Description rdf:about="http://www.semanticweb.org/sc3/ontologies/2022/0/Planning-Ontology#hasEarliestReleaseDate">
        <rdfs:comment>This is the earliest time where the activities associated with a PLANNING OBJECT can start. Note that the parameter RELEASE DATE is exogenous, i.e. given, in contrast to the property TIME.</rdfs:comment>
    </rdf:Description>
    


    <!-- 
    ///////////////////////////////////////////////////////////////////////////////////////
    //
    // General axioms
    //
    ///////////////////////////////////////////////////////////////////////////////////////
     -->


    <rdf:Description>
        <rdf:type rdf:resource="http://www.w3.org/2002/07/owl#AllDisjointClasses"/>
        <owl:members rdf:parseType="Collection">
            <rdf:Description rdf:about="http://www.semanticweb.org/sc3/ontologies/2022/0/Planning-Ontology#Resource-Availability-Constraints"/>
            <rdf:Description rdf:about="http://www.semanticweb.org/sc3/ontologies/2022/0/Planning-Ontology#Resource-Compatibility-Constraints"/>
            <rdf:Description rdf:about="http://www.semanticweb.org/sc3/ontologies/2022/0/Planning-Ontology#Temporal-Constraints"/>
        </owl:members>
    </rdf:Description>
</rdf:RDF>



<!-- Generated by the OWL API (version 5.1.18) https://github.com/owlcs/owlapi/ -->


