@prefix : <http://www.semanticweb.org/sc3/ontologies/2022/0/Planning-Ontology#> .
@prefix owl: <http://www.w3.org/2002/07/owl#> .
@prefix rdf: <http://www.w3.org/1999/02/22-rdf-syntax-ns#> .
@prefix xml: <http://www.w3.org/XML/1998/namespace> .
@prefix xsd: <http://www.w3.org/2001/XMLSchema#> .
@prefix rdfs: <http://www.w3.org/2000/01/rdf-schema#> .
@base <http://www.semanticweb.org/sc3/ontologies/2022/0/Planning-Ontology#> .

<http://www.semanticweb.org/sc3/ontologies/2022/0/Planning-Ontology> rdf:type owl:Ontology ;
                                                                      owl:imports <http://www.semanticweb.org/sc3/ontologies/2022/0/ozone-ontology> ,
                                                                                  <http://www.w3.org/2006/time#2016> .

#################################################################
#    Annotation properties
#################################################################

###  http://www.semanticweb.org/sc3/ontologies/2022/0/Planning-Ontology#sc3:formula
:sc3:formula rdf:type owl:AnnotationProperty .


#################################################################
#    Datatypes
#################################################################

###  http://www.w3.org/2001/XMLSchema#dateTimeStamp
xsd:dateTimeStamp rdfs:label "sello de tiempo"@es .


###  http://www.w3.org/2001/XMLSchema#duration
xsd:duration rdf:type rdfs:Datatype .


###  http://www.w3.org/2006/time#generalDay
<http://www.w3.org/2006/time#generalDay> rdf:type rdfs:Datatype ;
                                         rdfs:comment """Day of month - formulated as a text string with a pattern constraint to reproduce the same lexical form as gDay, except that values up to 99 are permitted, in order to support calendars with more than 31 days in a month. 
Note that the value-space is not defined, so a generic OWL2 processor cannot compute ordering relationships of values of this type."""@en ,
                                                      """Día del mes - formulado como una cadena de texto con una restricción patrón para reproducir la misma forma léxica que gDay, excepto que se permiten valores hasta el 99, con el propósito de proporcionar soporte a calendarios con meses con más de 31 días.
            Nótese que el espacio de valores no está definido, por tanto, un procesador genérico de OWL2 no puede computar relaciones de orden de valores de este tipo."""@es ;
                                         rdfs:label "Día generalizado"@es ,
                                                    "Generalized day"@en ;
                                         <http://www.w3.org/2004/02/skos/core#definition> """Day of month - formulated as a text string with a pattern constraint to reproduce the same lexical form as gDay, except that values up to 99 are permitted, in order to support calendars with more than 31 days in a month. 
Note that the value-space is not defined, so a generic OWL2 processor cannot compute ordering relationships of values of this type."""@en ,
                                                                                          """Día del mes - formulado como una cadena de texto con una restricción patrón para reproducir la misma forma léxica que gDay, excepto que se permiten valores hasta el 99, con el propósito de proporcionar soporte a calendarios con meses con más de 31 días.
            Nótese que el espacio de valores no está definido, por tanto, un procesador genérico de OWL2 no puede computar relaciones de orden de valores de este tipo."""@es .


###  http://www.w3.org/2006/time#generalMonth
<http://www.w3.org/2006/time#generalMonth> rdf:type rdfs:Datatype ;
                                           rdfs:comment """Mes del año - formulado como una cadena de texto con una restricción patrón para reproducir la misma forma léxica que gMonth, excepto que se permiten valores hasta el 20, con el propósito de proporcionar soporte a calendarios con años con más de 12 meses.
            Nótese que el espacio de valores no está definido, por tanto, un procesador genérico de OWL2 no puede computar relaciones de orden de valores de este tipo."""@es ,
                                                        """Month of year - formulated as a text string with a pattern constraint to reproduce the same lexical form as gMonth, except that values up to 20 are permitted, in order to support calendars with more than 12 months in the year. 
Note that the value-space is not defined, so a generic OWL2 processor cannot compute ordering relationships of values of this type."""@en ;
                                           rdfs:label "Generalized month"@en ,
                                                      "Mes generalizado"@es ;
                                           <http://www.w3.org/2004/02/skos/core#definition> """Mes del año - formulado como una cadena de texto con una restricción patrón para reproducir la misma forma léxica que gMonth, excepto que se permiten valores hasta el 20, con el propósito de proporcionar soporte a calendarios con años con más de 12 meses.
            Nótese que el espacio de valores no está definido, por tanto, un procesador genérico de OWL2 no puede computar relaciones de orden de valores de este tipo."""@es ,
                                                                                            """Month of year - formulated as a text string with a pattern constraint to reproduce the same lexical form as gMonth, except that values up to 20 are permitted, in order to support calendars with more than 12 months in the year. 
Note that the value-space is not defined, so a generic OWL2 processor cannot compute ordering relationships of values of this type."""@en .


###  http://www.w3.org/2006/time#generalYear
<http://www.w3.org/2006/time#generalYear> rdf:type rdfs:Datatype ;
                                          rdfs:comment """Número de año - formulado como una cadena de texto con una restricción patrón para reproducir la misma forma léxica que gYear, aunque no está restringido a valores del calendario gregoriano.
            Nótese que el espacio de valores no está definido, por tanto, un procesador genérico de OWL2 no puede computar relaciones de orden de valores de este tipo."""@es ,
                                                       """Year number - formulated as a text string with a pattern constraint to reproduce the same lexical form as gYear, but not restricted to values from the Gregorian calendar. 
Note that the value-space is not defined, so a generic OWL2 processor cannot compute ordering relationships of values of this type."""@en ;
                                          rdfs:label "Año generalizado"@es ,
                                                     "Generalized year"@en ;
                                          <http://www.w3.org/2004/02/skos/core#definition> """Número de año - formulado como una cadena de texto con una restricción patrón para reproducir la misma forma léxica que gYear, aunque no está restringido a valores del calendario gregoriano.
            Nótese que el espacio de valores no está definido, por tanto, un procesador genérico de OWL2 no puede computar relaciones de orden de valores de este tipo."""@es ,
                                                                                           """Year number - formulated as a text string with a pattern constraint to reproduce the same lexical form as gYear, but not restricted to values from the Gregorian calendar. 
Note that the value-space is not defined, so a generic OWL2 processor cannot compute ordering relationships of values of this type."""@en .


#################################################################
#    Object Properties
#################################################################

###  http://www.semanticweb.org/sc3/ontologies/2022/0/Planning-Ontology#hasActivities
:hasActivities rdf:type owl:ObjectProperty ;
               rdfs:subPropertyOf owl:topObjectProperty ;
               rdfs:domain :PlanningObject ,
                           :RequiredCapacity ,
                           <http://www.semanticweb.org/sc3/ontologies/2022/0/ozone-ontology#Product> ;
               rdfs:range :Activity ;
               rdfs:comment """This property describes the set of activities that must be carried out to produce the goods that are associated with the PLANNING OBJECT.

Moreover, there are additional parameters for most types of PLANNING OBJECTS.""" .


###  http://www.semanticweb.org/sc3/ontologies/2022/0/Planning-Ontology#hasBillOfMaterial
:hasBillOfMaterial rdf:type owl:ObjectProperty ;
                   rdfs:domain :Part ,
                               <http://www.semanticweb.org/sc3/ontologies/2022/0/ozone-ontology#Product> ;
                   rdfs:range :BillOfMaterial ;
                   rdfs:comment "A set of potentially alternative BOMs can be used to meet the demand of a certain product" .


###  http://www.semanticweb.org/sc3/ontologies/2022/0/Planning-Ontology#hasBin
:hasBin rdf:type owl:ObjectProperty ;
        rdfs:domain :Binning ;
        rdfs:range :Bin .


###  http://www.semanticweb.org/sc3/ontologies/2022/0/Planning-Ontology#hasCapacity
:hasCapacity rdf:type owl:ObjectProperty ;
             rdfs:domain :Process ,
                         <http://www.semanticweb.org/sc3/ontologies/2022/0/ozone-ontology#Resource> ;
             rdfs:range :AvailableCapacity .


###  http://www.semanticweb.org/sc3/ontologies/2022/0/Planning-Ontology#hasChildProductAggregate
:hasChildProductAggregate rdf:type owl:ObjectProperty ;
                          rdfs:domain :ProductHierarchy ;
                          rdfs:range :ProductHierarchy .


###  http://www.semanticweb.org/sc3/ontologies/2022/0/Planning-Ontology#hasComponentLocation
:hasComponentLocation rdf:type owl:ObjectProperty ;
                      rdfs:domain :BillOfMaterial ;
                      rdfs:range :Location .


###  http://www.semanticweb.org/sc3/ontologies/2022/0/Planning-Ontology#hasComponentPart
:hasComponentPart rdf:type owl:ObjectProperty ;
                  rdfs:subPropertyOf owl:topObjectProperty ;
                  rdfs:domain :BillOfMaterial ,
                              :Process ;
                  rdfs:range :ComponentPart .


###  http://www.semanticweb.org/sc3/ontologies/2022/0/Planning-Ontology#hasComponentProcess
:hasComponentProcess rdf:type owl:ObjectProperty ;
                     rdfs:domain :BillOfMaterial ;
                     rdfs:range :Process .


###  http://www.semanticweb.org/sc3/ontologies/2022/0/Planning-Ontology#hasConnection
:hasConnection rdf:type owl:ObjectProperty ;
               rdfs:subPropertyOf owl:topObjectProperty ;
               rdfs:domain :DecisionMakingUnit ,
                           :PlanningProcess ;
               rdfs:range :Edge ;
               rdfs:comment "If a vertex provides instruction or a reaction to another vertex than the two vertices are connected by a directed edge." .


###  http://www.semanticweb.org/sc3/ontologies/2022/0/Planning-Ontology#hasConstraint
:hasConstraint rdf:type owl:ObjectProperty .


###  http://www.semanticweb.org/sc3/ontologies/2022/0/Planning-Ontology#hasCriterias
:hasCriterias rdf:type owl:ObjectProperty ;
              rdfs:domain :PlaningPurpose ;
              rdfs:range :Criteria ;
              rdfs:comment "A criterion is assigned to each performance measure that belongs to a PLANNING PURPOSE. Typical criteria are maximization, minimization, i.e. if an optimization problem is considered, or larger or smaller than a prescribed value of the certain performance measure, a so-called target, i.e. if a satisfaction problem is solved. In a multi-criteria setting, the dominance concept for plans is of interest." .


###  http://www.semanticweb.org/sc3/ontologies/2022/0/Planning-Ontology#hasDMUa
:hasDMUa rdf:type owl:ObjectProperty ;
         rdfs:subPropertyOf owl:topObjectProperty ;
         rdfs:domain :Vertex ;
         rdfs:range :DecisionMakingUnit ;
         rdfs:comment "First DMU of the Vertex" .


###  http://www.semanticweb.org/sc3/ontologies/2022/0/Planning-Ontology#hasDMUb
:hasDMUb rdf:type owl:ObjectProperty ;
         rdfs:subPropertyOf owl:topObjectProperty ;
         rdfs:domain :Edge ;
         rdfs:range :DecisionMakingUnit ;
         rdfs:comment "Second DMU of the Vertex" .


###  http://www.semanticweb.org/sc3/ontologies/2022/0/Planning-Ontology#hasDecisionMakerType
:hasDecisionMakerType rdf:type owl:ObjectProperty ;
                      rdfs:subPropertyOf owl:topObjectProperty ;
                      rdfs:domain :DecisionMakingUnit ;
                      rdfs:range :DecisionMakerType ;
                      rdfs:comment "Specifies the concrete type of a DMU" .


###  http://www.semanticweb.org/sc3/ontologies/2022/0/Planning-Ontology#hasDecisionMakingInitiative
:hasDecisionMakingInitiative rdf:type owl:ObjectProperty ;
                             rdfs:subPropertyOf owl:topObjectProperty ;
                             rdfs:domain :DecisionMakingUnit ;
                             rdfs:range :DecisionMakingInitiative ;
                             rdfs:comment "We distinguish fully autonomous DECISION-MAKING UNITS from DECISION-MAKING UNITS where the decision-making activities are triggered by other DECISION-MAKING UNITS. Note that the decision-making initiative can change over time in a situation-dependent manner." .


###  http://www.semanticweb.org/sc3/ontologies/2022/0/Planning-Ontology#hasDecisionMakingUnit
:hasDecisionMakingUnit rdf:type owl:ObjectProperty ;
                       rdfs:subPropertyOf owl:topObjectProperty ;
                       rdfs:domain :PlanningSituation ,
                                   :Vertex ;
                       rdfs:range :DecisionMakingUnit ;
                       rdfs:comment "This property describes the set of DECISION-MAKING UNITS that constitutes the planning situation. We refer to the elements of the set as vertices." .


###  http://www.semanticweb.org/sc3/ontologies/2022/0/Planning-Ontology#hasDecisionMakingUnitCharcters
:hasDecisionMakingUnitCharcters rdf:type owl:ObjectProperty ;
                                rdfs:subPropertyOf owl:topObjectProperty ;
                                rdfs:domain :PlanningSituation ;
                                rdfs:range :DecisonMakingUnitCharacter .


###  http://www.semanticweb.org/sc3/ontologies/2022/0/Planning-Ontology#hasDefined
:hasDefined rdf:type owl:ObjectProperty ;
            rdfs:subPropertyOf owl:topObjectProperty ;
            rdfs:domain :PlanExecutuon ;
            rdfs:range :PerformanceMeasure ;
            rdfs:comment "Values for certain PERFORMANCE MEASURES can be computed after a plan is executed. This always requires that the consequences of a PLAN are assessed in the base system." .


###  http://www.semanticweb.org/sc3/ontologies/2022/0/Planning-Ontology#hasEarliestReleaseDate
:hasEarliestReleaseDate rdf:type owl:ObjectProperty ;
                        rdfs:subPropertyOf owl:topObjectProperty ;
                        rdfs:domain :PlanningObject ;
                        rdfs:range <http://www.w3.org/2006/time#TemporalDuration> .


###  http://www.semanticweb.org/sc3/ontologies/2022/0/Planning-Ontology#hasEventTrigger
:hasEventTrigger rdf:type owl:ObjectProperty ;
                 rdfs:subPropertyOf owl:topObjectProperty ;
                 rdfs:domain :PlanningProcess ;
                 rdfs:range :Trigger ;
                 rdfs:comment "This property determines which events result in replanning (Vieria et al. 2003). For instance, replanning can be the result of the breakdown of a bottleneck resource." .


###  http://www.semanticweb.org/sc3/ontologies/2022/0/Planning-Ontology#hasFrozenFence
:hasFrozenFence rdf:type owl:ObjectProperty ;
                rdfs:subPropertyOf owl:topObjectProperty ;
                rdfs:domain :PlanningProcess ;
                rdfs:range :PlanningDecision ;
                rdfs:comment "This property specifies which planning decisions are remain unchanged in the case of replanning activities." .


###  http://www.semanticweb.org/sc3/ontologies/2022/0/Planning-Ontology#hasHierarchicalSituation
:hasHierarchicalSituation rdf:type owl:ObjectProperty ;
                          rdfs:subPropertyOf owl:topObjectProperty ;
                          rdfs:domain :PlanningSituation ;
                          rdfs:range :HierarchicalSituation .


###  http://www.semanticweb.org/sc3/ontologies/2022/0/Planning-Ontology#hasInvolvedPlanningObjects
:hasInvolvedPlanningObjects rdf:type owl:ObjectProperty ;
                            rdfs:subPropertyOf owl:topObjectProperty ;
                            rdfs:domain :PlanningInstance ;
                            rdfs:range :PlanningObject ;
                            rdfs:comment "This property specifies the involved PLANNING OBJECTS." .


###  http://www.semanticweb.org/sc3/ontologies/2022/0/Planning-Ontology#hasLocation
:hasLocation rdf:type owl:ObjectProperty ;
             rdfs:subPropertyOf owl:topObjectProperty ;
             rdfs:domain :BillOfMaterial ,
                         :Binning ,
                         :Capacity ,
                         :FrozenFence ,
                         :Inventory ,
                         :InventoryPolicy ,
                         :LotSizingRule ,
                         :PlanningObject ,
                         :Process ,
                         :ProjectedWip ,
                         :Substitution ,
                         :SupplyInformation ,
                         :Yield ,
                         <http://www.semanticweb.org/sc3/ontologies/2022/0/ozone-ontology#Product> ;
             rdfs:range :Location ;
             rdfs:comment "This property describes the place or places, for instance nodes of the semiconductor supply chain or specific machines of a work center where the ACTIVITIES associated with the PLANNING OBJECT have to be executed." .


###  http://www.semanticweb.org/sc3/ontologies/2022/0/Planning-Ontology#hasObjectives
:hasObjectives rdf:type owl:ObjectProperty ;
               rdfs:domain :PlanningProcess ;
               rdfs:range :PlaningPurpose ;
               rdfs:comment """: The property specifies the objectives of a certain planning activity.
Moreover, there are additional parameters for most types of PLANNING PROCESS.""" .


###  http://www.semanticweb.org/sc3/ontologies/2022/0/Planning-Ontology#hasOperations
:hasOperations rdf:type owl:ObjectProperty ;
               rdfs:domain :Route ;
               rdfs:range :MacroOperation .


###  http://www.semanticweb.org/sc3/ontologies/2022/0/Planning-Ontology#hasOrder
:hasOrder rdf:type owl:ObjectProperty ;
          rdfs:domain :In-TransitInventory ;
          rdfs:range :Order .


###  http://www.semanticweb.org/sc3/ontologies/2022/0/Planning-Ontology#hasOwner
:hasOwner rdf:type owl:ObjectProperty ;
          rdfs:subPropertyOf owl:topObjectProperty ;
          rdfs:domain :PlanningObject ;
          rdfs:range :Owner ;
          rdfs:comment "A PLANNING OBJECT is rarely considered in isolation. Usually it belongs to a set of PLANNING OBJECTS, for example, a planning instance." .


###  http://www.semanticweb.org/sc3/ontologies/2022/0/Planning-Ontology#hasParentProductAggregate
:hasParentProductAggregate rdf:type owl:ObjectProperty ;
                           rdfs:domain :ProductHierarchy ;
                           rdfs:range :ProductHierarchy .


###  http://www.semanticweb.org/sc3/ontologies/2022/0/Planning-Ontology#hasPart
:hasPart rdf:type owl:ObjectProperty ;
         rdfs:domain :Bin ,
                     :Binning ,
                     :ProjectedWip ,
                     :Yield ;
         rdfs:range :Part .


###  http://www.semanticweb.org/sc3/ontologies/2022/0/Planning-Ontology#hasPerformanceMeasures
:hasPerformanceMeasures rdf:type owl:ObjectProperty ;
                        rdfs:subPropertyOf owl:topObjectProperty ;
                        rdfs:domain :PlaningPurpose ;
                        rdfs:range :PerformanceMeasure ;
                        rdfs:comment "Each PLANNING PURPOSE is determined by a set of performance measures. Each measure is defined by a calculation procedure. Performance measures can be blended using weights to express the importance of the different measures." .


###  http://www.semanticweb.org/sc3/ontologies/2022/0/Planning-Ontology#hasPeriodicTrigger
:hasPeriodicTrigger rdf:type owl:ObjectProperty ;
                    rdfs:subPropertyOf owl:topObjectProperty ;
                    rdfs:domain :PlanningProcess ;
                    rdfs:range :Trigger ;
                    rdfs:comment "This property defines after which amount of time a replanning activity is initiated in a periodic manner (Vieria et al. 2003). Rolling horizon approaches are triggered by such a periodic approach." .


###  http://www.semanticweb.org/sc3/ontologies/2022/0/Planning-Ontology#hasPlan
:hasPlan rdf:type owl:ObjectProperty ;
         rdfs:subPropertyOf owl:topObjectProperty ;
         rdfs:domain :PlanningProcess ;
         rdfs:range :Plan ;
         rdfs:comment "Activities associated with a PLANNING PROCESS require an instance of the concept PLAN." .


###  http://www.semanticweb.org/sc3/ontologies/2022/0/Planning-Ontology#hasPlanningConstraints
:hasPlanningConstraints rdf:type owl:ObjectProperty ;
                        rdfs:subPropertyOf owl:topObjectProperty ;
                        rdfs:domain :PlanningInstance ;
                        rdfs:range :PlanningConstraint ;
                        rdfs:comment "This property specifies which constraints must be ensured." .


###  http://www.semanticweb.org/sc3/ontologies/2022/0/Planning-Ontology#hasPlanningInstance
:hasPlanningInstance rdf:type owl:ObjectProperty ;
                     rdfs:subPropertyOf owl:topObjectProperty ;
                     rdfs:domain :PlanningProcess ;
                     rdfs:range :PlanningInstance ;
                     rdfs:comment "Activities associated with PLANNING PROCESS require an instance of the concept PLANNING INSTANCE." .


###  http://www.semanticweb.org/sc3/ontologies/2022/0/Planning-Ontology#hasPlanningObject
:hasPlanningObject rdf:type owl:ObjectProperty ;
                   rdfs:domain :FrozenFence ;
                   rdfs:range :PlanningObject .


###  http://www.semanticweb.org/sc3/ontologies/2022/0/Planning-Ontology#hasPlanningObjects
:hasPlanningObjects rdf:type owl:ObjectProperty ;
                    rdfs:subPropertyOf owl:topObjectProperty ;
                    rdfs:domain :Part ,
                                :PlaningPurpose ;
                    rdfs:range :PlanningObject ;
                    rdfs:comment "A set of planning objects is required to determine the performance measure values belonging to the PLANNING PURPOSE. The set of planning objects is often determined by the planning window." .


###  http://www.semanticweb.org/sc3/ontologies/2022/0/Planning-Ontology#hasPlanningProcess
:hasPlanningProcess rdf:type owl:ObjectProperty ;
                    rdfs:subPropertyOf owl:topObjectProperty ;
                    rdfs:domain :DecisionMakingUnit ;
                    rdfs:range :PlanningProcess ;
                    rdfs:comment "This property specifies under which circumstances which (re)planning activities are performed by a DECISION-MAKING UNIT." .


###  http://www.semanticweb.org/sc3/ontologies/2022/0/Planning-Ontology#hasPlanningPurpose
:hasPlanningPurpose rdf:type owl:ObjectProperty ;
                    rdfs:domain :PlanningProcess ;
                    rdfs:range :PlaningPurpose .


###  http://www.semanticweb.org/sc3/ontologies/2022/0/Planning-Ontology#hasPredecessor
:hasPredecessor rdf:type owl:ObjectProperty ;
                rdfs:domain :Location ;
                rdfs:range :Location .


###  http://www.semanticweb.org/sc3/ontologies/2022/0/Planning-Ontology#hasProcess
:hasProcess rdf:type owl:ObjectProperty ;
            rdfs:domain :BillOfMaterial ,
                        :Binning ,
                        :RequiredCapacity ,
                        :Yield ;
            rdfs:range :Process .


###  http://www.semanticweb.org/sc3/ontologies/2022/0/Planning-Ontology#hasProduct
:hasProduct rdf:type owl:ObjectProperty ;
            rdfs:domain :BillOfMaterial ,
                        :Binning ,
                        :Capacity ,
                        :In-TransitInventory ,
                        :Inventory ,
                        :InventoryPolicy ,
                        :LotSizingRule ,
                        :Part ,
                        :PlanningObject ,
                        :Process ,
                        :ProductAggregate ,
                        :ProjectedWip ,
                        :Substitution ,
                        :SupplyInformation ,
                        <http://www.semanticweb.org/sc3/ontologies/2022/0/ozone-ontology#Demand> ;
            rdfs:range <http://www.semanticweb.org/sc3/ontologies/2022/0/ozone-ontology#Product> .


###  http://www.semanticweb.org/sc3/ontologies/2022/0/Planning-Ontology#hasReceivingLocation
:hasReceivingLocation rdf:type owl:ObjectProperty ;
                      rdfs:domain :In-TransitInventory ;
                      rdfs:range :Location .


###  http://www.semanticweb.org/sc3/ontologies/2022/0/Planning-Ontology#hasReplanningDegree
:hasReplanningDegree rdf:type owl:ObjectProperty ;
                     rdfs:subPropertyOf owl:topObjectProperty ;
                     rdfs:domain :PlanningProcess ;
                     rdfs:range :ReplanningDegree ;
                     rdfs:comment "he degree distinguishes replanning from scratch and repair of existing plans (Vieria et al. 2003)." .


###  http://www.semanticweb.org/sc3/ontologies/2022/0/Planning-Ontology#hasResources
:hasResources rdf:type owl:ObjectProperty ;
              rdfs:subPropertyOf owl:topObjectProperty ;
              rdfs:domain :Capacity ,
                          <http://www.semanticweb.org/sc3/ontologies/2022/0/ozone-ontology#Product> ;
              rdfs:range <http://www.semanticweb.org/sc3/ontologies/2022/0/ozone-ontology#Resource> ;
              rdfs:comment "the  set  of  resources  that  can be  utilized  to  execute  various  ACTIVITIES  of  the PRODUCT  plan." .


###  http://www.semanticweb.org/sc3/ontologies/2022/0/Planning-Ontology#hasScope
:hasScope rdf:type owl:ObjectProperty ;
          rdfs:subPropertyOf owl:topObjectProperty ;
          rdfs:domain :DecisionMakingUnit ;
          rdfs:range :PlanningFunction ;
          rdfs:comment "This property defines which planning function is addressed by the DECISION-MAKING UNIT (planning scope). It also described to which part of the base system the DECISION-MAKING UNIT belongs (physical scope)." .


###  http://www.semanticweb.org/sc3/ontologies/2022/0/Planning-Ontology#hasSetOfPlanningObjects
:hasSetOfPlanningObjects rdf:type owl:ObjectProperty ;
                         rdfs:subPropertyOf owl:topObjectProperty ;
                         rdfs:domain :Plan ;
                         rdfs:range :PlanningObject ;
                         rdfs:comment "This property specifies a set of planning objects from a given planning instance where all attributes are supplied with values that are determined as the result of a planning decisions." .


###  http://www.semanticweb.org/sc3/ontologies/2022/0/Planning-Ontology#hasSubProcesses
:hasSubProcesses rdf:type owl:ObjectProperty ;
                 rdfs:domain :Process ;
                 rdfs:range :Process .


###  http://www.semanticweb.org/sc3/ontologies/2022/0/Planning-Ontology#hasSubstitutes
:hasSubstitutes rdf:type owl:ObjectProperty ;
                rdfs:domain :Substitution ;
                rdfs:range <http://www.semanticweb.org/sc3/ontologies/2022/0/ozone-ontology#Product> .


###  http://www.semanticweb.org/sc3/ontologies/2022/0/Planning-Ontology#hasSuccessor
:hasSuccessor rdf:type owl:ObjectProperty ;
              rdfs:domain :Location ;
              rdfs:range :Location .


###  http://www.semanticweb.org/sc3/ontologies/2022/0/Planning-Ontology#hasSupplyingLocation
:hasSupplyingLocation rdf:type owl:ObjectProperty ;
                      rdfs:domain :In-TransitInventory ;
                      rdfs:range :Location .


###  http://www.semanticweb.org/sc3/ontologies/2022/0/Planning-Ontology#hasTargets
:hasTargets rdf:type owl:ObjectProperty ;
            rdfs:subPropertyOf owl:topObjectProperty ;
            rdfs:domain :PlaningPurpose ;
            rdfs:range :Target .


###  http://www.semanticweb.org/sc3/ontologies/2022/0/Planning-Ontology#hasTrigger
:hasTrigger rdf:type owl:ObjectProperty ;
            rdfs:domain :PlanningProcess ;
            rdfs:range :Trigger .


###  http://www.semanticweb.org/sc3/ontologies/2022/0/Planning-Ontology#hasVertex
:hasVertex rdf:type owl:ObjectProperty ;
           rdfs:domain :PlanningSituation ;
           rdfs:range :Vertex .


###  http://www.semanticweb.org/sc3/ontologies/2022/0/Planning-Ontology#hasYield
:hasYield rdf:type owl:ObjectProperty ;
          rdfs:domain :Process ;
          rdfs:range :Yield .


###  http://www.semanticweb.org/sc3/ontologies/2022/0/Planning-Ontology#usesPlanningApproach
:usesPlanningApproach rdf:type owl:ObjectProperty ;
                      rdfs:subPropertyOf owl:topObjectProperty ;
                      rdfs:domain :PlanningProcess ;
                      rdfs:range :PlanningApproach ;
                      rdfs:comment "This property defines which algorithm is used to make the required decisions." .


###  http://www.w3.org/2002/07/owl#topObjectProperty
owl:topObjectProperty rdfs:range <http://www.w3.org/2006/time#TemporalEntity> .


###  http://www.w3.org/2006/time#after
<http://www.w3.org/2006/time#after> rdf:type owl:ObjectProperty ;
                                    rdfs:domain <http://www.w3.org/2006/time#TemporalEntity> ;
                                    rdfs:range <http://www.w3.org/2006/time#TemporalEntity> ;
                                    rdfs:comment "Asume una dirección en el tiempo. Si una entidad temporal T1 está después de otra entidad temporal T2, entonces el principio de T1 está después del final de T2."@es ,
                                                 "Gives directionality to time. If a temporal entity T1 is after another temporal entity T2, then the beginning of T1 is after the end of T2."@en ;
                                    rdfs:label "after"@en ,
                                               "después"@es ;
                                    <http://www.w3.org/2004/02/skos/core#definition> "Asume una dirección en el tiempo. Si una entidad temporal T1 está después de otra entidad temporal T2, entonces el principio de T1 está después del final de T2."@es ,
                                                                                     "Gives directionality to time. If a temporal entity T1 is after another temporal entity T2, then the beginning of T1 is after the end of T2."@en .


###  http://www.w3.org/2006/time#before
<http://www.w3.org/2006/time#before> rdf:type owl:ObjectProperty ;
                                     owl:inverseOf <http://www.w3.org/2006/time#after> ;
                                     rdf:type owl:TransitiveProperty ;
                                     rdfs:domain <http://www.w3.org/2006/time#TemporalEntity> ;
                                     rdfs:range <http://www.w3.org/2006/time#TemporalEntity> ;
                                     rdfs:comment "Asume una dirección en el tiempo. Si una entidad temporal T1 está antes que otra entidad temporal T2, entonces el final de T1 está antes que el principio de T2. Así, \"antes\" se puede considerar básica para instantes y derivada para intervalos."@es ,
                                                  "Gives directionality to time. If a temporal entity T1 is before another temporal entity T2, then the end of T1 is before the beginning of T2. Thus, \"before\" can be considered to be basic to instants and derived for intervals."@en ;
                                     rdfs:label "antes"@es ,
                                                "before"@en ;
                                     <http://www.w3.org/2004/02/skos/core#definition> "Asume una dirección en el tiempo. Si una entidad temporal T1 está antes que otra entidad temporal T2, entonces el final de T1 está antes que el principio de T2. Así, \"antes\" se puede considerar básica para instantes y derivada para intervalos."@es ,
                                                                                      "Gives directionality to time. If a temporal entity T1 is before another temporal entity T2, then the end of T1 is before the beginning of T2. Thus, \"before\" can be considered to be basic to instants and derived for intervals."@en .


###  http://www.w3.org/2006/time#dayOfWeek
<http://www.w3.org/2006/time#dayOfWeek> rdf:type owl:ObjectProperty ;
                                        rdfs:domain <http://www.w3.org/2006/time#GeneralDateTimeDescription> ;
                                        rdfs:range <http://www.w3.org/2006/time#DayOfWeek> ;
                                        rdfs:comment "The day of week, whose value is a member of the class time:DayOfWeek"@en ,
                                                     "El día de la semana, cuyo valor es un miembro de la clase 'día de la semana'." ;
                                        rdfs:label "day of week"@en ,
                                                   "día de la semana"@es ;
                                        <http://www.w3.org/2004/02/skos/core#definition> "El día de la semana, cuyo valor es un miembro de la clase 'día de la semana'."@es ,
                                                                                         "The day of week, whose value is a member of the class time:DayOfWeek"@en .


###  http://www.w3.org/2006/time#hasBeginning
<http://www.w3.org/2006/time#hasBeginning> rdf:type owl:ObjectProperty ;
                                           rdfs:subPropertyOf <http://www.w3.org/2006/time#hasTime> ;
                                           rdfs:domain <http://www.w3.org/2006/time#TemporalEntity> ;
                                           rdfs:range <http://www.w3.org/2006/time#Instant> ;
                                           rdfs:comment "Beginning of a temporal entity"@en ,
                                                        "Comienzo de una entidad temporal."@es ;
                                           rdfs:label "has beginning"@en ,
                                                      "tiene principio"@es ;
                                           <http://www.w3.org/2004/02/skos/core#definition> "Beginning of a temporal entity."@en ,
                                                                                            "Comienzo de una entidad temporal."@es .


###  http://www.w3.org/2006/time#hasDateTimeDescription
<http://www.w3.org/2006/time#hasDateTimeDescription> rdf:type owl:ObjectProperty ;
                                                     rdfs:domain <http://www.w3.org/2006/time#DateTimeInterval> ;
                                                     rdfs:range <http://www.w3.org/2006/time#GeneralDateTimeDescription> ;
                                                     rdfs:comment "Valor de intervalo de fecha-hora expresado como un valor estructurado. El principio y el final del intervalo coincide con los límites del elemento más corto en la descripción."@es ,
                                                                  "Value of DateTimeInterval expressed as a structured value. The beginning and end of the interval coincide with the limits of the shortest element in the description."@en ;
                                                     rdfs:label "has Date-Time description"@en ,
                                                                "tiene descripción fecha-hora"@es ;
                                                     <http://www.w3.org/2004/02/skos/core#definition> "Valor de intervalo de fecha-hora expresado como un valor estructurado. El principio y el final del intervalo coincide con los límites del elemento más corto en la descripción."@es ,
                                                                                                      "Value of DateTimeInterval expressed as a structured value. The beginning and end of the interval coincide with the limits of the shortest element in the description."@en .


###  http://www.w3.org/2006/time#hasDuration
<http://www.w3.org/2006/time#hasDuration> rdf:type owl:ObjectProperty ;
                                          rdfs:subPropertyOf <http://www.w3.org/2006/time#hasTemporalDuration> ;
                                          rdfs:range <http://www.w3.org/2006/time#Duration> ;
                                          rdfs:comment "Duración de una entidad temporal, expresada como un valor escalado o un valor nominal."@es ,
                                                       "Duration of a temporal entity, expressed as a scaled value or nominal value"@en ;
                                          rdfs:label "has duration"@en ,
                                                     "tiene duración"@es ;
                                          <http://www.w3.org/2004/02/skos/core#definition> "Duración de una entidad temporal, evento o actividad, o cosa, expresada como un valor escalado."@es ,
                                                                                           "Duration of a temporal entity, event or activity, or thing, expressed as a scaled value"@en .


###  http://www.w3.org/2006/time#hasDurationDescription
<http://www.w3.org/2006/time#hasDurationDescription> rdf:type owl:ObjectProperty ;
                                                     rdfs:subPropertyOf <http://www.w3.org/2006/time#hasTemporalDuration> ;
                                                     rdfs:range <http://www.w3.org/2006/time#GeneralDurationDescription> ;
                                                     rdfs:comment "Duración de una entidad temporal, expresada utilizando una descripción estructurada."@es ,
                                                                  "Duration of a temporal entity, expressed using a structured description"@en ;
                                                     rdfs:label "has duration description"@en ,
                                                                "tiene descripción de duración"@es ;
                                                     <http://www.w3.org/2004/02/skos/core#definition> "Duración de una entidad temporal, expresada utilizando una descripción estructurada."@es ,
                                                                                                      "Duration of a temporal entity, expressed using a structured description"@en .


###  http://www.w3.org/2006/time#hasEnd
<http://www.w3.org/2006/time#hasEnd> rdf:type owl:ObjectProperty ;
                                     rdfs:subPropertyOf <http://www.w3.org/2006/time#hasTime> ;
                                     rdfs:domain <http://www.w3.org/2006/time#TemporalEntity> ;
                                     rdfs:range <http://www.w3.org/2006/time#Instant> ;
                                     rdfs:comment "End of a temporal entity."@en ,
                                                  "Final de una entidad temporal."@es ;
                                     rdfs:label "has end"@en ,
                                                "tiene fin"@es ;
                                     <http://www.w3.org/2004/02/skos/core#definition> "End of a temporal entity."@en ,
                                                                                      "Final de una entidad temporal."@es .


###  http://www.w3.org/2006/time#hasTRS
<http://www.w3.org/2006/time#hasTRS> rdf:type owl:ObjectProperty ,
                                              owl:FunctionalProperty ;
                                     rdfs:domain [ rdf:type owl:Class ;
                                                   owl:unionOf ( <http://www.w3.org/2006/time#GeneralDurationDescription>
                                                                 <http://www.w3.org/2006/time#TemporalPosition>
                                                               )
                                                 ] ;
                                     rdfs:range <http://www.w3.org/2006/time#TRS> ;
                                     rdfs:comment "El sistema de referencia temporal utilizado por una posición temporal o descripción de extensión."@es ,
                                                  "The temporal reference system used by a temporal position or extent description. "@en ;
                                     rdfs:label "Temporal reference system used"@en ,
                                                "sistema de referencia temporal utilizado"@es ;
                                     <http://www.w3.org/2004/02/skos/core#definition> "El sistema de referencia temporal utilizado por una posición temporal o descripción de extensión."@es ,
                                                                                      "The temporal reference system used by a temporal position or extent description. "@en .


###  http://www.w3.org/2006/time#hasTemporalDuration
<http://www.w3.org/2006/time#hasTemporalDuration> rdf:type owl:ObjectProperty ;
                                                  rdfs:domain <http://www.w3.org/2006/time#TemporalEntity> ;
                                                  rdfs:range <http://www.w3.org/2006/time#TemporalDuration> ;
                                                  rdfs:comment "Duración de una entidad temporal."@es ,
                                                               "Duration of a temporal entity."@en ;
                                                  rdfs:label "has temporal duration"@en ,
                                                             "tiene duración temporal"@es ;
                                                  <http://www.w3.org/2004/02/skos/core#definition> "Duración de una entidad temporal."@es ,
                                                                                                   "Duration of a temporal entity."@en .


###  http://www.w3.org/2006/time#hasTime
<http://www.w3.org/2006/time#hasTime> rdf:type owl:ObjectProperty ;
                                      rdfs:range <http://www.w3.org/2006/time#TemporalEntity> ;
                                      rdfs:comment "Proporciona soporte a la asociación de una entidad temporal (instante o intervalo) a cualquier cosa."@es ,
                                                   "Supports the association of a temporal entity (instant or interval) to any thing"@en ;
                                      rdfs:label "has time"@en ,
                                                 "tiene tiempo"@es ;
                                      <http://www.w3.org/2004/02/skos/core#definition> "Proporciona soporte a la asociación de una entidad temporal (instante o intervalo) a cualquier cosa."@es ,
                                                                                       "Supports the association of a temporal entity (instant or interval) to any thing"@en ;
                                      <http://www.w3.org/2004/02/skos/core#editorialNote> "Característica arriesgada -añadida en la revisión del 2017 que no ha sido todavía utilizada de forma amplia."@es ,
                                                                                          "Feature at risk - added in 2017 revision, and not yet widely used. "@en .


###  http://www.w3.org/2006/time#inDateTime
<http://www.w3.org/2006/time#inDateTime> rdf:type owl:ObjectProperty ;
                                         rdfs:subPropertyOf <http://www.w3.org/2006/time#inTemporalPosition> ;
                                         rdfs:domain <http://www.w3.org/2006/time#Instant> ;
                                         rdfs:range <http://www.w3.org/2006/time#GeneralDateTimeDescription> ;
                                         rdfs:comment "Posición de un instante, expresada utilizando una descripción estructurada."@es ,
                                                      "Position of an instant, expressed using a structured description"@en ;
                                         rdfs:label "en descripción de fecha-hora"@es ,
                                                    "in date-time description"@en ;
                                         <http://www.w3.org/2004/02/skos/core#definition> "Posición de un instante, expresada utilizando una descripción estructurada."@es ,
                                                                                          "Position of an instant, expressed using a structured description"@en .


###  http://www.w3.org/2006/time#inTemporalPosition
<http://www.w3.org/2006/time#inTemporalPosition> rdf:type owl:ObjectProperty ;
                                                 rdfs:domain <http://www.w3.org/2006/time#Instant> ;
                                                 rdfs:range <http://www.w3.org/2006/time#TemporalPosition> ;
                                                 rdfs:comment "Posición de un instante de tiempo."@es ,
                                                              "Position of a time instant"@en ;
                                                 rdfs:label "Temporal position"@en ,
                                                            "posición temporal"@es ;
                                                 <http://www.w3.org/2004/02/skos/core#definition> "Posición de un instante de tiempo."@es ,
                                                                                                  "Position of a time instant"@en .


###  http://www.w3.org/2006/time#inTimePosition
<http://www.w3.org/2006/time#inTimePosition> rdf:type owl:ObjectProperty ;
                                             rdfs:subPropertyOf <http://www.w3.org/2006/time#inTemporalPosition> ;
                                             rdfs:domain <http://www.w3.org/2006/time#Instant> ;
                                             rdfs:range <http://www.w3.org/2006/time#TimePosition> ;
                                             rdfs:comment "Posición de un instante, expresada como una coordenada temporal o un valor nominal."@es ,
                                                          "Position of an instant, expressed as a temporal coordinate or nominal value"@en ;
                                             rdfs:label "Time position"@en ,
                                                        "posición de tiempo"@es ;
                                             <http://www.w3.org/2004/02/skos/core#definition> "Posición de un instante, expresada como una coordenada temporal o un valor nominal."@es ,
                                                                                              "Position of a time instant expressed as a TimePosition"@en .


###  http://www.w3.org/2006/time#inside
<http://www.w3.org/2006/time#inside> rdf:type owl:ObjectProperty ;
                                     rdfs:domain <http://www.w3.org/2006/time#Interval> ;
                                     rdfs:range <http://www.w3.org/2006/time#Instant> ;
                                     rdfs:comment "An instant that falls inside the interval. It is not intended to include beginnings and ends of intervals."@en ,
                                                  "Un instante que cae dentro del intervalo. Se asume que no es ni el principio ni el final de ningún intervalo."@es ;
                                     rdfs:label "has time instant inside"@en ,
                                                "tiene instante de tiempo dentro"@es ;
                                     <http://www.w3.org/2004/02/skos/core#definition> "An instant that falls inside the interval. It is not intended to include beginnings and ends of intervals."@en ,
                                                                                      "Un instante que cae dentro del intervalo. Se asume que no es ni el principio ni el final de ningún intervalo."@es .


###  http://www.w3.org/2006/time#intervalAfter
<http://www.w3.org/2006/time#intervalAfter> rdf:type owl:ObjectProperty ;
                                            rdfs:subPropertyOf <http://www.w3.org/2006/time#after> ,
                                                               <http://www.w3.org/2006/time#intervalDisjoint> ;
                                            owl:inverseOf <http://www.w3.org/2006/time#intervalBefore> ;
                                            rdfs:domain <http://www.w3.org/2006/time#ProperInterval> ;
                                            rdfs:range <http://www.w3.org/2006/time#ProperInterval> ;
                                            rdfs:comment "If a proper interval T1 is intervalAfter another proper interval T2, then the beginning of T1 is after the end of T2."@en ,
                                                         "Si un intervalo propio T1 es posterior a otro intervalo propio T2, entonces el principio de T1 está después que el final de T2." ;
                                            rdfs:label "interval after"@en ,
                                                       "intervalo posterior"@es ;
                                            <http://www.w3.org/2004/02/skos/core#definition> "If a proper interval T1 is intervalAfter another proper interval T2, then the beginning of T1 is after the end of T2."@en ,
                                                                                             "Si un intervalo propio T1 es posterior a otro intervalo propio T2, entonces el principio de T1 está después que el final de T2."@es .


###  http://www.w3.org/2006/time#intervalBefore
<http://www.w3.org/2006/time#intervalBefore> rdf:type owl:ObjectProperty ;
                                             rdfs:subPropertyOf <http://www.w3.org/2006/time#before> ,
                                                                <http://www.w3.org/2006/time#intervalDisjoint> ;
                                             rdfs:domain <http://www.w3.org/2006/time#ProperInterval> ;
                                             rdfs:range <http://www.w3.org/2006/time#ProperInterval> ;
                                             rdfs:comment "If a proper interval T1 is intervalBefore another proper interval T2, then the end of T1 is before the beginning of T2."@en ,
                                                          "Si un intervalo propio T1 está antes que otro intervalo propio T2, entonces el final de T1 está antes que el principio de T2."@es ;
                                             rdfs:label "interval before"@en ,
                                                        "intervalo anterior"@es ;
                                             <http://www.w3.org/2004/02/skos/core#definition> "If a proper interval T1 is intervalBefore another proper interval T2, then the end of T1 is before the beginning of T2."@en ,
                                                                                              "Si un intervalo propio T1 está antes que otro intervalo propio T2, entonces el final de T1 está antes que el principio de T2."@es .


###  http://www.w3.org/2006/time#intervalContains
<http://www.w3.org/2006/time#intervalContains> rdf:type owl:ObjectProperty ;
                                               rdfs:domain <http://www.w3.org/2006/time#ProperInterval> ;
                                               rdfs:range <http://www.w3.org/2006/time#ProperInterval> ;
                                               rdfs:comment "If a proper interval T1 is intervalContains another proper interval T2, then the beginning of T1 is before the beginning of T2, and the end of T1 is after the end of T2."@en ,
                                                            "Si un intervalo propio T1 contiene otro intervalo propio T2, entonces el principio de T1 está antes que el principio de T2, y el final de T1 está después del final de T2."@es ;
                                               rdfs:label "interval contains"@en ,
                                                          "intervalo contiene"@es ;
                                               <http://www.w3.org/2004/02/skos/core#definition> "If a proper interval T1 is intervalContains another proper interval T2, then the beginning of T1 is before the beginning of T2, and the end of T1 is after the end of T2."@en ,
                                                                                                "Si un intervalo propio T1 contiene otro intervalo propio T2, entonces el principio de T1 está antes que el principio de T2, y el final de T1 está después del final de T2."@es .


###  http://www.w3.org/2006/time#intervalDisjoint
<http://www.w3.org/2006/time#intervalDisjoint> rdf:type owl:ObjectProperty ;
                                               rdfs:domain <http://www.w3.org/2006/time#ProperInterval> ;
                                               rdfs:range <http://www.w3.org/2006/time#ProperInterval> ;
                                               rdfs:comment "If a proper interval T1 is intervalDisjoint another proper interval T2, then the beginning of T1 is after the end of T2, or the end of T1 is before the beginning of T2, i.e. the intervals do not overlap in any way, but their ordering relationship is not known."@en ,
                                                            "Si un intervalo propio T1 es disjunto con otro intervalo propio T2, entonces el principio de T1 está después del final de T2, o el final de T1 está antes que el principio de T2, es decir, los intervalos no se solapan de ninguna forma, aunque su relación de orden no se conozca."@es ;
                                               rdfs:label "interval disjoint"@en ,
                                                          "intervalo disjunto"@es ;
                                               <http://www.w3.org/2004/02/skos/core#definition> "If a proper interval T1 is intervalDisjoint another proper interval T2, then the beginning of T1 is after the end of T2, or the end of T1 is before the beginning of T2, i.e. the intervals do not overlap in any way, but their ordering relationship is not known."@en ,
                                                                                                "Si un intervalo propio T1 es disjunto con otro intervalo propio T2, entonces el principio de T1 está después del final de T2, o el final de T1 está antes que el principio de T2, es decir, los intervalos no se solapan de ninguna forma, aunque su relación de orden no se conozca."@es ;
                                               <http://www.w3.org/2004/02/skos/core#note> "Esta relación entre intervalos no estaba incluida en las 13 relaciones básicas definidas por Allen (1984), pero está definida en T.3 como la unión de 'intervalo anterior' con 'intervalo posterior'. Sin embargo, esto está fuera de la expresividad de OWL2, por tanto, está implementado como una propiedad explícita, con 'intervalo anterior' e 'intervalo posterior' como sub-propiedades."@es ,
                                                                                          "This interval relation is not included in the 13 basic relationships defined in Allen (1984), but is defined in (T.3) as the union of :intervalBefore v :intervalAfter . However, that is outside OWL2 expressivity, so is implemented as an explicit property, with :intervalBefore , :intervalAfter as sub-properties"@en .


###  http://www.w3.org/2006/time#intervalDuring
<http://www.w3.org/2006/time#intervalDuring> rdf:type owl:ObjectProperty ;
                                             rdfs:subPropertyOf <http://www.w3.org/2006/time#intervalIn> ;
                                             owl:inverseOf <http://www.w3.org/2006/time#intervalContains> ;
                                             rdfs:domain <http://www.w3.org/2006/time#ProperInterval> ;
                                             rdfs:range <http://www.w3.org/2006/time#ProperInterval> ;
                                             rdfs:comment "If a proper interval T1 is intervalDuring another proper interval T2, then the beginning of T1 is after the beginning of T2, and the end of T1 is before the end of T2."@en ,
                                                          "Si un intervalo propio T1 está durante otro intervalo propio T2, entonces del principio de T1 está después del principio de T2, y el final de T1 está antes que el final de T2."@es ;
                                             rdfs:label "interval during"@en ,
                                                        "intervalo durante"@es ;
                                             <http://www.w3.org/2004/02/skos/core#definition> "If a proper interval T1 is intervalDuring another proper interval T2, then the beginning of T1 is after the beginning of T2, and the end of T1 is before the end of T2."@en ,
                                                                                              "Si un intervalo propio T1 está durante otro intervalo propio T2, entonces del principio de T1 está después del principio de T2, y el final de T1 está antes que el final de T2."@es .


###  http://www.w3.org/2006/time#intervalEquals
<http://www.w3.org/2006/time#intervalEquals> rdf:type owl:ObjectProperty ;
                                             rdfs:domain <http://www.w3.org/2006/time#ProperInterval> ;
                                             rdfs:range <http://www.w3.org/2006/time#ProperInterval> ;
                                             owl:propertyDisjointWith <http://www.w3.org/2006/time#intervalIn> ;
                                             rdfs:comment "If a proper interval T1 is intervalEquals another proper interval T2, then the beginning of T1 is coincident with the beginning of T2, and the end of T1 is coincident with the end of T2."@en ,
                                                          "Si un intervalo propio T1 es igual a otro intervalo propio T2, entonces el principio de T1 coincide con el principio de T2, y el final de T1 coincide con el final de T2."@es ;
                                             rdfs:label "interval equals"@en ,
                                                        "intervalo igual"@es ;
                                             <http://www.w3.org/2004/02/skos/core#definition> "If a proper interval T1 is intervalEquals another proper interval T2, then the beginning of T1 is coincident with the beginning of T2, and the end of T1 is coincident with the end of T2."@en ,
                                                                                              "Si un intervalo propio T1 es igual a otro intervalo propio T2, entonces el principio de T1 coincide con el principio de T2, y el final de T1 coincide con el final de T2."@es .


###  http://www.w3.org/2006/time#intervalFinishedBy
<http://www.w3.org/2006/time#intervalFinishedBy> rdf:type owl:ObjectProperty ;
                                                 owl:inverseOf <http://www.w3.org/2006/time#intervalFinishes> ;
                                                 rdfs:domain <http://www.w3.org/2006/time#ProperInterval> ;
                                                 rdfs:range <http://www.w3.org/2006/time#ProperInterval> ;
                                                 rdfs:comment "If a proper interval T1 is intervalFinishedBy another proper interval T2, then the beginning of T1 is before the beginning of T2, and the end of T1 is coincident with the end of T2."@en ,
                                                              "Si un intervalo propio T1 está terminado por otro intervalo propio T2, entonces el principio de T1 está antes que el principio de T2, y el final de T1 coincide con el final de T2."@es ;
                                                 rdfs:label "interval finished by"@en ,
                                                            "intervalo terminado por"@es ;
                                                 <http://www.w3.org/2004/02/skos/core#definition> "If a proper interval T1 is intervalFinishedBy another proper interval T2, then the beginning of T1 is before the beginning of T2, and the end of T1 is coincident with the end of T2."@en ,
                                                                                                  "Si un intervalo propio T1 está terminado por otro intervalo propio T2, entonces el principio de T1 está antes que el principio de T2, y el final de T1 coincide con el final de T2."@es .


###  http://www.w3.org/2006/time#intervalFinishes
<http://www.w3.org/2006/time#intervalFinishes> rdf:type owl:ObjectProperty ;
                                               rdfs:subPropertyOf <http://www.w3.org/2006/time#intervalIn> ;
                                               rdfs:domain <http://www.w3.org/2006/time#ProperInterval> ;
                                               rdfs:range <http://www.w3.org/2006/time#ProperInterval> ;
                                               rdfs:comment "If a proper interval T1 is intervalFinishes another proper interval T2, then the beginning of T1 is after the beginning of T2, and the end of T1 is coincident with the end of T2."@en ,
                                                            "Si un intervalo propio T1 termina otro intervalo propio T2, entonces del principio de T1 está después del principio de T2, y el final de T1 coincide con el final de T2."@es ;
                                               rdfs:label "interval finishes"@en ,
                                                          "intervalo termina"@es ;
                                               <http://www.w3.org/2004/02/skos/core#definition> "If a proper interval T1 is intervalFinishes another proper interval T2, then the beginning of T1 is after the beginning of T2, and the end of T1 is coincident with the end of T2."@en ,
                                                                                                "Si un intervalo propio T1 termina otro intervalo propio T2, entonces del principio de T1 está después del principio de T2, y el final de T1 coincide con el final de T2."@es .


###  http://www.w3.org/2006/time#intervalIn
<http://www.w3.org/2006/time#intervalIn> rdf:type owl:ObjectProperty ;
                                         rdfs:domain <http://www.w3.org/2006/time#ProperInterval> ;
                                         rdfs:range <http://www.w3.org/2006/time#ProperInterval> ;
                                         rdfs:comment "If a proper interval T1 is intervalIn another proper interval T2, then the beginning of T1 is after the beginning of T2 or is coincident with the beginning of T2, and the end of T1 is before the end of T2, or is coincident with the end of T2, except that end of T1 may not be coincident with the end of T2 if the beginning of T1 is coincident with the beginning of T2."@en ,
                                                      "Si un intervalo propio T1 es un intervalo interior a otro intervalo propio T2, entonces el principio de T1 está después del principio de T2 o coincide con el principio de T2, y el final de T1 está antes que el final de T2, o coincide con el final de T2, excepto que el final de T1 puede no coincidir con el final de T2 si el principio de T1 coincide con el principio de T2."@es ;
                                         rdfs:label "interval in"@en ,
                                                    "intervalo interior"@es ;
                                         <http://www.w3.org/2004/02/skos/core#definition> "If a proper interval T1 is intervalIn another proper interval T2, then the beginning of T1 is after the beginning of T2 or is coincident with the beginning of T2, and the end of T1 is before the end of T2, or is coincident with the end of T2, except that end of T1 may not be coincident with the end of T2 if the beginning of T1 is coincident with the beginning of T2."@en ,
                                                                                          "Si un intervalo propio T1 es un intervalo interior a otro intervalo propio T2, entonces el principio de T1 está después del principio de T2 o coincide con el principio de T2, y el final de T1 está antes que el final de T2, o coincide con el final de T2, excepto que el final de T1 puede no coincidir con el final de T2 si el principio de T1 coincide con el principio de T2."@es ;
                                         <http://www.w3.org/2004/02/skos/core#note> "Esta relación entre intervalos no estaba incluida en las 13 relaciones básicas definidas por Allen (1984), pero se hace referencia a ella como \"una relación importante\" en Allen y Ferguson (1997). Es la unión disjunta de 'intervalo empieza', 'intervalo durante' y con 'intervalo termina'. Sin embargo, esto está fuera de la expresividad de OWL2, por tanto, se implementa como una propiedad explícita, con 'intervalo empieza', 'intervalo durante' e 'intervalo termina' como sub-propiedades."@es ,
                                                                                    "This interval relation is not included in the 13 basic relationships defined in Allen (1984), but is referred to as 'an important relationship' in Allen and Ferguson (1997). It is the disjoint union of :intervalStarts v :intervalDuring v :intervalFinishes . However, that is outside OWL2 expressivity, so is implemented as an explicit property, with :intervalStarts , :intervalDuring , :intervalFinishes as sub-properties"@en .


###  http://www.w3.org/2006/time#intervalMeets
<http://www.w3.org/2006/time#intervalMeets> rdf:type owl:ObjectProperty ;
                                            rdfs:domain <http://www.w3.org/2006/time#ProperInterval> ;
                                            rdfs:range <http://www.w3.org/2006/time#ProperInterval> ;
                                            rdfs:comment "If a proper interval T1 is intervalMeets another proper interval T2, then the end of T1 is coincident with the beginning of T2."@en ,
                                                         "Si un intervalo propio T1 se encuentra con otro intervalo propio T2, entonces el final de T1 coincide con el principio de T2."@es ;
                                            rdfs:label "interval meets"@en ,
                                                       "intervalo se encuentra"@es ;
                                            <http://www.w3.org/2004/02/skos/core#definition> "If a proper interval T1 is intervalMeets another proper interval T2, then the end of T1 is coincident with the beginning of T2."@en ,
                                                                                             "Si un intervalo propio T1 se encuentra con otro intervalo propio T2, entonces el final de T1 coincide con el principio de T2."@es .


###  http://www.w3.org/2006/time#intervalMetBy
<http://www.w3.org/2006/time#intervalMetBy> rdf:type owl:ObjectProperty ;
                                            owl:inverseOf <http://www.w3.org/2006/time#intervalMeets> ;
                                            rdfs:domain <http://www.w3.org/2006/time#ProperInterval> ;
                                            rdfs:range <http://www.w3.org/2006/time#ProperInterval> ;
                                            rdfs:comment "If a proper interval T1 is intervalMetBy another proper interval T2, then the beginning of T1 is coincident with the end of T2."@en ,
                                                         "Si un intervalo propio T1 es 'intervalo encontrado por' otro intervalo propio T2, entonces el principio de T1 coincide con el final de T2."@es ;
                                            rdfs:label "interval met by"@en ,
                                                       "intervalo encontrado por"@es ;
                                            <http://www.w3.org/2004/02/skos/core#definition> "If a proper interval T1 is intervalMetBy another proper interval T2, then the beginning of T1 is coincident with the end of T2."@en ,
                                                                                             "Si un intervalo propio T1 es 'intervalo encontrado por' otro intervalo propio T2, entonces el principio de T1 coincide con el final de T2."@es .


###  http://www.w3.org/2006/time#intervalOverlappedBy
<http://www.w3.org/2006/time#intervalOverlappedBy> rdf:type owl:ObjectProperty ;
                                                   rdfs:domain <http://www.w3.org/2006/time#ProperInterval> ;
                                                   rdfs:range <http://www.w3.org/2006/time#ProperInterval> ;
                                                   rdfs:comment "If a proper interval T1 is intervalOverlappedBy another proper interval T2, then the beginning of T1 is after the beginning of T2, the beginning of T1 is before the end of T2, and the end of T1 is after the end of T2."@en ,
                                                                "Si un intervalo propio T1 es 'intervalo solapado por' otro intervalo propio T2, entonces el principio de T1 es posterior al principio de T2, y el principio de T1 es anterior al final de T2, y el final de T1 es posterior al final de T2."@es ;
                                                   rdfs:label "interval overlapped by"@en ,
                                                              "intervalo solapado por"@es ;
                                                   <http://www.w3.org/2004/02/skos/core#definition> "If a proper interval T1 is intervalOverlappedBy another proper interval T2, then the beginning of T1 is after the beginning of T2, the beginning of T1 is before the end of T2, and the end of T1 is after the end of T2."@en ,
                                                                                                    "Si un intervalo propio T1 es 'intervalo solapado por' otro intervalo propio T2, entonces el principio de T1 es posterior al principio de T2, y el principio de T1 es anterior al final de T2, y el final de T1 es posterior al final de T2."@es .


###  http://www.w3.org/2006/time#intervalOverlaps
<http://www.w3.org/2006/time#intervalOverlaps> rdf:type owl:ObjectProperty ;
                                               owl:inverseOf <http://www.w3.org/2006/time#intervalOverlappedBy> ;
                                               rdfs:domain <http://www.w3.org/2006/time#ProperInterval> ;
                                               rdfs:range <http://www.w3.org/2006/time#ProperInterval> ;
                                               rdfs:comment "Asume una dirección en el tiempo. Si una entidad temporal T1 está después de otra entidad temporal T2, entonces el principio de T1 está después del final de T2."@es ,
                                                            "If a proper interval T1 is intervalOverlaps another proper interval T2, then the beginning of T1 is before the beginning of T2, the end of T1 is after the beginning of T2, and the end of T1 is before the end of T2."@en ,
                                                            "Si un intervalo propio T1 se solapa con otro intervalo propio T2, entonces el principio de T1 es anterior al principio de T2, el final de T1 es posterior al principio de T2, y el final de T1 es anterior al final de T2."@es ;
                                               rdfs:label "interval overlaps"@en ,
                                                          "intervalo se solapa"@es ;
                                               <http://www.w3.org/2004/02/skos/core#definition> "If a proper interval T1 is intervalOverlaps another proper interval T2, then the beginning of T1 is before the beginning of T2, the end of T1 is after the beginning of T2, and the end of T1 is before the end of T2."@en ,
                                                                                                "Si un intervalo propio T1 se solapa con otro intervalo propio T2, entonces el principio de T1 es anterior al principio de T2, el final de T1 es posterior al principio de T2, y el final de T1 es anterior al final de T2."@es .


###  http://www.w3.org/2006/time#intervalStartedBy
<http://www.w3.org/2006/time#intervalStartedBy> rdf:type owl:ObjectProperty ;
                                                rdfs:domain <http://www.w3.org/2006/time#ProperInterval> ;
                                                rdfs:range <http://www.w3.org/2006/time#ProperInterval> ;
                                                rdfs:comment "If a proper interval T1 is intervalStarted another proper interval T2, then the beginning of T1 is coincident with the beginning of T2, and the end of T1 is after the end of T2."@en ,
                                                             "Si un intervalo propio T1 es empezado por otro intervalo propio T2, entonces el principio de T1 coincide con el principio de T2, y el final de T1 es posterior al final de T2."@es ;
                                                rdfs:label "interval started by"@en ;
                                                <http://www.w3.org/2004/02/skos/core#definition> "If a proper interval T1 is intervalStarted another proper interval T2, then the beginning of T1 is coincident with the beginning of T2, and the end of T1 is after the end of T2."@en ,
                                                                                                 "Si un intervalo propio T1 es empezado por otro intervalo propio T2, entonces el principio de T1 coincide con el principio de T2, y el final de T1 es posterior al final de T2."@es .


###  http://www.w3.org/2006/time#intervalStarts
<http://www.w3.org/2006/time#intervalStarts> rdf:type owl:ObjectProperty ;
                                             rdfs:subPropertyOf <http://www.w3.org/2006/time#intervalIn> ;
                                             owl:inverseOf <http://www.w3.org/2006/time#intervalStartedBy> ;
                                             rdfs:domain <http://www.w3.org/2006/time#ProperInterval> ;
                                             rdfs:range <http://www.w3.org/2006/time#ProperInterval> ;
                                             rdfs:comment "If a proper interval T1 is intervalStarts another proper interval T2, then the beginning of T1 is coincident with the beginning of T2, and the end of T1 is before the end of T2."@en ,
                                                          "Si un intervalo propio T1 empieza otro intervalo propio T2, entonces del principio de T1 con el principio de T2, y el final de T1 es anterior al final de T2."@es ;
                                             rdfs:label "interval starts"@en ,
                                                        "intervalo empieza"@es ;
                                             <http://www.w3.org/2004/02/skos/core#definition> "If a proper interval T1 is intervalStarts another proper interval T2, then the beginning of T1 is coincident with the beginning of T2, and the end of T1 is before the end of T2."@en ,
                                                                                              "Si un intervalo propio T1 empieza otro intervalo propio T2, entonces del principio de T1 con el final de T2, y el final de T1 es anterior al final de T2."@es .


###  http://www.w3.org/2006/time#monthOfYear
<http://www.w3.org/2006/time#monthOfYear> rdf:type owl:ObjectProperty ;
                                          rdfs:domain <http://www.w3.org/2006/time#GeneralDateTimeDescription> ;
                                          rdfs:range <http://www.w3.org/2006/time#MonthOfYear> ;
                                          rdfs:comment "El mes del año, cuyo valor es un miembro de la clase 'mes del año'."@es ,
                                                       "The month of the year, whose value is a member of the class time:MonthOfYear"@en ;
                                          rdfs:label "mes del año"@es ,
                                                     "month of year"@en ;
                                          <http://www.w3.org/2004/02/skos/core#definition> "El mes del año, cuyo valor es un miembro de la clase 'mes del año'."@es ,
                                                                                           "The month of the year, whose value is a member of the class time:MonthOfYear"@en ;
                                          <http://www.w3.org/2004/02/skos/core#editorialNote> "Característica arriesgada - añadida en la revisión de 2017, y todavía no ampliamente utilizada."@es ,
                                                                                              "Feature at risk - added in 2017 revision, and not yet widely used. "@en .


###  http://www.w3.org/2006/time#timeZone
<http://www.w3.org/2006/time#timeZone> rdf:type owl:ObjectProperty ;
                                       rdfs:domain <http://www.w3.org/2006/time#GeneralDateTimeDescription> ;
                                       rdfs:range <http://www.w3.org/2006/time#TimeZone> ;
                                       rdfs:comment "The time zone for clock elements in the temporal position"@en ;
                                       rdfs:label "en huso horario"@es ,
                                                  "in time zone"@en ;
                                       <http://www.w3.org/2004/02/skos/core#historyNote> """En la versión original de OWL-Time de 2006, el rango de 'en huso horario' se definió en un espacio de nombres diferente \"http://www.w3.org/2006/timezone#\".
            Un axioma de alineación permite que los datos codificados de acuerdo con la versión anterior sean consistentes con la ontología actualizada."""@es ,
                                                                                         """In the original 2006 version of OWL-Time, the range of time:timeZone was a TimeZone class in a separate namespace \"http://www.w3.org/2006/timezone#\". 
An alignment axiom 
	tzont:TimeZone rdfs:subClassOf time:TimeZone . 
allows data encoded according to the previous version to be consistent with the updated ontology. """ ;
                                       <http://www.w3.org/2004/02/skos/core#note> """IANA mantiene una base de datos de husos horarios. Éstas están bien mantenidas y generalmente se consideran autorizadas, pero los ítems individuales no están disponibles en URIs individuales, por tanto, no se pueden utilizar directamente en datos expresados utilizando OWL-Time.
            La BDPedia proporciona un conjunto de recursos correspondientes a los husos horarios de IANA, con una URI para cada uno (por ejemplo, http://dbpedia.org/resource/Australia/Eucla). El Servicio de Reloj Mundial también proporciona una lista de husos horarios con la descripción de cada uno de los disponibles como una página Web individual con una URI adecuada individual (por ejemplo, https://www.timeanddate.com/time/zones/acwst). Éstos, y otros recursos similares, se puden usar como un valor de la propiedad 'huso horario'."""@es ,
                                                                                  """IANA maintains a database of timezones. These are well maintained and generally considered authoritative, but individual items are not available at individual URIs, so cannot be used directly in data expressed using OWL-Time.

DBPedia provides a set of resources corresponding to the IANA timezones, with a URI for each (e.g. http://dbpedia.org/resource/Australia/Eucla). The World Clock service also provides a list of time zones with the description of each available as an individual webpage with a convenient individual URI (e.g. https://www.timeanddate.com/time/zones/acwst). These or other, similar, resources might be used as a value of the time:timeZone property.""" .


###  http://www.w3.org/2006/time#unitType
<http://www.w3.org/2006/time#unitType> rdf:type owl:ObjectProperty ;
                                       rdfs:domain [ rdf:type owl:Class ;
                                                     owl:unionOf ( <http://www.w3.org/2006/time#Duration>
                                                                   <http://www.w3.org/2006/time#GeneralDateTimeDescription>
                                                                 )
                                                   ] ;
                                       rdfs:range <http://www.w3.org/2006/time#TemporalUnit> ;
                                       rdfs:comment "La unidad de tiempo que proporciona la precisión de un valor fecha-hora o la escala de una extensión temporal."@es ,
                                                    "The temporal unit which provides the precision of a date-time value or scale of a temporal extent"@en ;
                                       rdfs:label "temporal unit type"@en ,
                                                  "tipo de unidad temporal"@es .


#################################################################
#    Data properties
#################################################################

###  http://www.semanticweb.org/sc3/ontologies/2022/0/Planning-Ontology#hasAnticipationCapabilities
:hasAnticipationCapabilities rdf:type owl:DatatypeProperty ;
                             rdfs:subPropertyOf owl:topDataProperty ;
                             rdfs:domain :DecisionMakingUnit ;
                             rdfs:range xsd:string ;
                             rdfs:comment "Anticipatory activities are used by a DECISION-MAKING UNIT to take into account the characteristics and the situation of other DECISION-MAKING UNITs in course of its own decision making (Schneeweiss 2003)." .


###  http://www.semanticweb.org/sc3/ontologies/2022/0/Planning-Ontology#hasAvailabilityDate
:hasAvailabilityDate rdf:type owl:DatatypeProperty ;
                     rdfs:domain :SupplyInformation ;
                     rdfs:range xsd:string .


###  http://www.semanticweb.org/sc3/ontologies/2022/0/Planning-Ontology#hasBinningPercentage
:hasBinningPercentage rdf:type owl:DatatypeProperty ;
                      rdfs:domain :Process ;
                      rdfs:range xsd:int .


###  http://www.semanticweb.org/sc3/ontologies/2022/0/Planning-Ontology#hasCapacityUnit
:hasCapacityUnit rdf:type owl:DatatypeProperty ;
                 rdfs:domain :Capacity ;
                 rdfs:range xsd:string .


###  http://www.semanticweb.org/sc3/ontologies/2022/0/Planning-Ontology#hasCommitDate
:hasCommitDate rdf:type owl:DatatypeProperty ;
               rdfs:domain <http://www.semanticweb.org/sc3/ontologies/2022/0/ozone-ontology#Demand> ;
               rdfs:range xsd:string .


###  http://www.semanticweb.org/sc3/ontologies/2022/0/Planning-Ontology#hasConsumedQuantity
:hasConsumedQuantity rdf:type owl:DatatypeProperty ;
                     rdfs:domain :RequiredCapacity ;
                     rdfs:range xsd:int .


###  http://www.semanticweb.org/sc3/ontologies/2022/0/Planning-Ontology#hasCosts
:hasCosts rdf:type owl:DatatypeProperty ;
          rdfs:subPropertyOf owl:topDataProperty ;
          rdfs:domain :PlaningPurpose ,
                      :Substitution ;
          rdfs:range xsd:string ;
          rdfs:comment "Cost refers to the amount of money that is needed to do a certain action for a unit of a certain good, for instance, store or produce a unit of a product." .


###  http://www.semanticweb.org/sc3/ontologies/2022/0/Planning-Ontology#hasCurrentStockLevel
:hasCurrentStockLevel rdf:type owl:DatatypeProperty ;
                      rdfs:domain :Inventory ;
                      rdfs:range xsd:int .


###  http://www.semanticweb.org/sc3/ontologies/2022/0/Planning-Ontology#hasDecision-Rights
:hasDecision-Rights rdf:type owl:DatatypeProperty ;
                    rdfs:subPropertyOf owl:topDataProperty ;
                    rdfs:domain :DecisionMakingUnit ;
                    rdfs:range xsd:string ;
                    rdfs:comment "This property will allow a DECISION-MAKING UNIT to negotiate the instruction provided by other DECISION-MAKING UNIT. In a conventional or strict hierarchical setting, negotiations of instruction provided by superior DECISION-MAKING UNITs are impossible. In a distributed hierarchical setting in the sense of Schneeweiss (2003) reactions of the DECISION-MAKING UNIT which can lead to negotiations are possible (Schneeweiss 2003)." .


###  http://www.semanticweb.org/sc3/ontologies/2022/0/Planning-Ontology#hasDecisionTime
:hasDecisionTime rdf:type owl:DatatypeProperty ;
                 rdfs:subPropertyOf owl:topDataProperty ;
                 rdfs:domain :DecisionMakingUnit ;
                 rdfs:range xsd:string ;
                 rdfs:comment "This property describes the point of time when a decision is made by the DECISION-MAKING UNIT." .


###  http://www.semanticweb.org/sc3/ontologies/2022/0/Planning-Ontology#hasDemandClass
:hasDemandClass rdf:type owl:DatatypeProperty ;
                rdfs:domain <http://www.semanticweb.org/sc3/ontologies/2022/0/ozone-ontology#Demand> ;
                rdfs:range xsd:string .


###  http://www.semanticweb.org/sc3/ontologies/2022/0/Planning-Ontology#hasDistribution
:hasDistribution rdf:type owl:DatatypeProperty ;
                 rdfs:domain :Binning ;
                 rdfs:range xsd:int .


###  http://www.semanticweb.org/sc3/ontologies/2022/0/Planning-Ontology#hasDueDate
:hasDueDate rdf:type owl:DatatypeProperty ;
            rdfs:subPropertyOf owl:topDataProperty ;
            rdfs:domain :Activity ,
                        :Part ,
                        :PlanningObject ,
                        :SupplyInformation ;
            rdfs:range xsd:dateTime ;
            rdfs:comment "This is the latest time where the activities associated with a PLANNING OBJECT have to be finished. Note that the parameter DUE DATE is exogenous, i.e. given, in contrast to the property TIME." .


###  http://www.semanticweb.org/sc3/ontologies/2022/0/Planning-Ontology#hasEarliestReleaseDate
:hasEarliestReleaseDate rdf:type owl:DatatypeProperty ;
                        rdfs:domain :Part ;
                        rdfs:range xsd:string .


###  http://www.semanticweb.org/sc3/ontologies/2022/0/Planning-Ontology#hasEffectiveDate
:hasEffectiveDate rdf:type owl:DatatypeProperty ;
                  rdfs:domain :Yield ;
                  rdfs:range xsd:string .


###  http://www.semanticweb.org/sc3/ontologies/2022/0/Planning-Ontology#hasEffectiveStartDate
:hasEffectiveStartDate rdf:type owl:DatatypeProperty ;
                       rdfs:domain :Capacity ;
                       rdfs:range xsd:string .


###  http://www.semanticweb.org/sc3/ontologies/2022/0/Planning-Ontology#hasEndDate
:hasEndDate rdf:type owl:DatatypeProperty ;
            rdfs:domain :Binning ,
                        :FrozenFence ,
                        :InventoryPolicy ,
                        :LotSizingRule ,
                        :Substitution ;
            rdfs:range xsd:string .


###  http://www.semanticweb.org/sc3/ontologies/2022/0/Planning-Ontology#hasEndTime
:hasEndTime rdf:type owl:DatatypeProperty ;
            rdfs:subPropertyOf owl:topDataProperty ;
            rdfs:domain :PlanningConstraint ;
            rdfs:range xsd:string ;
            rdfs:comment "This is the latest point in time when the PLANNING CONSTRAINT is active." .


###  http://www.semanticweb.org/sc3/ontologies/2022/0/Planning-Ontology#hasFeasibilityStatus
:hasFeasibilityStatus rdf:type owl:DatatypeProperty ;
                      rdfs:subPropertyOf owl:topDataProperty ;
                      rdfs:domain :Plan ;
                      rdfs:range xsd:string ;
                      rdfs:comment "A PLAN is feasible if all PLANNING CONSTAINTS of the PLANNING INSTANCE on which the plan is based are fulfilled, otherwise, the plan is infeasible." .


###  http://www.semanticweb.org/sc3/ontologies/2022/0/Planning-Ontology#hasHardConstraints
:hasHardConstraints rdf:type owl:DatatypeProperty ;
                    rdfs:subPropertyOf owl:topDataProperty ;
                    rdfs:domain :PlanningConstraint ;
                    rdfs:range xsd:string ;
                    rdfs:comment "PLANNING CONSTRAINTS with this property cannot be violated." .


###  http://www.semanticweb.org/sc3/ontologies/2022/0/Planning-Ontology#hasIdentifier
:hasIdentifier rdf:type owl:DatatypeProperty ;
               rdfs:subPropertyOf owl:topDataProperty ;
               rdfs:domain :PlanningObject ;
               rdfs:range xsd:string ;
               rdfs:comment "Each PLANNING OBJECT has a unique identifier, abbreviated by ID." .


###  http://www.semanticweb.org/sc3/ontologies/2022/0/Planning-Ontology#hasInformationStatus
:hasInformationStatus rdf:type owl:DatatypeProperty ;
                      rdfs:subPropertyOf owl:topDataProperty ;
                      rdfs:domain :DecisionMakingUnit ;
                      rdfs:range xsd:string ;
                      rdfs:comment "This property describes the own internal, but also the external situation of the DECISION-MAKING UNIT. At the same time, it describes information about the internal and external situation of other DECISION-MAKING UNITs and their information status (Schneeweiss 2003)." .


###  http://www.semanticweb.org/sc3/ontologies/2022/0/Planning-Ontology#hasLeadTime
:hasLeadTime rdf:type owl:DatatypeProperty ;
             rdfs:domain :Process ;
             rdfs:range xsd:int .


###  http://www.semanticweb.org/sc3/ontologies/2022/0/Planning-Ontology#hasLevel
:hasLevel rdf:type owl:DatatypeProperty ;
          rdfs:subPropertyOf owl:topDataProperty ;
          rdfs:domain :Edge ,
                      :PlanningSituation ;
          rdfs:range xsd:string ;
          rdfs:comment "Each vertex has a level. The highest level is assigned to vertices that do not receive instructions from other vertices. The vertices belonging to the second highest level receive instructions only from vertices of the highest level. This definition can be repeated in a recursive manner. Reactions are only possible from vertices of level k-1 to vertices of level k or level k-1." .


###  http://www.semanticweb.org/sc3/ontologies/2022/0/Planning-Ontology#hasMaximumCapacity
:hasMaximumCapacity rdf:type owl:DatatypeProperty ;
                    rdfs:domain :AvailableCapacity ;
                    rdfs:range xsd:int .


###  http://www.semanticweb.org/sc3/ontologies/2022/0/Planning-Ontology#hasMaximumComputingTime
:hasMaximumComputingTime rdf:type owl:DatatypeProperty ;
                         rdfs:subPropertyOf owl:topDataProperty ;
                         rdfs:domain :PlanningProcess ;
                         rdfs:range xsd:string ;
                         rdfs:comment "This property specifies which maximum time is allowed to perform a certain planning activity." .


###  http://www.semanticweb.org/sc3/ontologies/2022/0/Planning-Ontology#hasMaximumLotSize
:hasMaximumLotSize rdf:type owl:DatatypeProperty ;
                   rdfs:domain :LotSizingRule ;
                   rdfs:range xsd:int .


###  http://www.semanticweb.org/sc3/ontologies/2022/0/Planning-Ontology#hasMaximumSupply
:hasMaximumSupply rdf:type owl:DatatypeProperty ;
                  rdfs:domain :SupplyInformation ;
                  rdfs:range xsd:string .


###  http://www.semanticweb.org/sc3/ontologies/2022/0/Planning-Ontology#hasMinimumCapacity
:hasMinimumCapacity rdf:type owl:DatatypeProperty ;
                    rdfs:domain :AvailableCapacity ;
                    rdfs:range xsd:int .


###  http://www.semanticweb.org/sc3/ontologies/2022/0/Planning-Ontology#hasMinimumLotSize
:hasMinimumLotSize rdf:type owl:DatatypeProperty ;
                   rdfs:domain :LotSizingRule ;
                   rdfs:range xsd:int .


###  http://www.semanticweb.org/sc3/ontologies/2022/0/Planning-Ontology#hasMinimumSupply
:hasMinimumSupply rdf:type owl:DatatypeProperty ;
                  rdfs:domain :SupplyInformation ;
                  rdfs:range xsd:string .


###  http://www.semanticweb.org/sc3/ontologies/2022/0/Planning-Ontology#hasOffsetPeriods
:hasOffsetPeriods rdf:type owl:DatatypeProperty ;
                  rdfs:domain :RequiredCapacity ;
                  rdfs:range xsd:int .


###  http://www.semanticweb.org/sc3/ontologies/2022/0/Planning-Ontology#hasOrigin
:hasOrigin rdf:type owl:DatatypeProperty ;
           rdfs:domain <http://www.semanticweb.org/sc3/ontologies/2022/0/ozone-ontology#Demand> ;
           rdfs:range xsd:string .


###  http://www.semanticweb.org/sc3/ontologies/2022/0/Planning-Ontology#hasPartType
:hasPartType rdf:type owl:DatatypeProperty ;
             rdfs:domain :ProjectedWip ;
             rdfs:range xsd:string .


###  http://www.semanticweb.org/sc3/ontologies/2022/0/Planning-Ontology#hasPenalityCosts
:hasPenalityCosts rdf:type owl:DatatypeProperty ;
                  rdfs:subPropertyOf owl:topDataProperty ;
                  rdfs:domain :PlaningPurpose ;
                  rdfs:range xsd:string ;
                  rdfs:comment "If CONSTRAINTS are violated by a plan penalties might be used to change the performance measure values to express that the violations are undesired." .


###  http://www.semanticweb.org/sc3/ontologies/2022/0/Planning-Ontology#hasPerformanceCriteria
:hasPerformanceCriteria rdf:type owl:DatatypeProperty ;
                        rdfs:domain :PlaningPurpose ;
                        rdfs:range xsd:string .


###  http://www.semanticweb.org/sc3/ontologies/2022/0/Planning-Ontology#hasPerformanceMeasure
:hasPerformanceMeasure rdf:type owl:DatatypeProperty ;
                       rdfs:domain :PlaningPurpose ;
                       rdfs:range xsd:string .


###  http://www.semanticweb.org/sc3/ontologies/2022/0/Planning-Ontology#hasPeriod
:hasPeriod rdf:type owl:DatatypeProperty ;
           rdfs:range xsd:int .


###  http://www.semanticweb.org/sc3/ontologies/2022/0/Planning-Ontology#hasPlanningPeriod
:hasPlanningPeriod rdf:type owl:DatatypeProperty ;
                   rdfs:subPropertyOf owl:topDataProperty ;
                   rdfs:domain :PlanningInstance ;
                   rdfs:range xsd:int ;
                   rdfs:comment "This property defines a certain fraction of a planning window. Equidistant periods are common for many supply chain planning problems." .


###  http://www.semanticweb.org/sc3/ontologies/2022/0/Planning-Ontology#hasPlanningWindow
:hasPlanningWindow rdf:type owl:DatatypeProperty ;
                   rdfs:subPropertyOf owl:topDataProperty ;
                   rdfs:domain :PlaningPurpose ,
                               :PlanningInstance ;
                   rdfs:range xsd:int ;
                   rdfs:comment "A planning window described for which amount of periods or which time span the performance measure values have to be calculated. In some situations, the planning window will determine the set of planning objects, for instance, lots completed within the planning window." .


###  http://www.semanticweb.org/sc3/ontologies/2022/0/Planning-Ontology#hasPriority
:hasPriority rdf:type owl:DatatypeProperty ;
             rdfs:subPropertyOf owl:topDataProperty ;
             rdfs:domain :PlanningObject ;
             rdfs:range xsd:int ;
             rdfs:comment "This property describes the relative importance of the PLANNING OBJECT. It provided the base for establishing a partial ordering of the importance of the set of planning objects." .


###  http://www.semanticweb.org/sc3/ontologies/2022/0/Planning-Ontology#hasProjectedDate
:hasProjectedDate rdf:type owl:DatatypeProperty ;
                  rdfs:domain :In-TransitInventory ,
                              :ProjectedWip ;
                  rdfs:range xsd:string .


###  http://www.semanticweb.org/sc3/ontologies/2022/0/Planning-Ontology#hasProjectedQuantity
:hasProjectedQuantity rdf:type owl:DatatypeProperty ;
                      rdfs:domain :In-TransitInventory ,
                                  :ProjectedWip ;
                      rdfs:range xsd:int .


###  http://www.semanticweb.org/sc3/ontologies/2022/0/Planning-Ontology#hasQuantity
:hasQuantity rdf:type owl:DatatypeProperty ;
             rdfs:subPropertyOf owl:topDataProperty ;
             rdfs:domain :PlanningObject ,
                         <http://www.semanticweb.org/sc3/ontologies/2022/0/ozone-ontology#Demand> ;
             rdfs:range xsd:int ;
             rdfs:comment "This property describes given, i.e. fixed, size of a PLANNING OBJECT, for instance, the number of wafers that belong to a lot. Note that the parameter QUANTITY is exogenous, i.e. given, in contrast to the property QUANTITY where the amount of the quantity has to be decided." .


###  http://www.semanticweb.org/sc3/ontologies/2022/0/Planning-Ontology#hasReleaseDate
:hasReleaseDate rdf:type owl:DatatypeProperty ;
                rdfs:subPropertyOf owl:topDataProperty ;
                rdfs:domain :Activity ,
                            :PlanningObject ;
                rdfs:range xsd:dateTime .


###  http://www.semanticweb.org/sc3/ontologies/2022/0/Planning-Ontology#hasRequestedDate
:hasRequestedDate rdf:type owl:DatatypeProperty ;
                  rdfs:domain <http://www.semanticweb.org/sc3/ontologies/2022/0/ozone-ontology#Demand> ;
                  rdfs:range xsd:string .


###  http://www.semanticweb.org/sc3/ontologies/2022/0/Planning-Ontology#hasRevenue
:hasRevenue rdf:type owl:DatatypeProperty ;
            rdfs:subPropertyOf owl:topDataProperty ;
            rdfs:domain :PlaningPurpose ;
            rdfs:range xsd:string ;
            rdfs:comment "Revenue refers to the amount of income, earning generated by the sale of one unit of a certain good." .


###  http://www.semanticweb.org/sc3/ontologies/2022/0/Planning-Ontology#hasSafetyStockLevel
:hasSafetyStockLevel rdf:type owl:DatatypeProperty ;
                     rdfs:domain :InventoryPolicy ;
                     rdfs:range xsd:int .


###  http://www.semanticweb.org/sc3/ontologies/2022/0/Planning-Ontology#hasSafetyStockTime
:hasSafetyStockTime rdf:type owl:DatatypeProperty ;
                    rdfs:domain :InventoryPolicy ;
                    rdfs:range xsd:string .


###  http://www.semanticweb.org/sc3/ontologies/2022/0/Planning-Ontology#hasSetOfConnections
:hasSetOfConnections rdf:type owl:DatatypeProperty ;
                     rdfs:subPropertyOf owl:topDataProperty ;
                     rdfs:domain :PlanningSituation ;
                     rdfs:range xsd:string .


###  http://www.semanticweb.org/sc3/ontologies/2022/0/Planning-Ontology#hasSoftConstraints
:hasSoftConstraints rdf:type owl:DatatypeProperty ;
                    rdfs:subPropertyOf owl:topDataProperty ;
                    rdfs:domain :PlanningConstraint ;
                    rdfs:range xsd:string ;
                    rdfs:comment "PLANNING CONSTRAINTS with this property can be violated. This means that the degree of violation is typically penalized in a related criterion or performance measure." .


###  http://www.semanticweb.org/sc3/ontologies/2022/0/Planning-Ontology#hasStartDate
:hasStartDate rdf:type owl:DatatypeProperty ;
              rdfs:domain :Binning ,
                          :InventoryPolicy ,
                          :LotSizingRule ,
                          :Substitution ;
              rdfs:range xsd:string .


###  http://www.semanticweb.org/sc3/ontologies/2022/0/Planning-Ontology#hasStartTime
:hasStartTime rdf:type owl:DatatypeProperty ;
              rdfs:subPropertyOf owl:topDataProperty ;
              rdfs:domain :PlanningConstraint ;
              rdfs:range xsd:string ;
              rdfs:comment "This is the earliest point in time when the PLANNING CONSTRAINT is active." .


###  http://www.semanticweb.org/sc3/ontologies/2022/0/Planning-Ontology#hasSubstitutionQuantity
:hasSubstitutionQuantity rdf:type owl:DatatypeProperty ;
                         rdfs:domain :Substitution ;
                         rdfs:range xsd:int .


###  http://www.semanticweb.org/sc3/ontologies/2022/0/Planning-Ontology#hasTime
:hasTime rdf:type owl:DatatypeProperty ;
         rdfs:subPropertyOf owl:topDataProperty ;
         rdfs:domain :PlanningObject ;
         rdfs:range xsd:string ;
         rdfs:comment "This property is required to manage timing aspects of a PLANNING OBJECT. It can be a release time, a finishing time, a single start time, or a set of start time for certain ACTIVITIES to be fulfilled." .


###  http://www.semanticweb.org/sc3/ontologies/2022/0/Planning-Ontology#hasType
:hasType rdf:type owl:DatatypeProperty ;
         rdfs:domain :InventoryPolicy ,
                     :Order ,
                     :SupplyInformation ;
         rdfs:range xsd:string .


###  http://www.semanticweb.org/sc3/ontologies/2022/0/Planning-Ontology#hasWeights
:hasWeights rdf:type owl:DatatypeProperty ;
            rdfs:subPropertyOf owl:topDataProperty ;
            rdfs:domain :PlaningPurpose ;
            rdfs:range xsd:int ;
            rdfs:comment "Weights can be used to express preferences of the decision makers among the different performance measures and related criteria. This is, for instance, useful if a lexicographic approach is used." .


###  http://www.semanticweb.org/sc3/ontologies/2022/0/Planning-Ontology#numberOfOperationsOnSameResource
:numberOfOperationsOnSameResource rdf:type owl:DatatypeProperty ;
                                  rdfs:domain <http://www.semanticweb.org/sc3/ontologies/2022/0/ozone-ontology#Product> ;
                                  rdfs:range xsd:int .


###  http://www.w3.org/2002/07/owl#topDataProperty
owl:topDataProperty rdfs:comment "This is the earliest time where the activities associated with a PLANNING OBJECT can start. Note that the parameter RELEASE DATE is exogenous, i.e. given, in contrast to the property TIME." .


###  http://www.w3.org/2006/time#day
<http://www.w3.org/2006/time#day> rdf:type owl:DatatypeProperty ;
                                  rdfs:domain <http://www.w3.org/2006/time#GeneralDateTimeDescription> ;
                                  rdfs:comment """Day position in a calendar-clock system.

The range of this property is not specified, so can be replaced by any specific representation of a calendar day from any calendar. """@en ,
                                               "Posición de día en un sistema calendario-reloj."@es ;
                                  rdfs:label "day"@en ,
                                             "día"@es ;
                                  <http://www.w3.org/2004/02/skos/core#definition> """Day position in a calendar-clock system.

The range of this property is not specified, so can be replaced by any specific representation of a calendar day from any calendar. """@en ,
                                                                                   """Posición de día en un sistema calendario-reloj.

El rango de esta propiedad no está especificado, por tanto, se puede reemplazar por una representación específica de un día de calendario de cualquier calendario."""@es .


###  http://www.w3.org/2006/time#dayOfYear
<http://www.w3.org/2006/time#dayOfYear> rdf:type owl:DatatypeProperty ;
                                        rdfs:domain <http://www.w3.org/2006/time#GeneralDateTimeDescription> ;
                                        rdfs:range xsd:nonNegativeInteger ;
                                        rdfs:comment "El número de día en el año."@es ,
                                                     "The number of the day within the year"@en ;
                                        rdfs:label "day of year"@en ,
                                                   "día del año"@es ;
                                        <http://www.w3.org/2004/02/skos/core#definition> "El número de día en el año."@es ,
                                                                                         "The number of the day within the year"@en .


###  http://www.w3.org/2006/time#days
<http://www.w3.org/2006/time#days> rdf:type owl:DatatypeProperty ;
                                   rdfs:domain <http://www.w3.org/2006/time#GeneralDurationDescription> ;
                                   rdfs:range xsd:decimal ;
                                   rdfs:comment "Longitud de, o elemento de la longitud de, una extensión temporal expresada en días."@es ,
                                                "length of, or element of the length of, a temporal extent expressed in days"@en ;
                                   rdfs:label "days duration"@en ,
                                              "duración en días"@es ;
                                   <http://www.w3.org/2004/02/skos/core#definition> "Longitud de, o elemento de la longitud de, una extensión temporal expresada en días."@es ,
                                                                                    "length of, or element of the length of, a temporal extent expressed in days"@en .


###  http://www.w3.org/2006/time#hasXSDDuration
<http://www.w3.org/2006/time#hasXSDDuration> rdf:type owl:DatatypeProperty ;
                                             rdfs:domain <http://www.w3.org/2006/time#TemporalEntity> ;
                                             rdfs:range xsd:duration ;
                                             rdfs:comment "Extensión de una entidad temporal, expresada utilizando xsd:duration."@es ,
                                                          "Extent of a temporal entity, expressed using xsd:duration"@en ;
                                             rdfs:label "has XSD duration"@en ,
                                                        "tiene duración XSD"@es ;
                                             <http://www.w3.org/2004/02/skos/core#definition> "Extensión de una entidad temporal, expresada utilizando xsd:duration."@es ,
                                                                                              "Extent of a temporal entity, expressed using xsd:duration"@en ;
                                             <http://www.w3.org/2004/02/skos/core#editorialNote> "Característica arriesgada - añadida en la revisión de 2017, y todavía no ampliamente utilizada."@es ,
                                                                                                 "Feature at risk - added in 2017 revision, and not yet widely used. "@en .


###  http://www.w3.org/2006/time#hour
<http://www.w3.org/2006/time#hour> rdf:type owl:DatatypeProperty ;
                                   rdfs:domain <http://www.w3.org/2006/time#GeneralDateTimeDescription> ;
                                   rdfs:range xsd:nonNegativeInteger ;
                                   rdfs:comment "Hour position in a calendar-clock system."@en ,
                                                "Posición de hora en un sistema calendario-reloj."@es ;
                                   rdfs:label "hora"@es ,
                                              "hour"@en ;
                                   <http://www.w3.org/2004/02/skos/core#definition> "Hour position in a calendar-clock system."@en ,
                                                                                    "Posición de hora en un sistema calendario-reloj."@es .


###  http://www.w3.org/2006/time#hours
<http://www.w3.org/2006/time#hours> rdf:type owl:DatatypeProperty ;
                                    rdfs:domain <http://www.w3.org/2006/time#GeneralDurationDescription> ;
                                    rdfs:range xsd:decimal ;
                                    rdfs:comment "Longitud de, o elemento de la longitud de, una extensión temporal expresada en horas."@es ,
                                                 "length of, or element of the length of, a temporal extent expressed in hours"@en ;
                                    rdfs:label "duración en horas"@es ,
                                               "hours duration"@en ;
                                    <http://www.w3.org/2004/02/skos/core#definition> "Longitud de, o elemento de la longitud de, una extensión temporal expresada en horas."@es ,
                                                                                     "length of, or element of the length of, a temporal extent expressed in hours"@en .


###  http://www.w3.org/2006/time#inXSDDate
<http://www.w3.org/2006/time#inXSDDate> rdf:type owl:DatatypeProperty ;
                                        rdfs:domain <http://www.w3.org/2006/time#Instant> ;
                                        rdfs:range xsd:date ;
                                        rdfs:comment "Posición de un instante, expresado utilizando xsd:date."@es ,
                                                     "Position of an instant, expressed using xsd:date"@en ;
                                        rdfs:label "en fecha XSD"@es ,
                                                   "in XSD date"@en ;
                                        <http://www.w3.org/2004/02/skos/core#definition> "Posición de un instante, expresado utilizando xsd:date."@es ,
                                                                                         "Position of an instant, expressed using xsd:date"@en .


###  http://www.w3.org/2006/time#inXSDDateTime
<http://www.w3.org/2006/time#inXSDDateTime> rdf:type owl:DatatypeProperty ;
                                            rdfs:domain <http://www.w3.org/2006/time#Instant> ;
                                            rdfs:range xsd:dateTime ;
                                            rdfs:comment "Posición de un instante, expresado utilizando xsd:dateTime."@es ,
                                                         "Position of an instant, expressed using xsd:dateTime"@en ;
                                            rdfs:label "en fecha-tiempo XSD"@es ,
                                                       "in XSD Date-Time"@en ;
                                            owl:deprecated "true"^^xsd:boolean ;
                                            <http://www.w3.org/2004/02/skos/core#definition> "Posición de un instante, expresado utilizando xsd:dateTime."@es ,
                                                                                             "Position of an instant, expressed using xsd:dateTime"@en ;
                                            <http://www.w3.org/2004/02/skos/core#note> "La propiedad 'en fecha-hora XSD' ha sido reemplazada por 'en fecha-sello de tiempo XSD' que hace obligatorio el campo 'huso horario'."@es ,
                                                                                       "The property :inXSDDateTime is replaced by :inXSDDateTimeStamp which makes the time-zone field mandatory."@en .


###  http://www.w3.org/2006/time#inXSDDateTimeStamp
<http://www.w3.org/2006/time#inXSDDateTimeStamp> rdf:type owl:DatatypeProperty ;
                                                 rdfs:domain <http://www.w3.org/2006/time#Instant> ;
                                                 rdfs:range xsd:dateTimeStamp ;
                                                 rdfs:comment "Posición de un instante, expresado utilizando xsd:dateTimeStamp."@es ,
                                                              "Position of an instant, expressed using xsd:dateTimeStamp"@en ;
                                                 rdfs:label "en fecha-sello de tiempo XSD"@es ,
                                                            "in XSD Date-Time-Stamp"@en ;
                                                 <http://www.w3.org/2004/02/skos/core#definition> "Posición de un instante, expresado utilizando xsd:dateTimeStamp."@es ,
                                                                                                  "Position of an instant, expressed using xsd:dateTimeStamp"@en .


###  http://www.w3.org/2006/time#inXSDgYear
<http://www.w3.org/2006/time#inXSDgYear> rdf:type owl:DatatypeProperty ;
                                         rdfs:domain <http://www.w3.org/2006/time#Instant> ;
                                         rdfs:range xsd:gYear ;
                                         rdfs:comment "Posición de un instante, expresado utilizando xsd:gYear."@es ,
                                                      "Position of an instant, expressed using xsd:gYear"@en ;
                                         rdfs:label "en año gregoriano XSD"@es ,
                                                    "in XSD g-Year"@en ;
                                         <http://www.w3.org/2004/02/skos/core#definition> "Posición de un instante, expresado utilizando xsd:gYear."@es ,
                                                                                          "Position of an instant, expressed using xsd:gYear"@en .


###  http://www.w3.org/2006/time#inXSDgYearMonth
<http://www.w3.org/2006/time#inXSDgYearMonth> rdf:type owl:DatatypeProperty ;
                                              rdfs:domain <http://www.w3.org/2006/time#Instant> ;
                                              rdfs:range xsd:gYearMonth ;
                                              rdfs:comment "Posición de un instante, expresado utilizando xsd:gYearMonth."@es ,
                                                           "Position of an instant, expressed using xsd:gYearMonth"@en ;
                                              rdfs:label "en año-mes gregoriano XSD"@es ,
                                                         "in XSD g-YearMonth"@en ;
                                              <http://www.w3.org/2004/02/skos/core#definition> "Posición de un instante, expresado utilizando xsd:gYearMonth."@es ,
                                                                                               "Position of an instant, expressed using xsd:gYearMonth"@en .


###  http://www.w3.org/2006/time#minute
<http://www.w3.org/2006/time#minute> rdf:type owl:DatatypeProperty ;
                                     rdfs:domain <http://www.w3.org/2006/time#GeneralDateTimeDescription> ;
                                     rdfs:range xsd:nonNegativeInteger ;
                                     rdfs:comment "Minute position in a calendar-clock system."@en ,
                                                  "Posición de minuto en un sistema calendario-reloj."@es ;
                                     rdfs:label "minute"@en ,
                                                "minuto"@es ;
                                     <http://www.w3.org/2004/02/skos/core#definition> "Minute position in a calendar-clock system."@en ,
                                                                                      "Posición de minuto en un sistema calendario-reloj."@es .


###  http://www.w3.org/2006/time#minutes
<http://www.w3.org/2006/time#minutes> rdf:type owl:DatatypeProperty ;
                                      rdfs:domain <http://www.w3.org/2006/time#GeneralDurationDescription> ;
                                      rdfs:range xsd:decimal ;
                                      rdfs:comment "Longitud de, o elemento de la longitud de, una extensión temporal expresada en minutos."@es ,
                                                   "length, or element of, a temporal extent expressed in minutes"@en ;
                                      rdfs:label "minutes"@en ,
                                                 "minutos"@es ;
                                      <http://www.w3.org/2004/02/skos/core#definition> "Longitud de, o elemento de la longitud de, una extensión temporal expresada en minutos."@es ,
                                                                                       "length, or element of, a temporal extent expressed in minutes"@en .


###  http://www.w3.org/2006/time#month
<http://www.w3.org/2006/time#month> rdf:type owl:DatatypeProperty ;
                                    rdfs:domain <http://www.w3.org/2006/time#GeneralDateTimeDescription> ;
                                    rdfs:comment """Month position in a calendar-clock system.

The range of this property is not specified, so can be replaced by any specific representation of a calendar month from any calendar. """@en ,
                                                 """Posición de mes en un sistema calendario-reloj.
    El rango de esta propiedad no está especificado, por tanto, se puede reemplazar por cualquier representación específica de un mes de calendario de un calendario cualquiera."""@es ;
                                    rdfs:label "mes"@es ,
                                               "month"@en ;
                                    <http://www.w3.org/2004/02/skos/core#definition> """Month position in a calendar-clock system.

The range of this property is not specified, so can be replaced by any specific representation of a calendar month from any calendar. """@en ,
                                                                                     """Posición de mes en un sistema calendario-reloj.
            El rango de esta propiedad no está especificado, por tanto, se puede reemplazar por cualquier representación específica de un mes de calendario de un calendario cualquiera."""@es .


###  http://www.w3.org/2006/time#months
<http://www.w3.org/2006/time#months> rdf:type owl:DatatypeProperty ;
                                     rdfs:domain <http://www.w3.org/2006/time#GeneralDurationDescription> ;
                                     rdfs:range xsd:decimal ;
                                     rdfs:comment "Longitud de, o elemento de la longitud de, una extensión temporal expresada en meses."@es ,
                                                  "length of, or element of the length of, a temporal extent expressed in months"@en ;
                                     rdfs:label "duración en meses"@es ,
                                                "months duration"@en ;
                                     <http://www.w3.org/2004/02/skos/core#definition> "Longitud de, o elemento de la longitud de, una extensión temporal expresada en meses."@es ,
                                                                                      "length of, or element of the length of, a temporal extent expressed in months"@en .


###  http://www.w3.org/2006/time#nominalPosition
<http://www.w3.org/2006/time#nominalPosition> rdf:type owl:DatatypeProperty ;
                                              rdfs:domain <http://www.w3.org/2006/time#TimePosition> ;
                                              rdfs:range xsd:string ;
                                              rdfs:comment "El valor (nominal) que indica posición temporal en un sistema de referencia ordinal."@es ,
                                                           "The (nominal) value indicating temporal position in an ordinal reference system "@en ;
                                              rdfs:label "Name of temporal position"@en ,
                                                         "nombre de posición temporal"@es ;
                                              <http://www.w3.org/2004/02/skos/core#definition> "El valor (nominal) que indica posición temporal en un sistema de referencia ordinal."@es ,
                                                                                               "The (nominal) value indicating temporal position in an ordinal reference system "@en .


###  http://www.w3.org/2006/time#numericDuration
<http://www.w3.org/2006/time#numericDuration> rdf:type owl:DatatypeProperty ;
                                              rdfs:domain <http://www.w3.org/2006/time#Duration> ;
                                              rdfs:range xsd:decimal ;
                                              rdfs:comment "Valor de una extensión temporal expresada como un número decimal escalado por una unidad de tiempo."@es ,
                                                           "Value of a temporal extent expressed as a decimal number scaled by a temporal unit"@en ;
                                              rdfs:label "Numeric value of temporal duration"@en ,
                                                         "valor numérico de duración temporal"@es ;
                                              <http://www.w3.org/2004/02/skos/core#definition> "Valor de una extensión temporal expresada como un número decimal escalado por una unidad de tiempo."@es ,
                                                                                               "Value of a temporal extent expressed as a decimal number scaled by a temporal unit"@en .


###  http://www.w3.org/2006/time#numericPosition
<http://www.w3.org/2006/time#numericPosition> rdf:type owl:DatatypeProperty ;
                                              rdfs:domain <http://www.w3.org/2006/time#TimePosition> ;
                                              rdfs:range xsd:decimal ;
                                              rdfs:comment "El valor (numérico) que indica posición temporal en un sistema de referencia ordinal."@es ,
                                                           "The (numeric) value indicating position within a temporal coordinate system "@en ;
                                              rdfs:label "Numeric value of temporal position"@en ,
                                                         "valor numérico de posición temporal"@es ;
                                              <http://www.w3.org/2004/02/skos/core#definition> "El valor (numérico) que indica posición temporal en un sistema de referencia ordinal."@es ,
                                                                                               "The (numeric) value indicating position within a temporal coordinate system "@en .


###  http://www.w3.org/2006/time#second
<http://www.w3.org/2006/time#second> rdf:type owl:DatatypeProperty ;
                                     rdfs:domain <http://www.w3.org/2006/time#GeneralDateTimeDescription> ;
                                     rdfs:range xsd:decimal ;
                                     rdfs:comment "Posición de segundo en un sistema calendario-reloj."@es ,
                                                  "Second position in a calendar-clock system."@en ;
                                     rdfs:label "second"@en ,
                                                "segundo"@es .


###  http://www.w3.org/2006/time#seconds
<http://www.w3.org/2006/time#seconds> rdf:type owl:DatatypeProperty ;
                                      rdfs:domain <http://www.w3.org/2006/time#GeneralDurationDescription> ;
                                      rdfs:range xsd:decimal ;
                                      rdfs:comment "Longitud de, o elemento de la longitud de, una extensión temporal expresada en segundos."@es ,
                                                   "length of, or element of the length of, a temporal extent expressed in seconds"@en ;
                                      rdfs:label "duración en segundos"@es ,
                                                 "seconds duration"@en ;
                                      rdfs:seeAlso <http://www.bipm.org/en/publications/si-brochure/second.html> .


###  http://www.w3.org/2006/time#week
<http://www.w3.org/2006/time#week> rdf:type owl:DatatypeProperty ;
                                   rdfs:domain <http://www.w3.org/2006/time#GeneralDateTimeDescription> ;
                                   rdfs:range xsd:nonNegativeInteger ;
                                   rdfs:comment "Número de semana en el año."@es ,
                                                "Week number within the year."@en ;
                                   rdfs:label "semana"@es ,
                                              "week"@en ;
                                   <http://www.w3.org/2004/02/skos/core#note> "Weeks are numbered differently depending on the calendar in use and the local language or cultural conventions (locale). ISO-8601 specifies that the first week of the year includes at least four days, and that Monday is the first day of the week. In that system, week 1 is the week that contains the first Thursday in the year."@en ;
                                   <http://www.w3.org/2004/02/skos/core#scopeNote> "Las semanas están numeradas de forma diferente dependiendo del calendario en uso y de las convenciones lingüísticas y culturales locales (locale en inglés). El ISO-8601 especifica que la primera semana del año incluye al menos cuatro días, y que el lunes es el primer día de la semana. En ese sistema, la semana 1 es la semana que contiene el primer jueves del año."@es .


###  http://www.w3.org/2006/time#weeks
<http://www.w3.org/2006/time#weeks> rdf:type owl:DatatypeProperty ;
                                    rdfs:domain <http://www.w3.org/2006/time#GeneralDurationDescription> ;
                                    rdfs:range xsd:decimal ;
                                    rdfs:comment "Longitud de, o elemento de la longitud de, una extensión temporal expresada en semanas."@es ,
                                                 "length of, or element of the length of, a temporal extent expressed in weeks"@en ;
                                    rdfs:label "duración en semanas"@es ,
                                               "weeks duration"@en .


###  http://www.w3.org/2006/time#xsdDateTime
<http://www.w3.org/2006/time#xsdDateTime> rdf:type owl:DatatypeProperty ;
                                          rdfs:domain <http://www.w3.org/2006/time#DateTimeInterval> ;
                                          rdfs:range xsd:dateTime ;
                                          rdfs:comment "Valor de 'intervalo de fecha-hora' expresado como un valor compacto."@es ,
                                                       "Value of DateTimeInterval expressed as a compact value."@en ;
                                          rdfs:label "has XSD date-time"@en ,
                                                     "tiene fecha-hora XSD"@es ;
                                          owl:deprecated "true"^^xsd:boolean ;
                                          <http://www.w3.org/2004/02/skos/core#note> "Using xsd:dateTime in this place means that the duration of the interval is implicit: it corresponds to the length of the smallest non-zero element of the date-time literal. However, this rule cannot be used for intervals whose duration is more than one rank smaller than the starting time - e.g. the first minute or second of a day, the first hour of a month, or the first day of a year. In these cases the desired interval cannot be distinguished from the interval corresponding to the next rank up. Because of this essential ambiguity, use of this property is not recommended and it is deprecated."@en ,
                                                                                     "Utilizando xsd:dateTime en este lugar significa que la duración del intervalo está implícita: se corresponde con la longitud del elemento más pequeño distinto de cero del literal fecha-hora. Sin embargo, esta regla no se puede utilizar para intervalos cuya duración es mayor que un rango más pequeño que el tiempo de comienzo - p.ej. el primer minuto o segundo del día, la primera hora del mes, o el primer día del año. En estos casos el intervalo deseado no se puede distinguir del intervalo correspondiente al próximo rango más alto. Debido a esta ambigüedad esencial, no se recomienda el uso de esta propiedad y está desaprobada." .


###  http://www.w3.org/2006/time#year
<http://www.w3.org/2006/time#year> rdf:type owl:DatatypeProperty ;
                                   rdfs:domain <http://www.w3.org/2006/time#GeneralDateTimeDescription> ;
                                   rdfs:comment """Posición de año en un sistema calendario-reloj.

l rango de esta propiedad no está especificado, por tanto, se puede reemplazar por cualquier representación específica de un año de calendario de un calendario cualquiera."""@es ,
                                                """Year position in a calendar-clock system.

The range of this property is not specified, so can be replaced by any specific representation of a calendar year from any calendar. """@en ;
                                   rdfs:label "year"@en .


###  http://www.w3.org/2006/time#years
<http://www.w3.org/2006/time#years> rdf:type owl:DatatypeProperty ;
                                    rdfs:domain <http://www.w3.org/2006/time#GeneralDurationDescription> ;
                                    rdfs:range xsd:decimal ;
                                    rdfs:comment "Longitud de, o elemento de la longitud de, una extensión temporal expresada en años."@es ,
                                                 "length of, or element of the length of, a temporal extent expressed in years"@en ;
                                    rdfs:label "duración en años"@es ,
                                               "years duration"@en .


#################################################################
#    Classes
#################################################################

###  http://www.semanticweb.org/sc3/ontologies/2022/0/Planning-Ontology#Activity
:Activity rdf:type owl:Class .


###  http://www.semanticweb.org/sc3/ontologies/2022/0/Planning-Ontology#Automated
:Automated rdf:type owl:Class ;
           rdfs:subClassOf :DecisionMakerType .


###  http://www.semanticweb.org/sc3/ontologies/2022/0/Planning-Ontology#Autonomous
:Autonomous rdf:type owl:Class ;
            rdfs:subClassOf :DecisionMakingInitiative .


###  http://www.semanticweb.org/sc3/ontologies/2022/0/Planning-Ontology#AvailableCapacity
:AvailableCapacity rdf:type owl:Class ;
                   rdfs:subClassOf :Capacity ;
                   rdfs:comment ": The AVAILABLE CAPACITY describes the ability of a resource within a period of time to perform activities or processes. Elmaghraby (2011) refers to this as operational capacity, i.e. the productive capacity that is obtained from the nominal capacity by subtracting the anticipated and unavoidable loss in productivity, for instance, due to machine breakdowns in a wafer fab." .


###  http://www.semanticweb.org/sc3/ontologies/2022/0/Planning-Ontology#BillOfMaterial
:BillOfMaterial rdf:type owl:Class ;
                rdfs:comment "A BILL OF MATERIALS (BOM) describes the component products used to make another product. Substitution, often associated with binning, is based on the possibility that alternative items might be used to finish a process step." .


###  http://www.semanticweb.org/sc3/ontologies/2022/0/Planning-Ontology#Bin
:Bin rdf:type owl:Class .


###  http://www.semanticweb.org/sc3/ontologies/2022/0/Planning-Ontology#Binning
:Binning rdf:type owl:Class ;
         rdfs:comment "BINNING refers to the process of testing and categorizing parts against defined measures and sort them into different bins (Degbotse 2013). Each bin belongs to certain levels of defined measures (e.g. chip speed, current, voltage, energy consumption). Binning is often combined with SUBSTITUTION." .


###  http://www.semanticweb.org/sc3/ontologies/2022/0/Planning-Ontology#Capacity
:Capacity rdf:type owl:Class .


###  http://www.semanticweb.org/sc3/ontologies/2022/0/Planning-Ontology#ComponentPart
:ComponentPart rdf:type owl:Class ;
               rdfs:subClassOf :Part .


###  http://www.semanticweb.org/sc3/ontologies/2022/0/Planning-Ontology#Criteria
:Criteria rdf:type owl:Class ;
          rdfs:comment "Typical criteria are maximization, minimization, i.e. if an optimization problem is considered, or larger or smaller than a prescribed value of the certain performance measure, a so-called target, i.e. if a satisfaction problem is solved. In a multi-criteria setting, the dominance concept for plans is of interest." .


###  http://www.semanticweb.org/sc3/ontologies/2022/0/Planning-Ontology#DecisionMakerType
:DecisionMakerType rdf:type owl:Class ;
                   rdfs:comment "We distinguish human decision-makers (human DECISION-MAKING UNITS) from fully automated DECISION-MAKING UNITS where computers make fully automated decisions. Between these two extremes there are semi-automated decisions, where a computer provides several decision alternatives and a human decision-maker chooses among them. Note that the decision-maker type can change over time." .


###  http://www.semanticweb.org/sc3/ontologies/2022/0/Planning-Ontology#DecisionMakingInitiative
:DecisionMakingInitiative rdf:type owl:Class ;
                          rdfs:comment "We distinguish fully autonomous DECISION-MAKING UNITS from DECISION-MAKING UNITS where the decision-making activities are triggered by other DECISION-MAKING UNITS. Note that the decision-making initiative can change over time in a situation-dependent manner." .


###  http://www.semanticweb.org/sc3/ontologies/2022/0/Planning-Ontology#DecisionMakingUnit
:DecisionMakingUnit rdf:type owl:Class ;
                    rdfs:comment "The DECISION-MAKING UNIT specifies an instance that makes decisions." .


###  http://www.semanticweb.org/sc3/ontologies/2022/0/Planning-Ontology#DecisonMakingUnitCharacter
:DecisonMakingUnitCharacter rdf:type owl:Class ;
                            rdfs:comment "In an ANTAGO¬NISTIC SETTING, the different DECISION-MAKING UNITS try to meet their own objectives which are in conflict. In a non-antagonistic setting, the DECISION-MAKING UNITS do not exploit their private knowledge in an opportunistic way." .


###  http://www.semanticweb.org/sc3/ontologies/2022/0/Planning-Ontology#Dependent
:Dependent rdf:type owl:Class ;
           rdfs:subClassOf :DecisionMakingInitiative .


###  http://www.semanticweb.org/sc3/ontologies/2022/0/Planning-Ontology#DistributedHierarchicalSituation
:DistributedHierarchicalSituation rdf:type owl:Class ;
                                  rdfs:subClassOf :HierarchicalSituation ;
                                  rdfs:comment "In this situation, edges referring to instructions and reactions are possible." .


###  http://www.semanticweb.org/sc3/ontologies/2022/0/Planning-Ontology#Edge
:Edge rdf:type owl:Class .


###  http://www.semanticweb.org/sc3/ontologies/2022/0/Planning-Ontology#FrozenFence
:FrozenFence rdf:type owl:Class ;
             rdfs:comment "FROZEN FENCE is used to set a frozen interval  in which decision making is not allowed to change the previously determined values." .


###  http://www.semanticweb.org/sc3/ontologies/2022/0/Planning-Ontology#HeterarchicalSituation
:HeterarchicalSituation rdf:type owl:Class ;
                        rdfs:subClassOf :HierarchicalSituation ;
                        rdfs:comment "All the vertices have level 1." .


###  http://www.semanticweb.org/sc3/ontologies/2022/0/Planning-Ontology#HierarchicalSituation
:HierarchicalSituation rdf:type owl:Class .


###  http://www.semanticweb.org/sc3/ontologies/2022/0/Planning-Ontology#Human
:Human rdf:type owl:Class ;
       rdfs:subClassOf :DecisionMakerType .


###  http://www.semanticweb.org/sc3/ontologies/2022/0/Planning-Ontology#In-TransitInventory
:In-TransitInventory rdf:type owl:Class ;
                     rdfs:comment "The IN-TRANSIT INVENTORY describes the quantity of a certain product that is shipped from one location to another. This quantity has left the inventory of one location, but has not yet been received into the inventory of the receiving location." .


###  http://www.semanticweb.org/sc3/ontologies/2022/0/Planning-Ontology#Inventory
:Inventory rdf:type owl:Class ;
           rdfs:comment "The INVENTORY describes the quantity of a certain product that is available in stock to be used to meet demand." .


###  http://www.semanticweb.org/sc3/ontologies/2022/0/Planning-Ontology#InventoryPolicy
:InventoryPolicy rdf:type owl:Class ;
                 rdfs:comment "An INVENTORY POLICY indicates how much earlier or how much more (safety stock) needs to be built than that required to satisfy demand on time. Inventory Policies define the rules which have to be implemented at a specific inventory location such as safety stock or product mix for supporting the production process flow as well as fulfilling customer demand." .


###  http://www.semanticweb.org/sc3/ontologies/2022/0/Planning-Ontology#Location
:Location rdf:type owl:Class ;
          rdfs:comment "" .


###  http://www.semanticweb.org/sc3/ontologies/2022/0/Planning-Ontology#LotSizingRule
:LotSizingRule rdf:type owl:Class ;
               rdfs:comment "A LOT SIZING RULE defines a rule to specify the lot size for a specific part. The lot size on the other hand defines the number of pieces belonging to a part. The lot size is the result of applying lot sizing rules." .


###  http://www.semanticweb.org/sc3/ontologies/2022/0/Planning-Ontology#MacroOperation
:MacroOperation rdf:type owl:Class .


###  http://www.semanticweb.org/sc3/ontologies/2022/0/Planning-Ontology#Order
:Order rdf:type owl:Class .


###  http://www.semanticweb.org/sc3/ontologies/2022/0/Planning-Ontology#Owner
:Owner rdf:type owl:Class .


###  http://www.semanticweb.org/sc3/ontologies/2022/0/Planning-Ontology#Part
:Part rdf:type owl:Class ;
      rdfs:comment "A PART represents a physical instance of a product in the manufacturing process. It therefore realizes a product. A part moves through the system and is manufactured according to its product specification. A part is associated to exactly one product. During the production process it is typically tested several times. The binning rules of the associated product specification can be applied to the respective part. A part can be substituted by another part according to the associated product specification" .


###  http://www.semanticweb.org/sc3/ontologies/2022/0/Planning-Ontology#PerformanceMeasure
:PerformanceMeasure rdf:type owl:Class ;
                    rdfs:comment "Each measure is defined by a calculation procedure. Performance measures can be blended using weights to express the importance of the different measures." .


###  http://www.semanticweb.org/sc3/ontologies/2022/0/Planning-Ontology#Plan
:Plan rdf:type owl:Class ;
      rdfs:comment "A PLAN is an activity specification with an intended purpose." .


###  http://www.semanticweb.org/sc3/ontologies/2022/0/Planning-Ontology#PlanExecutuon
:PlanExecutuon rdf:type owl:Class ;
               rdfs:comment "A PLAN EXECUTION is related to performing the activities according to a PLAN either directly in the base system, for instance, releasing lots into a wafer fab, or as instructions for another DECISION-MAKING UNIT." .


###  http://www.semanticweb.org/sc3/ontologies/2022/0/Planning-Ontology#PlaningPurpose
:PlaningPurpose rdf:type owl:Class ;
                rdfs:comment "" ,
                             "The PLANNING PURPOSE specifies the objectives of a certain planning activity. It is given by a set of performance measures that are related to a set of PLANNING OBJECTS." .


###  http://www.semanticweb.org/sc3/ontologies/2022/0/Planning-Ontology#PlanningApproach
:PlanningApproach rdf:type owl:Class ;
                  rdfs:comment "Specific planning algorithm which is used in a deticated planning process" .


###  http://www.semanticweb.org/sc3/ontologies/2022/0/Planning-Ontology#PlanningConstraint
:PlanningConstraint rdf:type owl:Class ;
                    rdfs:comment "A PLANNING CONSTRAINT restricts the action space. This space is formed by alternative actions that are a result of the planning decisions (Schneeweis 2003). In the planning domain, PLANNING CONSTRAINTS, often the capacity offered by resources, limit the quantities that are assigned to the PLANNING OBJECTS or impact the temporal properties of PLANNING OBJECTS." .


###  http://www.semanticweb.org/sc3/ontologies/2022/0/Planning-Ontology#PlanningDecision
:PlanningDecision rdf:type owl:Class ;
                  rdfs:comment "Decisions determined by a Decision Making Unit" .


###  http://www.semanticweb.org/sc3/ontologies/2022/0/Planning-Ontology#PlanningFunction
:PlanningFunction rdf:type owl:Class ;
                  rdfs:comment "Describes the different functions and its properies follwing the supply chain planning matrix." .


###  http://www.semanticweb.org/sc3/ontologies/2022/0/Planning-Ontology#PlanningInstance
:PlanningInstance rdf:type owl:Class ;
                  rdfs:comment "A PLANNING INSTANCE specifies the PLANNING OBJECTS and the values of related PLANNING CONSTRAINTS that form the basis for a planning decision." .


###  http://www.semanticweb.org/sc3/ontologies/2022/0/Planning-Ontology#PlanningObject
:PlanningObject rdf:type owl:Class ;
                rdfs:comment "A PLANNING OBJECT specifies what has to be planned as an atomic unit. A single PLANNING OBJECT typically represents a quantity of a certain product or product aggregate to be released or completed within a certain period in a certain node of the semiconductor supply chain. Other PLANNING OBJECTS can be orders or lots. Values are assigned to the attributes of a PLANNING OBJECT as a result of a planning decision." .


###  http://www.semanticweb.org/sc3/ontologies/2022/0/Planning-Ontology#PlanningProcess
:PlanningProcess rdf:type owl:Class ;
                 rdfs:comment "The PLANNING PROCESS specifies under which circumstances which (re)planning activities are performed by a DECISION-MAKING UNIT." .


###  http://www.semanticweb.org/sc3/ontologies/2022/0/Planning-Ontology#PlanningSituation
:PlanningSituation rdf:type owl:Class ;
                   rdfs:comment "The PLANNING SITUATION describes the organization of several DECISION-MAKING UNITS and also its environment." .


###  http://www.semanticweb.org/sc3/ontologies/2022/0/Planning-Ontology#Process
:Process rdf:type owl:Class ;
         rdfs:comment "A PROCESS specifies a method of making a product at a location. The process is expressed at a coarse level of granularity suitable for use in production planning." .


###  http://www.semanticweb.org/sc3/ontologies/2022/0/Planning-Ontology#ProductAggregate
:ProductAggregate rdf:type owl:Class ;
                  rdfs:comment "A PRODUCT AGGREGATE combines individual products into a few logical products groups. This results in a reduction of complexity, which enables a better overview." .


###  http://www.semanticweb.org/sc3/ontologies/2022/0/Planning-Ontology#ProductHierarchy
:ProductHierarchy rdf:type owl:Class ;
                  rdfs:comment "A PRODUCT HIERARCHY characterizes the top-down and bottom-up relationship between different product aggregates. It organizes the product aggregates according to defined criteria. A product aggregate is used to group different products based on certain criteria. The grouping criteria depend on the planning purpose (e.g. controlling, production). It is a certain view on a set of products." .


###  http://www.semanticweb.org/sc3/ontologies/2022/0/Planning-Ontology#ProjectedWip
:ProjectedWip rdf:type owl:Class ;
              rdfs:comment "The PROJECTED WIP describes the quantity of a certain product that is anticipated to be received into inventory at a particular location at a particular time." .


###  http://www.semanticweb.org/sc3/ontologies/2022/0/Planning-Ontology#ReplanningDegree
:ReplanningDegree rdf:type owl:Class ;
                  rdfs:comment "The degree distinguishes replanning from scratch and repair of existing plans (Vieria et al. 2003)." .


###  http://www.semanticweb.org/sc3/ontologies/2022/0/Planning-Ontology#RequiredCapacity
:RequiredCapacity rdf:type owl:Class ;
                  rdfs:subClassOf :Capacity .


###  http://www.semanticweb.org/sc3/ontologies/2022/0/Planning-Ontology#Resource-Availability-Constraints
:Resource-Availability-Constraints rdf:type owl:Class ;
                                   rdfs:subClassOf :PlanningConstraint ;
                                   rdfs:comment "This type of constraints has an impact on the assignment of activities to RESOURCES and to START/END TIMES to ACTIVITIES." .


###  http://www.semanticweb.org/sc3/ontologies/2022/0/Planning-Ontology#Resource-Compatibility-Constraints
:Resource-Compatibility-Constraints rdf:type owl:Class ;
                                    rdfs:subClassOf :PlanningConstraint ;
                                    rdfs:comment "This type of constraints ensures that only allowed activities are performed using a given RESOURCE." .


###  http://www.semanticweb.org/sc3/ontologies/2022/0/Planning-Ontology#Route
:Route rdf:type owl:Class .


###  http://www.semanticweb.org/sc3/ontologies/2022/0/Planning-Ontology#SemiAutomated
:SemiAutomated rdf:type owl:Class ;
               rdfs:subClassOf :DecisionMakerType ;
               rdfs:comment "Between these two extremes there are semi-automated decisions, where a computer provides several decision alternatives and a human decision-maker chooses among them." .


###  http://www.semanticweb.org/sc3/ontologies/2022/0/Planning-Ontology#StrictHierarchicalSituation
:StrictHierarchicalSituation rdf:type owl:Class ;
                             rdfs:subClassOf :HierarchicalSituation ;
                             rdfs:comment "There are only edges between vertices of level k and vertices of level k-1, where k≥2." .


###  http://www.semanticweb.org/sc3/ontologies/2022/0/Planning-Ontology#Substitution
:Substitution rdf:type owl:Class ;
              rdfs:comment "SUBSTITUTION refers to using alternative parts. Depending on the product, each one could be replaced by using specific alternatives at the same stage of production, e.g. final product, raw material, or semi-finished products (Degbotse 2013) in order to complete a manufacturing step or fulfill a customer order." .


###  http://www.semanticweb.org/sc3/ontologies/2022/0/Planning-Ontology#SupplyInformation
:SupplyInformation rdf:type owl:Class ;
                   rdfs:comment "SUPPLY INFORMATION provides information of the used and unused supply of a supply chain network." .


###  http://www.semanticweb.org/sc3/ontologies/2022/0/Planning-Ontology#Target
:Target rdf:type owl:Class ;
        rdfs:comment "Targets are prescribed values for the different performance measures." .


###  http://www.semanticweb.org/sc3/ontologies/2022/0/Planning-Ontology#Temporal-Constraints
:Temporal-Constraints rdf:type owl:Class ;
                      rdfs:subClassOf :PlanningConstraint ;
                      rdfs:comment "This type of constraints restricts the values of temporal attributes, modeled by the property TIME, that belong to PLANNING OBJECTS. For instance, there might be a minimum amount of time between two consecutive operations of a certain product." .


###  http://www.semanticweb.org/sc3/ontologies/2022/0/Planning-Ontology#Trigger
:Trigger rdf:type owl:Class ;
         rdfs:comment "A mechanism that initiates an action when an event occurs such as reaching a certain time or date or upon receiving some type of input. A trigger generally causes a program routine to be executed." .


###  http://www.semanticweb.org/sc3/ontologies/2022/0/Planning-Ontology#Vertex
:Vertex rdf:type owl:Class .


###  http://www.semanticweb.org/sc3/ontologies/2022/0/Planning-Ontology#Yield
:Yield rdf:type owl:Class ;
       rdfs:comment "YIELD could be the fraction (percentage) of good dies resulting from total dies released." .


###  http://www.semanticweb.org/sc3/ontologies/2022/0/ozone-ontology#Demand
<http://www.semanticweb.org/sc3/ontologies/2022/0/ozone-ontology#Demand> rdf:type owl:Class .


###  http://www.semanticweb.org/sc3/ontologies/2022/0/ozone-ontology#Product
<http://www.semanticweb.org/sc3/ontologies/2022/0/ozone-ontology#Product> rdf:type owl:Class .


###  http://www.semanticweb.org/sc3/ontologies/2022/0/ozone-ontology#Resource
<http://www.semanticweb.org/sc3/ontologies/2022/0/ozone-ontology#Resource> rdf:type owl:Class .


###  http://www.w3.org/2006/time#DateTimeDescription
<http://www.w3.org/2006/time#DateTimeDescription> rdf:type owl:Class ;
                                                  rdfs:subClassOf <http://www.w3.org/2006/time#GeneralDateTimeDescription> ,
                                                                  [ rdf:type owl:Restriction ;
                                                                    owl:onProperty <http://www.w3.org/2006/time#hasTRS> ;
                                                                    owl:hasValue <http://www.opengis.net/def/uom/ISO-8601/0/Gregorian>
                                                                  ] ,
                                                                  [ rdf:type owl:Restriction ;
                                                                    owl:onProperty <http://www.w3.org/2006/time#day> ;
                                                                    owl:allValuesFrom xsd:gDay
                                                                  ] ,
                                                                  [ rdf:type owl:Restriction ;
                                                                    owl:onProperty <http://www.w3.org/2006/time#month> ;
                                                                    owl:allValuesFrom xsd:gMonth
                                                                  ] ,
                                                                  [ rdf:type owl:Restriction ;
                                                                    owl:onProperty <http://www.w3.org/2006/time#year> ;
                                                                    owl:allValuesFrom xsd:gYear
                                                                  ] ;
                                                  rdfs:comment "Descripción de fecha y tiempo estructurada con valores separados para los diferentes elementos de un sistema calendario-reloj. El sistema de referencia temporal está fijado al calendario gregoriano, y el rango de las propiedades año, mes, día restringidas a los correspondientes tipos del XML Schema xsd:gYear, xsd:gMonth y xsd:gDay respectivamente."@es ,
                                                               "Description of date and time structured with separate values for the various elements of a calendar-clock system. The temporal reference system is fixed to Gregorian Calendar, and the range of year, month, day properties restricted to corresponding XML Schema types xsd:gYear, xsd:gMonth and xsd:gDay, respectively."@en ;
                                                  rdfs:label "Date-Time description"@en ,
                                                             "descripción de fecha-tiempo"@es ;
                                                  <http://www.w3.org/2004/02/skos/core#definition> "Descripción de fecha y tiempo estructurada con valores separados para los diferentes elementos de un sistema calendario-reloj. El sistema de referencia temporal está fijado al calendario gregoriano, y el rango de las propiedades año, mes, día restringidas a los correspondientes tipos del XML Schema xsd:gYear, xsd:gMonth y xsd:gDay respectivamente."@es ,
                                                                                                   "Description of date and time structured with separate values for the various elements of a calendar-clock system. The temporal reference system is fixed to Gregorian Calendar, and the range of year, month, day properties restricted to corresponding XML Schema types xsd:gYear, xsd:gMonth and xsd:gDay, respectively."@en .


###  http://www.w3.org/2006/time#DateTimeInterval
<http://www.w3.org/2006/time#DateTimeInterval> rdf:type owl:Class ;
                                               rdfs:subClassOf <http://www.w3.org/2006/time#ProperInterval> ;
                                               rdfs:comment "'intervalo de fecha-hora' es una subclase de 'intervalo propio', definida utilizando el multi-elemento 'descripción de fecha-hora'."@es ,
                                                            "DateTimeInterval is a subclass of ProperInterval, defined using the multi-element DateTimeDescription."@en ;
                                               rdfs:label "Date-time interval"@en ,
                                                          "intervalo de fecha-hora"@es ;
                                               <http://www.w3.org/2004/02/skos/core#definition> "'intervalo de fecha-hora' es una subclase de 'intervalo propio', definida utilizando el multi-elemento 'descripción de fecha-hora'."@es ,
                                                                                                "DateTimeInterval is a subclass of ProperInterval, defined using the multi-element DateTimeDescription."@en ;
                                               <http://www.w3.org/2004/02/skos/core#note> "'intervalo de fecha-hora' se puede utilizar sólo para un intervalo cuyos límites coinciden con un elemento de fecha-hora alineados con el calendario y la zona horaria indicados. Por ejemplo, aunque ambos tienen una duración de un día, el intervalo de 24 horas que empieza en la media noche del comienzo del 8 mayo en Europa Central se puede expresar como un 'intervalo de fecha-hora', el intervalo de 24 horas que empieza a las 1:30pm no."@es ,
                                                                                          ":DateTimeInterval can only be used for an interval whose limits coincide with a date-time element aligned to the calendar and timezone indicated. For example, while both have a duration of one day, the 24-hour interval beginning at midnight at the beginning of 8 May in Central Europe can be expressed as a :DateTimeInterval, but the 24-hour interval starting at 1:30pm cannot."@en .


###  http://www.w3.org/2006/time#DayOfWeek
<http://www.w3.org/2006/time#DayOfWeek> rdf:type owl:Class ;
                                        rdfs:subClassOf owl:Thing ;
                                        rdfs:comment "El día de la semana"@es ,
                                                     "The day of week"@en ;
                                        rdfs:label "Day of week"@en ,
                                                   "día de la semana"@es ;
                                        <http://www.w3.org/2004/02/skos/core#changeNote> """Remove enumeration from definition, in order to allow other days to be used when required in other calendars. 
NOTE: existing days are still present as members of the class, but the class membership is now open. 

In the original OWL-Time the following constraint appeared: 
  owl:oneOf (
      time:Monday
      time:Tuesday
      time:Wednesday
      time:Thursday
      time:Friday
      time:Saturday
      time:Sunday
    ) ;"""@en ;
                                        <http://www.w3.org/2004/02/skos/core#definition> "El día de la semana"@es ,
                                                                                         "The day of week"@en ;
                                        <http://www.w3.org/2004/02/skos/core#note> "La pertenencia a la clase 'día de la semana' está abierta, para permitir longitudes de semana alternativas y diferentes nombres de días."@es ,
                                                                                   "Membership of the class :DayOfWeek is open, to allow for alternative week lengths and different day names."@en .


###  http://www.w3.org/2006/time#Duration
<http://www.w3.org/2006/time#Duration> rdf:type owl:Class ;
                                       rdfs:subClassOf <http://www.w3.org/2006/time#TemporalDuration> ,
                                                       [ rdf:type owl:Restriction ;
                                                         owl:onProperty <http://www.w3.org/2006/time#unitType> ;
                                                         owl:cardinality "1"^^xsd:nonNegativeInteger
                                                       ] ,
                                                       [ rdf:type owl:Restriction ;
                                                         owl:onProperty <http://www.w3.org/2006/time#numericDuration> ;
                                                         owl:cardinality "1"^^xsd:nonNegativeInteger
                                                       ] ;
                                       rdfs:comment "Duración de una extensión temporal expresada como un número escalado por una unidad temporal."@es ,
                                                    "Duration of a temporal extent expressed as a number scaled by a temporal unit"@en ;
                                       rdfs:label "Time duration"@en ,
                                                  "duración de tiempo" ;
                                       <http://www.w3.org/2004/02/skos/core#definition> "Duración de una extensión temporal expresada como un número escalado por una unidad temporal."@es ,
                                                                                        "Duration of a temporal extent expressed as a number scaled by a temporal unit"@en ;
                                       <http://www.w3.org/2004/02/skos/core#note> "Alternativa a 'descripción de tiempo' para proporcionar descripción soporte a una duración temporal diferente a utilizar un sistema de calendario/reloj."@es ,
                                                                                  "Alternative to time:DurationDescription to support description of a temporal duration other than using a calendar/clock system."@en .


###  http://www.w3.org/2006/time#DurationDescription
<http://www.w3.org/2006/time#DurationDescription> rdf:type owl:Class ;
                                                  rdfs:subClassOf <http://www.w3.org/2006/time#GeneralDurationDescription> ,
                                                                  [ rdf:type owl:Restriction ;
                                                                    owl:onProperty <http://www.w3.org/2006/time#hasTRS> ;
                                                                    owl:hasValue <http://www.opengis.net/def/uom/ISO-8601/0/Gregorian>
                                                                  ] ,
                                                                  [ rdf:type owl:Restriction ;
                                                                    owl:onProperty <http://www.w3.org/2006/time#days> ;
                                                                    owl:allValuesFrom xsd:decimal
                                                                  ] ,
                                                                  [ rdf:type owl:Restriction ;
                                                                    owl:onProperty <http://www.w3.org/2006/time#hours> ;
                                                                    owl:allValuesFrom xsd:decimal
                                                                  ] ,
                                                                  [ rdf:type owl:Restriction ;
                                                                    owl:onProperty <http://www.w3.org/2006/time#minutes> ;
                                                                    owl:allValuesFrom xsd:decimal
                                                                  ] ,
                                                                  [ rdf:type owl:Restriction ;
                                                                    owl:onProperty <http://www.w3.org/2006/time#months> ;
                                                                    owl:allValuesFrom xsd:decimal
                                                                  ] ,
                                                                  [ rdf:type owl:Restriction ;
                                                                    owl:onProperty <http://www.w3.org/2006/time#seconds> ;
                                                                    owl:allValuesFrom xsd:decimal
                                                                  ] ,
                                                                  [ rdf:type owl:Restriction ;
                                                                    owl:onProperty <http://www.w3.org/2006/time#weeks> ;
                                                                    owl:allValuesFrom xsd:decimal
                                                                  ] ,
                                                                  [ rdf:type owl:Restriction ;
                                                                    owl:onProperty <http://www.w3.org/2006/time#years> ;
                                                                    owl:allValuesFrom xsd:decimal
                                                                  ] ;
                                                  rdfs:comment "Descripción de extensión temporal estructurada con valores separados para los distintos elementos de un sistema de horario-calendario. El sistema de referencia temporal se fija al calendario gregoriano, y el intervalo de cada una de las propiedades numéricas se restringe a xsd:decimal."@es ,
                                                               "Description of temporal extent structured with separate values for the various elements of a calendar-clock system. The temporal reference system is fixed to Gregorian Calendar, and the range of each of the numeric properties is restricted to xsd:decimal"@en ;
                                                  rdfs:label "Duration description"@en ,
                                                             "descripción de duración"@es ;
                                                  <http://www.w3.org/2004/02/skos/core#definition> "Descripción de extensión temporal estructurada con valores separados para los distintos elementos de un sistema de horario-calendario. El sistema de referencia temporal se fija al calendario gregoriano, y el intervalo de cada una de las propiedades numéricas se restringe a xsd:decimal."@es ,
                                                                                                   "Description of temporal extent structured with separate values for the various elements of a calendar-clock system. The temporal reference system is fixed to Gregorian Calendar, and the range of each of the numeric properties is restricted to xsd:decimal"@en ;
                                                  <http://www.w3.org/2004/02/skos/core#note> "En el calendario gregoriano la longitud de los meses no es fija. Por lo tanto, un valor como \"2,5 meses\" no se puede comparar exactamente con una duración similar expresada en términos de semanas o días."@es ,
                                                                                             "In the Gregorian calendar the length of the month is not fixed. Therefore, a value like \"2.5 months\" cannot be exactly compared with a similar duration expressed in terms of weeks or days."@en .


###  http://www.w3.org/2006/time#GeneralDateTimeDescription
<http://www.w3.org/2006/time#GeneralDateTimeDescription> rdf:type owl:Class ;
                                                         rdfs:subClassOf <http://www.w3.org/2006/time#TemporalPosition> ,
                                                                         [ rdf:type owl:Restriction ;
                                                                           owl:onProperty <http://www.w3.org/2006/time#unitType> ;
                                                                           owl:cardinality "1"^^xsd:nonNegativeInteger
                                                                         ] ,
                                                                         [ rdf:type owl:Restriction ;
                                                                           owl:onProperty <http://www.w3.org/2006/time#dayOfWeek> ;
                                                                           owl:maxCardinality "1"^^xsd:nonNegativeInteger
                                                                         ] ,
                                                                         [ rdf:type owl:Restriction ;
                                                                           owl:onProperty <http://www.w3.org/2006/time#monthOfYear> ;
                                                                           owl:maxCardinality "1"^^xsd:nonNegativeInteger
                                                                         ] ,
                                                                         [ rdf:type owl:Restriction ;
                                                                           owl:onProperty <http://www.w3.org/2006/time#timeZone> ;
                                                                           owl:maxCardinality "1"^^xsd:nonNegativeInteger
                                                                         ] ,
                                                                         [ rdf:type owl:Restriction ;
                                                                           owl:onProperty <http://www.w3.org/2006/time#day> ;
                                                                           owl:maxCardinality "1"^^xsd:nonNegativeInteger
                                                                         ] ,
                                                                         [ rdf:type owl:Restriction ;
                                                                           owl:onProperty <http://www.w3.org/2006/time#dayOfYear> ;
                                                                           owl:maxCardinality "1"^^xsd:nonNegativeInteger
                                                                         ] ,
                                                                         [ rdf:type owl:Restriction ;
                                                                           owl:onProperty <http://www.w3.org/2006/time#hour> ;
                                                                           owl:maxCardinality "1"^^xsd:nonNegativeInteger
                                                                         ] ,
                                                                         [ rdf:type owl:Restriction ;
                                                                           owl:onProperty <http://www.w3.org/2006/time#minute> ;
                                                                           owl:maxCardinality "1"^^xsd:nonNegativeInteger
                                                                         ] ,
                                                                         [ rdf:type owl:Restriction ;
                                                                           owl:onProperty <http://www.w3.org/2006/time#month> ;
                                                                           owl:maxCardinality "1"^^xsd:nonNegativeInteger
                                                                         ] ,
                                                                         [ rdf:type owl:Restriction ;
                                                                           owl:onProperty <http://www.w3.org/2006/time#second> ;
                                                                           owl:maxCardinality "1"^^xsd:nonNegativeInteger
                                                                         ] ,
                                                                         [ rdf:type owl:Restriction ;
                                                                           owl:onProperty <http://www.w3.org/2006/time#week> ;
                                                                           owl:maxCardinality "1"^^xsd:nonNegativeInteger
                                                                         ] ,
                                                                         [ rdf:type owl:Restriction ;
                                                                           owl:onProperty <http://www.w3.org/2006/time#year> ;
                                                                           owl:maxCardinality "1"^^xsd:nonNegativeInteger
                                                                         ] ;
                                                         rdfs:comment "Descripción de fecha y hora estructurada con valores separados para los distintos elementos de un sistema calendario-reloj."@es ,
                                                                      "Description of date and time structured with separate values for the various elements of a calendar-clock system"@en ;
                                                         rdfs:label "Generalized date-time description"@en ,
                                                                    "descripción de fecha-hora generalizada"@es ;
                                                         <http://www.w3.org/2004/02/skos/core#definition> "Description of date and time structured with separate values for the various elements of a calendar-clock system"@en ,
                                                                                                          "Descripción de fecha y hora estructurada con valores separados para los distintos elementos de un sistema calendario-reloj." ;
                                                         <http://www.w3.org/2004/02/skos/core#note> "Algunas combinaciones de propiedades son redundantes - por ejemplo, dentro de un 'año' especificado si se proporciona 'día del año' entonces 'día' y 'mes' se pueden computar, y viceversa. Los valores individuales deberían ser consistentes entre ellos y con el calendario, indicado a través del valor de la propiedad 'tiene TRS'."@es ,
                                                                                                    "Some combinations of properties are redundant - for example, within a specified :year if :dayOfYear is provided then :day and :month can be computed, and vice versa. Individual values should be consistent with each other and the calendar, indicated through the value of the :hasTRS property." .


###  http://www.w3.org/2006/time#GeneralDurationDescription
<http://www.w3.org/2006/time#GeneralDurationDescription> rdf:type owl:Class ;
                                                         rdfs:subClassOf <http://www.w3.org/2006/time#TemporalDuration> ,
                                                                         [ rdf:type owl:Restriction ;
                                                                           owl:onProperty <http://www.w3.org/2006/time#hasTRS> ;
                                                                           owl:cardinality "1"^^xsd:nonNegativeInteger
                                                                         ] ,
                                                                         [ rdf:type owl:Restriction ;
                                                                           owl:onProperty <http://www.w3.org/2006/time#days> ;
                                                                           owl:maxCardinality "1"^^xsd:nonNegativeInteger
                                                                         ] ,
                                                                         [ rdf:type owl:Restriction ;
                                                                           owl:onProperty <http://www.w3.org/2006/time#hours> ;
                                                                           owl:maxCardinality "1"^^xsd:nonNegativeInteger
                                                                         ] ,
                                                                         [ rdf:type owl:Restriction ;
                                                                           owl:onProperty <http://www.w3.org/2006/time#minutes> ;
                                                                           owl:maxCardinality "1"^^xsd:nonNegativeInteger
                                                                         ] ,
                                                                         [ rdf:type owl:Restriction ;
                                                                           owl:onProperty <http://www.w3.org/2006/time#months> ;
                                                                           owl:maxCardinality "1"^^xsd:nonNegativeInteger
                                                                         ] ,
                                                                         [ rdf:type owl:Restriction ;
                                                                           owl:onProperty <http://www.w3.org/2006/time#seconds> ;
                                                                           owl:maxCardinality "1"^^xsd:nonNegativeInteger
                                                                         ] ,
                                                                         [ rdf:type owl:Restriction ;
                                                                           owl:onProperty <http://www.w3.org/2006/time#weeks> ;
                                                                           owl:maxCardinality "1"^^xsd:nonNegativeInteger
                                                                         ] ,
                                                                         [ rdf:type owl:Restriction ;
                                                                           owl:onProperty <http://www.w3.org/2006/time#years> ;
                                                                           owl:maxCardinality "1"^^xsd:nonNegativeInteger
                                                                         ] ;
                                                         rdfs:comment "Descripción de extensión temporal estructurada con valores separados para los distintos elementos de un sistema de horario-calendario."@es ,
                                                                      "Description of temporal extent structured with separate values for the various elements of a calendar-clock system."@en ;
                                                         rdfs:label "Generalized duration description"@en ,
                                                                    "descripción de duración generalizada"@es ;
                                                         <http://www.w3.org/2004/02/skos/core#definition> "Descripción de extensión temporal estructurada con valores separados para los distintos elementos de un sistema de horario-calendario."@es ,
                                                                                                          "Description of temporal extent structured with separate values for the various elements of a calendar-clock system."@en ;
                                                         <http://www.w3.org/2004/02/skos/core#note> "La extensión de una duración de tiempo expresada como una 'descripción de duración general' depende del Sistema de Referencia Temporal. En algunos calendarios la longitud de la semana o del mes no es constante a lo largo del año. Por tanto, un valor como \"25 meses\" puede no ser necesariamente ser comparado con un duración similar expresada en términos de semanas o días. Cuando se consideran calendarios que no están basados en el movimiento de la Tierra, se deben tomar incluso más precauciones en la comparación de duraciones."@es ,
                                                                                                    "The extent of a time duration expressed as a GeneralDurationDescription depends on the Temporal Reference System. In some calendars the length of the week or month is not constant within the year. Therefore, a value like \"2.5 months\" may not necessarily be exactly compared with a similar duration expressed in terms of weeks or days. When non-earth-based calendars are considered even more care must be taken in comparing durations."@en .


###  http://www.w3.org/2006/time#Instant
<http://www.w3.org/2006/time#Instant> rdf:type owl:Class ;
                                      rdfs:subClassOf <http://www.w3.org/2006/time#TemporalEntity> ;
                                      owl:disjointWith <http://www.w3.org/2006/time#ProperInterval> ;
                                      rdfs:comment "A temporal entity with zero extent or duration"@en ,
                                                   "Una entidad temporal con una extensión o duración cero."@es ;
                                      rdfs:label "Time instant"@en ,
                                                 "instante de tiempo."@es ;
                                      <http://www.w3.org/2004/02/skos/core#definition> "A temporal entity with zero extent or duration"@en ,
                                                                                       "Una entidad temporal con una extensión o duración cero."@es .


###  http://www.w3.org/2006/time#Interval
<http://www.w3.org/2006/time#Interval> rdf:type owl:Class ;
                                       rdfs:subClassOf <http://www.w3.org/2006/time#TemporalEntity> ;
                                       rdfs:comment "A temporal entity with an extent or duration"@en ,
                                                    "Una entidad temporal con una extensión o duración."@es ;
                                       rdfs:label "Time interval"@en ,
                                                  "intervalo de tiempo"@es ;
                                       <http://www.w3.org/2004/02/skos/core#definition> "A temporal entity with an extent or duration"@en ,
                                                                                        "Una entidad temporal con una extensión o duración."@es .


###  http://www.w3.org/2006/time#January
<http://www.w3.org/2006/time#January> rdf:type owl:Class ;
                                      rdfs:subClassOf <http://www.w3.org/2006/time#DateTimeDescription> ,
                                                      [ rdf:type owl:Restriction ;
                                                        owl:onProperty <http://www.w3.org/2006/time#unitType> ;
                                                        owl:hasValue <http://www.w3.org/2006/time#unitMonth>
                                                      ] ,
                                                      [ rdf:type owl:Restriction ;
                                                        owl:onProperty <http://www.w3.org/2006/time#month> ;
                                                        owl:hasValue "--01"
                                                      ] ;
                                      rdfs:label "January" ;
                                      owl:deprecated "true"^^xsd:boolean ;
                                      <http://www.w3.org/2004/02/skos/core#historyNote> "This class was present in the 2006 version of OWL-Time. It was presented as an example of how DateTimeDescription could be specialized, but does not belong in the revised ontology. " .


###  http://www.w3.org/2006/time#MonthOfYear
<http://www.w3.org/2006/time#MonthOfYear> rdf:type owl:Class ;
                                          rdfs:subClassOf <http://www.w3.org/2006/time#DateTimeDescription> ,
                                                          [ rdf:type owl:Restriction ;
                                                            owl:onProperty <http://www.w3.org/2006/time#unitType> ;
                                                            owl:hasValue <http://www.w3.org/2006/time#unitMonth>
                                                          ] ,
                                                          [ rdf:type owl:Restriction ;
                                                            owl:onProperty <http://www.w3.org/2006/time#day> ;
                                                            owl:cardinality "0"^^xsd:nonNegativeInteger
                                                          ] ,
                                                          [ rdf:type owl:Restriction ;
                                                            owl:onProperty <http://www.w3.org/2006/time#hour> ;
                                                            owl:cardinality "0"^^xsd:nonNegativeInteger
                                                          ] ,
                                                          [ rdf:type owl:Restriction ;
                                                            owl:onProperty <http://www.w3.org/2006/time#minute> ;
                                                            owl:cardinality "0"^^xsd:nonNegativeInteger
                                                          ] ,
                                                          [ rdf:type owl:Restriction ;
                                                            owl:onProperty <http://www.w3.org/2006/time#month> ;
                                                            owl:cardinality "1"^^xsd:nonNegativeInteger
                                                          ] ,
                                                          [ rdf:type owl:Restriction ;
                                                            owl:onProperty <http://www.w3.org/2006/time#second> ;
                                                            owl:cardinality "0"^^xsd:nonNegativeInteger
                                                          ] ,
                                                          [ rdf:type owl:Restriction ;
                                                            owl:onProperty <http://www.w3.org/2006/time#week> ;
                                                            owl:cardinality "0"^^xsd:nonNegativeInteger
                                                          ] ,
                                                          [ rdf:type owl:Restriction ;
                                                            owl:onProperty <http://www.w3.org/2006/time#year> ;
                                                            owl:cardinality "0"^^xsd:nonNegativeInteger
                                                          ] ;
                                          rdfs:comment "El mes del año."@es ,
                                                       "The month of the year"@en ;
                                          rdfs:label "Month of year"@en ,
                                                     "mes del año"@es ;
                                          <http://www.w3.org/2004/02/skos/core#definition> "El mes del año."@es ,
                                                                                           "The month of the year"@en ;
                                          <http://www.w3.org/2004/02/skos/core#editorialNote> "Característica en riesgo - añadida en la revisión de 2017, y no utilizada todavía de forma amplia."@es ,
                                                                                              "Feature at risk - added in 2017 revision, and not yet widely used. "@en ;
                                          <http://www.w3.org/2004/02/skos/core#note> "La pertenencia a la clase 'mes del año' está abierta, a permitir calendarios anuales alternativos y diferentes nombres de meses."@es ,
                                                                                     "Membership of the class :MonthOfYear is open, to allow for alternative annual calendars and different month names."@en .


###  http://www.w3.org/2006/time#ProperInterval
<http://www.w3.org/2006/time#ProperInterval> rdf:type owl:Class ;
                                             rdfs:subClassOf <http://www.w3.org/2006/time#Interval> ;
                                             rdfs:comment "A temporal entity with non-zero extent or duration, i.e. for which the value of the beginning and end are different"@en ,
                                                          "Una entidad temporal con extensión o duración distinta de cero, es decir, para la cual los valores de principio y fin del intervalo son diferentes."@es ;
                                             rdfs:label "Proper interval"@en ,
                                                        "intervalo propio"@es ;
                                             <http://www.w3.org/2004/02/skos/core#definition> "A temporal entity with non-zero extent or duration, i.e. for which the value of the beginning and end are different"@en ,
                                                                                              "Una entidad temporal con extensión o duración distinta de cero, es decir, para la cual los valores de principio y fin del intervalo son diferentes."@es .


###  http://www.w3.org/2006/time#TRS
<http://www.w3.org/2006/time#TRS> rdf:type owl:Class ;
                                  rdfs:comment """A temporal reference system, such as a temporal coordinate system (with an origin, direction, and scale), a calendar-clock combination, or a (possibly hierarchical) ordinal system. 

This is a stub class, representing the set of all temporal reference systems."""@en ,
                                               """Un sistema de referencia temporal, tal como un sistema de coordenadas temporales (con un origen, una dirección y una escala), una combinación calendario-reloj, o un sistema ordinal (posiblemente jerárquico).
        Esta clase comodín representa el conjunto de todos los sistemas de referencia temporal."""@es ;
                                  rdfs:label "Temporal Reference System"@en ,
                                             "sistema de referencia temporal"@es ;
                                  <http://www.w3.org/2004/02/skos/core#definition> """A temporal reference system, such as a temporal coordinate system (with an origin, direction, and scale), a calendar-clock combination, or a (possibly hierarchical) ordinal system. 

This is a stub class, representing the set of all temporal reference systems."""@en ,
                                                                                   """Un sistema de referencia temporal, tal como un sistema de coordenadas temporales (con un origen, una dirección y una escala), una combinación calendario-reloj, o un sistema ordinal (posiblemente jerárquico).
    Esta clase comodín representa el conjunto de todos los sistemas de referencia temporal."""@es ;
                                  <http://www.w3.org/2004/02/skos/core#note> "A taxonomy of temporal reference systems is provided in ISO 19108:2002 [ISO19108], including (a) calendar + clock systems; (b) temporal coordinate systems (i.e. numeric offset from an epoch); (c) temporal ordinal reference systems (i.e. ordered sequence of named intervals, not necessarily of equal duration)."@en ,
                                                                             "En el ISO 19108:2002 [ISO19108] se proporciona una taxonomía de sistemas de referencia temporal, incluyendo (a) sistemas de calendario + reloj; (b) sistemas de coordenadas temporales (es decir, desplazamiento numérico a partir de una época); (c) sistemas de referencia ordinales temporales (es decir, secuencia ordenada de intervalos nombrados, no necesariamente de igual duración)."@es .


###  http://www.w3.org/2006/time#TemporalDuration
<http://www.w3.org/2006/time#TemporalDuration> rdf:type owl:Class ;
                                               rdfs:comment "Extensión de tiempo; duración de un intervalo de tiempo independiente de su posición de inicio particular."@es ,
                                                            "Time extent; duration of a time interval separate from its particular start position"@en ;
                                               rdfs:label "Temporal duration"@en ,
                                                          "duración temporal"@es ;
                                               <http://www.w3.org/2004/02/skos/core#definition> "Extensión de tiempo; duración de un intervalo de tiempo independiente de su posición de inicio particular."@es ,
                                                                                                "Time extent; duration of a time interval separate from its particular start position"@en .


###  http://www.w3.org/2006/time#TemporalEntity
<http://www.w3.org/2006/time#TemporalEntity> rdf:type owl:Class ;
                                             owl:equivalentClass [ rdf:type owl:Class ;
                                                                   owl:unionOf ( <http://www.w3.org/2006/time#Instant>
                                                                                 <http://www.w3.org/2006/time#Interval>
                                                                               )
                                                                 ] ;
                                             rdfs:subClassOf owl:Thing ;
                                             rdfs:comment "A temporal interval or instant."@en ,
                                                          "Un intervalo temporal o un instante."@es ;
                                             rdfs:label "Temporal entity"@en ,
                                                        "entidad temporal"@es ;
                                             <http://www.w3.org/2004/02/skos/core#definition> "A temporal interval or instant."@en ,
                                                                                              "Un intervalo temporal o un instante."@es .


###  http://www.w3.org/2006/time#TemporalPosition
<http://www.w3.org/2006/time#TemporalPosition> rdf:type owl:Class ;
                                               rdfs:subClassOf [ rdf:type owl:Restriction ;
                                                                 owl:onProperty <http://www.w3.org/2006/time#hasTRS> ;
                                                                 owl:cardinality "1"^^xsd:nonNegativeInteger
                                                               ] ;
                                               rdfs:comment "A position on a time-line"@en ,
                                                            "Una posición sobre una línea de tiempo."@es ;
                                               rdfs:label "Temporal position"@en ,
                                                          "posición temporal"@es ;
                                               <http://www.w3.org/2004/02/skos/core#definition> "A position on a time-line"@en ,
                                                                                                "Una posición sobre una línea de tiempo."@es .


###  http://www.w3.org/2006/time#TemporalUnit
<http://www.w3.org/2006/time#TemporalUnit> rdf:type owl:Class ;
                                           rdfs:subClassOf <http://www.w3.org/2006/time#TemporalDuration> ;
                                           rdfs:comment "A standard duration, which provides a scale factor for a time extent, or the granularity or precision for a time position."@en ,
                                                        "Una duración estándar, que proporciona un factor de escala para una extensión de tiempo, o la granularidad o precisión para una posición de tiempo."@es ;
                                           rdfs:label "Temporal unit"@en ,
                                                      "unidad de tiempo"@es ;
                                           <http://www.w3.org/2004/02/skos/core#changeNote> """Remove enumeration from definition, in order to allow other units to be used when required in other coordinate systems. 
NOTE: existing units are still present as members of the class, but the class membership is now open. 

In the original OWL-Time the following constraint appeared: 
  owl:oneOf (
      time:unitSecond
      time:unitMinute
      time:unitHour
      time:unitDay
      time:unitWeek
      time:unitMonth
      time:unitYear
    ) ;"""@en ;
                                           <http://www.w3.org/2004/02/skos/core#definition> "A standard duration, which provides a scale factor for a time extent, or the granularity or precision for a time position."@en ,
                                                                                            "Una duración estándar, que proporciona un factor de escala para una extensión de tiempo, o la granularidad o precisión para una posición de tiempo."@es ;
                                           <http://www.w3.org/2004/02/skos/core#note> "La pertenencia de la clase 'unidad de tiempo' está abierta, para permitir otras unidades de tiempo utilizadas en algunas aplicaciones técnicas (por ejemplo, millones de años o el mes Baha'i)."@es ,
                                                                                      "Membership of the class TemporalUnit is open, to allow for other temporal units used in some technical applications (e.g. millions of years, Baha'i month)."@en .


###  http://www.w3.org/2006/time#TimePosition
<http://www.w3.org/2006/time#TimePosition> rdf:type owl:Class ;
                                           rdfs:subClassOf <http://www.w3.org/2006/time#TemporalPosition> ,
                                                           [ rdf:type owl:Class ;
                                                             owl:unionOf ( [ rdf:type owl:Restriction ;
                                                                             owl:onProperty <http://www.w3.org/2006/time#nominalPosition> ;
                                                                             owl:cardinality "1"^^xsd:nonNegativeInteger
                                                                           ]
                                                                           [ rdf:type owl:Restriction ;
                                                                             owl:onProperty <http://www.w3.org/2006/time#numericPosition> ;
                                                                             owl:cardinality "1"^^xsd:nonNegativeInteger
                                                                           ]
                                                                         )
                                                           ] ;
                                           rdfs:comment "A temporal position described using either a (nominal) value from an ordinal reference system, or a (numeric) value in a temporal coordinate system. "@en ,
                                                        "Una posición temporal descrita utilizando bien un valor (nominal) de un sistema de referencia ordinal, o un valor (numérico) en un sistema de coordenadas temporales."@es ;
                                           rdfs:label "Time position"@en ,
                                                      "posición de tiempo"@es ;
                                           <http://www.w3.org/2004/02/skos/core#definition> "A temporal position described using either a (nominal) value from an ordinal reference system, or a (numeric) value in a temporal coordinate system. "@en ,
                                                                                            "Una posición temporal descrita utilizando bien un valor (nominal) de un sistema de referencia ordinal, o un valor (numérico) en un sistema de coordenadas temporales."@es .


###  http://www.w3.org/2006/time#TimeZone
<http://www.w3.org/2006/time#TimeZone> rdf:type owl:Class ;
                                       rdfs:comment """A Time Zone specifies the amount by which the local time is offset from UTC. 
	A time zone is usually denoted geographically (e.g. Australian Eastern Daylight Time), with a constant value in a given region. 
The region where it applies and the offset from UTC are specified by a locally recognised governing authority."""@en ,
                                                    """Un huso horario especifica la cantidad en que la hora local está desplazada con respecto a UTC.
        Un huso horario normalmente se denota geográficamente (p.ej. el horario de verano del este de Australia), con un valor constante en una región dada.
        La región donde aplica y el desplazamiento desde UTC las especifica una autoridad gubernamental localmente reconocida."""@es ;
                                       rdfs:label "Time Zone"@en ,
                                                  "huso horario"@es ;
                                       <http://www.w3.org/2004/02/skos/core#definition> """A Time Zone specifies the amount by which the local time is offset from UTC. 
	A time zone is usually denoted geographically (e.g. Australian Eastern Daylight Time), with a constant value in a given region. 
The region where it applies and the offset from UTC are specified by a locally recognised governing authority."""@en ,
                                                                                        """Un huso horario especifica la cantidad en que la hora local está desplazada con respecto a UTC.
    Un huso horario normalmente se denota geográficamente (p.ej. el horario de verano del este de Australia), con un valor constante en una región dada.
    La región donde aplica y el desplazamiento desde UTC las especifica una autoridad gubernamental localmente reconocida."""@es ;
                                       <http://www.w3.org/2004/02/skos/core#historyNote> """En la versión original de OWL-Time de 2006, se definió, en un espacio de nombres diferente \"http://www.w3.org/2006/timezone#\", la clase 'huso horario', con varias propiedades específicas correspondientes a un modelo específico de huso horario.
    En la versión actual hay una clase con el mismo nombre local en el espacio de nombres de OWL-Time, eliminando la dependencia del espacio de nombres externo.
    Un axioma de alineación permite que los datos codificados de acuerdo con la versión anterior sean consistentes con la ontología actualizada."""@es ,
                                                                                         """In the original 2006 version of OWL-Time, the TimeZone class, with several properties corresponding to a specific model of time-zones, was defined in a separate namespace \"http://www.w3.org/2006/timezone#\". 

In the current version a class with same local name is put into the main OWL-Time namespace, removing the dependency on the external namespace. 

An alignment axiom 
	tzont:TimeZone rdfs:subClassOf time:TimeZone . 
allows data encoded according to the previous version to be consistent with the updated ontology. """ ;
                                       <http://www.w3.org/2004/02/skos/core#note> """A designated timezone is associated with a geographic region. However, for a particular region the offset from UTC often varies seasonally, and the dates of the changes may vary from year to year. The timezone designation usually changes for the different seasons (e.g. Australian Eastern Standard Time vs. Australian Eastern Daylight Time). Furthermore, the offset for a timezone may change over longer timescales, though its designation might not.  

Detailed guidance about working with time zones is given in http://www.w3.org/TR/timezone/ ."""@en ,
                                                                                  "An ontology for time zone descriptions was described in [owl-time-20060927] and provided as RDF in a separate namespace tzont:. However, that ontology was incomplete in scope, and the example datasets were selective. Furthermore, since the use of a class from an external ontology as the range of an ObjectProperty in OWL-Time creates a dependency, reference to the time zone class has been replaced with the 'stub' class in the normative part of this version of OWL-Time."@en ,
                                                                                  """Un huso horario designado está asociado con una región geográfica. Sin embargo, para una región particular el desplazamiento desde UTC a menudo varía según las estaciones, y las fechas de los cambios pueden variar de un año a otro. La designación de huso horario  normalmente cambia de una estación a otra (por ejemplo, el horario estándar frente al horario de verano ambos del este de Australia). Además, del desplazamiento para un huso horario puede cambiar sobre escalas de tiempo mayores, aunque su designación no lo haga.
    Se puede encontrar una guía detallada sobre el funcionamiento de husos horarios en http://www.w3.org/TR/timezone/.\"@es , \"En [owl-time-20060927] se describió una ontología para descripciones de husos horarios, y se proporcionó en un espacio de nombres separado tzont:. Sin embargo, dicha ontología estaba incompleta en su alcance, y el ejemplo de conjuntos de datos (datasets) era selectivo. Además, puesto que el uso de una clase de una ontología externa como el rango de una propiedad de objeto en OWL-Time crea una dependencia, la referencia a la clase huso horario se ha reemplazado por una clase que viene a ser un \"cajón de sastre\" en la en la parte normativa de esta versión de OWL-Time."""@es ;
                                       <http://www.w3.org/2004/02/skos/core#scopeNote> "En esta implementación 'huso horario' no tiene definidas propiedades. Se debería pensar como una superclase \"abstracta\" de todas las implementaciones de huso horario específicas."@es ,
                                                                                       "In this implementation TimeZone has no properties defined. It should be thought of as an 'abstract' superclass of all specific timezone implementations." .


###  http://www.w3.org/2006/time#Year
<http://www.w3.org/2006/time#Year> rdf:type owl:Class ;
                                   rdfs:subClassOf <http://www.w3.org/2006/time#DurationDescription> ,
                                                   [ rdf:type owl:Restriction ;
                                                     owl:onProperty <http://www.w3.org/2006/time#days> ;
                                                     owl:cardinality "0"^^xsd:nonNegativeInteger
                                                   ] ,
                                                   [ rdf:type owl:Restriction ;
                                                     owl:onProperty <http://www.w3.org/2006/time#hours> ;
                                                     owl:cardinality "0"^^xsd:nonNegativeInteger
                                                   ] ,
                                                   [ rdf:type owl:Restriction ;
                                                     owl:onProperty <http://www.w3.org/2006/time#minutes> ;
                                                     owl:cardinality "0"^^xsd:nonNegativeInteger
                                                   ] ,
                                                   [ rdf:type owl:Restriction ;
                                                     owl:onProperty <http://www.w3.org/2006/time#months> ;
                                                     owl:cardinality "0"^^xsd:nonNegativeInteger
                                                   ] ,
                                                   [ rdf:type owl:Restriction ;
                                                     owl:onProperty <http://www.w3.org/2006/time#seconds> ;
                                                     owl:cardinality "0"^^xsd:nonNegativeInteger
                                                   ] ,
                                                   [ rdf:type owl:Restriction ;
                                                     owl:onProperty <http://www.w3.org/2006/time#weeks> ;
                                                     owl:cardinality "0"^^xsd:nonNegativeInteger
                                                   ] ,
                                                   [ rdf:type owl:Restriction ;
                                                     owl:onProperty <http://www.w3.org/2006/time#years> ;
                                                     owl:cardinality "1"^^xsd:nonNegativeInteger
                                                   ] ;
                                   rdfs:comment "Year duration" ;
                                   rdfs:label "Year"@en ;
                                   owl:deprecated "true"^^xsd:boolean ;
                                   <http://www.w3.org/2004/02/skos/core#definition> "Year duration" ;
                                   <http://www.w3.org/2004/02/skos/core#historyNote> """Year was proposed in the 2006 version of OWL-Time as an example of how DurationDescription could be specialized to allow for a duration to be restricted to a number of years. 

It is deprecated in this edition of OWL-Time. """ ;
                                   <http://www.w3.org/2004/02/skos/core#prefLabel> "Anno"@it ,
                                                                                   "Année (calendrier)"@fr ,
                                                                                   "Ano"@pt ,
                                                                                   "Año"@es ,
                                                                                   "Jaar"@nl ,
                                                                                   "Jahr"@de ,
                                                                                   "Rok"@pl ,
                                                                                   "Year"@en ,
                                                                                   "Год"@ru ,
                                                                                   "سنة"@ar ,
                                                                                   "年"@ja ,
                                                                                   "年"@zh .


#################################################################
#    Individuals
#################################################################

###  http://www.semanticweb.org/sc3/ontologies/2022/0/Planning-Ontology#Activity_Etching
:Activity_Etching rdf:type owl:NamedIndividual ,
                           :Activity ;
                  :hasCapacity :RequiredCap1 ;
                  :hasResources :FE_Aligner .


###  http://www.semanticweb.org/sc3/ontologies/2022/0/Planning-Ontology#Activity_Oxide
:Activity_Oxide rdf:type owl:NamedIndividual ,
                         :Activity ;
                :hasCapacity :RequiredCap2 ;
                :hasResources :FE_Implanter .


###  http://www.semanticweb.org/sc3/ontologies/2022/0/Planning-Ontology#Activity_Photo
:Activity_Photo rdf:type owl:NamedIndividual ,
                         :Activity ;
                :hasCapacity :RequiredCap3 ;
                :hasResources :FE_Stepper_1 .


###  http://www.semanticweb.org/sc3/ontologies/2022/0/Planning-Ontology#Activity_UV_Bake
:Activity_UV_Bake rdf:type owl:NamedIndividual ,
                           :Activity ;
                  :hasCapacity :RequiredCap4 ;
                  :hasResources :FE_Stepper_2 .


###  http://www.semanticweb.org/sc3/ontologies/2022/0/Planning-Ontology#All_Planning_Objects_have_to_be_positive
:All_Planning_Objects_have_to_be_positive rdf:type owl:NamedIndividual ,
                                                   :PlanningConstraint ;
                                          :sc3:formula """forall($g in Products, $t in PlanningHorizon, $j in Frontends) -> FE_Y($j, $g, $t) >= 0;
forall($g in Products, $t in PlanningHorizon, $j in Frontends) -> FE_X($j, $g, $t) >= 0;
forall($g in Products, $t in PlanningHorizon, $j in Frontends) -> FE_Wip($j, $g, $t) >= 0;
forall($g in Products, $t in PlanningHorizon) -> FE_Inventory($g, $t) >= 0;
forall($g in Products, $t in PlanningHorizon) -> FE_Backlog($g, $t) >= 0;""" .


###  http://www.semanticweb.org/sc3/ontologies/2022/0/Planning-Ontology#AvailableCap1
:AvailableCap1 rdf:type owl:NamedIndividual ,
                        :AvailableCapacity .


###  http://www.semanticweb.org/sc3/ontologies/2022/0/Planning-Ontology#AvailableCap2
:AvailableCap2 rdf:type owl:NamedIndividual ,
                        :AvailableCapacity .


###  http://www.semanticweb.org/sc3/ontologies/2022/0/Planning-Ontology#AvailableCap3
:AvailableCap3 rdf:type owl:NamedIndividual ,
                        :AvailableCapacity .


###  http://www.semanticweb.org/sc3/ontologies/2022/0/Planning-Ontology#AvailableCap4
:AvailableCap4 rdf:type owl:NamedIndividual ,
                        :AvailableCapacity .


###  http://www.semanticweb.org/sc3/ontologies/2022/0/Planning-Ontology#AvailableCap5
:AvailableCap5 rdf:type owl:NamedIndividual ,
                        :AvailableCapacity .


###  http://www.semanticweb.org/sc3/ontologies/2022/0/Planning-Ontology#Bom_Product_1
:Bom_Product_1 rdf:type owl:NamedIndividual ,
                        :BillOfMaterial ;
               :hasLocation :Frontend_1 ;
               :hasProduct :Product_1 .


###  http://www.semanticweb.org/sc3/ontologies/2022/0/Planning-Ontology#Borderless_FE1_zu_FE2
:Borderless_FE1_zu_FE2 rdf:type owl:NamedIndividual ,
                                :PlanningObject ;
                       :hasActivities :Activity_Photo ;
                       :hasLocation :Frontend_2 ;
                       :hasOwner :FE1 ;
                       :hasProduct :Product_1 ;
                       :hasDueDate "1 week" ;
                       :hasQuantity 10 .


###  http://www.semanticweb.org/sc3/ontologies/2022/0/Planning-Ontology#Capacity_Restriction_Equation
:Capacity_Restriction_Equation rdf:type owl:NamedIndividual ,
                                        :PlanningConstraint ;
                               :sc3:formula """forall($k in WorkCenters, $j in Frontends, t in PlanningHorizon) sum($g in Products, $l in OperationCountOnWorkCenter($j, $k, $g) ->
		FE_Y($j, $g, $t, OperationsOnWorkCenter($j, $k, $g, $l)) * alpha($j, $g, OperationsOnWorkCenter($j, $k, $g, $l)) <= WorkCenterCapacity($t, $j, $k);
	

WorkCenters (Resources)=FE_Aligner, FE_Stepper_2, FE_Stepper_1, FE_Implanter
Frontends= Frontend_1, Frontend_2;
Products= Product_1;
OperationCountOnWorkCenter=Product($numberOfOperationsOnSameResource);
alpha= Activity($hasRequiredCapacity(Product($hasActivities)));
WorkCenterCapacity= FE_Aligner($hasAvailableCapacity, $hasLocation), FE_Stepper_2($hasAvailableCapacity, $hasLocation), FE_Stepper_1($hasAvailableCapacity, $hasLocation), FE_Implanter($hasAvailableCapacity, $hasLocation);""" .


###  http://www.semanticweb.org/sc3/ontologies/2022/0/Planning-Ontology#FE1
:FE1 rdf:type owl:NamedIndividual ,
              :Owner .


###  http://www.semanticweb.org/sc3/ontologies/2022/0/Planning-Ontology#FE1_CostMinimization
:FE1_CostMinimization rdf:type owl:NamedIndividual ,
                               :PlaningPurpose ;
                      :hasCriterias :Minimization ;
                      :hasPerformanceMeasures :MinimizeBacklog ,
                                              :MinimizeInventoryLevel ,
                                              :MinimizeWipCosts ;
                      :hasPlanningObjects :FE_Backlog ,
                                          :FE_Inventory ,
                                          :FE_Wip ,
                                          :FE_X ,
                                          :FE_Y ;
                      :hasCosts "backlog=150" ,
                                "inventory=15" ,
                                "wip=50" ;
                      :hasPlanningWindow "12 weeks" ;
                      :sc3:formula """sum($g in Products, $t in PlanningHorizon)--> sum($j in Frontends) (WipCosts($g, $t) * FE_Wip($j, $g, $t)) + InventoryCosts($g, $t) * FE_Inventory($g, $t) + BacklogCosts($g, $t) * FE_Backlog($g, $t);

Frontends= Frontend_1, Frontend_2;
Products= Product_1;
InventoryCosts= $(hasCosts($inventory));
BacklogCosts= $(hasCosts($backlog));
WipCosts= $(hasCosts($wip));""" .


###  http://www.semanticweb.org/sc3/ontologies/2022/0/Planning-Ontology#FE2
:FE2 rdf:type owl:NamedIndividual ,
              :Owner .


###  http://www.semanticweb.org/sc3/ontologies/2022/0/Planning-Ontology#FE_Aligner
:FE_Aligner rdf:type owl:NamedIndividual ,
                     <http://www.semanticweb.org/sc3/ontologies/2022/0/ozone-ontology#Resource> ;
            :hasCapacity :AvailableCap1 ;
            :hasLocation :Frontend_1 .


###  http://www.semanticweb.org/sc3/ontologies/2022/0/Planning-Ontology#FE_Backlog
:FE_Backlog rdf:type owl:NamedIndividual ,
                     :PlanningObject ;
            :hasLocation :Frontend_1 ,
                         :Frontend_2 ;
            :hasProduct :Product_1 ;
            :hasPeriod "" ;
            <http://www.w3.org/2006/time#day> "" .


###  http://www.semanticweb.org/sc3/ontologies/2022/0/Planning-Ontology#FE_Implanter
:FE_Implanter rdf:type owl:NamedIndividual ,
                       <http://www.semanticweb.org/sc3/ontologies/2022/0/ozone-ontology#Resource> ;
              :hasCapacity :AvailableCap2 ;
              :hasLocation :Frontend_1 .


###  http://www.semanticweb.org/sc3/ontologies/2022/0/Planning-Ontology#FE_Inventory
:FE_Inventory rdf:type owl:NamedIndividual ,
                       :PlanningObject ;
              :hasLocation :Frontend_1 ,
                           :Frontend_2 ;
              :hasProduct :Product_1 ,
                          :Product_2 ;
              :hasPeriod "" ;
              <http://www.w3.org/2006/time#day> "" .


###  http://www.semanticweb.org/sc3/ontologies/2022/0/Planning-Ontology#FE_Stepper_1
:FE_Stepper_1 rdf:type owl:NamedIndividual ,
                       <http://www.semanticweb.org/sc3/ontologies/2022/0/ozone-ontology#Resource> ;
              :hasCapacity :AvailableCap3 ;
              :hasLocation :Frontend_1 .


###  http://www.semanticweb.org/sc3/ontologies/2022/0/Planning-Ontology#FE_Stepper_2
:FE_Stepper_2 rdf:type owl:NamedIndividual ,
                       <http://www.semanticweb.org/sc3/ontologies/2022/0/ozone-ontology#Resource> ;
              :hasCapacity :AvailableCap4 ;
              :hasLocation :Frontend_1 .


###  http://www.semanticweb.org/sc3/ontologies/2022/0/Planning-Ontology#FE_Wip
:FE_Wip rdf:type owl:NamedIndividual ,
                 :PlanningObject ;
        :hasLocation :Frontend_1 ,
                     :Frontend_2 ;
        :hasProduct :Product_1 ,
                    :Product_2 ;
        :hasPeriod "" ;
        <http://www.w3.org/2006/time#day> "" .


###  http://www.semanticweb.org/sc3/ontologies/2022/0/Planning-Ontology#FE_X
:FE_X rdf:type owl:NamedIndividual ,
               :PlanningObject ;
      :hasLocation :Frontend_1 ,
                   :Frontend_2 ;
      :hasProduct :Product_1 ,
                  :Product_2 ;
      :hasPeriod "" ;
      <http://www.w3.org/2006/time#day> "" .


###  http://www.semanticweb.org/sc3/ontologies/2022/0/Planning-Ontology#FE_Y
:FE_Y rdf:type owl:NamedIndividual ,
               :PlanningObject ;
      :hasLocation :Frontend_1 ,
                   :Frontend_2 ;
      :hasProduct :Product_1 ,
                  :Product_2 ;
      :hasPeriod "" ;
      <http://www.w3.org/2006/time#day> "" .


###  http://www.semanticweb.org/sc3/ontologies/2022/0/Planning-Ontology#Frontend_1
:Frontend_1 rdf:type owl:NamedIndividual ,
                     :Location ;
            :hasProduct :Product_1 .


###  http://www.semanticweb.org/sc3/ontologies/2022/0/Planning-Ontology#Frontend_2
:Frontend_2 rdf:type owl:NamedIndividual ,
                     :Location ;
            :hasLocation :Frontend_1 ;
            :hasProduct :Product_1 .


###  http://www.semanticweb.org/sc3/ontologies/2022/0/Planning-Ontology#Inventory_Balance_Equation
:Inventory_Balance_Equation rdf:type owl:NamedIndividual ,
                                     :PlanningConstraint ;
                            :sc3:formula """forall($g in Products, $t in PlanningHorizon) -> FE_Inventory($p, $t) = FE_Inventory($g, $t-1) + sum(j in Frontends)(FE_Y($j,$g,$t) - FE_Backlog($g, $t-1) + FE_Backlog($g, $t) + sum(j in Frontends)(Inventory_DB($j, $g, $t) - Demand($g, $t);

Frontends= Frontend_1, Frontend_2;
Products= Product_1;""" .


###  http://www.semanticweb.org/sc3/ontologies/2022/0/Planning-Ontology#Inventory_DB
:Inventory_DB rdf:type owl:NamedIndividual ,
                       :Inventory ;
              :hasLocation :Frontend_1 ,
                           :Frontend_2 ;
              :hasProduct :Product_1 ,
                          :Product_2 ;
              :hasPeriod "" ;
              <http://www.w3.org/2006/time#day> "" .


###  http://www.semanticweb.org/sc3/ontologies/2022/0/Planning-Ontology#Material_Flow_Equation
:Material_Flow_Equation rdf:type owl:NamedIndividual ,
                                 :PlanningConstraint ;
                        :sc3:formula """forall($g in Products, $j in Frontends, $t in PlanningHorizon, $l in Steps($j, $g) -> FE_Y($j, $g, $t, $l) = FE_X($j, $g, $t - LeadTime($g, $l));
			

Frontends= Frontend_1, Frontend_2;
Products= Product_1;
Steps= Product($hasActivities);
LeadTime= Product($hasLeadTime);""" .


###  http://www.semanticweb.org/sc3/ontologies/2022/0/Planning-Ontology#Minimization
:Minimization rdf:type owl:NamedIndividual ,
                       :Criteria .


###  http://www.semanticweb.org/sc3/ontologies/2022/0/Planning-Ontology#MinimizeBacklog
:MinimizeBacklog rdf:type owl:NamedIndividual .


###  http://www.semanticweb.org/sc3/ontologies/2022/0/Planning-Ontology#MinimizeInventoryLevel
:MinimizeInventoryLevel rdf:type owl:NamedIndividual .


###  http://www.semanticweb.org/sc3/ontologies/2022/0/Planning-Ontology#MinimizeWipCosts
:MinimizeWipCosts rdf:type owl:NamedIndividual .


###  http://www.semanticweb.org/sc3/ontologies/2022/0/Planning-Ontology#Part1_Product_1
:Part1_Product_1 rdf:type owl:NamedIndividual ,
                          :Part ;
                 :hasPlanningObject :Borderless_FE1_zu_FE2 ;
                 :hasProduct :Product_1 ;
                 :hasDueDate "1 week" .


###  http://www.semanticweb.org/sc3/ontologies/2022/0/Planning-Ontology#Part2_Product_1
:Part2_Product_1 rdf:type owl:NamedIndividual ,
                          :Part ;
                 :hasPlanningObject :Borderless_FE1_zu_FE2 ;
                 :hasProduct :Product_1 ;
                 :hasDueDate "1 week" .


###  http://www.semanticweb.org/sc3/ontologies/2022/0/Planning-Ontology#Part3_Product_1
:Part3_Product_1 rdf:type owl:NamedIndividual ,
                          :Part ;
                 :hasProduct :Product_1 ;
                 :hasDueDate "3 weeks" .


###  http://www.semanticweb.org/sc3/ontologies/2022/0/Planning-Ontology#Part4_Product_1
:Part4_Product_1 rdf:type owl:NamedIndividual ,
                          :Part ;
                 :hasProduct :Product_1 ;
                 :hasDueDate "4 weeks" .


###  http://www.semanticweb.org/sc3/ontologies/2022/0/Planning-Ontology#Part5_Product_1
:Part5_Product_1 rdf:type owl:NamedIndividual ,
                          :Part ;
                 :hasProduct :Product_1 ;
                 :hasDueDate "5 weeks" .


###  http://www.semanticweb.org/sc3/ontologies/2022/0/Planning-Ontology#PeriodLength
:PeriodLength rdf:type owl:NamedIndividual ,
                       <http://www.w3.org/2006/time#Interval> ;
              <http://www.w3.org/2006/time#days> 1 .


###  http://www.semanticweb.org/sc3/ontologies/2022/0/Planning-Ontology#PlanningInstance_Frontend_1
:PlanningInstance_Frontend_1 rdf:type owl:NamedIndividual ,
                                      :PlanningInstance ;
                             :hasConstraint :Capacity_Restriction_Equation ,
                                            :Inventory_Balance_Equation ,
                                            :Material_Flow_Equation ,
                                            :Wip_Balance_Equation .


###  http://www.semanticweb.org/sc3/ontologies/2022/0/Planning-Ontology#Process_Product_1
:Process_Product_1 rdf:type owl:NamedIndividual .


###  http://www.semanticweb.org/sc3/ontologies/2022/0/Planning-Ontology#Product_1
:Product_1 rdf:type owl:NamedIndividual ,
                    <http://www.semanticweb.org/sc3/ontologies/2022/0/ozone-ontology#Product> ;
           :hasActivities :Activity_Etching ,
                          :Activity_Oxide ,
                          :Activity_Photo ,
                          :Activity_UV_Bake ;
           :hasLocation :Frontend_1 ;
           :hasProcess :Process_Product_1 ;
           :hasProduct :Product_1 .


###  http://www.semanticweb.org/sc3/ontologies/2022/0/Planning-Ontology#Product_2
:Product_2 rdf:type owl:NamedIndividual ,
                    <http://www.semanticweb.org/sc3/ontologies/2022/0/ozone-ontology#Product> .


###  http://www.semanticweb.org/sc3/ontologies/2022/0/Planning-Ontology#RequiredCap1
:RequiredCap1 rdf:type owl:NamedIndividual ,
                       :RequiredCapacity .


###  http://www.semanticweb.org/sc3/ontologies/2022/0/Planning-Ontology#RequiredCap2
:RequiredCap2 rdf:type owl:NamedIndividual ,
                       :RequiredCapacity .


###  http://www.semanticweb.org/sc3/ontologies/2022/0/Planning-Ontology#RequiredCap3
:RequiredCap3 rdf:type owl:NamedIndividual ,
                       :RequiredCapacity .


###  http://www.semanticweb.org/sc3/ontologies/2022/0/Planning-Ontology#RequiredCap4
:RequiredCap4 rdf:type owl:NamedIndividual ,
                       :RequiredCapacity .


###  http://www.semanticweb.org/sc3/ontologies/2022/0/Planning-Ontology#SimulationHorizon
:SimulationHorizon rdf:type owl:NamedIndividual ,
                            <http://www.w3.org/2006/time#Duration> ;
                   <http://www.w3.org/2006/time#weeks> 26 .


###  http://www.semanticweb.org/sc3/ontologies/2022/0/Planning-Ontology#Wip_Balance_Equation
:Wip_Balance_Equation rdf:type owl:NamedIndividual ,
                               :PlanningConstraint ;
                      :sc3:formula """forall($g in Products, $t in PlanningHorizon, $j in Frontends) -> FE_Wip($j, $g, $t) = FE_X($j, $g, $t) - FE_Y($j, $g, $t) + FE_Wip($j, $g, $t-1)

Frontends= Frontend_1, Frontend_2;
Products= Product_1;""" .


###  http://www.w3.org/2006/time#Friday
<http://www.w3.org/2006/time#Friday> rdf:type <http://www.w3.org/2006/time#DayOfWeek> ;
                                     rdfs:label "Friday"@en ;
                                     <http://www.w3.org/2004/02/skos/core#prefLabel> "Freitag"@de ,
                                                                                     "Friday"@en ,
                                                                                     "Piątek"@pl ,
                                                                                     "Sexta-feira"@pt ,
                                                                                     "Vendredi"@fr ,
                                                                                     "Venerdì"@it ,
                                                                                     "Viernes"@es ,
                                                                                     "Vrijdag"@nl ,
                                                                                     "Пятница"@ru ,
                                                                                     "الجمعة"@ar ,
                                                                                     "星期五"@zh ,
                                                                                     "金曜日"@ja .


###  http://www.w3.org/2006/time#Monday
<http://www.w3.org/2006/time#Monday> rdf:type <http://www.w3.org/2006/time#DayOfWeek> ;
                                     rdfs:label "Monday"@en ;
                                     <http://www.w3.org/2004/02/skos/core#prefLabel> "Lundi"@fr ,
                                                                                     "Lunedì"@it ,
                                                                                     "Lunes"@es ,
                                                                                     "Maandag"@nl ,
                                                                                     "Monday"@en ,
                                                                                     "Montag"@de ,
                                                                                     "Poniedziałek"@pl ,
                                                                                     "Segunda-feira"@pt ,
                                                                                     "Понедельник"@ru ,
                                                                                     "الاثنين"@ar ,
                                                                                     "星期一"@zh ,
                                                                                     "月曜日"@ja .


###  http://www.w3.org/2006/time#Saturday
<http://www.w3.org/2006/time#Saturday> rdf:type <http://www.w3.org/2006/time#DayOfWeek> ;
                                       rdfs:label "Saturday"@en ;
                                       <http://www.w3.org/2004/02/skos/core#prefLabel> "Sabato"@it ,
                                                                                       "Samedi"@fr ,
                                                                                       "Samstag"@de ,
                                                                                       "Saturday"@en ,
                                                                                       "Sobota"@pl ,
                                                                                       "Sábado"@es ,
                                                                                       "Sábado"@pt ,
                                                                                       "Zaterdag"@nl ,
                                                                                       "Суббота"@ru ,
                                                                                       "السبت"@ar ,
                                                                                       "土曜日"@ja ,
                                                                                       "星期六"@zh .


###  http://www.w3.org/2006/time#Sunday
<http://www.w3.org/2006/time#Sunday> rdf:type <http://www.w3.org/2006/time#DayOfWeek> ;
                                     rdfs:label "Sunday"@en ;
                                     <http://www.w3.org/2004/02/skos/core#prefLabel> "Dimanche"@fr ,
                                                                                     "Domenica"@it ,
                                                                                     "Domingo"@es ,
                                                                                     "Domingo"@pt ,
                                                                                     "Niedziela"@pl ,
                                                                                     "Sonntag"@de ,
                                                                                     "Sunday"@en ,
                                                                                     "Zondag"@nl ,
                                                                                     "Воскресенье"@ru ,
                                                                                     "الأحد (يوم)"@ar ,
                                                                                     "日曜日"@ja ,
                                                                                     "星期日"@zh .


###  http://www.w3.org/2006/time#Thursday
<http://www.w3.org/2006/time#Thursday> rdf:type <http://www.w3.org/2006/time#DayOfWeek> ;
                                       rdfs:label "Thursday"@en ;
                                       <http://www.w3.org/2004/02/skos/core#prefLabel> "Czwartek"@pl ,
                                                                                       "Donderdag"@nl ,
                                                                                       "Donnerstag"@de ,
                                                                                       "Giovedì"@it ,
                                                                                       "Jeudi"@fr ,
                                                                                       "Jueves"@es ,
                                                                                       "Quinta-feira"@pt ,
                                                                                       "Thursday"@en ,
                                                                                       "Четверг"@ru ,
                                                                                       "الخميس"@ar ,
                                                                                       "星期四"@zh ,
                                                                                       "木曜日"@ja .


###  http://www.w3.org/2006/time#Tuesday
<http://www.w3.org/2006/time#Tuesday> rdf:type <http://www.w3.org/2006/time#DayOfWeek> ;
                                      rdfs:label "Tuesday"@en ;
                                      <http://www.w3.org/2004/02/skos/core#prefLabel> "Dienstag"@de ,
                                                                                      "Dinsdag"@nl ,
                                                                                      "Mardi"@fr ,
                                                                                      "Martedì"@it ,
                                                                                      "Martes"@es ,
                                                                                      "Terça-feira"@pt ,
                                                                                      "Tuesday"@en ,
                                                                                      "Wtorek"@pl ,
                                                                                      "Вторник"@ru ,
                                                                                      "الثلاثاء"@ar ,
                                                                                      "星期二"@zh ,
                                                                                      "火曜日"@ja .


###  http://www.w3.org/2006/time#Wednesday
<http://www.w3.org/2006/time#Wednesday> rdf:type <http://www.w3.org/2006/time#DayOfWeek> ;
                                        rdfs:label "Wednesday"@en ;
                                        <http://www.w3.org/2004/02/skos/core#prefLabel> "Mercoledì"@it ,
                                                                                        "Mercredi"@fr ,
                                                                                        "Mittwoch"@de ,
                                                                                        "Miércoles"@es ,
                                                                                        "Quarta-feira"@pt ,
                                                                                        "Wednesday"@en ,
                                                                                        "Woensdag"@nl ,
                                                                                        "Środa"@pl ,
                                                                                        "Среда"@ru ,
                                                                                        "الأربعاء"@ar ,
                                                                                        "星期三"@zh ,
                                                                                        "水曜日"@ja .


###  http://www.w3.org/2006/time#unitDay
<http://www.w3.org/2006/time#unitDay> rdf:type <http://www.w3.org/2006/time#TemporalUnit> ;
                                      <http://www.w3.org/2006/time#days> 1 ;
                                      <http://www.w3.org/2006/time#hours> 0 ;
                                      <http://www.w3.org/2006/time#minutes> 0 ;
                                      <http://www.w3.org/2006/time#months> 0 ;
                                      <http://www.w3.org/2006/time#seconds> 0 ;
                                      <http://www.w3.org/2006/time#weeks> 0 ;
                                      <http://www.w3.org/2006/time#years> 0 ;
                                      rdfs:label "Day (unit of temporal duration)"@en ;
                                      <http://www.w3.org/2004/02/skos/core#prefLabel> "Tag"@de ,
                                                                                      "dag"@nl ,
                                                                                      "day"@en ,
                                                                                      "dia"@pt ,
                                                                                      "doba"@pl ,
                                                                                      "día"@es ,
                                                                                      "giorno"@it ,
                                                                                      "jour"@fr ,
                                                                                      "يوماً ما"@ar ,
                                                                                      "ある日"@jp ,
                                                                                      "一天"@zh ,
                                                                                      "언젠가"@kr .


###  http://www.w3.org/2006/time#unitHour
<http://www.w3.org/2006/time#unitHour> rdf:type <http://www.w3.org/2006/time#TemporalUnit> ;
                                       <http://www.w3.org/2006/time#days> 0 ;
                                       <http://www.w3.org/2006/time#hours> 1 ;
                                       <http://www.w3.org/2006/time#minutes> 0 ;
                                       <http://www.w3.org/2006/time#months> 0 ;
                                       <http://www.w3.org/2006/time#seconds> 0 ;
                                       <http://www.w3.org/2006/time#weeks> 0 ;
                                       <http://www.w3.org/2006/time#years> 0 ;
                                       rdfs:label "Hour (unit of temporal duration)"@en ;
                                       <http://www.w3.org/2004/02/skos/core#prefLabel> "Stunde"@de ,
                                                                                       "godzina"@pl ,
                                                                                       "heure"@fr ,
                                                                                       "hora"@es ,
                                                                                       "hora"@pt ,
                                                                                       "hour"@en ,
                                                                                       "ora"@it ,
                                                                                       "uur"@nl ,
                                                                                       "ساعة واحدة"@ar ,
                                                                                       "一小時"@zh ,
                                                                                       "一時間"@jp ,
                                                                                       "한 시간"@kr ,
                                                                                       "один час\"@ru" .


###  http://www.w3.org/2006/time#unitMinute
<http://www.w3.org/2006/time#unitMinute> rdf:type <http://www.w3.org/2006/time#TemporalUnit> ;
                                         <http://www.w3.org/2006/time#days> 0 ;
                                         <http://www.w3.org/2006/time#hours> 0 ;
                                         <http://www.w3.org/2006/time#minutes> 1 ;
                                         <http://www.w3.org/2006/time#months> 0 ;
                                         <http://www.w3.org/2006/time#seconds> 0 ;
                                         <http://www.w3.org/2006/time#weeks> 0 ;
                                         <http://www.w3.org/2006/time#years> 0 ;
                                         rdfs:label "Minute (unit of temporal duration)"@en ;
                                         <http://www.w3.org/2004/02/skos/core#prefLabel> "Minute"@de ,
                                                                                         "minuta"@pl ,
                                                                                         "minute"@en ,
                                                                                         "minute"@fr ,
                                                                                         "minuto"@es ,
                                                                                         "minuto"@it ,
                                                                                         "minuto"@pt ,
                                                                                         "minuut"@nl ,
                                                                                         "одна минута"@ru ,
                                                                                         "دقيقة واحدة"@ar ,
                                                                                         "一分"@jp ,
                                                                                         "等一下"@zh ,
                                                                                         "분"@kr .


###  http://www.w3.org/2006/time#unitMonth
<http://www.w3.org/2006/time#unitMonth> rdf:type <http://www.w3.org/2006/time#TemporalUnit> ;
                                        <http://www.w3.org/2006/time#days> 0 ;
                                        <http://www.w3.org/2006/time#hours> 0 ;
                                        <http://www.w3.org/2006/time#minutes> 0 ;
                                        <http://www.w3.org/2006/time#months> 1 ;
                                        <http://www.w3.org/2006/time#seconds> 0 ;
                                        <http://www.w3.org/2006/time#weeks> 0 ;
                                        <http://www.w3.org/2006/time#years> 0 ;
                                        rdfs:label "Month (unit of temporal duration)"@en ;
                                        <http://www.w3.org/2004/02/skos/core#prefLabel> "Monat"@de ,
                                                                                        "maand"@nl ,
                                                                                        "mes"@es ,
                                                                                        "mese"@it ,
                                                                                        "miesiąc"@pl ,
                                                                                        "mois"@fr ,
                                                                                        "month"@en ,
                                                                                        "один месяц"@ru ,
                                                                                        "شهر واحد"@ar ,
                                                                                        "一か月"@jp ,
                                                                                        "一個月"@zh ,
                                                                                        "한달"@kr .


###  http://www.w3.org/2006/time#unitSecond
<http://www.w3.org/2006/time#unitSecond> rdf:type <http://www.w3.org/2006/time#TemporalUnit> ;
                                         <http://www.w3.org/2006/time#days> 0 ;
                                         <http://www.w3.org/2006/time#hours> 0 ;
                                         <http://www.w3.org/2006/time#minutes> 0 ;
                                         <http://www.w3.org/2006/time#months> 0 ;
                                         <http://www.w3.org/2006/time#seconds> 1 ;
                                         <http://www.w3.org/2006/time#weeks> 0 ;
                                         <http://www.w3.org/2006/time#years> 0 ;
                                         rdfs:label "Second (unit of temporal duration)"@en ;
                                         <http://www.w3.org/2004/02/skos/core#prefLabel> "Sekunde"@de ,
                                                                                         "Sekundę"@pl ,
                                                                                         "second"@en ,
                                                                                         "seconde"@fr ,
                                                                                         "seconde"@nl ,
                                                                                         "secondo"@it ,
                                                                                         "segundo"@es ,
                                                                                         "segundo"@pt ,
                                                                                         "ثانية واحدة"@ar ,
                                                                                         "一秒"@jp ,
                                                                                         "一秒"@zh ,
                                                                                         "일초"@kr .


###  http://www.w3.org/2006/time#unitWeek
<http://www.w3.org/2006/time#unitWeek> rdf:type <http://www.w3.org/2006/time#TemporalUnit> ;
                                       <http://www.w3.org/2006/time#days> 0 ;
                                       <http://www.w3.org/2006/time#hours> 0 ;
                                       <http://www.w3.org/2006/time#minutes> 0 ;
                                       <http://www.w3.org/2006/time#months> 0 ;
                                       <http://www.w3.org/2006/time#seconds> 0 ;
                                       <http://www.w3.org/2006/time#weeks> 1 ;
                                       <http://www.w3.org/2006/time#years> 0 ;
                                       rdfs:label "Week (unit of temporal duration)"@en ;
                                       <http://www.w3.org/2004/02/skos/core#prefLabel> "Woche"@de ,
                                                                                       "semaine"@fr ,
                                                                                       "semana"@es ,
                                                                                       "semana"@pt ,
                                                                                       "settimana"@it ,
                                                                                       "tydzień"@pl ,
                                                                                       "week"@en ,
                                                                                       "week"@nl ,
                                                                                       "одна неделя"@ru ,
                                                                                       "سبوع واحد"@ar ,
                                                                                       "一周"@zh ,
                                                                                       "一週間"@jp ,
                                                                                       "일주일"@kr .


###  http://www.w3.org/2006/time#unitYear
<http://www.w3.org/2006/time#unitYear> rdf:type <http://www.w3.org/2006/time#TemporalUnit> ;
                                       <http://www.w3.org/2006/time#days> 0 ;
                                       <http://www.w3.org/2006/time#hours> 0 ;
                                       <http://www.w3.org/2006/time#minutes> 0 ;
                                       <http://www.w3.org/2006/time#months> 0 ;
                                       <http://www.w3.org/2006/time#seconds> 0 ;
                                       <http://www.w3.org/2006/time#weeks> 0 ;
                                       <http://www.w3.org/2006/time#years> 1 ;
                                       rdfs:label "Year (unit of temporal duration)"@en ;
                                       <http://www.w3.org/2004/02/skos/core#prefLabel> "1 년"@kr ,
                                                                                       "1年"@jp ,
                                                                                       "Jahr"@de ,
                                                                                       "an"@fr ,
                                                                                       "anno"@it ,
                                                                                       "ano"@pt ,
                                                                                       "jaar"@nl ,
                                                                                       "rok"@pl ,
                                                                                       "un año"@es ,
                                                                                       "year"@en ,
                                                                                       "один год"@ru ,
                                                                                       "سنة واحدة"@ar ,
                                                                                       "一年"@zh .


[ xsd:pattern "---(0[1-9]|[1-9][0-9])(Z|(\\+|-)((0[0-9]|1[0-3]):[0-5][0-9]|14:00))?"
] .

[ xsd:pattern "--(0[1-9]|1[0-9]|20)(Z|(\\+|-)((0[0-9]|1[0-3]):[0-5][0-9]|14:00))?"
 ] .

[ xsd:pattern "-?([1-9][0-9]{3,}|0[0-9]{3})(Z|(\\+|-)((0[0-9]|1[0-3]):[0-5][0-9]|14:00))?"
 ] .

#################################################################
#    Annotations
#################################################################

:hasEarliestReleaseDate rdfs:comment "This is the earliest time where the activities associated with a PLANNING OBJECT can start. Note that the parameter RELEASE DATE is exogenous, i.e. given, in contrast to the property TIME." .


#################################################################
#    General axioms
#################################################################

[ rdf:type owl:AllDisjointClasses ;
  owl:members ( :Resource-Availability-Constraints
                :Resource-Compatibility-Constraints
                :Temporal-Constraints
              )
] .


###  Generated by the OWL API (version 5.1.18) https://github.com/owlcs/owlapi/
